<rdf:RDF
    xmlns:rdf="http://www.w3.org/1999/02/22-rdf-syntax-ns#"
    xmlns="https://isotc211.geolexica.org/ld/concepts/11/"
    xmlns:ldapi="https://isotc211.geolexica.org/ld/ldapi#"
    xmlns:lang="https://isotc211.geolexica.org/ld/language#"
    xmlns:rdfs="http://www.w3.org/2000/01/rdf-schema#"
    xmlns:geolexica="https://isotc211.geolexica.org/ld/geolexica#"
    xmlns:dcterms="http://purl.org/dc/terms/"
    xmlns:notes="https://isotc211.geolexica.org/ld/notes#"
    xmlns:sources="https://isotc211.geolexica.org/ld/sources#"
    xmlns:owl="http://www.w3.org/2002/07/owl#"
    xmlns:dctype="http://purl.org/dc/dcmitype/"
    xmlns:skos="http://www.w3.org/2004/02/skos/core#"
    xmlns:void="http://vocab.deri.ie/void#"
    xmlns:info="https://isotc211.geolexica.org/ld/info#"
    xmlns:vann="http://purl.org/vocab/vann/"
    xmlns:xsd="http://www.w3.org/2001/XMLSchema#"
    xmlns:reviews="https://isotc211.geolexica.org/ld/reviews#" > 
  <rdf:Description rdf:about="https://isotc211.geolexica.org/ld/concepts/11/">
    <owl:versionIRI rdf:resource="https://isotc211.geolexica.org/ld/concepts/11/"/>
    <dcterms:created rdf:datatype="http://www.w3.org/2001/XMLSchema#date">2022-01-20</dcterms:created>
    <dcterms:issued> </dcterms:issued>
    <vann:preferredNamespaceUri>https://isotc211.geolexica.org/ld/concepts/11/</vann:preferredNamespaceUri>
    <vann:preferredNamespacePrefix>concept11</vann:preferredNamespacePrefix>
    <dcterms:modified rdf:datatype="http://www.w3.org/2001/XMLSchema#date">2022-01-28</dcterms:modified>
    <owl:imports rdf:resource="https://isotc211.geolexica.org/ld/notes#"/>
    <dcterms:contributor rdf:resource="https://www.linkedin.com/in/rhtse/"/>
    <dcterms:conformsTo rdf:resource="https://isotc211.geolexica.org/ld/geolexica/v1.0/"/>
    <owl:imports rdf:resource="https://isotc211.geolexica.org/ld/reviews#"/>
    <owl:imports rdf:resource="https://isotc211.geolexica.org/ld/ldapi#"/>
    <dcterms:creator rdf:resource="https://www.linkedin.com/in/lanemk"/>
    <dcterms:license>Copyright 2022 OSGeo</dcterms:license>
    <rdfs:label>aggregation (UML)</rdfs:label>
    <dcterms:title>aggregation (UML)</dcterms:title>
    <rdf:type rdf:resource="http://purl.org/dc/dcmitype/Dataset"/>
    <owl:imports rdf:resource="https://isotc211.geolexica.org/ld/geolexica"/>
    <owl:imports rdf:resource="https://isotc211.geolexica.org/ld/language#"/>
    <owl:imports rdf:resource="https://isotc211.geolexica.org/ld/sources#"/>
    <owl:imports rdf:resource="https://isotc211.geolexica.org/ld/info#"/>
  </rdf:Description>
  <rdf:Description rdf:about="http://purl.org/dc/terms/issued">
    <rdf:type rdf:resource="http://www.w3.org/2002/07/owl#AnnotationProperty"/>
  </rdf:Description>
  <rdf:Description rdf:about="http://purl.org/dc/dcmitype/Dataset">
    <owl:sameAs rdf:resource="http://vocab.deri.ie/void#Dataset"/>
  </rdf:Description>
  <rdf:Description rdf:about="https://isotc211.geolexica.org/ld/concepts/11/aggregation">
    <geolexica:origin rdf:resource="https://isotc211.geolexica.org/ld/language#danRegistry"/>
    <lang:eng-note xml:lang="en">Note to entry: See composition</lang:eng-note>
    <lang:spa-note xml:lang="es">Nota: Véase la composición</lang:spa-note>
    <skos:prefLabel xml:lang="fr">agrégation (UML)</skos:prefLabel>
    <skos:prefLabel xml:lang="ko">집합 연관 (UML)</skos:prefLabel>
    <geolexica:hasLangCode rdf:resource="https://isotc211.geolexica.org/ld/language#fin"/>
    <skos:definition xml:lang="en">special form of association that specifies a whole-part relationship between the aggregate (whole) and a component part</skos:definition>
    <skos:definition xml:lang="sv">special form of association that specifies a whole-part relationship between the aggregate (whole) and a component part</skos:definition>
    <skos:definition xml:lang="zh">(UML)关联的特殊形式，用以说明聚集(整体)与组成部分之间的整体-部分关系。</skos:definition>
    <geolexica:origin rdf:resource="https://isotc211.geolexica.org/ld/language#spaRegistry"/>
    <skos:prefLabel xml:lang="ar">تجميع (UML)</skos:prefLabel>
    <geolexica:hasLangCode rdf:resource="https://isotc211.geolexica.org/ld/language#kor"/>
    <skos:definition xml:lang="da">særlig form for association, der specificerer et helhed-del-forhold mellem en klasse, som indtager rollen som helheden, og en eller flere klasser, som indtager rollen som del</skos:definition>
    <geolexica:hasLangCode rdf:resource="https://isotc211.geolexica.org/ld/language#zho"/>
    <geolexica:hasLDAPI rdf:resource="https://isotc211.geolexica.org/ld/ldapi#ldapi11-rdfxml"/>
    <geolexica:hasLangCode rdf:resource="https://isotc211.geolexica.org/ld/language#deu"/>
    <geolexica:origin rdf:resource="https://isotc211.geolexica.org/ld/language#sweRegistry"/>
    <lang:deu-note rdf:resource="https://isotc211.geolexica.org/ld/notes#DefnTransUnavail"/>
    <lang:dan-note xml:lang="da">Bemærk til posten: Se komposition</lang:dan-note>
    <geolexica:hasLangCode rdf:resource="https://isotc211.geolexica.org/ld/language#ara"/>
    <skos:prefLabel xml:lang="zh">聚合(UML)</skos:prefLabel>
    <geolexica:hasLangCode rdf:resource="https://isotc211.geolexica.org/ld/language#rus"/>
    <lang:ara-note xml:lang="ar">ملاحظة: أنظر التركيب</lang:ara-note>
    <geolexica:origin rdf:resource="https://isotc211.geolexica.org/ld/language#rusRegistry"/>
    <lang:fin-note xml:lang="fi">HUOM.: Katso vahva/aito kooste (composition).</lang:fin-note>
    <geolexica:origin rdf:resource="https://isotc211.geolexica.org/ld/language#korRegistry"/>
    <geolexica:hasLDAPI rdf:resource="https://isotc211.geolexica.org/ld/ldapi#ldapi11-json"/>
    <geolexica:origin rdf:resource="https://isotc211.geolexica.org/ld/language#finRegistry"/>
    <skos:prefLabel xml:lang="sv">aggregering</skos:prefLabel>
    <geolexica:hasLangCode rdf:resource="https://isotc211.geolexica.org/ld/language#spa"/>
    <rdfs:label>aggregation (UML)</rdfs:label>
    <rdf:type rdf:resource="http://www.w3.org/2004/02/skos/core#Concept"/>
    <geolexica:origin rdf:resource="https://isotc211.geolexica.org/ld/language#engRegistry"/>
    <geolexica:hasLangCode rdf:resource="https://isotc211.geolexica.org/ld/language#swe"/>
    <skos:definition xml:lang="es">forma especial de asociación  que especifica una relación del todo con una parte entre el agregado (el todo) y una parte componente</skos:definition>
    <skos:altLabel xml:lang="fi">kokoelma (UML)</skos:altLabel>
    <geolexica:hasLangCode rdf:resource="https://isotc211.geolexica.org/ld/language#fra"/>
    <geolexica:hasReview rdf:resource="https://isotc211.geolexica.org/ld/reviews#Review11"/>
    <geolexica:hasLDAPI rdf:resource="https://isotc211.geolexica.org/ld/ldapi#ldapi11-skosrdf"/>
    <lang:kor-note xml:lang="ko">비고: 합성 참고</lang:kor-note>
    <geolexica:origin rdf:resource="https://isotc211.geolexica.org/ld/language#araRegistry"/>
    <rdf:type rdf:resource="http://www.w3.org/2002/07/owl#NamedIndividual"/>
    <skos:prefLabel xml:lang="fi">kooste (UML)</skos:prefLabel>
    <skos:definition xml:lang="ru">особая форма ассоциации, описывающая отношение «целое-часть» между агрегатом («целое») и компонентом («часть»)</skos:definition>
    <skos:definition xml:lang="ko">집합체와 컴포넌트 간의 관계를 설명한 연관의 특정 형태</skos:definition>
    <geolexica:hasInfo rdf:resource="https://isotc211.geolexica.org/ld/info#Info11"/>
    <skos:prefLabel xml:lang="en">aggregation (UML)</skos:prefLabel>
    <skos:prefLabel xml:lang="ru">агрегация (UML)</skos:prefLabel>
    <geolexica:origin rdf:resource="https://isotc211.geolexica.org/ld/language#fraRegistry"/>
    <skos:definition xml:lang="fi">assosiaation erityinen laji, joka määrittää kokonaisuuden (aggregaatin) ja sen osan välisen suhteen</skos:definition>
    <lang:rus-note xml:lang="ru">Примечание: См. термин «композиция»</lang:rus-note>
    <geolexica:hasLangCode rdf:resource="https://isotc211.geolexica.org/ld/language#dan"/>
    <skos:prefLabel xml:lang="es">agregación (UML)</skos:prefLabel>
    <lang:swe-note rdf:resource="https://isotc211.geolexica.org/ld/notes#NoteTransUnavail"/>
    <skos:definition xml:lang="fr">forme spéciale d&amp;#39;association qui spécifie une relation ensemble-composant entre l&amp;#39;agrégat (ensemble) et la partie composante</skos:definition>
    <lang:rus-note rdf:resource="https://isotc211.geolexica.org/ld/notes#NoteTransDiff"/>
    <dcterms:identifier rdf:datatype="http://www.w3.org/2001/XMLSchema#integer">11</dcterms:identifier>
    <skos:prefLabel xml:lang="da">aggregering (UML)</skos:prefLabel>
    <geolexica:origin rdf:resource="https://isotc211.geolexica.org/ld/language#jpnRegistry"/>
    <skos:inScheme rdf:resource="https://isotc211.geolexica.org/ld/geolexica#GeolexicaConceptScheme"/>
    <geolexica:hasLangCode rdf:resource="https://isotc211.geolexica.org/ld/language#eng"/>
    <skos:definition xml:lang="ar">شكل خاص من أشكال الترابط يصف علاقة &amp;quot;الكل والجزء&amp;quot; بين الكل والجزء المكون له.</skos:definition>
    <lang:deu-note rdf:resource="https://isotc211.geolexica.org/ld/notes#NoteTransUnavail"/>
    <lang:zho-note xml:lang="zh">注： 参见组合。</lang:zho-note>
    <geolexica:origin rdf:resource="https://isotc211.geolexica.org/ld/language#zhoRegistry"/>
    <skos:prefLabel xml:lang="de">Aggregation (UML)</skos:prefLabel>
    <skos:notation rdf:datatype="http://www.w3.org/2001/XMLSchema#integer">11</skos:notation>
    <geolexica:hasLDAPI rdf:resource="https://isotc211.geolexica.org/ld/ldapi#ldapi11-jsonld"/>
  </rdf:Description>
  <rdf:Description rdf:about="http://purl.org/vocab/vann/preferredNamespacePrefix">
    <rdf:type rdf:resource="http://www.w3.org/2002/07/owl#AnnotationProperty"/>
  </rdf:Description>
  <rdf:Description rdf:about="http://purl.org/vocab/vann/preferredNamespaceUri">
    <rdf:type rdf:resource="http://www.w3.org/2002/07/owl#AnnotationProperty"/>
  </rdf:Description>
  <rdf:Description rdf:about="http://purl.org/dc/terms/publisher">
    <rdf:type rdf:resource="http://www.w3.org/2002/07/owl#AnnotationProperty"/>
  </rdf:Description>
  <rdf:Description rdf:about="http://purl.org/dc/terms/source">
    <rdf:type rdf:resource="http://www.w3.org/2002/07/owl#AnnotationProperty"/>
  </rdf:Description>
  <rdf:Description rdf:about="http://purl.org/dc/terms/created">
    <rdf:type rdf:resource="http://www.w3.org/2002/07/owl#AnnotationProperty"/>
  </rdf:Description>
  <rdf:Description rdf:about="http://purl.org/dc/terms/conformsTo">
    <rdf:type rdf:resource="http://www.w3.org/2002/07/owl#AnnotationProperty"/>
  </rdf:Description>
  <rdf:Description rdf:about="http://purl.org/dc/terms/modified">
    <rdf:type rdf:resource="http://www.w3.org/2002/07/owl#AnnotationProperty"/>
  </rdf:Description>
  <rdf:Description rdf:about="http://purl.org/dc/terms/license">
    <rdf:type rdf:resource="http://www.w3.org/2002/07/owl#AnnotationProperty"/>
  </rdf:Description>
</rdf:RDF>
