<rdf:RDF
    xmlns:rdf="http://www.w3.org/1999/02/22-rdf-syntax-ns#"
    xmlns="https://isotc211.geolexica.org/ld/concepts/26/"
    xmlns:ldapi="https://isotc211.geolexica.org/ld/ldapi#"
    xmlns:lang="https://isotc211.geolexica.org/ld/language#"
    xmlns:rdfs="http://www.w3.org/2000/01/rdf-schema#"
    xmlns:geolexica="https://isotc211.geolexica.org/ld/geolexica#"
    xmlns:dcterms="http://purl.org/dc/terms/"
    xmlns:notes="https://isotc211.geolexica.org/ld/notes#"
    xmlns:sources="https://isotc211.geolexica.org/ld/sources#"
    xmlns:owl="http://www.w3.org/2002/07/owl#"
    xmlns:dctype="http://purl.org/dc/dcmitype/"
    xmlns:skos="http://www.w3.org/2004/02/skos/core#"
    xmlns:void="http://vocab.deri.ie/void#"
    xmlns:info="https://isotc211.geolexica.org/ld/info#"
    xmlns:vann="http://purl.org/vocab/vann/"
    xmlns:xsd="http://www.w3.org/2001/XMLSchema#"
    xmlns:reviews="https://isotc211.geolexica.org/ld/reviews#" > 
  <rdf:Description rdf:about="http://purl.org/dc/terms/issued">
    <rdf:type rdf:resource="http://www.w3.org/2002/07/owl#AnnotationProperty"/>
  </rdf:Description>
  <rdf:Description rdf:about="https://isotc211.geolexica.org/ld/concepts/26/base_standard">
    <geolexica:origin rdf:resource="https://isotc211.geolexica.org/ld/language#fraRegistry"/>
    <dcterms:identifier rdf:datatype="http://www.w3.org/2001/XMLSchema#integer">26</dcterms:identifier>
    <geolexica:hasLangCode rdf:resource="https://isotc211.geolexica.org/ld/language#dan"/>
    <skos:prefLabel xml:lang="fr">norme de base</skos:prefLabel>
    <skos:definition xml:lang="en">ISO geographic information standard or other information technology standard that is used as a source from which a profile may be constructed</skos:definition>
    <skos:prefLabel xml:lang="en">base standard</skos:prefLabel>
    <skos:prefLabel xml:lang="fi">perusstandardi</skos:prefLabel>
    <geolexica:hasLangCode rdf:resource="https://isotc211.geolexica.org/ld/language#spa"/>
    <geolexica:hasLangCode rdf:resource="https://isotc211.geolexica.org/ld/language#fra"/>
    <rdfs:label>base standard</rdfs:label>
    <skos:definition xml:lang="zh">能够用于构建专用标准的ISO地理信息标准或其他信息技术标准。</skos:definition>
    <skos:prefLabel xml:lang="ko">기반 표준</skos:prefLabel>
    <lang:deu-note rdf:resource="https://isotc211.geolexica.org/ld/notes#DefnTransUnavail"/>
    <geolexica:origin rdf:resource="https://isotc211.geolexica.org/ld/language#korRegistry"/>
    <skos:definition xml:lang="fr">norme d&amp;#39;information géographique ISO ou autre norme de technologie de l&amp;#39;information publiée comme une source et à partir de laquelle un profil peut être construit</skos:definition>
    <geolexica:hasLDAPI rdf:resource="https://isotc211.geolexica.org/ld/ldapi#ldapi26-rdfxml"/>
    <skos:prefLabel xml:lang="ar">مواصفة قياسية أساسية</skos:prefLabel>
    <skos:definition xml:lang="fi">paikkatietoa koskeva ISO-standardi tai muu tietotekniikkastandardi, jota voidaan käyttää profiilin laatimisen perustana</skos:definition>
    <skos:definition xml:lang="sv">standard som har ett brett syfte eller innehåller allmänna bestämmelser för ett visst område</skos:definition>
    <geolexica:origin rdf:resource="https://isotc211.geolexica.org/ld/language#sweRegistry"/>
    <geolexica:hasLangCode rdf:resource="https://isotc211.geolexica.org/ld/language#swe"/>
    <rdf:type rdf:resource="http://www.w3.org/2004/02/skos/core#Concept"/>
    <geolexica:origin rdf:resource="https://isotc211.geolexica.org/ld/language#zhoRegistry"/>
    <skos:definition xml:lang="ko">하나의 프로파일을 구성하는 데 활용될 수 있는 KS(ISO) 지리 정보 표준 또는 이외의 정보 기술 표준</skos:definition>
    <geolexica:origin rdf:resource="https://isotc211.geolexica.org/ld/language#engRegistry"/>
    <skos:definition xml:lang="es">norma ISO de información geográfica, u otra norma de tecnologías de la información, que se puede utilizar como fuente a partir de la cual es posible construir un perfil</skos:definition>
    <skos:prefLabel xml:lang="de">Basisstandard</skos:prefLabel>
    <geolexica:hasLangCode rdf:resource="https://isotc211.geolexica.org/ld/language#kor"/>
    <geolexica:hasLangCode rdf:resource="https://isotc211.geolexica.org/ld/language#eng"/>
    <skos:prefLabel xml:lang="ru">базовый стандарт</skos:prefLabel>
    <geolexica:origin rdf:resource="https://isotc211.geolexica.org/ld/language#araRegistry"/>
    <skos:prefLabel xml:lang="es">norma base</skos:prefLabel>
    <geolexica:hasLangCode rdf:resource="https://isotc211.geolexica.org/ld/language#ara"/>
    <skos:definition xml:lang="ru">стандарт ISO из серии  «Географическая информация» или другой технологический стандарт, который может служить источником для разработки профиля</skos:definition>
    <rdf:type rdf:resource="http://www.w3.org/2002/07/owl#NamedIndividual"/>
    <skos:definition xml:lang="da">SO geografisk informations-standard eller anden informationsteknologisk standard, der er udgivet som en kilde, hvorfra der kan opbygges en profil</skos:definition>
    <geolexica:hasLDAPI rdf:resource="https://isotc211.geolexica.org/ld/ldapi#ldapi26-skosrdf"/>
    <geolexica:hasLDAPI rdf:resource="https://isotc211.geolexica.org/ld/ldapi#ldapi26-jsonld"/>
    <geolexica:origin rdf:resource="https://isotc211.geolexica.org/ld/language#rusRegistry"/>
    <skos:prefLabel xml:lang="da">basisstandard</skos:prefLabel>
    <geolexica:origin rdf:resource="https://isotc211.geolexica.org/ld/language#finRegistry"/>
    <geolexica:origin rdf:resource="https://isotc211.geolexica.org/ld/language#spaRegistry"/>
    <skos:definition xml:lang="ar">مواصفة قياسية للمعلومات الجغرافية ( ISO ) أو مواصفة قياسية لتقنية المعلومات والتي صدرت كمصدر يمكن إنشاء مواصفة محددة منه</skos:definition>
    <skos:notation rdf:datatype="http://www.w3.org/2001/XMLSchema#integer">26</skos:notation>
    <geolexica:hasLDAPI rdf:resource="https://isotc211.geolexica.org/ld/ldapi#ldapi26-json"/>
    <geolexica:origin rdf:resource="https://isotc211.geolexica.org/ld/language#danRegistry"/>
    <geolexica:hasLangCode rdf:resource="https://isotc211.geolexica.org/ld/language#fin"/>
    <geolexica:hasLangCode rdf:resource="https://isotc211.geolexica.org/ld/language#zho"/>
    <geolexica:hasInfo rdf:resource="https://isotc211.geolexica.org/ld/info#Info26"/>
    <geolexica:origin rdf:resource="https://isotc211.geolexica.org/ld/language#deuRegistry"/>
    <skos:inScheme rdf:resource="https://isotc211.geolexica.org/ld/geolexica#GeolexicaConceptScheme"/>
    <geolexica:hasLangCode rdf:resource="https://isotc211.geolexica.org/ld/language#rus"/>
    <skos:prefLabel xml:lang="zh">基础标准</skos:prefLabel>
    <lang:fra-note rdf:resource="https://isotc211.geolexica.org/ld/notes#NoteTransDiff"/>
    <skos:prefLabel xml:lang="sv">grundstandard</skos:prefLabel>
  </rdf:Description>
  <rdf:Description rdf:about="http://purl.org/dc/dcmitype/Dataset">
    <owl:sameAs rdf:resource="http://vocab.deri.ie/void#Dataset"/>
  </rdf:Description>
  <rdf:Description rdf:about="http://purl.org/vocab/vann/preferredNamespacePrefix">
    <rdf:type rdf:resource="http://www.w3.org/2002/07/owl#AnnotationProperty"/>
  </rdf:Description>
  <rdf:Description rdf:about="http://purl.org/vocab/vann/preferredNamespaceUri">
    <rdf:type rdf:resource="http://www.w3.org/2002/07/owl#AnnotationProperty"/>
  </rdf:Description>
  <rdf:Description rdf:about="http://purl.org/dc/terms/publisher">
    <rdf:type rdf:resource="http://www.w3.org/2002/07/owl#AnnotationProperty"/>
  </rdf:Description>
  <rdf:Description rdf:about="http://purl.org/dc/terms/source">
    <rdf:type rdf:resource="http://www.w3.org/2002/07/owl#AnnotationProperty"/>
  </rdf:Description>
  <rdf:Description rdf:about="http://purl.org/dc/terms/created">
    <rdf:type rdf:resource="http://www.w3.org/2002/07/owl#AnnotationProperty"/>
  </rdf:Description>
  <rdf:Description rdf:about="http://purl.org/dc/terms/conformsTo">
    <rdf:type rdf:resource="http://www.w3.org/2002/07/owl#AnnotationProperty"/>
  </rdf:Description>
  <rdf:Description rdf:about="http://purl.org/dc/terms/modified">
    <rdf:type rdf:resource="http://www.w3.org/2002/07/owl#AnnotationProperty"/>
  </rdf:Description>
  <rdf:Description rdf:about="https://isotc211.geolexica.org/ld/concepts/26/">
    <owl:imports rdf:resource="https://isotc211.geolexica.org/ld/ldapi#"/>
    <owl:imports rdf:resource="https://isotc211.geolexica.org/ld/geolexica"/>
    <dcterms:modified rdf:datatype="http://www.w3.org/2001/XMLSchema#date">2022-01-28</dcterms:modified>
    <vann:preferredNamespacePrefix>concept26</vann:preferredNamespacePrefix>
    <dcterms:license>Copyright 2022 OSGeo</dcterms:license>
    <dcterms:contributor rdf:resource="https://www.linkedin.com/in/rhtse/"/>
    <owl:imports rdf:resource="https://isotc211.geolexica.org/ld/language#"/>
    <owl:versionIRI rdf:resource="https://isotc211.geolexica.org/ld/concepts/26/"/>
    <rdfs:label>base standard</rdfs:label>
    <dcterms:conformsTo rdf:resource="https://isotc211.geolexica.org/ld/geolexica/v1.0/"/>
    <dcterms:title>base standard</dcterms:title>
    <owl:imports rdf:resource="https://isotc211.geolexica.org/ld/reviews#"/>
    <owl:imports rdf:resource="https://isotc211.geolexica.org/ld/notes#"/>
    <dcterms:issued> </dcterms:issued>
    <owl:imports rdf:resource="https://isotc211.geolexica.org/ld/info#"/>
    <vann:preferredNamespaceUri>https://isotc211.geolexica.org/ld/concepts/26/</vann:preferredNamespaceUri>
    <rdf:type rdf:resource="http://purl.org/dc/dcmitype/Dataset"/>
    <owl:imports rdf:resource="https://isotc211.geolexica.org/ld/sources#"/>
    <dcterms:creator rdf:resource="https://www.linkedin.com/in/lanemk"/>
    <dcterms:created rdf:datatype="http://www.w3.org/2001/XMLSchema#date">2022-01-20</dcterms:created>
  </rdf:Description>
  <rdf:Description rdf:about="http://purl.org/dc/terms/license">
    <rdf:type rdf:resource="http://www.w3.org/2002/07/owl#AnnotationProperty"/>
  </rdf:Description>
</rdf:RDF>
