<rdf:RDF
    xmlns:rdf="http://www.w3.org/1999/02/22-rdf-syntax-ns#"
    xmlns="https://isotc211.geolexica.org/api/ld/concepts/30/"
    xmlns:ldapi="https://isotc211.geolexica.org/api/ld/ldapi#"
    xmlns:lang="https://isotc211.geolexica.org/api/ld/language#"
    xmlns:rdfs="http://www.w3.org/2000/01/rdf-schema#"
    xmlns:geolexica="https://isotc211.geolexica.org/api/ld/geolexica#"
    xmlns:dcterms="http://purl.org/dc/terms/"
    xmlns:notes="https://isotc211.geolexica.org/api/ld/notes#"
    xmlns:sources="https://isotc211.geolexica.org/api/ld/sources#"
    xmlns:owl="http://www.w3.org/2002/07/owl#"
    xmlns:dctype="http://purl.org/dc/dcmitype/"
    xmlns:skos="http://www.w3.org/2004/02/skos/core#"
    xmlns:void="http://vocab.deri.ie/void#"
    xmlns:info="https://isotc211.geolexica.org/api/ld/info#"
    xmlns:vann="http://purl.org/vocab/vann/"
    xmlns:xsd="http://www.w3.org/2001/XMLSchema#"
    xmlns:reviews="https://isotc211.geolexica.org/api/ld/reviews#" > 
  <rdf:Description rdf:about="https://isotc211.geolexica.org/api/ld/concepts/30/buffer">
    <geolexica:origin rdf:resource="https://isotc211.geolexica.org/api/ld/language#msaRegistry"/>
    <geolexica:hasLangCode rdf:resource="https://isotc211.geolexica.org/api/ld/language#ara"/>
    <skos:prefLabel xml:lang="ms">penampan</skos:prefLabel>
    <geolexica:hasLDAPI rdf:resource="https://isotc211.geolexica.org/api/ld/ldapi#ldapi30-rdfxml"/>
    <geolexica:hasLangCode rdf:resource="https://isotc211.geolexica.org/api/ld/language#msa"/>
    <geolexica:origin rdf:resource="https://isotc211.geolexica.org/api/ld/language#jpnRegistry"/>
    <geolexica:hasLangCode rdf:resource="https://isotc211.geolexica.org/api/ld/language#zho"/>
    <skos:definition xml:lang="ja">指定された幾何オブジェクトから与えられた距離以内のすべての直接位置を含む幾何オブジェクト。</skos:definition>
    <geolexica:origin rdf:resource="https://isotc211.geolexica.org/api/ld/language#korRegistry"/>
    <geolexica:origin rdf:resource="https://isotc211.geolexica.org/api/ld/language#finRegistry"/>
    <geolexica:hasLangCode rdf:resource="https://isotc211.geolexica.org/api/ld/language#eng"/>
    <skos:definition xml:lang="es">objeto geométrico que contiene todas las posiciones directas cuyas distancias a un objeto geométrico específico son menores o iguales que una distancia dada</skos:definition>
    <geolexica:origin rdf:resource="https://isotc211.geolexica.org/api/ld/language#zhoRegistry"/>
    <skos:prefLabel xml:lang="fi">vyöhyke</skos:prefLabel>
    <geolexica:origin rdf:resource="https://isotc211.geolexica.org/api/ld/language#spaRegistry"/>
    <skos:notation rdf:datatype="http://www.w3.org/2001/XMLSchema#integer">30</skos:notation>
    <geolexica:origin rdf:resource="https://isotc211.geolexica.org/api/ld/language#danRegistry"/>
    <geolexica:origin rdf:resource="https://isotc211.geolexica.org/api/ld/language#sweRegistry"/>
    <skos:prefLabel xml:lang="fr">tampon (buffer)</skos:prefLabel>
    <skos:prefLabel xml:lang="ja">バッファ</skos:prefLabel>
    <rdf:type rdf:resource="http://www.w3.org/2004/02/skos/core#Concept"/>
    <skos:definition xml:lang="pl">obiekt geometryczny zawierający wszystkie położenia bezpośrednie, których odległość od określonego obiektu geometrycznego jest równa danej odległości lub mniejsza</skos:definition>
    <geolexica:hasLangCode rdf:resource="https://isotc211.geolexica.org/api/ld/language#fin"/>
    <geolexica:hasLDAPI rdf:resource="https://isotc211.geolexica.org/api/ld/ldapi#ldapi30-jsonld"/>
    <skos:prefLabel xml:lang="de">Puffer</skos:prefLabel>
    <skos:definition xml:lang="zh">包含距一个指定几何对象的距离都小于或等于一个给定值的所有直接位置的几何对象。</skos:definition>
    <skos:inScheme rdf:resource="https://isotc211.geolexica.org/api/ld/geolexica#GeolexicaConceptScheme"/>
    <skos:definition xml:lang="ru">геометрический объект, содержащий все точки, расстояния от которых до заданного геометрического объекта меньше или равны заданной величине</skos:definition>
    <geolexica:origin rdf:resource="https://isotc211.geolexica.org/api/ld/language#rusRegistry"/>
    <geolexica:origin rdf:resource="https://isotc211.geolexica.org/api/ld/language#engRegistry"/>
    <geolexica:hasLangCode rdf:resource="https://isotc211.geolexica.org/api/ld/language#jpn"/>
    <geolexica:hasLDAPI rdf:resource="https://isotc211.geolexica.org/api/ld/ldapi#ldapi30-skosrdf"/>
    <skos:definition xml:lang="ms">Kawasan dalam ingatan utama yang telah dikhaskan untuk memegang data yang masih belum dapat dipindahkan kepada cakera</skos:definition>
    <skos:definition xml:lang="fi">geometrinen objekti, joka sisältää kaikki pisteet, joiden etäisyys annetusta geometrisestä objektista on pienempi tai yhtä suuri kuin tietty etäisyys</skos:definition>
    <skos:definition xml:lang="en">geometric object that contains all direct positions whose distance from a specified geometric object is less than or equal to a given distance</skos:definition>
    <skos:prefLabel xml:lang="pl">bufor</skos:prefLabel>
    <geolexica:origin rdf:resource="https://isotc211.geolexica.org/api/ld/language#deuRegistry"/>
    <skos:prefLabel xml:lang="es">buffer</skos:prefLabel>
    <skos:prefLabel xml:lang="en">buffer</skos:prefLabel>
    <skos:prefLabel xml:lang="da">buffer</skos:prefLabel>
    <geolexica:origin rdf:resource="https://isotc211.geolexica.org/api/ld/language#fraRegistry"/>
    <geolexica:hasInfo rdf:resource="https://isotc211.geolexica.org/api/ld/info#Info30"/>
    <geolexica:hasLangCode rdf:resource="https://isotc211.geolexica.org/api/ld/language#fra"/>
    <rdfs:label>buffer</rdfs:label>
    <geolexica:hasLangCode rdf:resource="https://isotc211.geolexica.org/api/ld/language#rus"/>
    <skos:prefLabel xml:lang="ko">영향 범위</skos:prefLabel>
    <geolexica:hasLangCode rdf:resource="https://isotc211.geolexica.org/api/ld/language#pol"/>
    <skos:definition xml:lang="ar">كيان هندسي يحتوي على جميع المواضع المباشرة التي تكون في نطاق يبعد عن كيان محدد مسافة محددة</skos:definition>
    <skos:prefLabel xml:lang="sv">buffertzon</skos:prefLabel>
    <geolexica:origin rdf:resource="https://isotc211.geolexica.org/api/ld/language#polRegistry"/>
    <rdf:type rdf:resource="http://www.w3.org/2002/07/owl#NamedIndividual"/>
    <skos:altLabel xml:lang="ko">버퍼</skos:altLabel>
    <geolexica:hasLangCode rdf:resource="https://isotc211.geolexica.org/api/ld/language#spa"/>
    <skos:prefLabel xml:lang="ru">буферная зона [буфер]</skos:prefLabel>
    <geolexica:hasLangCode rdf:resource="https://isotc211.geolexica.org/api/ld/language#deu"/>
    <geolexica:hasLangCode rdf:resource="https://isotc211.geolexica.org/api/ld/language#kor"/>
    <lang:deu-note rdf:resource="https://isotc211.geolexica.org/api/ld/notes#DefnTransUnavail"/>
    <dcterms:identifier rdf:datatype="http://www.w3.org/2001/XMLSchema#integer">30</dcterms:identifier>
    <geolexica:hasReview rdf:resource="https://isotc211.geolexica.org/api/ld/reviews#Review30"/>
    <skos:definition xml:lang="fr">objet géométrique contenant toutes les positions directes dont la distance à un objet géométrique spécifié est inférieure ou égale à une distance donnée</skos:definition>
    <skos:prefLabel xml:lang="zh">缓冲区</skos:prefLabel>
    <skos:prefLabel xml:lang="ar">نطاق</skos:prefLabel>
    <skos:definition xml:lang="da">geometrisk objekt, der indeholder alle de direkte positioner, hvis afstand fra et specificeret geometrisk objekt er mindre end eller lig med en given afstand</skos:definition>
    <skos:definition xml:lang="sv">område vars gränser befinner sig på givna avstånd från ett utvalt geografiskt objekt</skos:definition>
    <skos:definition xml:lang="ko">지정된 기하 객체로부터 주어진 거리 이내의 모든 직접 위치를 포함하는 기하 객체</skos:definition>
    <geolexica:hasLangCode rdf:resource="https://isotc211.geolexica.org/api/ld/language#dan"/>
    <geolexica:hasLDAPI rdf:resource="https://isotc211.geolexica.org/api/ld/ldapi#ldapi30-json"/>
    <geolexica:origin rdf:resource="https://isotc211.geolexica.org/api/ld/language#araRegistry"/>
    <geolexica:hasLangCode rdf:resource="https://isotc211.geolexica.org/api/ld/language#swe"/>
  </rdf:Description>
  <rdf:Description rdf:about="http://purl.org/dc/terms/issued">
    <rdf:type rdf:resource="http://www.w3.org/2002/07/owl#AnnotationProperty"/>
  </rdf:Description>
  <rdf:Description rdf:about="http://purl.org/dc/dcmitype/Dataset">
    <owl:sameAs rdf:resource="http://vocab.deri.ie/void#Dataset"/>
  </rdf:Description>
  <rdf:Description rdf:about="http://purl.org/vocab/vann/preferredNamespacePrefix">
    <rdf:type rdf:resource="http://www.w3.org/2002/07/owl#AnnotationProperty"/>
  </rdf:Description>
  <rdf:Description rdf:about="http://purl.org/vocab/vann/preferredNamespaceUri">
    <rdf:type rdf:resource="http://www.w3.org/2002/07/owl#AnnotationProperty"/>
  </rdf:Description>
  <rdf:Description rdf:about="http://purl.org/dc/terms/publisher">
    <rdf:type rdf:resource="http://www.w3.org/2002/07/owl#AnnotationProperty"/>
  </rdf:Description>
  <rdf:Description rdf:about="https://isotc211.geolexica.org/api/ld/concepts/30/">
    <vann:preferredNamespaceUri>https://isotc211.geolexica.org/api/ld/concepts/30/</vann:preferredNamespaceUri>
    <owl:imports rdf:resource="https://isotc211.geolexica.org/api/ld/reviews#"/>
    <dcterms:creator rdf:resource="https://www.linkedin.com/in/lanemk"/>
    <dcterms:modified rdf:datatype="http://www.w3.org/2001/XMLSchema#date">2022-01-28</dcterms:modified>
    <rdfs:label>buffer</rdfs:label>
    <owl:imports rdf:resource="https://isotc211.geolexica.org/api/ld/language#"/>
    <dcterms:license>Copyright 2022 OSGeo</dcterms:license>
    <owl:versionIRI rdf:resource="https://isotc211.geolexica.org/api/ld/concepts/30/"/>
    <dcterms:contributor rdf:resource="https://www.linkedin.com/in/rhtse/"/>
    <dcterms:conformsTo rdf:resource="https://isotc211.geolexica.org/api/ld/geolexica/v1.0/"/>
    <owl:imports rdf:resource="https://isotc211.geolexica.org/api/ld/notes#"/>
    <owl:imports rdf:resource="https://isotc211.geolexica.org/api/ld/sources#"/>
    <dcterms:title>buffer</dcterms:title>
    <owl:imports rdf:resource="https://isotc211.geolexica.org/api/ld/info#"/>
    <dcterms:created rdf:datatype="http://www.w3.org/2001/XMLSchema#date">2022-01-20</dcterms:created>
    <owl:imports rdf:resource="https://isotc211.geolexica.org/api/ld/geolexica"/>
    <vann:preferredNamespacePrefix>concept30</vann:preferredNamespacePrefix>
    <owl:imports rdf:resource="https://isotc211.geolexica.org/api/ld/ldapi#"/>
    <dcterms:issued> </dcterms:issued>
    <rdf:type rdf:resource="http://purl.org/dc/dcmitype/Dataset"/>
  </rdf:Description>
  <rdf:Description rdf:about="http://purl.org/dc/terms/source">
    <rdf:type rdf:resource="http://www.w3.org/2002/07/owl#AnnotationProperty"/>
  </rdf:Description>
  <rdf:Description rdf:about="http://purl.org/dc/terms/created">
    <rdf:type rdf:resource="http://www.w3.org/2002/07/owl#AnnotationProperty"/>
  </rdf:Description>
  <rdf:Description rdf:about="http://purl.org/dc/terms/conformsTo">
    <rdf:type rdf:resource="http://www.w3.org/2002/07/owl#AnnotationProperty"/>
  </rdf:Description>
  <rdf:Description rdf:about="http://purl.org/dc/terms/modified">
    <rdf:type rdf:resource="http://www.w3.org/2002/07/owl#AnnotationProperty"/>
  </rdf:Description>
  <rdf:Description rdf:about="http://purl.org/dc/terms/license">
    <rdf:type rdf:resource="http://www.w3.org/2002/07/owl#AnnotationProperty"/>
  </rdf:Description>
</rdf:RDF>
