@prefix : <https://isotc211.geolexica.org/ld/concepts#> .
@prefix owl: <http://www.w3.org/2002/07/owl#> .
@prefix rdf: <http://www.w3.org/1999/02/22-rdf-syntax-ns#> .
@prefix xml: <http://www.w3.org/XML/1998/namespace> .
@prefix xsd: <http://www.w3.org/2001/XMLSchema#> .
@prefix info: <https://isotc211.geolexica.org/ld/info#> .
@prefix lang: <https://isotc211.geolexica.org/ld/language#> .
@prefix rdfs: <http://www.w3.org/2000/01/rdf-schema#> .
@prefix skos: <http://www.w3.org/2004/02/skos/core#> .
@prefix vann: <http://purl.org/vocab/vann/> .
@prefix void: <http://vocab.deri.ie/void#> .
@prefix ldapi: <https://isotc211.geolexica.org/ld/ldapi#> .
@prefix notes: <https://isotc211.geolexica.org/ld/notes#> .
@prefix dctype: <http://purl.org/dc/dcmitype/> .
@prefix dcterms: <http://purl.org/dc/terms/> .
@prefix reviews: <https://isotc211.geolexica.org/ld/reviews#> .
@prefix sources: <https://isotc211.geolexica.org/ld/sources#> .
@prefix geolexica: <https://isotc211.geolexica.org/ld/geolexica#> .
@base <https://isotc211.geolexica.org/ld/concepts> .

<https://isotc211.geolexica.org/ld/concepts> rdf:type dctype:Dataset ;
        owl:versionIRI <https://isotc211.geolexica.org/ld/concepts/v1.0> ;
        owl:imports <https://isotc211.geolexica.org/ld/geolexica> ,
                    info: ,
                    lang: ,
                    ldapi: ,
                    notes: ,
                    reviews: ,
                    sources: ;
        dcterms:conformsTo <https://isotc211.geolexica.org/ld/geolexica/v1.0/> ;
        dcterms:contributor <https://www.linkedin.com/in/rhtse/> ;
        dcterms:created "2022-01-20"^^xsd:date ;
        dcterms:creator <https://www.linkedin.com/in/lanemk> ;
        dcterms:description "Concept serialization of ISO/TC 211 Multi-Lingual Glossary of Terms (MLGT)."@en ;
        dcterms:issued " " ;
        dcterms:license "Copyright 2022 OSGeo" ;
        dcterms:modified "2022-01-25"^^xsd:date ;
        dcterms:title "Concepts RDF Dataset: ISO/TC211 Multi-lingual Glossary of Terms (MLGT)"@en ;
        vann:preferredNamespacePrefix "mlgt-concepts" ;
        vann:preferredNamespaceUri "https://isotc211.geolexica.org/ld/concepts#" ;
        rdfs:label "Concepts RDF Dataset: (MLGT)"@en .


#################################################################
#    Annotation properties
#################################################################

###  http://purl.org/dc/terms/created
dcterms:created rdf:type owl:AnnotationProperty .
###  http://purl.org/dc/terms/issued
dcterms:issued rdf:type owl:AnnotationProperty .
###  http://purl.org/dc/terms/license
dcterms:license rdf:type owl:AnnotationProperty .
###  http://purl.org/dc/terms/modified
dcterms:modified rdf:type owl:AnnotationProperty .
###  http://purl.org/dc/terms/publisher
dcterms:publisher rdf:type owl:AnnotationProperty .
###  http://purl.org/vocab/vann/preferredNamespacePrefix
vann:preferredNamespacePrefix rdf:type owl:AnnotationProperty .
###  http://purl.org/vocab/vann/preferredNamespaceUri
vann:preferredNamespaceUri rdf:type owl:AnnotationProperty .


# ###  https://isotc211.geolexica.org/ld/geolexica#origin
# geolexica:origin rdf:type owl:AnnotationProperty .

# ###  https://isotc211.geolexica.org/ld/language#deu-note
# lang:deu-note rdf:type owl:AnnotationProperty .

# ###  https://isotc211.geolexica.org/ld/language#fra-note
# lang:fra-note rdf:type owl:AnnotationProperty .

# ###  https://isotc211.geolexica.org/ld/language#msa-note
# lang:msa-note rdf:type owl:AnnotationProperty .

# ###  https://isotc211.geolexica.org/ld/language#nld-note
# lang:nld-note rdf:type owl:AnnotationProperty .

#################################################################
#    Individuals
#################################################################

# ###  http://purl.org/dc/dcmitype/Dataset
# dctype:Dataset owl:sameAs void:Dataset .

###  http://vocab.deri.ie/void#Dataset

# ###  https://isotc211.geolexica.org/ld/concepts#
# <https://isotc211.geolexica.org/ld/concepts#> rdf:type owl:NamedIndividual ,
#                                                            dctype:Dataset .


###  https://isotc211.geolexica.org/ld/concepts#abbreviation
:abbreviation rdf:type owl:NamedIndividual ,
                       skos:Concept ;
              skos:inScheme geolexica:GeolexicaConceptScheme ;
              geolexica:hasInfo info:Info2 ;
              geolexica:hasLDAPI :abbreviation ,
                                 ldapi:ldapi2-json ,
                                 ldapi:ldapi2-jsonld ,
                                 ldapi:ldapi2-rdfxml ,
                                 ldapi:ldapi2-skosrdf ;
              geolexica:hasLangCode lang:ara ,
                                    lang:dan ,
                                    lang:deu ,
                                    lang:eng ,
                                    lang:kor ,
                                    lang:rus ,
                                    lang:spa ,
                                    lang:swe ;
              geolexica:hasReview reviews:Review2 ;
              dcterms:identifier 2 ;
              skos:notation 2 ;
              rdfs:label "abbreviation" ;
              skos:definition "benämning som skapats genom att ord eller bokstäver har utelämnats från en längre benämning och som står för samma begrepp som den längre benämningen"@sv ,
                              "betegnelse dannet ved at udelade ord eller bogstaver fra en længere form af et begreb som betegner det samme"@da ,
                              "designación formada por la omisión de palabras o letras de una denominación más larga y que designa al mismo concepto"@es ,
                              "designation formed by omitting words or letters from a longer form and designating the same concept"@en ,
                              "обозначение, образованное путём исключения слов или букв из более длинной формы и обозначающее  то же самое понятие"@ru ,
                              "دلالة تتشكل بعد حذف كلمات أو حروف من صيغة أطول وتدل عن نفس المفهوم"@ar ,
                              "축약하기 전의 용어와 동일한 개념을 나타내면서 글자 또는 단어를 생략한 용어"@ko ;
              skos:prefLabel "Abkürzung"@de ,
                             "abbreviation"@en ,
                             "abreviatura"@es ,
                             "forkortelse"@da ,
                             "förkortning"@sv ,
                             "аббревиатура"@ru ,
                             "اختصار"@ar ,
                             "약어"@ko ;
              geolexica:origin lang:araRegistry ,
                               lang:danRegistry ,
                               lang:deuRegistry ,
                               lang:engRegistry ,
                               lang:korRegistry ,
                               lang:rusRegistry ,
                               lang:spaRegistry ,
                               lang:sweRegistry ;
              lang:deu-note notes:DefnTransUnavail .


###  https://isotc211.geolexica.org/ld/concepts#abstract_test_case
:abstract_test_case rdf:type owl:NamedIndividual ,
                             skos:Concept ;
                    skos:inScheme geolexica:GeolexicaConceptScheme ;
                    geolexica:hasInfo info:Info3 ;
                    geolexica:hasLDAPI ldapi:ldapi3-json ,
                                       ldapi:ldapi3-jsonld ,
                                       ldapi:ldapi3-rdfxml ,
                                       ldapi:ldapi3-skosrdf ;
                    geolexica:hasLangCode lang:ara ,
                                          lang:dan ,
                                          lang:deu ,
                                          lang:eng ,
                                          lang:fin ,
                                          lang:fra ,
                                          lang:jpn ,
                                          lang:kor ,
                                          lang:rus ,
                                          lang:spa ,
                                          lang:swe ,
                                          lang:zho ;
                    geolexica:hasReview reviews:Review3 ;
                    dcterms:identifier 3 ;
                    skos:notation 3 ;
                    lang:ara-note "ملاحظة: حالة الاختبار التجريدي هي عبارة عن أساس منهجي لاشتقاق حالات اختبار قابلة للتطبيق. ويتم التعبير بشكل واضح ومقتضب عن غرض اختبار واحد أو أكثر في حالة الاختبار التجريدية. وتكون حالة الاختبار التجريدية مستقلة عن كل من التنفيذ والقيم. وينبغي أن تكون مكتملة بمعنى أن تشكل أساسا كافيا لإصدار حكم واضح وغير ملتبس مبني على نتيجة كل اختبار يتم إجراؤه ويخضع للملاحظة ( أي سلسلة الأحداث المتتالية للاختبار)"@ar ;
                    lang:dan-note "Bemærk til posten: Et abstrakt testforløb er et formelt grundlag for at kunne udvikle eksekverbare testforløb. Et eller flere testformål er samlet i det abstrakte testforløb. Et abstrakt testforløb er både uafhængigt af implementeringen og af værdierne. Testforløbet bør være fuldstændigt, dvs. tilstrækkeligt omfattende til at fremkomme med en testafgørelse, som kan knyttes utvetydigt til ethvert muligt testudfald (fx en sekvens af test events)."@da ;
                    lang:eng-note "Note to entry: An abstract test case is a formal basis for deriving executable test cases One or more test purposes are encapsulated in the abstract test case. An abstract test case is independent of both the implementation and the values. It should be complete in the sense that it is sufficient to enable a test verdict to be assigned unambiguously to each potentially observable test outcome (i.e. sequence of test events)."@en ;
                    lang:fin-note "HUOM.: Abstrakti testitapaus on suoritettavissa olevien testitapausten johtamisen muodollinen perusta. Abstraktiin testitapaukseen liittyy yksi tai useampi testaustarkoitus. Abstrakti testitapaus on toteutuksesta ja arvoista riippumaton. Abstraktin testitapauksen tulisi olla täydellinen, eli sen tulisi mahdollistaa yksikäsitteisen lausunnon (hyväksyntä/hylkäys) antaminen jokaiselle mahdollisesti havaittavalle testitulokselle (testitapahtumajonolle)."@fi ;
                    lang:jpn-note "備考： 抽象試験項目は，実行可能試験項目を導き出すための基礎として用いられる。抽象試験項目は，一つ以上の試験目的を含む。抽象試験項目は，実装及び値の両方から独立している。観測可能なすべての試験結果（試験中の一連の出力）に対して，あいまい性がなく試験判定を下すことができるという意味で，抽象試験項目は，完全であることが望ましい"@ja ;
                    lang:kor-note "비고: 추상 시험 케이스는 실행 가능 시험 케이스에 대한 형식적인 틀을 제공하며 하나 이상의 시험 목적을 갖는다. 추상 시험 케이스는 구현과 값의 양쪽에 모두 독립해 있다. 관측 가능한 모든 시험 결과는 시험 판정을 내릴 수 있도록 명확해야 한다(예: 시험 이벤트의 연속)"@ko ;
                    lang:rus-note "Примечание: Абстрактный тест является формальной основой для случаев исполняемого теста. Абстрактный тест не зависит ни от реализации объекта, ни от определенных значений. Абстрактный тест должен быть выполнен в таком объеме, чтобы по его итогам можно было подготовить непротиворечивое заключение для каждого потенциально возможного результата тестирования (т.е. последовательности шагов тестирования) "@ru ;
                    lang:spa-note "Nota: Una prueba genérica es una base formal para obtener pruebas ejecutables. Uno o más propósitos de prueba se encapsulan en una prueba genérica. Una prueba genérica es independiente tanto de la implementación como de los valores. Debería ser completa en el sentido de ser suficiente para permitir asignar inequívocamente un veredicto de prueba a cada resultado de la prueba potencialmente observable (es decir secuencia de eventos de ensayo)."@es ;
                    lang:zho-note "果（即：测试事件的序列）当中。"@zh ,
                                  "注： 抽象测试用例是导出可执行测试用例的形式化基础。在抽象测试用例里包含有一个或多个测试目的。一个抽象测试用例不取决于实现，也不取决于数值。它应当是完整的，足以将测试判定被明确地分配到每个潜在的可观察的测试结"@zh ;
                    rdfs:label "abstract test case" ;
                    skos:definition "generaliseret test for et bestemt krav"@da ,
                                    "generalized test for a particular requirement"@en ,
                                    "prueba generalizada para un requisito particular"@es ,
                                    "specifikation av de åtgärder som ska vidtas för att avgöra om ett visst krav är uppfyllt eller ej"@sv ,
                                    "test généralisé relatif à une exigence particulière"@fr ,
                                    "tietyn vaatimuksen täyttymistä mittaava yleistetty testi"@fi ,
                                    "обобщенный тест на соответствие конкретным требованиям"@ru ,
                                    "اختبار عام لمتطلب محدد"@ar ,
                                    "特定の要件のために作成された試験"@ja ,
                                    "针对特定要求的一般性测试。"@zh ,
                                    "특정한 요구 사항을 수행하기 위한 일반화된 시험"@ko ;
                    skos:prefLabel "abstract test case"@en ,
                                   "abstrakt testfall"@sv ,
                                   "abstrakt testforløb"@da ,
                                   "abstrakter Testfall"@de ,
                                   "abstrakti testitapaus"@fi ,
                                   "cas de test abstrait"@fr ,
                                   "prueba abstracta"@es ,
                                   "абстрактный тест"@ru ,
                                   "حالة اختبار تجريدي"@ar ,
                                   "抽象测试用例"@zh ,
                                   "抽象試験項目"@ja ,
                                   "추상 시험 케이스"@ko ;
                    geolexica:origin lang:araRegistry ,
                                     lang:danRegistry ,
                                     lang:deuRegistry ,
                                     lang:engRegistry ,
                                     lang:finRegistry ,
                                     lang:fraRegistry ,
                                     lang:jpnRegistry ,
                                     lang:korRegistry ,
                                     lang:rusRegistry ,
                                     lang:spaRegistry ,
                                     lang:sweRegistry ,
                                     lang:zhoRegistry ;
                    lang:deu-note notes:DefnTransUnavail ,
                                  notes:NoteTransUnavail ;
                    lang:swe-note notes:NoteTransUnavail .


###  https://isotc211.geolexica.org/ld/concepts#abstract_test_method
:abstract_test_method rdf:type owl:NamedIndividual ,
                               skos:Concept ;
                      skos:inScheme geolexica:GeolexicaConceptScheme ;
                      geolexica:hasInfo info:Info4 ;
                      geolexica:hasLDAPI ldapi:ldapi4-json ,
                                         ldapi:ldapi4-jsonld ,
                                         ldapi:ldapi4-rdfxml ,
                                         ldapi:ldapi4-skosrdf ;
                      geolexica:hasLangCode lang:ara ,
                                            lang:dan ,
                                            lang:deu ,
                                            lang:eng ,
                                            lang:fin ,
                                            lang:fra ,
                                            lang:jpn ,
                                            lang:kor ,
                                            lang:rus ,
                                            lang:spa ,
                                            lang:swe ,
                                            lang:zho ;
                      geolexica:hasReview reviews:Review4 ;
                      dcterms:identifier 4 ;
                      skos:notation 4 ;
                      rdfs:label "abstract test method" ;
                      skos:definition "method for testing implementation independent of any particular test procedure"@en ,
                                      "metode til at teste implementering uafhængigt af testprocedure"@da ,
                                      "méthode de test d&#39;implémentation indépendante de toute procédure de test"@fr ,
                                      "método para probar implementaciones independientemente de cualquier procedimiento de prueba particular"@es ,
                                      "testausmenettelystä riippumaton menetelmä toteutuksen testaamiseksi"@fi ,
                                      "testmetod som är oberoende oavsett typ av implementering"@sv ,
                                      "метод тестирования реализации, не зависящий от конкретной процедуры тестирования"@ru ,
                                      "طريقة لاختبار التنفيذ مستقلة عن أي إجراءات اختبار محددة"@ar ,
                                      "特定の試験手続から独立した実装の試験の方法。"@ja ,
                                      "用于实现测试的方法，它与特定测试过程无关。"@zh ,
                                      "특정 시험 절차와 상관 없이 독립적인 시험 구현을 위한 방법"@ko ;
                      skos:prefLabel "abstract test method"@en ,
                                     "abstrakt testmetode"@da ,
                                     "abstrakte Prüfmethode"@de ,
                                     "abstrakti testausmenetelmä"@fi ,
                                     "implementeringsoberoende testmetod"@sv ,
                                     "méthode de test abstrait"@fr ,
                                     "método de prueba abstracta"@es ,
                                     "метод абстрактного теста"@ru ,
                                     "طريقة اختبار تجريدي"@ar ,
                                     "抽象测试方法"@zh ,
                                     "抽象試験方法"@ja ,
                                     "추상 시험 방법"@ko ;
                      geolexica:origin lang:araRegistry ,
                                       lang:danRegistry ,
                                       lang:deuRegistry ,
                                       lang:engRegistry ,
                                       lang:finRegistry ,
                                       lang:fraRegistry ,
                                       lang:jpnRegistry ,
                                       lang:korRegistry ,
                                       lang:rusRegistry ,
                                       lang:spaRegistry ,
                                       lang:sweRegistry ,
                                       lang:zhoRegistry ;
                      lang:deu-note notes:DefnTransUnavail .


###  https://isotc211.geolexica.org/ld/concepts#abstract_test_module
:abstract_test_module rdf:type owl:NamedIndividual ,
                               skos:Concept ;
                      skos:inScheme geolexica:GeolexicaConceptScheme ;
                      geolexica:hasInfo info:Info5 ;
                      geolexica:hasLDAPI ldapi:ldapi5-json ,
                                         ldapi:ldapi5-jsonld ,
                                         ldapi:ldapi5-rdfxml ,
                                         ldapi:ldapi5-skosrdf ;
                      geolexica:hasLangCode lang:ara ,
                                            lang:dan ,
                                            lang:deu ,
                                            lang:eng ,
                                            lang:fin ,
                                            lang:fra ,
                                            lang:jpn ,
                                            lang:kor ,
                                            lang:rus ,
                                            lang:spa ,
                                            lang:swe ,
                                            lang:zho ;
                      geolexica:hasReview reviews:Review5 ;
                      dcterms:identifier 5 ;
                      skos:notation 5 ;
                      lang:ara-note "ملاحظة: الوحدات التكاملية المستقلة للاختبار التجريدي يمكن تعشيشها على نسق تسلسل هرمي"@ar ;
                      lang:dan-note "Bemærk til posten: Abstrakte testmoduler kan hænge hierarkisk sammen."@da ;
                      lang:eng-note "Note to entry: Abstract test modules may be nested in a hierarchical way."@en ;
                      lang:fin-note "HUOM.: Abstrakteja testausmoduuleja voi sijoittaa sisäkkäin hierarkkisesti."@fi ;
                      lang:jpn-note "備考： 抽象試験モジュールは，階層的な方法で，入れ子になってもよい。"@ja ;
                      lang:kor-note "비고: 추상 시험 모듈은 계층적 구조를 가질 수 있다."@ko ;
                      lang:rus-note "Примечание: Модули абстрактных тестов могут вкладываться друг в друга, образуя иерархическую структуру"@ru ;
                      lang:spa-note "Nota: Los módulos de pruebas genéricas pueden estar anidados de un modo jerárquico."@es ;
                      lang:zho-note "注： 抽象测试模块可以层次镶嵌。"@zh ;
                      rdfs:label "abstract test module" ;
                      skos:definition "conjunto de pruebas genéricas relacionadas entre sí"@es ,
                                      "ensemble de cas de test abstraits liés"@fr ,
                                      "joukko toisiinsa liittyviä abstrakteja testitapauksia"@fi ,
                                      "samling av samhörande abstrakta testfall"@sv ,
                                      "set of related abstract test cases"@en ,
                                      "sæt af forbundne abstrakte testforløb"@da ,
                                      "набор взаимосвязанных абстрактных тестов"@ru ,
                                      "مجموعة حالات اختبار تجريدي مرتبطة ببعضها"@ar ,
                                      "相关抽象测试用例的集合。"@zh ,
                                      "関係する抽象試験項目の集合。"@ja ,
                                      "관련된 추상 시험 케이스의 집합"@ko ;
                      skos:prefLabel "abstract test module"@en ,
                                     "abstrakt testmodul"@da ,
                                     "abstrakt testmodul"@sv ,
                                     "abstraktes  Prüfmodul"@de ,
                                     "abstrakti testausmoduuli"@fi ,
                                     "module de test abstrait"@fr ,
                                     "módulo de pruebas abstractas"@es ,
                                     "модуль  абстрактных тестов"@ru ,
                                     "نموذج اختبار تجريدي"@ar ,
                                     "抽象测试模块"@zh ,
                                     "抽象試験モジュール"@ja ,
                                     "추상 시험 모듈"@ko ;
                      geolexica:origin lang:araRegistry ,
                                       lang:danRegistry ,
                                       lang:deuRegistry ,
                                       lang:engRegistry ,
                                       lang:finRegistry ,
                                       lang:fraRegistry ,
                                       lang:jpnRegistry ,
                                       lang:korRegistry ,
                                       lang:rusRegistry ,
                                       lang:spaRegistry ,
                                       lang:sweRegistry ,
                                       lang:zhoRegistry ;
                      lang:deu-note notes:DefnTransUnavail ,
                                    notes:NoteTransUnavail ;
                      lang:swe-note notes:NoteTransUnavail .


###  https://isotc211.geolexica.org/ld/concepts#abstract_test_suite
:abstract_test_suite rdf:type owl:NamedIndividual ,
                              skos:Concept ;
                     skos:inScheme geolexica:GeolexicaConceptScheme ;
                     geolexica:hasInfo info:Info6 ;
                     geolexica:hasLDAPI ldapi:ldapi6-json ,
                                        ldapi:ldapi6-jsonld ,
                                        ldapi:ldapi6-rdfxml ,
                                        ldapi:ldapi6-skosrdf ;
                     geolexica:hasLangCode lang:ara ,
                                           lang:dan ,
                                           lang:deu ,
                                           lang:eng ,
                                           lang:fin ,
                                           lang:fra ,
                                           lang:jpn ,
                                           lang:kor ,
                                           lang:rus ,
                                           lang:spa ,
                                           lang:swe ,
                                           lang:zho ;
                     geolexica:hasReview reviews:Review6 ;
                     dcterms:identifier 6 ;
                     skos:notation 6 ;
                     geolexica:abbreviation "ATS"@da ,
                                            "ATS"@de ,
                                            "ATS"@en ,
                                            "ATS"@es ,
                                            "ATS"@ja ,
                                            "ATS"@ko ,
                                            "ATS"@sv ,
                                            "ATS"@zh ,
                                            "م ا ت"@ar ;
                     lang:ara-note "ملاحظة: توصف مجموعات الاختبار التجريدي في فقرة للمطابقة"@ar ;
                     lang:dan-note "Bemærk til posten: Abstrakte testsuiter er beskrevet i en overensstemmelsesklausul."@da ;
                     lang:eng-note "Note to entry: Abstract test suites are described in a conformance clause."@en ;
                     lang:fin-note "HUOM.: Abstraktit testisarjat on kuvattu vaatimuksenmukaisuuden määrittelyssä."@fi ;
                     lang:jpn-note "備考： 抽象試験項目群は，適合性の箇条において記述する。"@ja ;
                     lang:kor-note "비고: 추상 시험 스위트는 적합성 조항에서 기술되어 있다."@ko ;
                     lang:rus-note "Примечание: Комплексы абстрактных тестов описываются в разделе «Соответствие» международного стандарта"@ru ;
                     lang:spa-note "Nota: Los conjuntos de pruebas genéricas se describen en un capítulo de conformidad."@es ;
                     lang:zho-note "注： 抽象测试套件由一致性条款进行描述。"@zh ;
                     rdfs:label "abstract test suite" ;
                     skos:definition "abstract test module specifying all the requirements to be satisfied for conformance"@en ,
                                     "abstrakt testmodul, som specificerer alle krav, der skal opfyldes for, at der er overensstemmelse"@da ,
                                     "abstrakti testausmoduuli, jossa on määritelty kaikki laatuvaatimustason täyttymiseen edellytettävät vaatimukset"@fi ,
                                     "module de test abstrait spécifiant toutes les exigences de satisfaction par conformité"@fr ,
                                     "módulo de pruebas genéricas que especifica todos los requisitos que deben ser satisfechos para la conformidad"@es ,
                                     "samling abstrakta testfall som tillsammans kan avgöra om överensstämmelse råder med alla uppställda krav"@sv ,
                                     "тестовый модуль, определяющий все требования, которые должны быть удовлетворены для заключения о соответствии"@ru ,
                                     "نموذج اختبار تجريدي يحدد جميع المتطلبات اللازم تحقيقها للتطابق"@ar ,
                                     "満たされなければならないすべての要件を規定する抽象試験モジュール。"@ja ,
                                     "规定了实现一致性所要满足的全部要求的抽象测试模块。"@zh ,
                                     "적합성 시험에 요구되는 모든 사항들을 규정한 추상 시험 모듈"@ko ;
                     skos:prefLabel "abstract test suite"@en ,
                                    "abstrakt testsuite"@da ,
                                    "abstrakt testsvit"@sv ,
                                    "abstrakte Test-Suite"@de ,
                                    "abstrakti testisarja"@fi ,
                                    "conjunto de pruebas abstractas"@es ,
                                    "suite de tests abstraits"@fr ,
                                    "комплекс абстрактных тестов"@ru ,
                                    "مجموعة اختبار تجريدي"@ar ,
                                    "抽象测试套件"@zh ,
                                    "抽象試験項目群，ATS"@ja ,
                                    "추상 시험 스위트"@ko ;
                     geolexica:origin lang:araRegistry ,
                                      lang:danRegistry ,
                                      lang:deuRegistry ,
                                      lang:engRegistry ,
                                      lang:finRegistry ,
                                      lang:fraRegistry ,
                                      lang:jpnRegistry ,
                                      lang:korRegistry ,
                                      lang:rusRegistry ,
                                      lang:spaRegistry ,
                                      lang:sweRegistry ,
                                      lang:zhoRegistry ;
                     lang:deu-note notes:DefnTransUnavail ,
                                   notes:NoteTransUnavail ;
                     lang:swe-note notes:NoteTransUnavail .


###  https://isotc211.geolexica.org/ld/concepts#acceptance_testing
:acceptance_testing rdf:type owl:NamedIndividual ,
                             skos:Concept ;
                    skos:inScheme geolexica:GeolexicaConceptScheme ;
                    geolexica:hasInfo info:Info7 ;
                    geolexica:hasLDAPI ldapi:ldapi7-json ,
                                       ldapi:ldapi7-jsonld ,
                                       ldapi:ldapi7-rdfxml ,
                                       ldapi:ldapi7-skosrdf ;
                    geolexica:hasLangCode lang:ara ,
                                          lang:dan ,
                                          lang:deu ,
                                          lang:eng ,
                                          lang:fin ,
                                          lang:fra ,
                                          lang:jpn ,
                                          lang:kor ,
                                          lang:msa ,
                                          lang:rus ,
                                          lang:spa ,
                                          lang:swe ,
                                          lang:zho ;
                    dcterms:identifier 7 ;
                    skos:notation 7 ;
                    lang:ara-note "ملاحظة 1: هذا يشمل تخطيط وتنفيذ عدة أنواع من الاختبارات (مثل الاختبارات الوظيفية واختبارات الحجم واختبارات الأداء) التي تثبت أن التنفيذ يفي بجميع شروط ومتطلبات المستخدم"@ar ,
                                  "ملاحظة 2: هذا لا يشكل جزءا من اختبار المطابقة."@ar ;
                    lang:dan-note "Bemærk 1 til posten: Dette omfatter planlægning og gennemførelse af forskellige slags test (fx funktions-, volumen-, performancetest), som viser, at implementeringen opfylder brugerens krav."@da ,
                                  "Bemærk 2 til posten: Dette indgår ikke i overensstemmelsestest."@da ;
                    lang:eng-note "Note 1 to entry: This includes the planning and execution of several kinds of tests (e.g. functional, volume, performance tests) that demonstrate that the implementation satisfies the user requirements."@en ,
                                  "Note 2 to entry: This is not a part of conformance testing "@en ;
                    lang:fin-note "HUOM. 1: Hyväksymistestaukseen kuuluu monenlaisten käyttäjävaatimusten täyttymistä mittaavien testien (esim. toiminnallisuus-, kuormitus- ja suorituskykytestit) suunnittelua ja toteuttamista."@fi ,
                                  "HUOM. 2: Hyväksymistestaus ei kuulu vaatimuksenmukaisuuden testaukseen."@fi ;
                    lang:jpn-note "備考 1： 受入試験には，実装が利用者の要求を満たしていることを立証するための，種々の試験（機能性試験，数量試験，性能試験など）の計画及び実行が含まれる。"@ja ,
                                  "備考 2： 受入試験は，適合性試験の一部ではない。"@ja ;
                    lang:kor-note "비고 1: 사용자 요구 사항에 맞게 구현되는지를 시연하는 여러 종류의 시험(기능 시험, 용량 시험, 성능 시험 등)을 기획하고 실행하는 것이 검수 시험에 포함된다."@ko ,
                                  "비고 2: 검수 시험은 적합성 시험의 일부가 아니다."@ko ;
                    lang:rus-note "Примечание 1: Включает планирование и выполнение различных видов тестов, например, на функциональность, полноту, эффективность, которые показывают, удовлетворяет ли реализация требованиям пользователя"@ru ,
                                  "Примечание 2: Не является частью тестирования на соответствие"@ru ;
                    lang:spa-note "Nota 1: Esto incluye la planificación y ejecución de varias clases de pruebas (por ejemplo funcionales, de volumen, de desempeño) que demues¬tran que la implementación satisface los requisitos de usuario."@es ,
                                  "Nota 2: No es una parte de la prueba de conformidad."@es ;
                    lang:zho-note "注 1： 这个过程包括几种类型测试（例如：功能、容量、性能测试）的设计和执行，用来表明该实现是否满足的用户要求。"@zh ,
                                  "注 2： 验收测试不作为一致性测试的组成部分。"@zh ;
                    rdfs:label "acceptance testing (user)" ;
                    skos:definition "(用户)决定一个实现是否满足验收准则以及用户能否决定接受该实现的过程。"@zh ,
                                    "proces til bestemmelse af, om en implementering opfylder acceptance-kriterier og sætter brugeren i stand til at afgøre, om implementeringen skal accepteres"@da ,
                                    "proceso de determinación de si una implementación satisface o no los criterios de aceptación y permite al usuario determinar si acepta o no la implementación"@es ,
                                    "process of determining whether an implementation satisfies acceptance criteria and enables the user to determine whether to accept the implementation"@en ,
                                    "processus déterminant si une implémentation satisfait un critère d&#39;acceptation et permet à l&#39;utilisateur de déterminer s&#39;il accepte l&#39;implémentation"@fr ,
                                    "prosessi, jossa määritetään, täyttääkö toteutus hyväksyttävyyskriteerit ja jossa käyttäjälle annetaan mahdollisuus päättää toteutuksen hyväksymisestä"@fi ,
                                    "testning i syfte att bestämma om en implementering ska accepteras eller ej med hänsyn till användarnas behov och krav"@sv ,
                                    "процесс, позволяющий оценить, удовлетворяет ли реализация критериям приемлемости и дающий пользователю возможность вынести решение об этом"@ru ,
                                    "عملية تحديد ما إذا كان التنفيذ يحقق معيار القبول ويمكن المستخدم من قبول التنفيذ ."@ar ,
                                    "ある実装が利用者の受入基準を満たすかどうかを決定し，利用者がそれを受け入れるかどうかを判断するための試験。"@ja ,
                                    "구현된 결과가 검수 기준을 만족하는지에 대한 결정 과정"@ko ;
                    skos:prefLabel "Akzeptanzprüfung"@de ,
                                   "acceptance test (bruger)"@da ,
                                   "acceptance testing (user)"@en ,
                                   "acceptanstestning"@sv ,
                                   "hyväksymistestaus (käyttäjän)"@fi ,
                                   "prueba de aceptación (usuario)"@es ,
                                   "test d&#39;acceptation (utilisateur)"@fr ,
                                   "ujian penerimaan"@ms ,
                                   "тестирование на приемлемость для пользователя"@ru ,
                                   "اختبار القبول (المستخدم)"@ar ,
                                   "受入試験"@ja ,
                                   "验收测试(用户)"@zh ,
                                   "검수 시험(사용자)"@ko ;
                    geolexica:origin lang:araRegistry ,
                                     lang:danRegistry ,
                                     lang:deuRegistry ,
                                     lang:engRegistry ,
                                     lang:finRegistry ,
                                     lang:fraRegistry ,
                                     lang:jpnRegistry ,
                                     lang:korRegistry ,
                                     lang:msaRegistry ,
                                     lang:rusRegistry ,
                                     lang:spaRegistry ,
                                     lang:sweRegistry ,
                                     lang:zhoRegistry ;
                    lang:deu-note notes:DefnTransUnavail ,
                                  notes:NoteTransUnavail ;
                    lang:fra-note notes:NoteTransUnavail ;
                    lang:swe-note notes:NoteTransUnavail .


###  https://isotc211.geolexica.org/ld/concepts#accuracy
:accuracy rdf:type owl:NamedIndividual ,
                   skos:Concept ;
          skos:inScheme geolexica:GeolexicaConceptScheme ;
          geolexica:hasInfo info:Info8 ;
          geolexica:hasLDAPI ldapi:ldapi8-json ,
                             ldapi:ldapi8-jsonld ,
                             ldapi:ldapi8-rdfxml ,
                             ldapi:ldapi8-skosrdf ;
          geolexica:hasLangCode lang:ara ,
                                lang:dan ,
                                lang:eng ,
                                lang:fin ,
                                lang:fra ,
                                lang:jpn ,
                                lang:kor ,
                                lang:msa ,
                                lang:rus ,
                                lang:spa ,
                                lang:swe ,
                                lang:zho ;
          geolexica:hasReview reviews:Review8 ;
          dcterms:identifier 8 ;
          skos:notation 8 ;
          lang:ara-note "ملاحظة: نتيجة الاختبار يمكن أن تكون عملية مراقبة ورصد أو عملية قياس"@ar ;
          lang:dan-note "Bemærk til posten: Et testresultat kan være observationer eller målinger."@da ;
          lang:eng-note "A test result can be observations or measurements."@en ;
          lang:fin-note "HUOM.: Testitulos voi olla havainto tai mittaus."@fi ;
          lang:jpn-note "備考 1： 試験結果は，観測値又は測定値として得ることができる。"@ja ,
                        "備考 2： 参照値は，論議領域を実現するものとして採択された値である。"@ja ;
          lang:kor-note "비고: 시험 결과는 관측 값 또는 측정 값이 될 수 있다."@ko ;
          lang:rus-note "Примечание: Результат проверки может быть получен путем наблюдения или измерения"@ru ;
          lang:spa-note "Nota: Un resultado pueden ser observaciones o medidas"@es ;
          lang:swe-note "Anm. till termpost: Ibland talar man hellre om onoggrannhet istället för noggrannhet, om medelfelet ökar, ökar också onoggrannheten."@sv ;
          lang:zho-note "注： 测试结果可以是观测结果或量测结果。"@zh ;
          rdfs:label "accuracy" ;
          skos:definition "Nilai pengukuran yang sama atau menghampiri nilai kiraan atau jangkaan"@ms ,
                          "closeness of agreement between a test result and the accepted reference value"@en ,
                          "grad af overensstemmelse mellem et testresultat og den accepterede referenceværdi"@da ,
                          "graden av överensstämmelse mellan ett observerat, beräknat eller skattat värde och ett värde som betraktas som sant"@sv ,
                          "grado de acuerdo entre el resultado de una prueba y el valor de referencia aceptado"@es ,
                          "justesse de l&#39;accord entre un résultat de test et la valeur de référence"@fr ,
                          "testituloksen ja hyväksytyn viitearvon yhtäpitävyys"@fi ,
                          "близость результата проверки к принятому нормальному значению величины"@ru ,
                          "درجة اقتراب نتيجة الاختبار من القيمة المرجعية المعتمدة"@ar ,
                          "品質評価の試験結果得られた値と参照値との近さ。"@ja ,
                          "测试结果与公认的参考值间的接近程度。"@zh ,
                          "시험 결과와 기준 값 간의 일치도를 표시하는 척도"@ko ;
          skos:prefLabel "accuracy"@en ,
                         "exactitud"@es ,
                         "exactitude"@fr ,
                         "ketepatan"@ms ,
                         "noggrannhet"@sv ,
                         "nøjagtighed"@da ,
                         "ulkoinen tarkkuus"@fi ,
                         "точность"@ru ,
                         "الدقة"@ar ,
                         "准确度"@zh ,
                         "正確度"@ja ,
                         "정확도"@ko ;
          geolexica:origin lang:araRegistry ,
                           lang:danRegistry ,
                           lang:engRegistry ,
                           lang:finRegistry ,
                           lang:fraRegistry ,
                           lang:jpnRegistry ,
                           lang:korRegistry ,
                           lang:msaRegistry ,
                           lang:rusRegistry ,
                           lang:spaRegistry ,
                           lang:sweRegistry ,
                           lang:zhoRegistry ;
          lang:fra-note notes:NoteTransDiff ;
          lang:msa-note notes:NoteTransUnavail .


###  https://isotc211.geolexica.org/ld/concepts#actor
:actor rdf:type owl:NamedIndividual ,
                skos:Concept ;
       skos:inScheme geolexica:GeolexicaConceptScheme ;
       geolexica:hasInfo info:Info9 ;
       geolexica:hasLDAPI ldapi:ldapi9-json ,
                          ldapi:ldapi9-jsonld ,
                          ldapi:ldapi9-rdfxml ,
                          ldapi:ldapi9-skosrdf ;
       geolexica:hasLangCode lang:ara ,
                             lang:dan ,
                             lang:eng ,
                             lang:fin ,
                             lang:fra ,
                             lang:kor ,
                             lang:rus ,
                             lang:spa ,
                             lang:swe ,
                             lang:zho ;
       geolexica:hasReview reviews:Review9 ;
       dcterms:identifier 9 ;
       skos:notation 9 ;
       lang:ara-note "ملاحظة: نتيجة الاختبار يمكن أن تكون عملية مراقبة ورصد أو عملية قياس"@ar ;
       lang:dan-note "Bemærk til posten: Et testresultat kan være observationer eller målinger."@da ;
       lang:eng-note "Note to entry: A test result can be observations or measurements."@en ;
       lang:fin-note "HUOM.: Testitulos voi olla havainto tai mittaus."@fi ;
       lang:jpn-note "備考 1： 試験結果は，観測値又は測定値として得ることができる。"@ja ,
                     "備考 2： 参照値は，論議領域を実現するものとして採択された値である"@ja ;
       lang:kor-note "비고: 시험 결과는 관측 값 또는 측정 값이 될 수 있다."@ko ;
       lang:rus-note "Примечание: Результат проверки может быть получен путем наблюдения или измерения"@ru ;
       lang:spa-note "Nota: Un resultado pueden ser observaciones o medidas"@es ;
       lang:swe-note "Anm. till termpost: Ibland talar man hellre om onoggrannhet istället för noggrannhet, om medelfelet ökar, ökar också onoggrannheten."@sv ;
       lang:zho-note "注： 测试结果可以是观测结果或量测结果。"@zh ;
       rdfs:label "actor (UML)" ;
       skos:definition "(UML)当用例的用户与这些用例交互时，所扮演的相关角色的集合。"@zh ,
                       "coherent set of roles that users of use cases play when interacting with these use cases"@en ,
                       "conjunto coherente de roles que los usuarios de unos casos de uso jue gan cuando interaccionan con esos casos de uso"@es ,
                       "ensemble cohérent de rôles que les utilisateurs de cas d&#39;utilisation jouent en interagissant avec ces cas d&#39;utilisation"@fr ,
                       "något utanför ett system som växelverkar med systemet genom att delta i ett användningsfall"@sv ,
                       "sammenhængende sæt af roller, som brugere af use cases spiller i forhold til disse use cases"@da ,
                       "yhtenäinen joukko rooleja, joita käyttäjillä on käyttötapausten toiminnoissa"@fi ,
                       "множество логически связанных  ролей, выполняемых пользователями вариантов использования при взаимодействии с  ними"@ru ,
                       "مجموعة أدوار مترابطة منطقيا يقوم بها مستخدمو أدوات النمذجة عند التفاعل معها ."@ar ,
                       "유즈 케이스와 상호 작용 시, 그 유즈 케이스의 사용자가 수행하는 역할의 집합"@ko ;
       skos:prefLabel "Akteur (UML)"@de ,
                      "acteur (UML)"@fr ,
                      "actor (UML)"@en ,
                      "actor (UML)"@es ,
                      "aktör (UML)"@sv ,
                      "aktør (UML)"@da ,
                      "toimija (UML)"@fi ,
                      "действующее лицо (UML)"@ru ,
                      "لغة &quot;الممثل&quot; UML"@ar ,
                      "参与者(UML)"@zh ,
                      "행위자 (UML)"@ko ;
       geolexica:origin lang:araRegistry ,
                        lang:danRegistry ,
                        lang:engRegistry ,
                        lang:finRegistry ,
                        lang:fraRegistry ,
                        lang:korRegistry ,
                        lang:rusRegistry ,
                        lang:spaRegistry ,
                        lang:sweRegistry ,
                        lang:zhoRegistry ;
       lang:deu-note notes:DefnTransUnavail ,
                     notes:NoteTransUnavail ;
       lang:fra-note notes:NoteTransDiff ;
       lang:msa-note notes:NoteTransUnavail .


###  https://isotc211.geolexica.org/ld/concepts#admitted_term
:admitted_term rdf:type owl:NamedIndividual ,
                        skos:Concept ;
               skos:inScheme geolexica:GeolexicaConceptScheme ;
               geolexica:hasInfo info:Info10 ;
               geolexica:hasLDAPI ldapi:ldapi10-json ,
                                  ldapi:ldapi10-jsonld ,
                                  ldapi:ldapi10-rdfxml ,
                                  ldapi:ldapi10-skosrdf ;
               geolexica:hasLangCode lang:ara ,
                                     lang:dan ,
                                     lang:deu ,
                                     lang:eng ,
                                     lang:kor ,
                                     lang:rus ,
                                     lang:spa ,
                                     lang:swe ;
               geolexica:hasReview reviews:Review10 ;
               dcterms:identifier 10 ;
               skos:notation 10 ;
               rdfs:label "admitted term" ;
               skos:definition "term rated according to the scale of the term acceptability rating as a synonym for a preferred term"@en ,
                               "term som bedömts vara lämplig för ett visst begrepp och som används vid sidan av en rekommenderad term"@sv ,
                               "term, klassificeret efter en skala for tilladte termer, anvendt som synonym for en foretrukket term"@da ,
                               "término clasificado de acuerdo a la escala de aceptanción como un sinónimo de un término preferente"@es ,
                               "термин, оцененный по шкале рейтинга приемлемости термина как синоним предпочтительного термина"@ru ,
                               "مصطلح صنف وفقا لمقياس تصنيف قبول المصطلحات كمرادف للمصطلح المفضل"@ar ,
                               "상용 용어의 동의어로써 용어 수용가능성 등급체계에 의거하여 등급이 부여된 용어"@ko ;
               skos:prefLabel "admitted term"@en ,
                              "tilladt term"@da ,
                              "tillåten term"@sv ,
                              "término admitido"@es ,
                              "zugelassener Begriff"@de ,
                              "допустимый термин"@ru ,
                              "مصطلح معترف به"@ar ,
                              "승인 용어"@ko ;
               geolexica:origin lang:araRegistry ,
                                lang:danRegistry ,
                                lang:deuRegistry ,
                                lang:engRegistry ,
                                lang:korRegistry ,
                                lang:rusRegistry ,
                                lang:spaRegistry ,
                                lang:sweRegistry ;
               lang:deu-note notes:DefnTransUnavail .


###  https://isotc211.geolexica.org/ld/concepts#aggregation
:aggregation rdf:type owl:NamedIndividual ,
                      skos:Concept ;
             skos:inScheme geolexica:GeolexicaConceptScheme ;
             geolexica:hasInfo info:Info11 ;
             geolexica:hasLDAPI ldapi:ldapi11-json ,
                                ldapi:ldapi11-jsonld ,
                                ldapi:ldapi11-rdfxml ,
                                ldapi:ldapi11-skosrdf ;
             geolexica:hasLangCode lang:ara ,
                                   lang:dan ,
                                   lang:deu ,
                                   lang:eng ,
                                   lang:fin ,
                                   lang:fra ,
                                   lang:kor ,
                                   lang:rus ,
                                   lang:spa ,
                                   lang:swe ,
                                   lang:zho ;
             geolexica:hasReview reviews:Review11 ;
             dcterms:identifier 11 ;
             skos:notation 11 ;
             lang:ara-note "ملاحظة: أنظر التركيب"@ar ;
             lang:dan-note "Bemærk til posten: Se komposition"@da ;
             lang:eng-note "Note to entry: See composition"@en ;
             lang:fin-note "HUOM.: Katso vahva/aito kooste (composition)."@fi ;
             lang:kor-note "비고: 합성 참고"@ko ;
             lang:rus-note "Примечание: См. термин «композиция»"@ru ;
             lang:spa-note "Nota: Véase la composición"@es ;
             lang:zho-note "注： 参见组合。"@zh ;
             rdfs:label "aggregation (UML)" ;
             skos:altLabel "kokoelma (UML)"@fi ;
             skos:definition "(UML)关联的特殊形式，用以说明聚集(整体)与组成部分之间的整体-部分关系。"@zh ,
                             "assosiaation erityinen laji, joka määrittää kokonaisuuden (aggregaatin) ja sen osan välisen suhteen"@fi ,
                             "forma especial de asociación  que especifica una relación del todo con una parte entre el agregado (el todo) y una parte componente"@es ,
                             "forme spéciale d&#39;association qui spécifie une relation ensemble-composant entre l&#39;agrégat (ensemble) et la partie composante"@fr ,
                             "special form of association that specifies a whole-part relationship between the aggregate (whole) and a component part"@en ,
                             "special form of association that specifies a whole-part relationship between the aggregate (whole) and a component part"@sv ,
                             "særlig form for association, der specificerer et helhed-del-forhold mellem en klasse, som indtager rollen som helheden, og en eller flere klasser, som indtager rollen som del"@da ,
                             "особая форма ассоциации, описывающая отношение «целое-часть» между агрегатом («целое») и компонентом («часть»)"@ru ,
                             "شكل خاص من أشكال الترابط يصف علاقة &quot;الكل والجزء&quot; بين الكل والجزء المكون له."@ar ,
                             "집합체와 컴포넌트 간의 관계를 설명한 연관의 특정 형태"@ko ;
             skos:prefLabel "Aggregation (UML)"@de ,
                            "aggregation (UML)"@en ,
                            "aggregering"@sv ,
                            "aggregering (UML)"@da ,
                            "agregación (UML)"@es ,
                            "agrégation (UML)"@fr ,
                            "kooste (UML)"@fi ,
                            "агрегация (UML)"@ru ,
                            "تجميع (UML)"@ar ,
                            "聚合(UML)"@zh ,
                            "집합 연관 (UML)"@ko ;
             geolexica:origin lang:araRegistry ,
                              lang:danRegistry ,
                              lang:engRegistry ,
                              lang:finRegistry ,
                              lang:fraRegistry ,
                              lang:jpnRegistry ,
                              lang:korRegistry ,
                              lang:rusRegistry ,
                              lang:spaRegistry ,
                              lang:sweRegistry ,
                              lang:zhoRegistry ;
             lang:deu-note notes:DefnTransUnavail ,
                           notes:NoteTransUnavail ;
             lang:rus-note notes:NoteTransDiff ;
             lang:swe-note notes:NoteTransUnavail .


###  https://isotc211.geolexica.org/ld/concepts#altitude
:altitude rdf:type owl:NamedIndividual ,
                   skos:Concept ;
          skos:inScheme geolexica:GeolexicaConceptScheme ;
          geolexica:hasInfo info:Info12 ;
          geolexica:hasLDAPI ldapi:ldapi12-json ,
                             ldapi:ldapi12-jsonld ,
                             ldapi:ldapi12-rdfxml ,
                             ldapi:ldapi12-skosrdf ;
          geolexica:hasLangCode lang:ara ,
                                lang:dan ,
                                lang:deu ,
                                lang:eng ,
                                lang:fin ,
                                lang:fra ,
                                lang:kor ,
                                lang:msa ,
                                lang:rus ,
                                lang:spa ,
                                lang:swe ,
                                lang:zho ;
          geolexica:hasReview reviews:Review12 ;
          dcterms:identifier 12 ;
          skos:notation 12 ;
          geolexica:abbreviation "h or H"@en ,
                                 "h or H"@es ,
                                 "h or H"@sv ,
                                 "h or H"@zh ,
                                 "h; H"@fi ,
                                 "h; H"@ko ,
                                 "ع, ر"@ar ;
          lang:ara-note "ملاحظة 1: أنظر ارتفاع مجسم القطع الناقص والارتفاع المتصل بالجاذبية"@ar ,
                        "ملاحظة 2: ارتفاع نقطة تقع خارج السطح ويعامل كقيمة موجبة ؛ أما الارتفاع ذو القيمة السالبة فيصنف على أنه عمق."@ar ;
          lang:eng-note "Note 1 to entry: See ellipsoidal height and gravity-related height."@en ,
                        "Note 2 to entry: Height of a point outside the surface treated as positive; negative height is designated as depth."@en ;
          lang:fin-note "HUOM. 1: Katso myös ellipsoidinen korkeus ja painovoimaan perustuva korkeus."@fi ,
                        "HUOM. 2: Termillä korkeus viitataan pinnan yläpuolella olevan pisteen etäisyyteen pinnasta; negatiivista korkeutta nimitetään syvyydeksi."@fi ;
          lang:kor-note "비고 1: 타원체의 높이와 중력과 관련된 높이 참조"@ko ,
                        "비고 2: 양으로 여겨지는 표면 외부 지점의 높이, 음의 높이는 깊이라고 불린다."@ko ;
          lang:rus-note "Примечание 1: Высота точки, расположенная выше отсчетной поверхности, является положительной, а ниже нее – отрицательной"@ru ,
                        "Примечание 2: Высота точки над поверхностью считается положительной; отрицательная высота называется глубиной"@ru ;
          lang:spa-note "Nota 1: Véase altitud elipsoidal y altitud ligada a la gravedad."@es ,
                        "Nota 2: La altitud de un punto, sí es hacia el exterior de la superficie, se considera positiva; la altitud negativa se designa como profundidad."@es ;
          lang:zho-note "注 1： 参加椭球面高和重力高"@zh ,
                        "注 2： 向地表面外的高度视为正，相反的高度视为深度"@zh ;
          rdfs:label "altitude" ;
          skos:altLabel "altitud ortométrica"@es ,
                        "height"@ar ,
                        "height"@en ,
                        "height"@fr ,
                        "height"@ms ,
                        "height"@ru ,
                        "height"@sv ,
                        "height"@zh ;
          skos:definition "distance d&#39;un point à une surface de référence choisie, selon une ligne perpendiculaire à cette surface"@fr ,
                          "distance of a point from a chosen reference surface along a line perpendicular to that surface"@en ,
                          "distancia de un punto a una superficie de referencia escogida a lo largo de una línea perpendicular a esta superficie"@es ,
                          "höjd där den valda referensytan är världshavens medelvattenyta"@sv ,
                          "ketinggian sesuatu tempat (kawasan) yg biasanya diukur dr aras laut."@ms ,
                          "pisteen etäisyys valitusta vertauspinnasta kyseistä pintaa vastaan kohtisuorassa olevaa viivaa pitkin"@fi ,
                          "расстояние от отсчетной поверхности до выбранной точки по нормали к этой поверхности"@ru ,
                          "مسافة نقطة عن سطح إسناد مرجعي مختار على خط رأسي متعامد مع ذلك السطح"@ar ,
                          "地球自然表面点到所选择的参照面间的垂直距离"@zh ,
                          "선택된 기준면으로부터 그 면의 수직선으로 연결된 어떤 지점까지의 거리"@ko ;
          skos:prefLabel "Altitud"@ms ,
                         "altitud"@es ,
                         "altitud"@sv ,
                         "altitude"@en ,
                         "altitude"@fr ,
                         "korkeus"@fi ,
                         "высота"@ru ,
                         "الارتفاع"@ar ,
                         "海拔"@zh ,
                         "높이"@ko ;
          geolexica:origin geolexica:engRegistry ,
                           lang:araRegistry ,
                           lang:danRegistry ,
                           lang:finRegistry ,
                           lang:fraRegistry ,
                           lang:jpnRegistry ,
                           lang:korRegistry ,
                           lang:msaRegistry ,
                           lang:rusRegistry ,
                           lang:spaRegistry ,
                           lang:sweRegistry ,
                           lang:zhoRegistry ;
          lang:fra-note notes:NoteTransDiff ;
          lang:msa-note notes:NoteTransUnavail ;
          lang:swe-note notes:NoteTransUnavail .


###  https://isotc211.geolexica.org/ld/concepts#annotation
:annotation rdf:type owl:NamedIndividual ,
                     skos:Concept ;
            skos:inScheme geolexica:GeolexicaConceptScheme ;
            geolexica:hasInfo info:Info13 ;
            geolexica:hasLDAPI ldapi:ldapi13-json ,
                               ldapi:ldapi13-jsonld ,
                               ldapi:ldapi13-rdfxml ,
                               ldapi:ldapi13-skosrdf ;
            geolexica:hasLangCode lang:ara ,
                                  lang:dan ,
                                  lang:deu ,
                                  lang:eng ,
                                  lang:fin ,
                                  lang:fra ,
                                  lang:kor ,
                                  lang:msa ,
                                  lang:pol ,
                                  lang:rus ,
                                  lang:spa ,
                                  lang:swe ,
                                  lang:zho ;
            geolexica:hasReview reviews:Review13 ;
            dcterms:identifier 13 ;
            skos:notation 13 ;
            lang:ara-note "ملاحظة: الأرقام والحروف والرموز والعلامات كلها أمثلة للحاشية"@ar ;
            lang:dan-note "Bemærk til posten: Tal, bogstaver, symboler og signaturer er eksempler på annotation."@da ;
            lang:eng-note "Note to entry: Numbers, letters, symbols, and signs are examples of annotation"@en ;
            lang:fin-note "HUOM.: Viitemerkintöjä ovat esimerkiksi numerot, kirjaimet, symbolit ja merkit."@fi ;
            lang:kor-note "비고: 숫자, 문자, 기호 및 부호 등"@ko ;
            lang:pol-note "UWAGA: Przykładami adnotacji są liczby, litery, symbole i znak."@po ;
            lang:rus-note "Примечание: Примерами аннотаций служат цифры, буквы, обозначения и подписи"@ru ;
            lang:spa-note "Nota: son ejemplos de anotaciones los números, letras, símbolos y signos."@es ;
            lang:zho-note "注： 数字,字母,符号和标记是注记的例子。"@zh ;
            rdfs:label "annotation" ;
            skos:definition "any marking on illustrative material for the purpose of clarification"@en ,
                            "cualquier marca hecha en las ilustraciones con el objetivo de clarificar"@es ,
                            "jakiekolwiek oznaczenie na materiale ilustracyjnym, stosowane w celach wyjaśniających"@pl ,
                            "jede Kennzeichnung für illustrierendes Material zur Klarstellung"@de ,
                            "kort kommentar eller anteckning"@sv ,
                            "markering på illustrativt materiale med henblik på tydeliggørelse"@da ,
                            "mikä hyvänsä selvennykseksi tarkoitettu merkintä havainnollistavassa aineistossa"@fi ,
                            "nota atau catatan (sbg penerangan, komen dsb) yg ditambahkan pd teks penulisan sastera atau bahan bertulis yg lain."@ms ,
                            "note explicative sur un objet illustratif dans un but de clarification"@fr ,
                            "любые пояснительные метки, размещаемые на иллюстративном материале"@ru ,
                            "أي كتابة تكتب على مادة توضيحية بقصد التفسير والإيضاح"@ar ,
                            "以说明为目的，在诠释材料上作的标记。"@zh ,
                            "명시를 목적으로 해설 자료에 넣는 표기"@ko ;
            skos:prefLabel "Anmerkung"@de ,
                           "Anotasi"@ms ,
                           "adnotacja"@pl ,
                           "annotation"@da ,
                           "annotation"@en ,
                           "annotation"@fr ,
                           "annotation"@sv ,
                           "anotación"@es ,
                           "viitemerkintä"@fi ,
                           "аннотация"@ru ,
                           "حاشية"@ar ,
                           "注记"@zh ,
                           "주석"@ko ;
            geolexica:origin lang:araRegistry ,
                             lang:danRegistry ,
                             lang:deuRegistry ,
                             lang:engRegistry ,
                             lang:finRegistry ,
                             lang:fraRegistry ,
                             lang:korRegistry ,
                             lang:msaRegistry ,
                             lang:polRegistry ,
                             lang:rusRegistry ,
                             lang:spaRegistry ,
                             lang:sweRegistry ,
                             lang:zhoRegistry ;
            lang:deu-note notes:NoteTransUnavail ;
            lang:msa-note notes:NoteTransUnavail ;
            lang:rus-note notes:NoteTransDiff ;
            lang:swe-note notes:NoteTransUnavail .


###  https://isotc211.geolexica.org/ld/concepts#application
:application rdf:type owl:NamedIndividual ,
                      skos:Concept ;
             skos:inScheme geolexica:GeolexicaConceptScheme ;
             geolexica:hasInfo info:Info14 ;
             geolexica:hasLDAPI ldapi:ldapi14-json ,
                                ldapi:ldapi14-jsonld ,
                                ldapi:ldapi14-rdfxml ,
                                ldapi:ldapi14-skosrdf ;
             geolexica:hasLangCode lang:ara ,
                                   lang:dan ,
                                   lang:deu ,
                                   lang:eng ,
                                   lang:fin ,
                                   lang:fra ,
                                   lang:kor ,
                                   lang:msa ,
                                   lang:rus ,
                                   lang:spa ,
                                   lang:swe ,
                                   lang:zho ;
             geolexica:hasReview reviews:Review14 ;
             dcterms:identifier 14 ;
             skos:notation 14 ;
             rdfs:label "application" ;
             skos:altLabel "sovelma"@fi ;
             skos:definition "Be- und Verarbeitung von Daten zur Unterstützung von Nutzeranforderungen"@de ,
                             "hantering och bearbetning av data utifrån användarens behov"@sv ,
                             "ist atur cara atau program komputer yg direka khusus utk kegunaan tertentu"@ms ,
                             "manipulación y procesamiento de datos para satisfacer los requerimientos del usuario"@es ,
                             "manipulation and processing of data in support of user requirements"@en ,
                             "manipulation et traitement de données supportant des besoins d&#39;utilisateurs"@fr ,
                             "manipulation og behandling af data for at opfylde brugerkrav"@da ,
                             "tiedon käsittely ja prosessointi käyttäjävaatimusten mukaisesti"@fi ,
                             "манипулирование данными и их обработка с целью удовлетворения потребностей пользователя"@ru ,
                             "معالجة وتجهيز البيانات فيما يدعم متطلبات المستخدم"@ar ,
                             "支持用户需求的数据操作和处理。"@zh ,
                             "사용자 요구 사항의 지원을 위한 데이터의 조작 및 처리"@ko ;
             skos:prefLabel "Anwendung"@de ,
                            "Aplikasi"@ms ,
                            "aplicación"@es ,
                            "application"@en ,
                            "application"@fr ,
                            "applikation"@da ,
                            "applikation"@sv ,
                            "sovellus"@fi ,
                            "приложение"@ru ,
                            "تطبيق"@ar ,
                            "应用"@zh ,
                            "응용"@ko ;
             geolexica:origin lang:araRegistry ,
                              lang:danRegistry ,
                              lang:deuRegistry ,
                              lang:engRegistry ,
                              lang:finRegistry ,
                              lang:fraRegistry ,
                              lang:korRegistry ,
                              lang:msaRegistry ,
                              lang:rusRegistry ,
                              lang:spaRegistry ,
                              lang:sweRegistry ,
                              lang:zhoRegistry .


###  https://isotc211.geolexica.org/ld/concepts#application_schema
:application_schema rdf:type owl:NamedIndividual ,
                             skos:Concept ;
                    skos:inScheme geolexica:GeolexicaConceptScheme ;
                    geolexica:hasInfo info:Info15 ;
                    geolexica:hasLDAPI ldapi:ldapi15-json ,
                                       ldapi:ldapi15-jsonld ,
                                       ldapi:ldapi15-rdfxml ,
                                       ldapi:ldapi15-skosrdf ;
                    geolexica:hasLangCode lang:ara ,
                                          lang:dan ,
                                          lang:deu ,
                                          lang:eng ,
                                          lang:fin ,
                                          lang:fra ,
                                          lang:kor ,
                                          lang:msa ,
                                          lang:nld ,
                                          lang:rus ,
                                          lang:spa ,
                                          lang:swe ,
                                          lang:zho ;
                    geolexica:hasReview reviews:Review15 ;
                    dcterms:identifier 15 ;
                    skos:notation 15 ;
                    lang:rus-note "Примечание: Прикладная схема описывает содержимое, структуру и ограничения, накладываемые на информацию (4.22) в определенной области применения."@ru ;
                    rdfs:label "application schema" ;
                    skos:definition "conceptual schema for data required by one or more applications"@en ,
                                    "esquema conceptual de los datos requeridos por una o más aplicaciones"@es ,
                                    "formell beskrivning av den logiska strukturen"@sv ,
                                    "informatiemodel dat gegevens beschrijft die worden gebruikt door een of meer applicaties"@nl ,
                                    "konceptuel datamodel, der er nødvendig for en eller flere applikationer"@da ,
                                    "konzeptuelles Schema für Daten, das für eine oder mehrere Anwendungen erforderlich ist"@de ,
                                    "schéma conceptuel de données requis pour une ou plusieurs applications"@fr ,
                                    "skeema, joka kuvaa yhden tai useamman sovellusalan tarvitsemaa tietoa"@fi ,
                                    "skema konseptual bagi data yang diperlukan oleh satu atau lebih aplikasi"@ms ,
                                    "концептуальная схема для данных, которые требуются одному или  нескольким приложениям"@ru ,
                                    "مخطط تصوري للبيانات المطلوبة لتطبيق واحد أو أكثر"@ar ,
                                    "一个或多个应用所需数据的概念模式。"@zh ,
                                    "하나 이상의 응용에서 요구되는 데이터의 개념적 스키마"@ko ;
                    skos:prefLabel "Anwendungsschema"@de ,
                                   "Skema Aplikasi"@ms ,
                                   "applicatie schema"@nl ,
                                   "application schema"@en ,
                                   "applikationsmodel"@da ,
                                   "applikationsschema"@sv ,
                                   "esquema de aplicación"@es ,
                                   "schéma d&#39;application"@fr ,
                                   "sovellusskeema"@fi ,
                                   "схема приложения"@ru ,
                                   "مخطط التطبيق"@ar ,
                                   "应用模式"@zh ,
                                   "응용 스키마"@ko ;
                    geolexica:origin lang:araRegistry ,
                                     lang:danRegistry ,
                                     lang:deuRegistry ,
                                     lang:engRegistry ,
                                     lang:finRegistry ,
                                     lang:fraRegistry ,
                                     lang:korRegistry ,
                                     lang:msaRegistry ,
                                     lang:nldRegistry ,
                                     lang:rusRegistry ,
                                     lang:spaRegistry ,
                                     lang:sweRegistry ,
                                     lang:zhoRegistry .


###  https://isotc211.geolexica.org/ld/concepts#association
:association rdf:type owl:NamedIndividual ,
                      skos:Concept ;
             skos:inScheme geolexica:GeolexicaConceptScheme ;
             geolexica:hasInfo info:Info17 ;
             geolexica:hasLDAPI ldapi:ldapi17-json ,
                                ldapi:ldapi17-jsonld ,
                                ldapi:ldapi17-rdfxml ,
                                ldapi:ldapi17-skosrdf ;
             geolexica:hasLangCode lang:ara ,
                                   lang:dan ,
                                   lang:deu ,
                                   lang:eng ,
                                   lang:fin ,
                                   lang:fra ,
                                   lang:kor ,
                                   lang:rus ,
                                   lang:spa ,
                                   lang:swe ,
                                   lang:zho ;
             geolexica:hasReview reviews:Review17 ;
             dcterms:identifier 17 ;
             skos:notation 17 ;
             lang:ara-note "ملاحظة: الربط الثنائي هو عبارة عن ربط بين مصنِّفَيْن بالضبط ( ويشمل ذلك إمكانية الربط من مصنِّف إلى نفسه)"@ar ;
             lang:dan-note "Bemærk til posten: En binær association er en association imellem nøjagtig to klassifikatorer (inkl. muligheden for en association fra en klassifikator til sig selv)."@da ;
             lang:eng-note "Note to entry: A binary association is an association among exactly two classifiers (including the possibility of an association from a classifier to itself)."@en ;
             lang:fin-note "HUOM.: Binäärinen assosiaatio määrittää suhteen täsmälleen kahden luokittelijan välillä (mukaan lukien luokittelijan assosiaatiosuhde itseensä)."@fi ;
             lang:kor-note "비고: 이진 연관 관계는 정확하게 두 분류자 간의 연관 관계이다."@ko ;
             lang:rus-note "Примечание: Бинарная ассоциация является ассоциацией между двумя классификаторами, включая возможность ассоциации классификатора с самим собой"@ru ;
             lang:spa-note "Nota: son ejemplos de anotaciones los números, letras, símbolos y signos."@es ;
             lang:zho-note "注： 二元关联确指两个类元之间的关联（包括一个类元与其本身的关联）"@zh ;
             rdfs:label "association (UML);" ;
             skos:altLabel "assosiaatiosuhde (UML)"@fi ;
             skos:definition "(UML)两个或两个以上类之间的语义关系，定义了类中实例间的连接。"@zh ,
                             "UML-element som anger hur instanser kan eller ska referera till varandra"@sv ,
                             "kahden tai useamman luokittelijan välinen semanttinen suhde, joka määrittää luokittelijoiden mukaisten ilmentymien väliset yhteydet"@fi ,
                             "relación semántica entre dos o más clasificadores que especifica conexiones entre sus instancias"@es ,
                             "relation sémantique entre deux ou plusieurs classificateurs qui spécifient des connections parmi leurs instances"@fr ,
                             "semantic relationship between two or more classifiers that specifies connections among their instances"@en ,
                             "semantisk sammenhæng imellem to eller flere klassifikatorer, som specificerer forbindelser mellem deres instanser"@da ,
                             "семантическое отношение двух или более классификаторов, определяющее взаимосвязи между их экземплярами"@ru ,
                             "العلاقة اللغوية القائمة بين مصنِّفَيْن أو أكثر التي تحدد الترابط بين عناصرها"@ar ,
                             "인스턴스간의 연결을 규정하는 두 개 이상 분류자 간의 의미론적 관계"@ko ;
             skos:prefLabel "Relation (UML) (Synonym: Beziehung, Assoziation)"@de ,
                            "asociación (UML)"@es ,
                            "association (UML)"@da ,
                            "association (UML)"@en ,
                            "association (UML)"@fr ,
                            "assosiaatio (UML)"@fi ,
                            "samband (UML)"@sv ,
                            "ассоциация (UML)"@ru ,
                            "ارتباط UML"@ar ,
                            "关联(UML)"@zh ,
                            "연관 (UML)"@ko ;
             geolexica:origin lang:araRegistry ,
                              lang:danRegistry ,
                              lang:deuRegistry ,
                              lang:engRegistry ,
                              lang:finRegistry ,
                              lang:fraRegistry ,
                              lang:korRegistry ,
                              lang:rusRegistry ,
                              lang:spaRegistry ,
                              lang:sweRegistry ,
                              lang:zhoRegistry ;
             lang:deu-note notes:DefnTransUnavail ,
                           notes:NoteTransUnavail ;
             lang:swe-note notes:NoteTransUnavail .


###  https://isotc211.geolexica.org/ld/concepts#attitude
:attitude rdf:type owl:NamedIndividual ,
                   skos:Concept ;
          skos:inScheme geolexica:GeolexicaConceptScheme ;
          geolexica:hasInfo info:Info18 ;
          geolexica:hasLDAPI ldapi:ldapi18-json ,
                             ldapi:ldapi18-jsonld ,
                             ldapi:ldapi18-rdfxml ,
                             ldapi:ldapi18-skosrdf ;
          geolexica:hasLangCode lang:ara ,
                                lang:dan ,
                                lang:deu ,
                                lang:eng ,
                                lang:fin ,
                                lang:fra ,
                                lang:kor ,
                                lang:msa ,
                                lang:rus ,
                                lang:spa ,
                                lang:swe ,
                                lang:zho ;
          geolexica:hasReview reviews:Review18 ;
          dcterms:identifier 18 ;
          skos:notation 18 ;
          lang:ara-note "ملاحظة: في خدمات تحديد المواقع ، يشير هذا عادة إلى اتجاه قواعد أداء المعدات لدى المستخدم مثل الطائرة ، أو المركب (قارب) أو السيارة"@ar ;
          lang:dan-note "Bemærk til posten: I stedsbestemmelsestjenester er dette normalt orienteringen af brugerens platform, såsom et luftfartøj, en båd eller en bil."@da ;
          lang:eng-note "Note to entry: In positioning services, this is usually the orientation of the user's platform, such as an aircraft, boat, or automobile."@en ;
          lang:fin-note "HUOM.: Paikannuspalveluissa termillä suuntaus viitataan tavallisesti käyttäjän alustan, esimerkiksi lentokoneen, laivan tai auton, suuntaan."@fi ;
          lang:kor-note "비고: 측위 서비스의 경우, 보통 항공기, 배, 자동차 등 사용자 플랫폼의 방향을 의미한다."@ko ;
          lang:rus-note "Примечание: В системах позиционирования это обычно ориентация платформы пользователя, например, самолета, судна или автомобиля"@ru ;
          lang:zho-note "注： 在定位服务中，这通常是指用户平台（如：飞行器、轮船或汽车）的定向。"@zh ;
          rdfs:label "attitude" ;
          skos:definition "(vid positionering) riktning hos ett objekt, beskrivet som vinklar mellan axlarna hos objektets interna koordinatsystem och axlarna i ett valt referenssystem"@sv ,
                          "kappaleen suunta, joka on ilmaistu kappaleen paikallisen koordinaatiston akseleiden ja ulkoisen koordinaatiston akseleiden välisten kulmien avulla"@fi ,
                          "orientación de un cuerpo, descrita mediante los ángulos entre los ejes del sistema de coordenadas del cuerpo y los ejes de un sistema de coordenadas externo"@es ,
                          "orientation d&#39;un objet décrite par les angles entre les axes du système de coordonnées de cet objet et les axes du système de coordonnées externe"@fr ,
                          "orientation of a body, described by the angles between the axes of that body&#39;s coordinate system and the axes of an external coordinate system"@en ,
                          "orientering af et legeme beskrevet ved vinklerne mellem akserne i legemets koordinatsystem og akserne i et eksternt koordinatsystem"@da ,
                          "perbuatan atau pandangan yg berdasarkan sesuatu pendapat"@ms ,
                          "ориентация тела, описываемая углами между осями его [собственной] системы координат и осями внешней системы координат"@ru ,
                          "اتجاه جسم ما كما تصفه الزوايا التي بين محاور نظام إحداثيات ذلك الجسم ومحاور نظام إحداثيات خارجي آخر"@ar ,
                          "一个物体的定向，由物体坐标系的轴和外部坐标系的轴之间的夹角来描述。"@zh ,
                          "물체의 좌표 체계 축과 외부 좌표 체계 축 사이의 각도를 통해 기술되는 물체의 방향"@ko ;
          skos:prefLabel "Einstellung"@de ,
                         "actitud"@es ,
                         "attitude"@en ,
                         "attitude"@fr ,
                         "attityd"@sv ,
                         "sikap"@ms ,
                         "suuntaus"@fi ,
                         "ydre orientering"@da ,
                         "пространственное положение"@ru ,
                         "الوضع"@ar ,
                         "姿态"@zh ,
                         "자세"@ko ;
          geolexica:origin lang:araRegistry ,
                           lang:danRegistry ,
                           lang:deuRegistry ,
                           lang:engRegistry ,
                           lang:finRegistry ,
                           lang:fraRegistry ,
                           lang:korRegistry ,
                           lang:msaRegistry ,
                           lang:rusRegistry ,
                           lang:spaRegistry ,
                           lang:sweRegistry ,
                           lang:zhoRegistry ;
          lang:deu-note notes:DefnTransUnavail ,
                        notes:NoteTransUnavail ;
          lang:msa-note notes:NoteTransUnavail ;
          lang:swe-note notes:NoteTransUnavail .


###  https://isotc211.geolexica.org/ld/concepts#attribute
:attribute rdf:type owl:NamedIndividual ,
                    skos:Concept ;
           skos:inScheme geolexica:GeolexicaConceptScheme ;
           geolexica:hasInfo info:Info19 ;
           geolexica:hasLDAPI ldapi:ldapi19-json ,
                              ldapi:ldapi19-jsonld ,
                              ldapi:ldapi19-rdfxml ,
                              ldapi:ldapi19-skosrdf ;
           geolexica:hasLangCode lang:ara ,
                                 lang:deu ,
                                 lang:eng ,
                                 lang:kor ,
                                 lang:msa ,
                                 lang:nld ,
                                 lang:rus ,
                                 lang:spa ,
                                 lang:swe ;
           geolexica:hasReview reviews:Review19 ;
           dcterms:identifier 19 ;
           skos:notation 19 ;
           lang:ara-note "ملاحظة: عبارة عن وصف لخاصية هندسية ، أو طوبولوجية ، أو موضوعية أو أي خاصية أخرى للكيان المعني."@ar ;
           lang:eng-note "Note to entry: Describes a geometrical, topological, thematic, or other characteristic of an entity"@en ;
           lang:rus-note "Примечание: Описывает геометрическую, топологическую, тематическую и другие характеристики сущности"@ru ;
           lang:spa-note "Nota: Describe una característica geométrica, topológica, temática o cualquier otra característica de una entidad"@es ;
           lang:zho-note "注： 在定位服务中，这通常是指用户平台（如：飞行器、轮船或汽车）的定向。"@zh ;
           rdfs:label "attribute" ;
           skos:definition "benannte Eigenschaft einer Einheit"@de ,
                           "ciri-ciri bagi sesuatu fitur"@ms ,
                           "kenmerk van een geo-object"@nl ,
                           "named property of an entity"@en ,
                           "namngiven egenskap hos objekt"@sv ,
                           "nombre de una propiedad de una entidad"@es ,
                           "именованное свойство сущности"@ru ,
                           "اسم خاصية لكيان ما"@ar ,
                           "실체의 속성"@ko ;
           skos:prefLabel "Attribut"@de ,
                          "atribut"@ms ,
                          "atributo"@es ,
                          "attribut"@sv ,
                          "attribute"@en ,
                          "attribuut"@nl ,
                          "атрибут"@ru ,
                          "صفة"@ar ,
                          "속성"@ko ;
           geolexica:origin lang:araRegistry ,
                            lang:deuRegistry ,
                            lang:engRegistry ,
                            lang:korRegistry ,
                            lang:msaRegistry ,
                            lang:nldRegistry ,
                            lang:rusRegistry ,
                            lang:spaRegistry ,
                            lang:sweRegistry ;
           lang:deu-note notes:NoteTransUnavail ;
           lang:kor-note notes:NoteTransUnavail ;
           lang:msa-note notes:NoteTransUnavail ;
           lang:nld-note notes:NoteTransUnavail ;
           lang:swe-note notes:NoteTransUnavail .


###  https://isotc211.geolexica.org/ld/concepts#attributeUML
:attributeUML rdf:type owl:NamedIndividual ,
                       skos:Concept ;
              skos:inScheme geolexica:GeolexicaConceptScheme ;
              geolexica:hasInfo info:Info20 ;
              geolexica:hasLDAPI ldapi:ldapi20-json ,
                                 ldapi:ldapi20-jsonld ,
                                 ldapi:ldapi20-rdfxml ,
                                 ldapi:ldapi20-skosrdf ;
              geolexica:hasLangCode lang:ara ,
                                    lang:dan ,
                                    lang:eng ,
                                    lang:fin ,
                                    lang:fra ,
                                    lang:kor ,
                                    lang:nld ,
                                    lang:rus ,
                                    lang:spa ,
                                    lang:swe ,
                                    lang:zho ;
              geolexica:hasReview reviews:Review20 ;
              dcterms:identifier 20 ;
              skos:notation 20 ;
              lang:ara-note "ملاحظة 1: الصفة لغة تعادل ربط التركيب ؛ ولكن المقصد والاستخدام يختلفان دائما"@ar ,
                            "ملاحظة 2: استخدم مصطلح (معلم) في هذا التعريف بمعناه المعتمد في اللغة الموحَّدة للنمذجة UML وهو مختلف عن تعريفه المنصوص عليه في الفقرة 4-1 من هذه المواصفة الفنية."@ar ;
              lang:dan-note "Bemærk til posten: En attribut svarer semantisk til en sammensætningsassociation; men formål og anvendelse er normalt forskellig fra denne."@da ;
              lang:eng-note "Note 1 to entry: An attribute is semantically equivalent to a composition association; however, the intent and usage is normally different."@en ,
                            "Note 2 to entry:-Feature- used in this definition is the UML meaning of the term and is not meant as defined in 4.1 of this Technical Specification. "@en ;
              lang:kor-note "비고 1: 속성은 의미적으로 합성 연관과 동일하다. 그러나 의미와 용법은 일반적으로 다르다."@ko ,
                            "비고 2: 정의에 사용된 “특성(Feature)”은 KS X ISO 19103에 정의된 의미가 아닌 UML 용어이다."@ko ;
              lang:rus-note "Примечание 1: Атрибут семантически эквивалентен ассоциации композиции, однако их содержание и использование обычно различаются"@ru ,
                            "Примечание 2: -Объект-, исходя из этого определения, это объект в терминологии UML."@ru ;
              lang:spa-note "Nota 1: Un atributo es semánticamente equivalente a una asociación de composición; sin embargo, la intención y el uso normalmente es diferente."@es ,
                            "Nota 2: -Aspecto- tal y como se ha usado en esta definición, tiene el significado UML del término y no aquel definido en el apartado 4.1 de esta Especificación Técnica."@es ;
              lang:zho-note "注 1： 一个属性语义上等同于一个组合关联，但是，目的和用途是不同的。"@zh ,
                            "注 2： 该定义使用的“特性（feature)”是UML的术语含义，不是本技术规范第4.1章定义的含义。"@zh ;
              rdfs:label "attribute (UML)" ;
              skos:altLabel "määrite (UML)"@fi ;
              skos:definition "aspecto dentro de un clasificador, que describe un rango de valores que las instancias del clasificador pueden tener"@es ,
                              "caractéristique d&#39;un classificateur décrivant une gamme de valeurs que les instances du classificateur peuvent avoir"@fr ,
                              "egenskab ved en klassifikator, der beskriver en række værdier, som instanser af klassifikatoren kan indeholde"@da ,
                              "element binnen een objecttype waarmee waarden worden beschreven die instanties van het object kunnen hebben"@nl ,
                              "feature within a classifier that describes a range of values that instances of the classifier may hold"@en ,
                              "kombination av en attributtyp och ett attributvärde, knutet till ett visst objekt"@sv ,
                              "luokittelijaan sisältyvä piirre, joka määrittelee niiden arvojen joukon, joita luokittelijan ilmentymät voivat saada"@fi ,
                              "свойство в классификаторе, описывающее множество значений, которые могут принимать экземпляры данного классификатора"@ru ,
                              "ميزة المصنِّف التي تصف نطاق من القيم التي يمكن لعناصر ذلك المصنِّف أن تحملها"@ar ,
                              "类元的特性，描述该类元的实例可能有的值的范围。"@zh ,
                              "분류자의 특성으로 분류자의 인스턴스가 가질 수 있는 값의 범위를 기술"@ko ;
              skos:prefLabel "Attribut (UML)"@de ,
                             "UML-attribut"@sv ,
                             "atributo (UML)"@es ,
                             "attribut (UML)"@da ,
                             "attribut (UML)"@fr ,
                             "attribute (UML)"@en ,
                             "attribuut (UML)"@nl ,
                             "attribuutti (UML)"@fi ,
                             "атрибут(UML)"@ru ,
                             "صفة (UML)"@ar ,
                             "属性(UML)"@zh ,
                             "속성 (UML)"@ko ;
              geolexica:origin lang:araRegistry ,
                               lang:danRegistry ,
                               lang:deuRegistry ,
                               lang:engRegistry ,
                               lang:finRegistry ,
                               lang:fraRegistry ,
                               lang:korRegistry ,
                               lang:nldRegistry ,
                               lang:rusRegistry ,
                               lang:spaRegistry ,
                               lang:sweRegistry ,
                               lang:zhoRegistry ;
              lang:deu-note notes:DefnTransUnavail ,
                            notes:NoteTransUnavail ;
              lang:kor-note notes:NoteTransUnavail ;
              lang:nld-note notes:NoteTransUnavail ;
              lang:rus-note notes:NoteTransDiff ;
              lang:swe-note notes:NoteTransUnavail .


###  https://isotc211.geolexica.org/ld/concepts#bag
:bag rdf:type owl:NamedIndividual ,
              skos:Concept ;
     skos:inScheme geolexica:GeolexicaConceptScheme ;
     geolexica:hasInfo info:Info24 ;
     geolexica:hasLDAPI ldapi:ldapi24-json ,
                        ldapi:ldapi24-jsonld ,
                        ldapi:ldapi24-rdfxml ,
                        ldapi:ldapi24-skosrdf ;
     geolexica:hasLangCode lang:ara ,
                           lang:dan ,
                           lang:eng ,
                           lang:fin ,
                           lang:fra ,
                           lang:kor ,
                           lang:nld ,
                           lang:rus ,
                           lang:spa ,
                           lang:swe ,
                           lang:zho ;
     geolexica:hasReview reviews:Review24 ;
     dcterms:identifier 24 ;
     skos:notation 24 ;
     lang:ara-note "ملاحظة: منطقيا ، الحقيبة هي عبارة عن مجموعة مكونة من أزواج < البند ، الإحصاء>"@ar ;
     lang:dan-note "Bemærk til posten: Logisk set er en samling organiseret i par <element, antal>"@da ;
     lang:eng-note "Note to entry: Logically, a bag is a set of pairs <item, count>."@en ;
     lang:fin-note "HUOM.: Monijoukkoa voidaan loogisesti kuvata parien <tietokohde, lukumäärä> joukkona."@fi ;
     lang:jpn-note "備考： 論理的には，多重集合は，＜項目，項数＞の対の集合である。"@ja ;
     lang:kor-note "비고: 논리적으로 다중 집합은 <항목, 수>쌍의 집합이다."@ko ;
     lang:pol-note "UWAGA: W sensie logicznym wielozbiór można uważać za kolekcję par typu <element, krotność tego elementu w kolekcji>."@po ;
     lang:rus-note "Примечание: Логически, мультимножество – это набор пар < item, count >."@ru ;
     lang:spa-note "Nota: Lógicamente, una bolsa es un conjunto de pares <item, contador>"@es ;
     lang:zho-note "注： 逻辑上，包是<项,数目>对的集合。"@zh ;
     rdfs:label "bag" ;
     skos:altLabel "백"@ko ;
     skos:definition "bekas utk mengisi, menyimpan atau membawa pakaian, surat, buku, dll yg dibuat drpd kulit dll"@ms ,
                     "colección finita y desordenada de ítems relacionados (objetos o valores) que pueden estar repetidos"@es ,
                     "collection limitée et non-ordonnée d&#39;éléments liés (objets ou valeurs) pouvant être répétés"@fr ,
                     "finit, uordnet samling af beslægtede elementer (objekter eller værdier), som kan gentages"@da ,
                     "finite, unordered collection of related items (objects or values) that may be repeated"@en ,
                     "oordnad, ändlig mängd av samhörande data"@sv ,
                     "skończona, nieuporządkowana kolekcja powiązanych pozycji (obiektów lub wartości), które mogą się powtarzać"@pl ,
                     "äärellinen, järjestämätön kokoelma yhteenliittyviä tietokohteita (objekteja tai arvoja), jotka voivat toistua"@fi ,
                     "конечная неупорядоченная совокупность элементов (объектов или значений), в которой  допускается их повторение"@ru ,
                     "مجموعة محدودة غير مرتبة من البنود (كيانات أو قيم) ذات ارتباط ببعضها ويمكن تكرارها"@ar ,
                     "可以重复的相关项（对象或值）的有限、无序的集合。"@zh ,
                     "繰返しのある，関連する項目（オブジェクト又は値）の，有限非順序な集まり。"@ja ,
                     "유한하며 순서가 없는, 반복 가능한 항목(객체 또는 값)의 모음"@ko ;
     skos:prefLabel "Multimenge"@de ,
                    "bag"@en ,
                    "bag"@sv ,
                    "beg"@ms ,
                    "bolsa"@es ,
                    "monijoukko"@fi ,
                    "multimængde"@da ,
                    "sac"@fr ,
                    "wielozbiór"@pl ,
                    "мультимножество"@ru ,
                    "مجموعة"@ar ,
                    "包"@zh ,
                    "多重集合"@ja ,
                    "다중 집합"@ko ;
     geolexica:origin lang:araRegistry ,
                      lang:danRegistry ,
                      lang:deuRegistry ,
                      lang:engRegistry ,
                      lang:finRegistry ,
                      lang:fraRegistry ,
                      lang:jpnRegistry ,
                      lang:korRegistry ,
                      lang:msaRegistry ,
                      lang:polRegistry ,
                      lang:rusRegistry ,
                      lang:spaRegistry ,
                      lang:sweRegistry ,
                      lang:zhoRegistry ;
     lang:deu-note notes:DefnTransUnavail ,
                   notes:NoteTransUnavail ;
     lang:msa-note notes:NoteTransUnavail ;
     lang:nld-note notes:NoteTransUnavail ;
     lang:swe-note notes:NoteTransUnavail .


###  https://isotc211.geolexica.org/ld/concepts#base_standard
:base_standard rdf:type owl:NamedIndividual ,
                        skos:Concept ;
               skos:inScheme geolexica:GeolexicaConceptScheme ;
               geolexica:hasInfo info:Info26 ;
               geolexica:hasLDAPI ldapi:ldapi26-json ,
                                  ldapi:ldapi26-jsonld ,
                                  ldapi:ldapi26-rdfxml ,
                                  ldapi:ldapi26-skosrdf ;
               geolexica:hasLangCode lang:ara ,
                                     lang:dan ,
                                     lang:eng ,
                                     lang:fin ,
                                     lang:fra ,
                                     lang:kor ,
                                     lang:rus ,
                                     lang:spa ,
                                     lang:swe ,
                                     lang:zho ;
               dcterms:identifier 26 ;
               skos:notation 26 ;
               rdfs:label "base standard" ;
               skos:definition "ISO geographic information standard or other information technology standard that is used as a source from which a profile may be constructed"@en ,
                               "SO geografisk informations-standard eller anden informationsteknologisk standard, der er udgivet som en kilde, hvorfra der kan opbygges en profil"@da ,
                               "norma ISO de información geográfica, u otra norma de tecnologías de la información, que se puede utilizar como fuente a partir de la cual es posible construir un perfil"@es ,
                               "norme d&#39;information géographique ISO ou autre norme de technologie de l&#39;information publiée comme une source et à partir de laquelle un profil peut être construit"@fr ,
                               "paikkatietoa koskeva ISO-standardi tai muu tietotekniikkastandardi, jota voidaan käyttää profiilin laatimisen perustana"@fi ,
                               "standard som har ett brett syfte eller innehåller allmänna bestämmelser för ett visst område"@sv ,
                               "стандарт ISO из серии  «Географическая информация» или другой технологический стандарт, который может служить источником для разработки профиля"@ru ,
                               "مواصفة قياسية للمعلومات الجغرافية ( ISO ) أو مواصفة قياسية لتقنية المعلومات والتي صدرت كمصدر يمكن إنشاء مواصفة محددة منه"@ar ,
                               "能够用于构建专用标准的ISO地理信息标准或其他信息技术标准。"@zh ,
                               "하나의 프로파일을 구성하는 데 활용될 수 있는 KS(ISO) 지리 정보 표준 또는 이외의 정보 기술 표준"@ko ;
               skos:prefLabel "Basisstandard"@de ,
                              "base standard"@en ,
                              "basisstandard"@da ,
                              "grundstandard"@sv ,
                              "norma base"@es ,
                              "norme de base"@fr ,
                              "perusstandardi"@fi ,
                              "базовый стандарт"@ru ,
                              "مواصفة قياسية أساسية"@ar ,
                              "基础标准"@zh ,
                              "기반 표준"@ko ;
               geolexica:origin lang:araRegistry ,
                                lang:danRegistry ,
                                lang:deuRegistry ,
                                lang:engRegistry ,
                                lang:finRegistry ,
                                lang:fraRegistry ,
                                lang:korRegistry ,
                                lang:rusRegistry ,
                                lang:spaRegistry ,
                                lang:sweRegistry ,
                                lang:zhoRegistry ;
               lang:deu-note notes:DefnTransUnavail ;
               lang:fra-note notes:NoteTransDiff .


###  https://isotc211.geolexica.org/ld/concepts#basic_test
:basic_test rdf:type owl:NamedIndividual ,
                     skos:Concept ;
            skos:inScheme geolexica:GeolexicaConceptScheme ;
            geolexica:hasInfo info:Info27 ;
            geolexica:hasLDAPI ldapi:ldapi27-json ,
                               ldapi:ldapi27-jsonld ,
                               ldapi:ldapi27-rdfxml ,
                               ldapi:ldapi27-skosrdf ;
            geolexica:hasLangCode lang:ara ,
                                  lang:dan ,
                                  lang:eng ,
                                  lang:fin ,
                                  lang:fra ,
                                  lang:jpn ,
                                  lang:kor ,
                                  lang:rus ,
                                  lang:spa ,
                                  lang:swe ,
                                  lang:zho ;
            geolexica:hasReview reviews:Review27 ;
            dcterms:identifier 27 ;
            skos:notation 27 ;
            rdfs:label "basic test" ;
            skos:definition "aluksi suoritettava kelpoisuustesti, jonka tarkoituksena on tunnistaa tapaukset, joissa vaatimuksenmukaisuusehdot eivät selvästi täyty"@fi ,
                            "duglighetstest som görs som första steg för att identifiera uppenbara fall av icke-överensstämmelse"@sv ,
                            "indledende egnethedstest, der har til formål at identificere tydelige tilfælde af afvigelse"@da ,
                            "initial capability test intended to identify clear cases of non-conformance"@en ,
                            "prueba de funcionalidad inicial que pretende identificar casos claros de no conformidad"@es ,
                            "test fonctionnel initial ayant pour but d&#39;identifier clairement des cas de non-conformité"@fr ,
                            "начальный тест на функциональное соответствие,  предназначенный для выявления очевидных случаев несоответствия"@ru ,
                            "اختبار قدرة أولي الغرض منه تحديد الحالات الواضحة من عدم المطابقة"@ar ,
                            "初始能力测试，目的是确定那些明显的不一致内容。"@zh ,
                            "明らかな不適合のケースを識別するために実施する最初の機能試験。"@ja ,
                            "부적합 경우와 적합한 경우를 명확하게 식별하기 위해 실시하는 최초의 기능 시험"@ko ;
            skos:prefLabel "Basistest"@de ,
                           "basic test"@en ,
                           "basistest"@da ,
                           "grundtest"@sv ,
                           "perustesti"@fi ,
                           "prueba básica"@es ,
                           "test de base"@fr ,
                           "базовый  тест"@ru ,
                           "اختبار أساسي"@ar ,
                           "基本测试"@zh ,
                           "基本試験"@ja ,
                           "기본 시험"@ko ;
            geolexica:origin lang:araRegistry ,
                             lang:danRegistry ,
                             lang:deuRegistry ,
                             lang:engRegistry ,
                             lang:finRegistry ,
                             lang:fraRegistry ,
                             lang:jpnRegistry ,
                             lang:korRegistry ,
                             lang:rusRegistry ,
                             lang:spaRegistry ,
                             lang:sweRegistry ,
                             lang:zhoRegistry ;
            lang:deu-note notes:DefnTransUnavail .


###  https://isotc211.geolexica.org/ld/concepts#behaviour
:behaviour rdf:type owl:NamedIndividual ,
                    skos:Concept ;
           skos:inScheme geolexica:GeolexicaConceptScheme ;
           geolexica:hasInfo info:Info28 ;
           geolexica:hasLDAPI ldapi:ldapi28-json ,
                              ldapi:ldapi28-jsonld ,
                              ldapi:ldapi28-rdfxml ,
                              ldapi:ldapi28-skosrdf ;
           geolexica:hasLangCode lang:ara ,
                                 lang:dan ,
                                 lang:deu ,
                                 lang:eng ,
                                 lang:fin ,
                                 lang:fra ,
                                 lang:kor ,
                                 lang:msa ,
                                 lang:rus ,
                                 lang:spa ,
                                 lang:swe ,
                                 lang:zho ;
           geolexica:hasReview reviews:Review28 ;
           dcterms:identifier 28 ;
           skos:notation 28 ;
           rdfs:label "behaviour (UML)" ;
           skos:definition "efectos observables de una operación o de un evento, incluyendo sus resultados"@es ,
                           "effets observables d&#39;une opération ou d&#39;un événement, incluant ses résultats"@fr ,
                           "iagttagelige virkninger af en handling eller hændelse, herunder dens resultater"@da ,
                           "kelakuan atau tingkah laku"@ms ,
                           "observable effects of an operation or event, including its results"@en ,
                           "observable effects of an operation or event, including its results"@sv ,
                           "toiminnon tai tapahtuman havaittavissa olevat vaikutukset ja tulokset"@fi ,
                           "доступные для наблюдения последствия выполнения операции или события, в том числе, ее (его)  результаты"@ru ,
                           "الآثار التي يمكن رصدها لعملية أو حدث ، بما في ذلك نتائجها ."@ar ,
                           "由操作或事件产生的可观测的影响及其结果。"@zh ,
                           "연산, 사건 또는 그 결과 값까지 포함하여 관측 가능한 효과"@ko ;
           skos:prefLabel "Verhalten (UML)"@de ,
                          "behaviour (UML)"@en ,
                          "behaviour (UML)"@sv ,
                          "comportamiento (UML)"@es ,
                          "comportement (UML)"@fr ,
                          "käyttäytyminen (UML)"@fi ,
                          "opførsel (UML)"@da ,
                          "perangai"@ms ,
                          "поведение (UML)"@ru ,
                          "سلوك (UML)"@ar ,
                          "行为(UML)"@zh ,
                          "행태 (UML)"@ko ;
           geolexica:origin lang:araRegistry ,
                            lang:danRegistry ,
                            lang:deuRegistry ,
                            lang:engRegistry ,
                            lang:finRegistry ,
                            lang:fraRegistry ,
                            lang:korRegistry ,
                            lang:msaRegistry ,
                            lang:rusRegistry ,
                            lang:spaRegistry ,
                            lang:sweRegistry ,
                            lang:zhoRegistry ;
           lang:deu-note notes:DefnTransUnavail .


###  https://isotc211.geolexica.org/ld/concepts#boundary
:boundary rdf:type owl:NamedIndividual ,
                   skos:Concept ;
          skos:inScheme geolexica:GeolexicaConceptScheme ;
          geolexica:hasInfo info:Info29 ;
          geolexica:hasLDAPI ldapi:ldapi29-json ,
                             ldapi:ldapi29-jsonld ,
                             ldapi:ldapi29-rdfxml ,
                             ldapi:ldapi29-skosrdf ;
          geolexica:hasLangCode lang:ara ,
                                lang:dan ,
                                lang:deu ,
                                lang:eng ,
                                lang:fin ,
                                lang:fra ,
                                lang:jpn ,
                                lang:kor ,
                                lang:msa ,
                                lang:pol ,
                                lang:rus ,
                                lang:spa ,
                                lang:swe ,
                                lang:zho ;
          geolexica:hasReview reviews:Review29 ;
          dcterms:identifier 29 ;
          skos:notation 29 ;
          lang:ara-note "ملاحظة: تستخدم كلمة الحد أكثر ما تستخدم في السياق الهندسي ، وفي هذا السياق تفهم المجموعة على أنها تعني مجموعة نقاط أو مجموعة من الأجسام التي تمثل تلك النقاط . و في حالات أخرى ، يستخدم المصطلح استخداما مجازيا لوصف حالة التحول بين كيان ما وبقية ما في المجال الذي ينتمي إليه"@ar ;
          lang:dan-note "Bemærk til posten: Afgrænsning anvendes almindeligvis inden for geometrien, hvor mængden er en samling af punkter eller en samling af objekter, der repræsenterer disse punkter. På andre områder anvendes termen metaforisk til at beskrive overgangen mellem en entitet og resten af dens universe of discourse"@da ;
          lang:eng-note "Note to entry: Boundary is most commonly used in the context of geometry, where the set is a collection of points or a collection of objects that represent those points. In other arenas, the term is used metaphorically to describe the transition between an entity and the rest of its domain of discourse."@en ;
          lang:fin-note "HUOM.: Käsitettä rajaus käytetään yleisimmin geometriassa, jossa määritelmän sanalla joukko tarkoitetaan kokoelmaa pisteitä tai pisteitä vastaavia objekteja. Muissa yhteyksissä termiä rajaus käytetään kuvaannollisesti viittaamaan tietyn kokonaisuuden ja sen ulkopuolisen maailman väliseen siirtymään."@fi ;
          lang:jpn-note "備考： 境界が最もよく使用されるのは，集合が点の集まり又はこれらの点を表すオブジェクトの集まりであるような幾何に関する記　述においてである。他の分野では，この用語を，実体とその論議領域での余事象との遷移領域を比ゆ（喩）的に記述するために使用する。"@ja ;
          lang:kor-note "비고: 경계는 기하 환경에서 가장 많이 사용된다. 기하는 점 집합체 또는 그 점들을 표현하는 객체 집합체로 구성된다. 다른 측면에서 경계는 어떤 개체와 그 개체를 제외한 논의의 영역 간의 전이역을 기술하기 위하여 은유적 용어로 사용된다."@ko ;
          lang:pol-note "UWAGA: Granica jest najczęściej używana w kontekście geometrii, gdzie zbiór stanowi kolekcję punktów lub kolekcję obiektów reprezentujących te punkty. W innych dziedzinach wyrażenie granica jest stosowane metaforycznie do opisu przejścia między obiektem a resztą rozważanej dziedziny."@po ;
          lang:rus-note "Примечание: Термин «граница» повсеместно используется в контексте геометрии, где множество представляет собой совокупность точек или совокупность объектов, состоящих из этих точек. В других сферах деятельности указанный термин используется образно для описания переходного участка между сущностью и остальной предметной областью"@ru ;
          lang:spa-note "Nota: El término frontera se usa normalmente en el contexto de geometría, siendo conjunto, una colección de puntos o de objetos que representan a esos puntos. En otros ámbitos, el término se usa metafóricamente para describir la transición entre una entidad y el resto del universo de discurso."@es ;
          lang:zho-note "注： 边界通常用在几何结构中，这里的几何是点的集合或代表这些点的对象的集合。在别的场合，这个术语通常隐喻在实体与论域其余部分间的跃迁。"@zh ;
          rdfs:label "boundary" ;
          skos:definition "Menge, die die Begrenzung einer Entität darstellt"@de ,
                          "bersempadankan mempunyai sesuatu sbg sempadan; berbataskan"@ms ,
                          "conjunto que representa el límite de una entidad"@es ,
                          "ensemble représentant les limites d&#39;une entité"@fr ,
                          "kokonaisuuden rajaava joukko"@fi ,
                          "mængde, som repræsenterer grænsen af en entitet"@da ,
                          "set that represents the limit of an entity"@en ,
                          "yttre begränsning hos ett objekt"@sv ,
                          "zbiór, który reprezentuje ograniczenie obiektu"@pl ,
                          "множество,  представляющее пределы данной сущности"@ru ,
                          "مجموعة من التحديدات تمثل حدود كيان ما"@ar ,
                          "実体の広がりの限界を示す集合。"@ja ,
                          "表示一个实体的界限的集合。"@zh ,
                          "개체의 한계를 표현하는 집합"@ko ;
          skos:prefLabel "Grenze"@de ,
                         "afgrænsning"@da ,
                         "avgränsning"@sv ,
                         "boundary"@en ,
                         "frontera"@es ,
                         "frontière"@fr ,
                         "granica"@pl ,
                         "rajaus"@fi ,
                         "sempadan"@ms ,
                         "граница"@ru ,
                         "حدود"@ar ,
                         "境界"@ja ,
                         "边界"@zh ,
                         "경계"@ko ;
          geolexica:origin lang:araRegistry ,
                           lang:danRegistry ,
                           lang:deuRegistry ,
                           lang:engRegistry ,
                           lang:finRegistry ,
                           lang:fraRegistry ,
                           lang:jpnRegistry ,
                           lang:korRegistry ,
                           lang:msaRegistry ,
                           lang:polRegistry ,
                           lang:rusRegistry ,
                           lang:spaRegistry ,
                           lang:sweRegistry ,
                           lang:zhoRegistry ;
          lang:deu-note notes:NoteTransUnavail ;
          lang:msa-note notes:NoteTransUnavail ;
          lang:swe-note notes:NoteTransUnavail .


###  https://isotc211.geolexica.org/ld/concepts#buffer
:buffer rdf:type owl:NamedIndividual ,
                 skos:Concept ;
        skos:inScheme geolexica:GeolexicaConceptScheme ;
        geolexica:hasInfo info:Info30 ;
        geolexica:hasLDAPI ldapi:ldapi30-json ,
                           ldapi:ldapi30-jsonld ,
                           ldapi:ldapi30-rdfxml ,
                           ldapi:ldapi30-skosrdf ;
        geolexica:hasLangCode lang:ara ,
                              lang:dan ,
                              lang:deu ,
                              lang:eng ,
                              lang:fin ,
                              lang:fra ,
                              lang:jpn ,
                              lang:kor ,
                              lang:msa ,
                              lang:pol ,
                              lang:rus ,
                              lang:spa ,
                              lang:swe ,
                              lang:zho ;
        geolexica:hasReview reviews:Review30 ;
        dcterms:identifier 30 ;
        skos:notation 30 ;
        rdfs:label "buffer" ;
        skos:altLabel "버퍼"@ko ;
        skos:definition "Kawasan dalam ingatan utama yang telah dikhaskan untuk memegang data yang masih belum dapat dipindahkan kepada cakera"@ms ,
                        "geometric object that contains all direct positions whose distance from a specified geometric object is less than or equal to a given distance"@en ,
                        "geometrinen objekti, joka sisältää kaikki pisteet, joiden etäisyys annetusta geometrisestä objektista on pienempi tai yhtä suuri kuin tietty etäisyys"@fi ,
                        "geometrisk objekt, der indeholder alle de direkte positioner, hvis afstand fra et specificeret geometrisk objekt er mindre end eller lig med en given afstand"@da ,
                        "obiekt geometryczny zawierający wszystkie położenia bezpośrednie, których odległość od określonego obiektu geometrycznego jest równa danej odległości lub mniejsza"@pl ,
                        "objet géométrique contenant toutes les positions directes dont la distance à un objet géométrique spécifié est inférieure ou égale à une distance donnée"@fr ,
                        "objeto geométrico que contiene todas las posiciones directas cuyas distancias a un objeto geométrico específico son menores o iguales que una distancia dada"@es ,
                        "område vars gränser befinner sig på givna avstånd från ett utvalt geografiskt objekt"@sv ,
                        "геометрический объект, содержащий все точки, расстояния от которых до заданного геометрического объекта меньше или равны заданной величине"@ru ,
                        "كيان هندسي يحتوي على جميع المواضع المباشرة التي تكون في نطاق يبعد عن كيان محدد مسافة محددة"@ar ,
                        "包含距一个指定几何对象的距离都小于或等于一个给定值的所有直接位置的几何对象。"@zh ,
                        "指定された幾何オブジェクトから与えられた距離以内のすべての直接位置を含む幾何オブジェクト。"@ja ,
                        "지정된 기하 객체로부터 주어진 거리 이내의 모든 직접 위치를 포함하는 기하 객체"@ko ;
        skos:prefLabel "Puffer"@de ,
                       "buffer"@da ,
                       "buffer"@en ,
                       "buffer"@es ,
                       "buffertzon"@sv ,
                       "bufor"@pl ,
                       "penampan"@ms ,
                       "tampon (buffer)"@fr ,
                       "vyöhyke"@fi ,
                       "буферная зона [буфер]"@ru ,
                       "نطاق"@ar ,
                       "バッファ"@ja ,
                       "缓冲区"@zh ,
                       "영향 범위"@ko ;
        geolexica:origin lang:araRegistry ,
                         lang:danRegistry ,
                         lang:deuRegistry ,
                         lang:engRegistry ,
                         lang:finRegistry ,
                         lang:fraRegistry ,
                         lang:jpnRegistry ,
                         lang:korRegistry ,
                         lang:msaRegistry ,
                         lang:polRegistry ,
                         lang:rusRegistry ,
                         lang:spaRegistry ,
                         lang:sweRegistry ,
                         lang:zhoRegistry ;
        lang:deu-note notes:DefnTransUnavail .


###  https://isotc211.geolexica.org/ld/concepts#calendar
:calendar rdf:type owl:NamedIndividual ,
                   skos:Concept ;
          skos:inScheme geolexica:GeolexicaConceptScheme ;
          geolexica:hasInfo info:Info31 ;
          geolexica:hasLDAPI ldapi:ldapi31-json ,
                             ldapi:ldapi31-jsonld ,
                             ldapi:ldapi31-rdfxml ,
                             ldapi:ldapi31-skosrdf ;
          geolexica:hasLangCode lang:ara ,
                                lang:dan ,
                                lang:deu ,
                                lang:eng ,
                                lang:fin ,
                                lang:fra ,
                                lang:jpn ,
                                lang:kor ,
                                lang:msa ,
                                lang:pol ,
                                lang:rus ,
                                lang:spa ,
                                lang:swe ,
                                lang:zho ;
          dcterms:identifier 31 ;
          skos:notation 31 ;
          rdfs:label "calendar" ;
          skos:altLabel "버퍼"@ko ;
          skos:definition "discrete temporal reference system that provides a basis for defining temporal position to a resolution of one day"@en ,
                          "diskreetti ajan vertausjärjestelmä, joka toimii pohjana temporaalisen sijainnin määrittelemiselle yhden vuorokauden tarkkuudella"@fi ,
                          "diskret tidsmæssigt referencesystem, der danner grundlag for at definere tidsmæssig position med en nøjagtighed på 1 døgn"@da ,
                          "dyskretny czasowy system odniesienia będący podstawą do definiowania położenia w czasie z dokładnością do jednego dnia"@pl ,
                          "senarai atau daftar hari bulan; takwim"@ms ,
                          "sistema de referencia temporal característico, que constituye una base para definir la posición temporal con una resolución de un día"@es ,
                          "system av regler för hur tid indelas och mäts"@sv ,
                          "système de référence temporelle discret fournissant une base pour définir la position temporelle avec une résolution d&#39;un jour"@fr ,
                          "дискретная система отсчета времени, которая образует основу для определения времени с разрешением в одни сутки"@ru ,
                          "نظام مرجعي زمني متميِّز يعتبر أساسا لتعريف الموضع الزمني بدرجة دقة تصل إلى يوم واحد"@ar ,
                          "一日をその分解能とする時間位置を定義するための基礎となる離散的な時間参照系の一つ。"@ja ,
                          "离散的时间参照系，提供了定义分辨率为一日的时间位置的基础。"@zh ,
                          "일 단위 시간 위치의 정의 근거를 제시하는 불연속 시간 참조 체계"@ko ;
          skos:prefLabel "Kalender"@de ,
                         "calendar"@en ,
                         "calendario"@es ,
                         "calendrier"@fr ,
                         "kalendar"@ms ,
                         "kalendarz"@pl ,
                         "kalender"@da ,
                         "kalender tideräkning"@sv ,
                         "kalenteri"@fi ,
                         "календарь"@ru ,
                         "تقويم"@ar ,
                         "日历"@zh ,
                         "暦"@ja ,
                         "달력"@ko ;
          geolexica:origin lang:araRegistry ,
                           lang:danRegistry ,
                           lang:deuRegistry ,
                           lang:engRegistry ,
                           lang:finRegistry ,
                           lang:fraRegistry ,
                           lang:jpnRegistry ,
                           lang:korRegistry ,
                           lang:msaRegistry ,
                           lang:polRegistry ,
                           lang:rusRegistry ,
                           lang:spaRegistry ,
                           lang:sweRegistry ,
                           lang:zhoRegistry ;
          lang:deu-note notes:DefnTransUnavail .

###  https://isotc211.geolexica.org/ld/concepts#calendar_era
:calendar_era rdf:type owl:NamedIndividual ,
                   skos:Concept ;
          skos:inScheme geolexica:GeolexicaConceptScheme ;
          geolexica:hasInfo info:Info32 ;
          geolexica:hasLDAPI ldapi:ldapi32-json ,
                             ldapi:ldapi32-jsonld ,
                             ldapi:ldapi32-rdfxml ,
                             ldapi:ldapi32-skosrdf ;
          geolexica:hasLangCode lang:ara ,
                                lang:dan ,
                                lang:deu ,
                                lang:eng ,
                                lang:fin ,
                                lang:fra ,
                                lang:jpn ,
                                lang:kor ,
                                lang:pol ,
                                lang:rus ,
                                lang:spa ,
                                lang:swe ,
                                lang:zho ;
          dcterms:identifier 32 ;
          skos:notation 32 ;
          rdfs:label "calendar era" ;
          skos:definition "sequence of periods of one of the types used in a calendar, counted from a specified event"@en ,
  "سلسلة من المدد الزمنية المتتالية من أحد الأنواع التي تستخدم في التقاويم ، تحسب اعتبارا من واقعة محددة"@ar ,
   "sekvens af perioder af en af de typer, der anvendes i en kalender, regnet fra en nærmere angivet hændelse"@da ,
   "kalenterissa käytössä olevien joidenkin aikajaksojen jono, joka aloitetaan tietystä ajanhetkestä"@fi ,
   "séquence de périodes de l&#39;un des types utilisés dans un calendrier, comptée à partir d&#39;un évenement particulier"@fr ,
   "暦の中で使用する型の一つとなり，ある特定の事象からその長さを数える期間。"@ja ,
   "기간의 연속을 표현하는 달력의 유형으로 특정 사건으로부터 계산된 기간 표시"@ko ,
   "zastosowany w kalendarzu ciąg okresów jednego typu,liczonych od określonego zdarzenia"@pl ,
   "последовательность периодов одного типа, используемого в календаре, с отсчетом от определенного события"@ru ,
   "secuencia de períodos de uno de los tipos utilizados en un calendario, contando a partir de un evento específico"@es ,
   "sequence of periods of one of the types used in a calendar, counted from a specified event"@sv ,
   "从特定事件起算的，日历中使用的一类时段序列。"@zh ;
            skos:prefLabel "calendar era"@en ,
   "حقبة تقويمية"@ar ,
   "kalenderinddeling"@da ,
   "kalendarischer Zeitraum"@de ,
   "kalenterikausi"@fi ,
   "ère calendaire"@fr ,
   "暦年代"@ja ,
   "달력 연대"@ko ,
   "era kalendarzowa"@pl ,
   "календарная эра"@ru ,
   "era de calendario"@es ,
   "kalenderera"@sv ,
   "日历时代"@zh ;
          geolexica:origin lang:araRegistry ,
                           lang:danRegistry ,
                           lang:deuRegistry ,
                           lang:engRegistry ,
                           lang:finRegistry ,
                           lang:fraRegistry ,
                           lang:jpnRegistry ,
                           lang:korRegistry ,
                           lang:polRegistry ,
                           lang:rusRegistry ,
                           lang:spaRegistry ,
                           lang:sweRegistry ,
                           lang:zhoRegistry ;
          lang:deu-note notes:DefnTransUnavail ;
          lang:fra-note notes:NoteTransDiff .


###  https://isotc211.geolexica.org/ld/concepts#candidate_route
:candidate_route rdf:type owl:NamedIndividual ,
                   skos:Concept ;
          skos:inScheme geolexica:GeolexicaConceptScheme ;
          geolexica:hasInfo info:Info34 ;
          geolexica:hasLDAPI ldapi:ldapi34-json ,
                             ldapi:ldapi34-jsonld ,
                             ldapi:ldapi34-rdfxml ,
                             ldapi:ldapi34-skosrdf ;
          geolexica:hasLangCode lang:ara ,
                                lang:dan ,
                                lang:deu ,
                                lang:eng ,
                                lang:fin ,
                                lang:fra ,
                                lang:kor ,
                                lang:rus ,
                                lang:spa ,
                                lang:swe ,
                                lang:zho ;
          dcterms:identifier 34 ;
          skos:notation 34 ;
          rdfs:label "candidate route" ;
          skos:definition "any route that satisfies all constraints of the routing request with the possible exception of optimality of the cost function"@en ,
                        "أي مسلك يكون مستوفيا لجميع القيود المشمولة في طلب تحديد مسلك أو مسار مع احتمال استثناء أفضلية دالة التكلفة"@ar ,
                        "enhver rute, der opfylder alle betingelser i ruteforespørgslen, dog evt. med undtagelse af optimering af omkostningsfunktionen"@da ,
                        "reitti, joka täyttää kaikki reitinhakupyynnön ehdot mahdollisesti lukuunottamatta kustannusten optimointitoimintoa"@fi ,
                        "itinéraire satisfaisant toutes les contraintes d&#39;une requête de routage à l&#39;exception possible de l&#39;optimalité de la fonction de coût"@fr ,
                        "라우팅 요청의 제약 조건에 대하여 최적화된 비용 함수를 만족시키는 경로"@ko ,
                        "любой из маршрутов, удовлетворяющий всем ограничениям из запроса, за исключением, возможно, требования на минимум функции  стоимости"@ru ,
                        "cualquier ruta que satisfaga todas las restricciones de una petición de enrutamiento con la posible excepción de la optimización de la función de costo"@es ,
                        "varje rutt som uppfyller kraven i ruttförfrågan, eventuellt frånsett kostnadsoptimering"@sv ,
                        "除了成本函数最优路径之外，还包含任何可满足路径请求的所有限制条件的路径。"@zh ;
            skos:prefLabel "candidate route"@en ,
                        "مسلك مرشح"@ar ,
                        "ruteforslag"@da ,
                        "mögliche Route"@de ,
                        "reittiehdokas"@fi ,
                        "itinéraire candidat"@fr ,
                        "후보 경로"@ko ,
                        "вариант маршрута"@ru ,
                        "ruta candidata"@es ,
                        "ruttkandidat"@sv ,
                        "候选路径"@zh ;
          geolexica:origin lang:araRegistry ,
                           lang:danRegistry ,
                           lang:deuRegistry ,
                           lang:engRegistry ,
                           lang:finRegistry ,
                           lang:fraRegistry ,
                           lang:korRegistry ,
                           lang:rusRegistry ,
                           lang:spaRegistry ,
                           lang:sweRegistry ,
                           lang:zhoRegistry ;
          lang:deu-note notes:DefnTransUnavail , notes:NoteTransUnavail ;
          lang:fra-note notes:NoteTransDiff ;
          lang:swe-note notes:NoteTransUnavail .

###  https://isotc211.geolexica.org/ld/concepts#capability_test
:capability_test rdf:type owl:NamedIndividual ,
                   skos:Concept ;
          skos:inScheme geolexica:GeolexicaConceptScheme ;
          geolexica:hasInfo info:Info35 ;
          geolexica:hasReview reviews:Review35 ;
          geolexica:hasLDAPI ldapi:ldapi35-json ,
                             ldapi:ldapi35-jsonld ,
                             ldapi:ldapi35-rdfxml ,
                             ldapi:ldapi35-skosrdf ;
          geolexica:hasLangCode lang:ara ,
                                lang:dan ,
                                lang:deu ,
                                lang:eng ,
                                lang:fin ,
                                lang:fra ,
                                lang:kor ,
                                lang:rus ,
                                lang:spa ,
                                lang:swe ,
                                lang:zho ;
          dcterms:identifier 35 ;
          skos:notation 35 ;
          rdfs:label "capability test" ;
          skos:definition "test designed to determine whether an IUT conforms to a particular characteristic of an International Standard as described in the test purpose"@en ,
   "اختبار صُمم لتحديد ما إذا كان التنفيذ تحت ظروف الاختبار في حالة معينة مطابقا لخاصية محددة لمقياس دولي ما بحسب الوصف الوارد في الغرض من إجراء الاختبار"@ar ,
   "test, der er udviklet med henblik på at afgøre, om en IUT (Implementation Under Test) opfylder kravene til en bestemt egenskab i en international standard som beskrevet i testformålet"@da ,
   "testi, jonka tarkoituksena on määrittää, onko testattavana oleva toteutus (Implementation Under Test, IUT) kansainvälisen standardin tietyn vaatimuksen mukainen siten kuin testin tarkoituksessa on kuvattu"@fi ,
   "test destiné à déterminer si une implémentation soumise à test est conforme à une caractéristique particulière d&#39;une norme internationale, tel que décrit dans l&#39;objet du test"@fr ,
   "試験対象(IUT:implementation under test)が試験目的の記述どおりに規格の特定の性質に適合するかどうかを決定するための試験。"@ja ,
   "시험용 구현(IUT: Implementation under test)이 시험 목적에 기술된 바와 같이 표준 표준의 특정한 특성을 따르는지를 판단하기 위해 설계된 시험"@ko ,
   "тест, призванный установить, обладает ли объект проверки конкретным свойством, которое предусмотрено международным стандартом и объявлено целью тестирования"@ru ,
   "prueba diseñada para determinar si un IUT es conforme a una característica particular de una norma internacional tal y como se describe en el propósito de la prueba"@es ,
   "test som är framtagen för att avgöra om en implementering av en standard överensstämmer med en viss egenskap hos standarden och i enlighet med testens syfte"@sv ,
   "为确定被测实现（IUT)是否符合测试目的所描述的标准的特性而设计的测试。"@zh ;
             skos:prefLabel "capability test"@en ,
   "اختبار القدرة"@ar ,
   "egnethedstest"@da ,
   "Fähigkeitstest"@de ,
   "kelpoisuustesti"@fi ,
   "test fonctionnel"@fr ,
   "機能試験"@ja ,
   "기능 시험"@ko ,
   "тест на функциональное соответствие"@ru ,
   "prueba de capacidad"@es ,
   "duglighetstest"@sv ,
   "能力测试"@zh ;
          geolexica:origin lang:araRegistry ,
                           lang:danRegistry ,
                           lang:deuRegistry ,
                           lang:engRegistry ,
                           lang:finRegistry ,
                           lang:fraRegistry ,
                           lang:korRegistry ,
                           lang:rusRegistry ,
                           lang:spaRegistry ,
                           lang:sweRegistry ,
                           lang:zhoRegistry ;
          lang:deu-note notes:DefnTransUnavail .

###  https://isotc211.geolexica.org/ld/concepts#cardinalityUML
:cardinalityUML rdf:type owl:NamedIndividual ,
                   skos:Concept ;
          skos:inScheme geolexica:GeolexicaConceptScheme ;
          geolexica:hasInfo info:Info36 ;
          geolexica:hasReview reviews:Review36 ;
          geolexica:hasLDAPI ldapi:ldapi36-json ,
                             ldapi:ldapi36-jsonld ,
                             ldapi:ldapi36-rdfxml ,
                             ldapi:ldapi36-skosrdf ;
          geolexica:hasLangCode lang:ara ,
                                lang:dan ,
                                lang:deu ,
                                lang:eng ,
                                lang:fin ,
                                lang:fra ,
                                lang:kor ,
                                lang:rus ,
                                lang:spa ,
                                lang:swe ,
                                lang:zho ;
          dcterms:identifier 36 ;
          skos:notation 36 ;
          rdfs:label "cardinality (UML)" ;
          skos:definition "number of elements in a set"@en ,
                "عدد العناصر في مجموعة معينة"@ar ,
                "antal elementer i en mængde"@da ,
                "joukon elementtien lukumäärä"@fi ,
                "nombre d&#39;éléments dans un ensemble"@fr ,
                "집합 내 요소의 수"@ko ,
                "число элементов  множества"@ru ,
                "número de elementos en un conjunto"@es ,
                "number of elements in a set"@sv ,
                "集合中元素的个数。"@zh ;
             skos:prefLabel "cardinality (UML)"@en ,
                "عدد العلاقات (UML)"@ar ,
                "kardinalitet (UML)"@da ,
                "Kardinalität"@de ,
                "mahtavuus (UML)"@fi ,
                "cardinalité (UML)"@fr ,
                "관계 수 (UML)"@ko ,
                "кардинальное число (UML)"@ru ,
                "cardinalidad(UML)"@es ,
                "cardinality (UML)"@sv ,
                "基数(UML)"@zh ;
          skos:altLabel "kardinaliteetti (UML)"@fi ;
          geolexica:origin lang:araRegistry ,
                           lang:danRegistry ,
                           lang:deuRegistry ,
                           lang:engRegistry ,
                           lang:finRegistry ,
                           lang:fraRegistry ,
                           lang:korRegistry ,
                           lang:rusRegistry ,
                           lang:spaRegistry ,
                           lang:sweRegistry ,
                           lang:zhoRegistry ;
          lang:deu-note notes:DefnTransUnavail , notes:NoteTransUnavail ;
          lang:swe-note notes:NoteTransUnavail ;
          lang:rus-note notes:NoteTransDiff .

###  https://isotc211.geolexica.org/ld/concepts#cartesian_coordinate_system
:cartesian_coordinate_system rdf:type owl:NamedIndividual ,
                   skos:Concept ;
          skos:inScheme geolexica:GeolexicaConceptScheme ;
          geolexica:hasInfo info:Info37 ;
          geolexica:hasReview reviews:Review37 ;
          geolexica:hasLDAPI ldapi:ldapi37-json ,
                             ldapi:ldapi37-jsonld ,
                             ldapi:ldapi37-rdfxml ,
                             ldapi:ldapi37-skosrdf ;
          geolexica:hasLangCode lang:ara ,
                                lang:dan ,
                                lang:deu ,
                                lang:eng ,
                                lang:fin ,
                                lang:fra ,
                                lang:kor ,
                                lang:nld ,
                                lang:pol ,
                                lang:rus ,
                                lang:spa ,
                                lang:swe ,
                                lang:zho ;
          dcterms:identifier 37 ;
          skos:notation 37 ;
          rdfs:label "Cartesian coordinate system" ;
          skos:definition "coordinate system which gives the position of points relative to n mutually perpendicular axes"@en ,
                "نظام إحداثيات يحدد موقع النقاط بالنسبة إلى عدد (ع) من المحاور المتعامدة على بعضها البعض"@ar ,
                "koordinatsystem, der angiver punkters position i forhold til n akser, som er vinkelret på hinanden"@da ,
                "Koordinatensystem, das die Punktposition in Bezug auf n zueinander orthogonale Achsen angibt"@de ,
                "koordinaatisto, jossa pisteen sijainti ilmoitetaan suhteessa n:ään toisiaan vastaan kohtisuorassa olevaan akseliin"@fi ,
                "système de coordonnées donnant la position des points relativement à n axes perpendiculaires deux à deux"@fr ,
                "상호 직교하는 n개의 축을 기준으로 점의 위치를 나타내는 좌표 체계"@ko ,
                "Coördinaat systeem wat de positie geeft van punten ten opzichte van loodrecht op elkaar staande assen."@nl ,
                "układ współrzędnych, który podaje pozycję punktów względem n wzajemnie prostopadłych osi"@pl ,
                "система координат, определяющая положение точек по отношению к N взаимно перпендикулярным осям, исходящим из одной точки"@ru ,
                "sistema de coordenadas que da la posición de los puntos en relación a n ejes mutuamente perpendiculares"@es ,
                "koordinatsystem som består av minst två axlar, vilka skär varandra under rät vinkel i ett origo, och där en punkts position anges som avstånd till axlarna"@sv ,
                "给出相对与n个相互垂直坐标轴的点位置的坐标系。"@zh ;
             skos:prefLabel "Cartesian coordinate system"@en ,
                "نظام الإحداثيات الديكارتي"@ar ,
                "kartesisk koordinatsystem"@da ,
                "kartesisches Koordinatensystem"@de ,
                "suorakulmainen koordinaatisto"@fi ,
                "système cartésien de coordonnées"@fr ,
                "직각 좌표계"@ko ,
                "Cartesiaans Coördinaat Systeem"@nl ,
                "kartezjański układ współrzędnych"@pl ,
                "прямоугольная система координат"@ru ,
                "sistema de coordenadas cartesianas"@es ,
                "kartesiskt koordinatsystem"@sv ,
                "笛卡尔坐标系"@zh ;
  skos:altLabel "karteesinen koordinaatisto"@fi ;
          geolexica:origin lang:araRegistry ,
                           lang:danRegistry ,
                           lang:deuRegistry ,
                           lang:engRegistry ,
                           lang:finRegistry ,
                           lang:fraRegistry ,
                           lang:korRegistry ,
                           lang:nldRegistry ,
                           lang:rusRegistry ,
                           lang:polRegistry ,
                           lang:spaRegistry ,
                           lang:sweRegistry ,
                           lang:zhoRegistry ;
          lang:deu-note notes:DefnTransUnavail .

###  https://isotc211.geolexica.org/ld/concepts#character
:character rdf:type owl:NamedIndividual ,
                   skos:Concept ;
          skos:inScheme geolexica:GeolexicaConceptScheme ;
          geolexica:hasInfo info:Info39 ;
          geolexica:hasReview reviews:Review39 ;
          geolexica:hasLDAPI ldapi:ldapi39-json ,
                             ldapi:ldapi39-jsonld ,
                             ldapi:ldapi39-rdfxml ,
                             ldapi:ldapi39-skosrdf ;
          geolexica:hasLangCode lang:ara ,
                                lang:dan ,
                                lang:deu ,
                                lang:eng ,
                                lang:fin ,
                                lang:fra ,
                                lang:kor ,
                                lang:msa ,
                                lang:rus ,
                                lang:spa ,
                                lang:swe ,
                                lang:zho ;
          dcterms:identifier 39 ;
          skos:notation 39 ;
          rdfs:label "character" ;
          skos:definition "member of a set of elements that is used for the representation, organization, or control of data"@en ,
                "واحد من مجموعة عناصر تستخدم لعرض البيانات أو تنظيمها أو السيطرة عليها"@ar ,
                "et af en mængde elementer, som anvendes til angivelse, organisering eller styring af data"@da ,
                "tiedon esittämiseen, järjestelyyn tai hallintaan käytetyn elementtijoukon jäsen"@fi ,
                "membre d’un ensemble d’éléments utilisé pour la représentation, l’organisation ou le contrôle des données"@fr ,
                "데이터를 표현, 구성 또는 제어하기 위해 사용되는 요소 집합의 원소"@ko ,
                "1 huruf. 2 ist huruf, angka, atau simbol dsb yg dpt dilambangkan dgn kod komputer."@ms ,
                "элемент множества, используемого для представления и организации данных, а также управления ими"@ru ,
                "miembro de un conjunto de elementos que se usa para la representación, organización o control de datos"@es ,
                "element som ingår i en mängd av vedertagen sammansättning och som används för att bilda, styra eller representera data"@sv ,
                "用于数据的表示、组织或控制的元素集合的成员。"@zh ;
          skos:prefLabel "character"@en ,
                "حرف"@ar ,
                "karakter; tegn"@da ,
                "Zeichen"@de ,
                "merkki"@fi ,
                "caractère"@fr ,
                "문자"@ko ,
                "aksara"@ms ,
                "символ"@ru ,
                "carácter"@es ,
                "tecken"@sv ,
                "字符"@zh ;
          geolexica:origin lang:araRegistry ,
                           lang:danRegistry ,
                           lang:deuRegistry ,
                           lang:engRegistry ,
                           lang:finRegistry ,
                           lang:fraRegistry ,
                           lang:korRegistry ,
                           lang:rusRegistry ,
                           lang:msaRegistry ,
                           lang:spaRegistry ,
                           lang:sweRegistry ,
                           lang:zhoRegistry ;
          lang:deu-note notes:DefnTransUnavail .

###  https://isotc211.geolexica.org/ld/concepts#circular_sequence
:circular_sequence rdf:type owl:NamedIndividual ,
                   skos:Concept ;
          skos:inScheme geolexica:GeolexicaConceptScheme ;
          geolexica:hasInfo info:Info41 ;
          geolexica:hasReview reviews:Review41 ;
          geolexica:hasLDAPI ldapi:ldapi41-json ,
                             ldapi:ldapi41-jsonld ,
                             ldapi:ldapi41-rdfxml ,
                             ldapi:ldapi41-skosrdf ;
          geolexica:hasLangCode lang:ara ,
                                lang:dan ,
                                lang:deu ,
                                lang:eng ,
                                lang:fin ,
                                lang:fra ,
                                lang:kor ,
                                lang:jpn ,
                                lang:pol ,
                                lang:rus ,
                                lang:spa ,
                                lang:swe ,
                                lang:zho ;
          dcterms:identifier 41 ;
          skos:notation 41 ;
          rdfs:label "circular sequence" ;
          skos:definition "sequence which has no logical beginning and is therefore equivalent to any circular shift of itself; hence the last item in the sequence is considered to precede the first item in the sequence"@en ,
   "تسلسل ليس له بداية منطقية ولهذا يعتبر مماثلا لأي تحول دائري يتم تلقائيا ؛ لذا فإن الجزء الأخير في التسلسل يعتبر متقدماً على الجزء الأول فيه"@ar ,
   "sekvens, der ikke har nogen logisk begyndelse og derfor er ækvivalent med enhver cirkulær forskydning af sig selv; derfor anses det sidste element i en sekvens at stå foran det første element i sekvensen"@da ,
   "jono, jolla ei ole käsitteellistä alkua ja joka loogisesti voidaan aloittaa mistä tahansa alkiosta; jonon viimeisen jäsenen katsotaan näin ollen edeltävän ensimmäistä alkiota jonossa"@fi ,
   "séquence n&#39;ayant aucun début logique et étant donc équivalente à n&#39;importe quelle permutation circulaire d&#39;elle-même; par conséquent, le dernier élément de la séquence est considéré comme celui qui précède le premier"@fr ,
   "論理的な開始点をもたないために，それ自身のどのような循環的なシフトとも同一になり，結果として最後の項目が順列の最初の項目に先行するとみなされる列。"@ja ,
   "논리적인 시작점이 존재하지 않기 때문에 어떤 한 점에서 수열을 이동하더라도 항상 동일한 연속; 따라서 연속의 마지막 항목이 첫 항목에 앞서는 것으로 간주됨"@ko ,
   "sekwencja, która nie ma logicznego początku i w tym sensie jest równoważna każdemu cyklicznemu przesunięciu samej siebie; ostatni element w sekwencji traktuje się jako poprzednik pierwszego elementu w sekwencji"@pl ,
   "последовательность, которая не имеет логического начала и, следовательно, эквивалентна любому циклу, сдвинутому относительно себя; в результате этого последний элемент последовательности считается предшествующим первому элементу"@ru ,
   "secuencia que no tiene un principio lógico y en consecuencia es equivalente a cualquier desplazamiento de sí mismo; de ahí que se considere que el último ítem de la secuencia precede al primero"@es ,
   "sekvens som upprepas från början när den kommit till sista elementet"@sv ,
   "没有逻辑起始，因而等同于任何自身循环移位的序列，因此可认为序列的最后一数据项位于该序列的第一项之前。"@zh ;
          skos:prefLabel "circular sequence"@en ,
   "تسلسل دائري"@ar ,
   "cirkulær sekvens"@da ,
   "Kreissequenz"@de ,
   "kehäjono"@fi ,
   "séquence circulaire"@fr ,
   "環状列"@ja ,
   "순환 연속"@ko ,
   "sekwencja cykliczna"@pl ,
   "циклическая [круговая] последовательность"@ru ,
   "secuencia circular"@es ,
   "cirkulär sekvens"@sv ,
   "循环序列"@zh ;
          geolexica:origin lang:araRegistry ,
                           lang:danRegistry ,
                           lang:deuRegistry ,
                           lang:engRegistry ,
                           lang:finRegistry ,
                           lang:fraRegistry ,
                           lang:korRegistry ,
                           lang:jpnRegistry ,
                           lang:rusRegistry ,
                           lang:polRegistry ,
                           lang:spaRegistry ,
                           lang:sweRegistry ,
                           lang:zhoRegistry ;
          lang:deu-note notes:DefnTransUnavail .

###  https://isotc211.geolexica.org/ld/concepts#classUML
:classUML rdf:type owl:NamedIndividual ,
                   skos:Concept ;
          skos:inScheme geolexica:GeolexicaConceptScheme ;
          geolexica:hasInfo info:Info43 ;
          geolexica:hasReview reviews:Review43 ;
          geolexica:hasLDAPI ldapi:ldapi43-json ,
                             ldapi:ldapi43-jsonld ,
                             ldapi:ldapi43-rdfxml ,
                             ldapi:ldapi43-skosrdf ;
          geolexica:hasLangCode lang:ara ,
                                lang:dan ,
                                lang:deu ,
                                lang:eng ,
                                lang:fin ,
                                lang:fra ,
                                lang:kor ,
                                lang:rus ,
                                lang:spa ,
                                lang:swe ,
                                lang:zho ;
          dcterms:identifier 43 ;
          skos:notation 43 ;
          rdfs:label "class (UML)" ;
          skos:definition "description of a set of objects that share the same attributes, operations, methods, relationships, and semantics"@en ,
   "وصف لمجموعة من البيانات التي لها بيانات وصفية ، وعمليات ، وطرق ، وعلاقات ، ودلالات لفظية مشتركة"@ar ,
   "beskrivelse af en mængde af objekter med samme attributter, operationer, metoder, relationer og semantik"@da ,
   "kuvaus joukosta objekteja, joilla on keskenään samat attribuutit, toiminnot, metodit, suhteet ja semantiikat"@fi ,
   "description d&#39;un ensemble d&#39;objets partageant les mêmes attributs, opérations, méthodes, relations et sémantique"@fr ,
   "동일한 속성, 연산, 방법 및 관계와 의미론을 공유하는 객체 집합의 기술"@ko ,
   "описание множества объектов, обладающих общими атрибутами, операциями, методами,  отношениями и семантикой"@ru ,
   "descripción de un conjunto de objetos que comparten los mismos atributos, operaciones, métodos, relaciones y semántica"@es ,
   "UML-element i klassdiagram för formell specifikation av datauppgifter och semantik för representation av likartade företeelser eller egenskaper"@sv ,
   "(UML)具有相同的属性（域）、操作方法、关系与语义的对象集的描述。"@zh ;
          skos:prefLabel "class (UML)"@en ,
   "فئة (UML)"@ar ,
   "klasse (UML)"@da ,
   "(Objekt-)Klasse"@de ,
   "luokka (UML)"@fi ,
   "classe (UML)"@fr ,
   "클래스 (UML)"@ko ,
   "класс (UML)"@ru ,
   "clase (UML)"@es ,
   "klass (UML)"@sv ,
   "类(UML)"@zh ;
          geolexica:origin lang:araRegistry ,
                           lang:danRegistry ,
                           lang:deuRegistry ,
                           lang:engRegistry ,
                           lang:finRegistry ,
                           lang:fraRegistry ,
                           lang:korRegistry ,
                           lang:spaRegistry ,
                           lang:sweRegistry ,
                           lang:zhoRegistry ;
          lang:deu-note notes:DefnTransUnavail , notes:NoteTransUnavail ;
          lang:swe-note notes:NoteTransUnavail ;
          lang:rus-note notes:NoteTransDiff .

###  https://isotc211.geolexica.org/ld/concepts#classifierUML
:classifierUML rdf:type owl:NamedIndividual ,
                   skos:Concept ;
          skos:inScheme geolexica:GeolexicaConceptScheme ;
          geolexica:hasInfo info:Info44 ;
          geolexica:hasReview reviews:Review44 ;
          geolexica:hasLDAPI ldapi:ldapi44-json ,
                             ldapi:ldapi44-jsonld ,
                             ldapi:ldapi44-rdfxml ,
                             ldapi:ldapi44-skosrdf ;
          geolexica:hasLangCode lang:ara ,
                                lang:dan ,
                                lang:deu ,
                                lang:eng ,
                                lang:fin ,
                                lang:fra ,
                                lang:kor ,
                                lang:rus ,
                                lang:spa ,
                                lang:swe ,
                                lang:zho ;
          dcterms:identifier 44 ;
          skos:notation 44 ;
          rdfs:label "classifier (UML)" ;
          skos:definition "mechanism that describes behavioural and structural features"@en ,
   "آلية تصف المعالم السلوكية والهيكلية"@ar ,
   "mekanisme, der beskriver adfærdsmæssige og strukturelle træk"@da ,
   "mekanismi, joka kuvaa käyttäytymiseen ja rakenteeseen liittyviä piirteitä"@fi ,
   "mécanisme décrivant les caractéristiques comportementales et structurelles"@fr ,
   "행위 및 구조적 특성을 기술하는 메커니즘"@ko ,
   "механизм, описывающий структурные и поведенческие особенности"@ru ,
   "mecanismo que describe objetos geográficos estructurados y con comportamiento"@es ,
   "mechanism that describes behavioural and structural features"@sv ,
   "描述行为和结构要素的机制。"@zh ;
  skos:prefLabel "classifier (UML);"@en ,
   "مصنِّف (UML);"@ar ,
   "klassifikator (UML);"@da ,
   "Klassifikator (UML);"@de ,
   "luokittelija (UML);"@fi ,
   "classificateur (UML);"@fr ,
   "분류자 (UML);"@ko ,
   "классификатор (UML);"@ru ,
   "clasificador (UML);"@es ,
   "classifier (UML);"@sv ,
   "类元(UML);"@zh ;
          geolexica:origin lang:araRegistry ,
                           lang:danRegistry ,
                           lang:deuRegistry ,
                           lang:engRegistry ,
                           lang:finRegistry ,
                           lang:fraRegistry ,
                           lang:korRegistry ,
                           lang:spaRegistry ,
                           lang:sweRegistry ,
                           lang:zhoRegistry ;
          lang:deu-note notes:DefnTransUnavail , notes:NoteTransUnavail ;
          lang:swe-note notes:NoteTransUnavail ;
          lang:rus-note notes:NoteTransDiff .

###  https://isotc211.geolexica.org/ld/concepts#client
:client rdf:type owl:NamedIndividual ,
                   skos:Concept ;
          skos:inScheme geolexica:GeolexicaConceptScheme ;
          geolexica:hasInfo info:Info45 ;
      #   geolexica:hasReview reviews:Review45 ;
          geolexica:hasLDAPI ldapi:ldapi45-json ,
                             ldapi:ldapi45-jsonld ,
                             ldapi:ldapi45-rdfxml ,
                             ldapi:ldapi45-skosrdf ;
          geolexica:hasLangCode lang:ara ,
                                lang:dan ,
                                lang:deu ,
                                lang:eng ,
                                lang:fin ,
                                lang:fra ,
                                lang:kor ,
                                lang:pol ,
                                lang:rus ,
                                lang:spa ,
                                lang:swe ,
                                lang:zho ;
          dcterms:identifier 45 ;
          skos:notation 45 ;
          rdfs:label "client" ;
          skos:definition "software component that can invoke an operation from a server"@en ,
                "أحد مكونات برنامج حاسب آلي قادر على تنفيذ التشغيل من خلال حاسب آلي خادم"@ar ,
                "softewarekomponent, der kan aktivere en operation fra en server"@da ,
                "Software-Komponente, die eine Operation von einem Server aufrufen kann"@de ,
                "ohjelmistokomponentti, joka voi kutsua operaatiota palvelimelta"@fi ,
                "composant logiciel pouvant invoquer une opération d&#39;un serveur"@fr ,
                "서버에게 연산을 호출할 수 있는 소프트웨어 컴포넌트"@ko ,
                "składnik oprogramowania, który może wywołać operację z serwera"@pl ,
                "компонент программного обеспечения, который   может вызвать операцию с сервера"@ru ,
                "componente software que puede solicitar una operación de un servidor"@es ,
                "program som kan begära en tjänst från en server"@sv ,
                "能从服务器端调用操作的软件组件。"@zh ;
          skos:prefLabel "client"@en ,
                "عميل"@ar ,
                "klient"@da ,
                "Client"@de ,
                "asiakassovellus"@fi ,
                "client"@fr ,
                "클라이언트"@ko ,
                "klient"@pl ,
                "клиент"@ru ,
                "cliente"@es ,
                "klient"@sv ,
                "客户端"@zh ;
          skos:altLabel "asiakasohjelma"@fi ;
          geolexica:origin lang:araRegistry ,
                           lang:danRegistry ,
                           lang:deuRegistry ,
                           lang:engRegistry ,
                           lang:finRegistry ,
                           lang:fraRegistry ,
                           lang:korRegistry ,
                           lang:polRegistry ,
                           lang:rusRegistry ,
                           lang:spaRegistry ,
                           lang:sweRegistry ,
                           lang:zhoRegistry ;
          lang:fra-note notes:NoteTransDiff .

###  https://isotc211.geolexica.org/ld/concepts#closure
:closure rdf:type owl:NamedIndividual ,
                   skos:Concept ;
          skos:inScheme geolexica:GeolexicaConceptScheme ;
          geolexica:hasInfo info:Info46 ;
          geolexica:hasReview reviews:Review46 ;
          geolexica:hasLDAPI ldapi:ldapi46-json ,
                             ldapi:ldapi46-jsonld ,
                             ldapi:ldapi46-rdfxml ,
                             ldapi:ldapi46-skosrdf ;
          geolexica:hasLangCode lang:ara ,
                                lang:dan ,
                                lang:deu ,
                                lang:eng ,
                                lang:fin ,
                                lang:fra ,
                                lang:kor ,
                                lang:pol ,
                                lang:rus ,
                                lang:spa ,
                                lang:swe ,
                                lang:zho ;
          dcterms:identifier 46 ;
          skos:notation 46 ;
          rdfs:label "closure" ;
          skos:definition "union of the interior and boundary of a topological or geometric object"@en ;
  skos:definition "اتحاد المكونات الداخلية والحدود ليكان طوبولوجي أو هندسي"@ar ;
  skos:definition "foreningsmængden af indholdet af og afgrænsningen af et topologisk eller geometrisk objekt"@da ;
  skos:definition "Vereinigung des Inneren und der Grenze eines topologischen oder geometrischen Objekts"@de ;
  skos:definition "topologisen tai geometrisen objektin sisäpuolen ja rajauksen muodostama kokonaisuus"@fi ;
  skos:definition "union de l&#39;intérieur et de la frontière d&#39;un objet topologique ou géométrique"@fr ;
  skos:definition "位相オブジェクト又は幾何オブジェクトの内部と境界との和集合。"@ja ;
  skos:definition "위상 객체 또는 기하 객체의 내부와 경계의 합집합"@ko ;
  skos:definition "sesuatu yang ditutup"@ms ;
  skos:definition "suma wnętrza i granicy obiektu topologicznego lub obiektu geometrycznego"@pl ;
  skos:definition "объединение внутренней области и границы топологического или геометрического объекта"@ru ;
  skos:definition "unión del interior y de la frontera de un objeto geométrico o topológico"@es ;
  skos:definition "unionen av avgränsningen hos ett rumsligt objekt och objektet självt"@sv ;
  skos:definition "拓扑对象或几何对象的内部与边界的并集。"@zh ;
  skos:prefLabel "closure"@en ;
  skos:prefLabel "مغلق"@ar ;
  skos:prefLabel "lukket enhed"@da ;
  skos:prefLabel "Abschluss"@de ;
  skos:prefLabel "sulkeuma"@fi ;
  skos:prefLabel "fermeture"@fr ;
  skos:prefLabel "閉包"@ja ;
  skos:prefLabel "폐합"@ko ;
  skos:prefLabel "tutupan"@ms ;
  skos:prefLabel "domknięcie"@pl ;
  skos:prefLabel "замкнутая область"@ru ;
  skos:prefLabel "cerramiento"@es ;
  skos:prefLabel "inneslutning"@sv ;
  skos:prefLabel "闭包"@zh ;
          geolexica:origin lang:araRegistry ,
                           lang:danRegistry ,
                           lang:deuRegistry ,
                           lang:engRegistry ,
                           lang:finRegistry ,
                           lang:fraRegistry ,
                           lang:korRegistry ,
                           lang:polRegistry ,
                           lang:rusRegistry ,
                           lang:spaRegistry ,
                           lang:sweRegistry ,
                           lang:zhoRegistry .

###  https://isotc211.geolexica.org/ld/concepts#cluster2
:cluster2 rdf:type owl:NamedIndividual ,
                   skos:Concept ;
          skos:inScheme geolexica:GeolexicaConceptScheme ;
          geolexica:hasInfo info:Info47 ;
        #   geolexica:hasReview reviews:Review47 ;
          geolexica:hasLDAPI ldapi:ldapi47-json ,
                             ldapi:ldapi47-jsonld ,
                             ldapi:ldapi47-rdfxml ,
                             ldapi:ldapi47-skosrdf ;
          geolexica:hasLangCode lang:ara ,
                                lang:dan ,
                                lang:deu ,
                                lang:eng ,
                                lang:fin ,
                                lang:fra ,
                                lang:kor ,
                                lang:pol ,
                                lang:rus ,
                                lang:spa ,
                                lang:swe ,
                                lang:zho ;
          dcterms:identifier 47 ;
          skos:notation 47 ;
          rdfs:label "cluster" ;

  skos:definition "union of the interior and boundary of a topological or geometric object"@en ;
  skos:definition "collection of targets potentially heterogeneous (each satisfying a different query criteria) whose locations fall within a small neighbourhood."@en ;
  skos:definition "مجموعة أهداف غير متجانسة  ( كلاً منها يحقق معيار استعلام مختلف) تقع مواضيعها ضمن جوار قريب"@ar ;
  skos:definition "kokoelma mahdollisesti heterogeenisia (eri hakuehdot täyttäviä) kohteita, jotka sijaitsevat lähekkäin"@fi ;
  skos:definition "ensemble de cibles potentiellement hétérogènes (chacun satisfaisant un critère de requête différent) dont la localisation se trouve dans un voisinage proche"@fr ;
  skos:definition "그 위치가 소규모 인접군 지역 내에 존재하는 잠재적으로 이질적인(서로 다른 질의 기준을 만족할 수 있는) 대상들의 모음"@ko ;
  skos:definition "beberapa benda (spt pulau) yg berada dlm kumpulan dan dikira satu/ sesuatu yg berada dlm kelompok"@ms ;
  skos:definition "совокупность целей, потенциально гетерогенных (каждая цель удовлетворяет своему критерию запроса), попадающих в некоторую малую окрестность"@ru ;
  skos:definition "colección de objetivos potencialmente heterogéneos (cada uno satisfaciendo un criterio de consulta diferente), cuyas ubicaciones caen dentro de una pequeña vecindad"@es ;
  skos:definition "samling av objekt som i något avseende liknar varandra eller ligger tillräckligt nära varandra och som därför behandlas som en enhet"@sv ;
  skos:definition "地点位于一个小区域内的具有潜在的不同类别的目标集合（每个目标都满足不同的查询准则）。"@zh ;

  skos:prefLabel "cluster"@en ;
  skos:prefLabel "تجميع"@ar ;
  skos:prefLabel "Cluster"@de ;
  skos:prefLabel "klusteri"@fi ;
  skos:prefLabel "grappe"@fr ;
  skos:prefLabel "클러스터"@ko ;
  skos:prefLabel "gugusan"@ms ;
  skos:prefLabel "кластер"@ru ;
  skos:prefLabel "cluster"@es ;
  skos:prefLabel "kluster"@sv ;
  skos:prefLabel "簇"@zh ;
  skos:altLabel "ryväs"@fi ;

          geolexica:origin lang:araRegistry ,
                           lang:danRegistry ,
                           lang:deuRegistry ,
                           lang:engRegistry ,
                           lang:finRegistry ,
                           lang:fraRegistry ,
                           lang:korRegistry ,
                           lang:rusRegistry ,
                           lang:msaRegistry ,
                           lang:spaRegistry ,
                           lang:sweRegistry ,
                           lang:zhoRegistry ;
          lang:deu-note notes:DefnTransUnavail ;
          lang:fra-note notes:NoteTransDiff .


###  https://isotc211.geolexica.org/ld/concepts#coboundary
:coboundary rdf:type owl:NamedIndividual ,
                   skos:Concept ;
          skos:inScheme geolexica:GeolexicaConceptScheme ;
          geolexica:hasInfo info:Info48 ;
          geolexica:hasReview reviews:Review48 ;
          geolexica:hasLDAPI ldapi:ldapi48-json ,
                             ldapi:ldapi48-jsonld ,
                             ldapi:ldapi48-rdfxml ,
                             ldapi:ldapi48-skosrdf ;
          geolexica:hasLangCode lang:ara ,
                                lang:dan ,
                                lang:deu ,
                                lang:eng ,
                                lang:fin ,
                                lang:fra ,
                                lang:kor ,
                                lang:pol ,
                                lang:rus ,
                                lang:spa ,
                                lang:swe ,
                                lang:zho ;
          dcterms:identifier 48 ;
          skos:notation 48 ;
          rdfs:label "coboundary" ;

skos:definition "set of topological primitives of higher topological dimension associated with a particular topological object, such that this topological object is in each of their boundaries"@en ;
  skos:definition "مجموعة عناصر طوبولوجية بدائية ذات بعد طوبولوجي أعلى ترتبط بكيان طوبولوجي معيَّن  بحيث يكون هذا الكيان الطوبولوجي في حدود كل منها"@ar ;
  skos:definition "en mængde af topologiske grundformer af højere topologisk dimension, som er forbundet med et bestemt topologisk objekt, således at dette topologiske objekt er i hver af deres afgrænsning"@da ;
  skos:definition "joukko korkeamman topologisen ulottuvuuden omaavia topologisia primitiivejä, jotka liittyvät tiettyyn topologiseen objektiin siten, että tämä topologinen objekti on mukana jokaisen primitiivin rajauksessa"@fi ;
  skos:definition "ensemble de primitives topologiques de dimension topologique supérieure associé à un objet topologique particulier, tel que cet objet topologique appartient à la frontière de chacune d&#39;elles."@fr ;
  skos:definition "ある位相オブジェクトに対応して，その位相オブジェクトを境界としてもつ，より高い位相次元の位相プリミティブの集合。"@ja ;
  skos:definition "특정 위상 객체를 구성하는 높은 위상 차원의 위상 원시 객체 집합으로, 이 위상 객체는 위상 원시 객체의 각 경계에 존재함"@ko ;
  skos:definition "zbiór prostych elementów topologicznych o większym wymiarze topologicznym, powiązanych z danym obiektem topologicznym w taki sposób, że ten topologiczny obiekt należy do granicy każdego z nich"@pl ;
  skos:definition "множество топологических примитивов более высокой топологической размерности, так ассоциированных с определенным топологическим объектом,  что  данный  топологический объект принадлежит границе каждого из них"@ru ;
  skos:definition "conjunto de primitivas topológicas, de dimensión topológica mayor, asociadas a un objeto topológico particular de tal modo, que este objeto topológico está en cada una de las fronteras del conjunto"@es ;
  skos:definition "samling av de topologiska objekt för vilka ett och samma topologiska objekt ingår i avgränsningen"@sv ;
  skos:definition "与特定的拓扑对象相关联，具有更高维数的拓扑单形的集合，这个拓扑对象在这些更高维数的拓扑单形的边界上。"@zh ;

  skos:prefLabel "coboundary"@en ;
  skos:prefLabel "حدود مشتركة"@ar ;
  skos:prefLabel "fællesgrænse"@da ;
  skos:prefLabel "kettenartig verknüpfte Grenze"@de ;
  skos:prefLabel "yhteisrajaus"@fi ;
  skos:prefLabel "co-frontière"@fr ;
  skos:prefLabel "双対境界"@ja ;
  skos:prefLabel "공유 경계"@ko ;
  skos:prefLabel "kosempadan"@ms ;
  skos:prefLabel "współgranica,  kogranica"@pl ;
  skos:prefLabel "кограница"@ru ;
  skos:prefLabel "cofrontera"@es ;
  skos:prefLabel "gränsberörda objekt"@sv ;
  skos:prefLabel "余边界"@zh ;
  
          geolexica:origin lang:araRegistry ,
                           lang:danRegistry ,
                           lang:deuRegistry ,
                           lang:engRegistry ,
                           lang:finRegistry ,
                           lang:fraRegistry ,
                           lang:korRegistry ,
                           lang:jpnRegistry ,
                           lang:rusRegistry ,
                           lang:polRegistry ,
                           lang:msaRegistry ,
                           lang:spaRegistry ,
                           lang:sweRegistry ,
                           lang:zhoRegistry ;
          lang:deu-note notes:DefnTransUnavail , notes:NoteTransUnavail ;
          lang:fra-note notes:NoteTransDiff .


###  https://isotc211.geolexica.org/ld/concepts#code
:code rdf:type owl:NamedIndividual ,
                   skos:Concept ;
          skos:inScheme geolexica:GeolexicaConceptScheme ;
          geolexica:hasInfo info:Info49 ;
          geolexica:hasReview reviews:Review49 ;
          geolexica:hasLDAPI ldapi:ldapi49-json ,
                             ldapi:ldapi49-jsonld ,
                             ldapi:ldapi49-rdfxml ,
                             ldapi:ldapi49-skosrdf ;
          geolexica:hasLangCode lang:ara ,
                                lang:dan ,
                                lang:deu ,
                                lang:eng ,
                                lang:fin ,
                                lang:fra ,
                                lang:kor ,
                              # lang:pol ,
                                lang:rus ,
                                lang:msa ,
                                lang:spa ,
                                lang:swe ,
                                lang:zho ;
          dcterms:identifier 49 ;
          skos:notation 49 ;
          rdfs:label "code" ;

  skos:definition "representation of a label according to a specified scheme"@en ;
  skos:definition "تمثيل لعلامة مميزة وفقاً لمخطط محدد"@ar ;
  skos:definition "angivelse af et label ud fra en specificeret skema"@da ;
  skos:definition "tunnuksen esitys tietyn mallin mukaisesti"@fi ;
  skos:definition "représentation d&#39;un libellé selon une méthode spécifiée"@fr ;
  skos:definition "특정한 형식에 따른 라벨의 표현"@ko ;
  skos:definition "1. Set peraturan tertentu yang menunjukkan cara bagaimana data boleh diwakili. 2. Peraturan dan resam yang menentukan bagaimana isyarat yang mewakili data boleh dibentuk, dihantar, diterima, dan diproses dalam suatu sistem perhubungan. 3. Bentuk berlambang yang mewakili data atau suruhan atur cara komputer atau mikropemproses yang boleh diterima dan diproses oleh mesin tersebut."@ms ;
  skos:definition "представление строки символов в соответствии со специфицированной схемой"@ru ;
  skos:definition "representación de una etiqueta de acuerdo a un esquema determinado"@es ;
  skos:definition "data som skapats enligt bestämda regler och som inte kan tolkas direkt"@sv ;
  skos:definition "基于所定义模式的符号表示。"@zh ;

  skos:prefLabel "code"@en ;
  skos:prefLabel "رمز"@ar ;
  skos:prefLabel "kode"@da ;
  skos:prefLabel "Code"@de ;
  skos:prefLabel "koodi"@fi ;
  skos:prefLabel "code"@fr ;
  skos:prefLabel "코드"@ko ;
  skos:prefLabel "kod"@ms ;
  skos:prefLabel "код"@ru ;
  skos:prefLabel "código"@es ;
  skos:prefLabel "kod"@sv ;
  skos:prefLabel "代码"@zh ;
  
          geolexica:origin lang:araRegistry ,
                           lang:danRegistry ,
                           lang:deuRegistry ,
                           lang:engRegistry ,
                           lang:finRegistry ,
                           lang:fraRegistry ,
                           lang:korRegistry ,
                           lang:jpnRegistry ,
                           lang:rusRegistry ,
                      #    lang:polRegistry ,
                           lang:msaRegistry ,
                           lang:spaRegistry ,
                           lang:sweRegistry ,
                           lang:zhoRegistry ;
          lang:deu-note notes:DefnTransUnavail .


###  https://isotc211.geolexica.org/ld/concepts#codelist
:codelist rdf:type owl:NamedIndividual ,
                   skos:Concept ;
          skos:inScheme geolexica:GeolexicaConceptScheme ;
          geolexica:hasInfo info:Info50 ;
          geolexica:hasReview reviews:Review50 ;
          geolexica:hasLDAPI ldapi:ldapi50-json ,
                             ldapi:ldapi50-jsonld ,
                             ldapi:ldapi50-rdfxml ,
                             ldapi:ldapi50-skosrdf ;
          geolexica:hasLangCode lang:ara ,
                                lang:dan ,
                                lang:deu ,
                                lang:eng ,
                                lang:fin ,
                                lang:fra ,
                                lang:kor ,
                                lang:pol ,
                                lang:rus ,
                                lang:spa ,
                                lang:swe ,
                                lang:zho ;
          dcterms:identifier 50 ;
          skos:notation 50 ;
          rdfs:label "codelist" ;

  skos:definition "value domain including a code for each permissible value"@en ;
  skos:definition "مجال للقيم يحتوي على رمز لكل قيمة مسموح بها"@ar ;
  skos:definition "Werteliste einschließlich eines Codes für jeden Wert"@de ;
  skos:definition "arvoalue, joka muodostuu arvojen luettelosta, jota voi laajentaa"@fi ;
  skos:definition "domaine de valeurs comprenant un code pour chaque valeur autorisée"@fr ;
  skos:definition "각 코드에 따른 허용 값을 제시하는 값 영역"@ko ;
  skos:definition "область значений,  содержащая код для каждого допустимого значения"@ru ;
  skos:definition "dominio de valores que incluye un código para cada uno de los valores permitidos"@es ;
  skos:definition "diskret värdedomän där varje värde tilldelats en inom listan unik beteckning"@sv ;
  skos:definition "包括每一个允许值代码的值域。"@zh ;

  skos:prefLabel "codelist"@en ;
  skos:prefLabel "قائمة الرموز"@ar ;
  skos:prefLabel "Codeliste"@de ;
  skos:prefLabel "koodiluettelo"@fi ;
  skos:prefLabel "liste de codes"@fr ;
  skos:prefLabel "코드 목록"@ko ;
  skos:prefLabel "кодовый спISOк"@ru ;
  skos:prefLabel "lista de códigos (codelist)"@es ;
  skos:prefLabel "kodlista"@sv ;
  skos:prefLabel "代码表"@zh ;
  
          geolexica:origin lang:araRegistry ,
                      #    lang:danRegistry ,
                           lang:deuRegistry ,
                           lang:engRegistry ,
                           lang:finRegistry ,
                           lang:fraRegistry ,
                           lang:korRegistry ,
                      #    lang:jpnRegistry ,
                           lang:rusRegistry ,
                      #    lang:polRegistry ,
                      #    lang:msaRegistry ,
                           lang:spaRegistry ,
                           lang:sweRegistry ,
                           lang:zhoRegistry .

###  https://isotc211.geolexica.org/ld/concepts#codespace
:codespace rdf:type owl:NamedIndividual ,
                   skos:Concept ;
          skos:inScheme geolexica:GeolexicaConceptScheme ;
          geolexica:hasInfo info:Info51 ;
          geolexica:hasReview reviews:Review51 ;
          geolexica:hasLDAPI ldapi:ldapi51-json ,
                             ldapi:ldapi51-jsonld ,
                             ldapi:ldapi51-rdfxml ,
                             ldapi:ldapi51-skosrdf ;
          geolexica:hasLangCode lang:ara ,
                                # lang:dan ,
                                lang:deu ,
                                lang:eng ,
                                lang:fin ,
                                lang:fra ,
                                lang:kor ,
                                # lang:pol ,
                                lang:rus ,
                                lang:spa ,
                                # lang:swe ,
                                lang:zho ;
          dcterms:identifier 51 ;
          skos:notation 51 ;
          rdfs:label "codespace" ;

  skos:definition "rule or authority for a code, name, term or category"@en ;
  skos:definition "قانون أو سلطة يستمد منها رمز أو اسم أو مصطلح أو فئة"@ar ;
  skos:definition "Regel oder Vorgabe für einen Code, Namen, Begriff oder Kategorie"@de ;
  skos:definition "valtuusalue koodille, nimelle, termille tai kategorialle"@fi ;
  skos:definition "règle ou autorité relative à un code, un nom, un terme ou une catégorie"@fr ;
  skos:definition "코드, 이름, 용어, 분류 체계 등에 대한 규정"@ko ;
  skos:definition "правило или уполномоченный орган,  определенные для назначения кода, имени, термина или категории"@ru ;
  skos:definition "regla o autoridad para un código, nombre, término o categoría"@es ;
  skos:definition "确认代码、名称、术语或类别的规则或者典据。"@zh ;

  skos:prefLabel "codespace"@en ;
  skos:prefLabel "حيز الرمز"@ar ;
  skos:prefLabel "Codespace"@de ;
  skos:prefLabel "koodiavaruus"@fi ;
  skos:prefLabel "espace de codage"@fr ;
  skos:prefLabel "코드 영역"@ko ;
  skos:prefLabel "пространство кодов"@ru ;
  skos:prefLabel "espacio de códigos (codespace)"@es ;
  skos:prefLabel "代码空间"@zh ;
  
          geolexica:origin lang:araRegistry ,
                        #    lang:danRegistry ,
                           lang:deuRegistry ,
                           lang:engRegistry ,
                           lang:finRegistry ,
                           lang:fraRegistry ,
                           lang:korRegistry ,
                        #    lang:jpnRegistry ,
                           lang:rusRegistry ,
                        #    lang:polRegistry ,
                        #    lang:msaRegistry ,
                           lang:spaRegistry ,
                        #    lang:sweRegistry ,
                           lang:zhoRegistry ;
          lang:deu-note notes:DefnTransUnavail .


###  https://isotc211.geolexica.org/ld/concepts#complex_feature
:complex_feature rdf:type owl:NamedIndividual ,
                   skos:Concept ;
          skos:inScheme geolexica:GeolexicaConceptScheme ;
          geolexica:hasInfo info:Info52 ;
          geolexica:hasReview reviews:Review52 ;
          geolexica:hasLDAPI ldapi:ldapi52-json ,
                             ldapi:ldapi52-jsonld ,
                             ldapi:ldapi52-rdfxml ,
                             ldapi:ldapi52-skosrdf ;
          geolexica:hasLangCode lang:ara ,
                                # lang:dan ,
                                lang:deu ,
                                lang:eng ,
                                lang:fin ,
                                lang:fra ,
                                lang:kor ,
                                # lang:pol ,
                                lang:rus ,
                                lang:spa ,
                                # lang:swe ,
                                lang:zho ;
          dcterms:identifier 52 ;
          skos:notation 52 ;
          rdfs:label "complex feature" ;

  skos:definition "feature composed of other features"@en ;
  skos:definition "معلم مؤلف من معالم أخرى"@ar ;
  skos:definition "Feature, das sich aus anderen Objekten zusammensetzt"@de ;
  skos:definition "kohde, joka geometrialtaan on muutakin kuin lineaarista kaksiulotteista geometriaa"@fi ;
  skos:definition "entité composée d&#39;autres entités"@fr ;
  skos:definition "다수의 피처들로 구성된 피처"@ko ;
  skos:definition "obiekt składający się z innych obiektów"@pl ;
  skos:definition "пространственный объект, состоящий из нескольких простых и/или сложных пространственных объектов"@ru ;
  skos:definition "objeto geográfico compuesto de otros objetos geográficos"@es ;
  skos:definition "objekt sammansatt av andra objekt"@sv ;
  skos:definition "由其它要素组合而成的要素。"@zh ;

  skos:prefLabel "complex feature"@en ;
  skos:prefLabel "معلم مركَّب"@ar ;
  skos:prefLabel "komplexes Feature"@de ;
  skos:prefLabel "kompleksinen kohde"@fi ;
  skos:prefLabel "entité complexe"@fr ;
  skos:prefLabel "복합 지형지물"@ko ;
  skos:prefLabel "kompleks fitur"@ms ;
  skos:prefLabel "złożony obiekt geograficzny"@pl ;
  skos:prefLabel "сложный (пространственный ) объект"@ru ;
  skos:prefLabel "objeto geográfico complejo"@es ;
  skos:prefLabel "sammansatt objekt"@sv ;
  skos:prefLabel "复杂要素"@zh ;
  skos:altLabel "복합 피처"@ko ;
  
          geolexica:origin lang:araRegistry ,
                        #    lang:danRegistry ,
                           lang:deuRegistry ,
                           lang:engRegistry ,
                           lang:finRegistry ,
                           lang:fraRegistry ,
                           lang:korRegistry ,
                        #    lang:jpnRegistry ,
                           lang:rusRegistry ,
                           lang:polRegistry ,
                           lang:msaRegistry ,
                           lang:spaRegistry ,
                        #    lang:sweRegistry ,
                           lang:zhoRegistry ;
          lang:msa-note notes:DefnTransUnavail, notes:NoteTransDiff ;
          lang:rus-note notes:NoteTransDiff .


###  https://isotc211.geolexica.org/ld/concepts#composite_curve
:composite_curve rdf:type owl:NamedIndividual ,
                   skos:Concept ;
          skos:inScheme geolexica:GeolexicaConceptScheme ;
          geolexica:hasInfo info:Info55 ;
          geolexica:hasReview reviews:Review55 ;
          geolexica:hasLDAPI ldapi:ldapi55-json ,
                             ldapi:ldapi55-jsonld ,
                             ldapi:ldapi55-rdfxml ,
                             ldapi:ldapi55-skosrdf ;
          geolexica:hasLangCode lang:ara ,
                                lang:dan ,
                                lang:deu ,
                                lang:eng ,
                                lang:fin ,
                                lang:fra ,
                                lang:kor ,
                                lang:pol ,
                                lang:jpn ,
                                lang:msa ,
                                lang:rus ,
                                lang:spa ,
                                lang:swe ,
                                lang:zho ;
          dcterms:identifier 55 ;
          skos:notation 55 ;
          rdfs:label "composite curve" ;

  skos:definition "sequence of curves such that each curve (except the first) starts at the end point of the previous curve in the sequence"@en ;
  skos:definition "سلسلة من المنحنيات  بحيث أن كل منحنى منها (باستثناء المنحنى الأول) يبدأ من النقطة التي ينتهي عندها المنحنى الذي يسبقه"@ar ;
  skos:definition "sekvens af kurver dannet således, at hver kurve (undtagen den første) starter ved slutpunktet af den foregående kurve i sekvensen."@da ;
  skos:definition "Sequenz von Kurven, wobei jede Kurve (außer der ersten) am Endpunkt der vorhergehenden Kurve einer Sequenz beginnt"@de ;
  skos:definition "komposiitti, joka koostuu toisissaan kiinni olevista peräkkäisistä käyristä"@fi ;
  skos:definition "séquence de courbes telle que chaque courbe (sauf la première) commence au point final de la courbe précédente dans la séquence"@fr ;
  skos:definition "列の各曲線が（最初のものを除き）直前の曲線の終点から開始するような曲線の列。"@ja ;
  skos:definition "첫 번째 곡선을 제외한 각각의 곡선이 연속적으로 앞 곡선의 끝점에서 시작되는 곡선의 연속"@ko ;
  skos:definition "sekwencja krzywych, w której każda krzywa (poza pierwszą) zaczyna się w punkcie końcowym poprzedniej krzywej w sekwencji"@pl ;
  skos:definition "последовательность кривых, каждая из которых (за исключением первой)  начинается в конечной точке предшествующей ей кривой"@ru ;
  skos:definition "secuencia de curvas tal que cada curva (excepto la primera) empieza en el punto final de la curva anterior en la secuencia"@es ;
  skos:definition "sekvens av linjer där varje linje utom den första startar där föregående linje slutar"@sv ;
  skos:definition "曲线的序列，其每条（第一条除外）在该序列的上一条曲线的结尾处开始。"@zh ;

  skos:prefLabel "composite curve"@en ;
  skos:prefLabel "منحنى مركَّب"@ar ;
  skos:prefLabel "sammensat kurve"@da ;
  skos:prefLabel "zusammenhängende Kurve"@de ;
  skos:prefLabel "komposiittikäyrä"@fi ;
  skos:prefLabel "courbe composite"@fr ;
  skos:prefLabel "合成曲線"@ja ;
  skos:prefLabel "합성 곡선"@ko ;
  skos:prefLabel "lengkok gabungan"@ms ;
  skos:prefLabel "krzywa kompozytowa"@pl ;
  skos:prefLabel "составная кривая"@ru ;
  skos:prefLabel "curva compuesta"@es ;
  skos:prefLabel "sammansatt linje"@sv ;
  skos:prefLabel "组合曲线"@zh ;
  
          geolexica:origin lang:araRegistry ,
                           lang:danRegistry ,
                           lang:deuRegistry ,
                           lang:engRegistry ,
                           lang:finRegistry ,
                           lang:fraRegistry ,
                           lang:korRegistry ,
                           lang:jpnRegistry ,
                           lang:rusRegistry ,
                           lang:polRegistry ,
                           lang:msaRegistry ,
                           lang:spaRegistry ,
                           lang:sweRegistry ,
                           lang:zhoRegistry ;
          lang:deu-note notes:NoteTransUnavail ;
          lang:swe-note notes:NoteTransUnavail ;
          lang:msa-note notes:DefnTransUnavail , notes:NoteTransDiff .



###  https://isotc211.geolexica.org/ld/concepts#composite_solid
:composite_solid rdf:type owl:NamedIndividual ,
                   skos:Concept ;
          skos:inScheme geolexica:GeolexicaConceptScheme ;
          geolexica:hasInfo info:Info56 ;
          geolexica:hasReview reviews:Review56 ;
          geolexica:hasLDAPI ldapi:ldapi56-json ,
                             ldapi:ldapi56-jsonld ,
                             ldapi:ldapi56-rdfxml ,
                             ldapi:ldapi56-skosrdf ;
          geolexica:hasLangCode lang:ara ,
                                lang:dan ,
                                lang:deu ,
                                lang:eng ,
                                lang:fin ,
                                lang:fra ,
                                lang:kor ,
                                lang:pol ,
                                lang:jpn ,
                                lang:msa ,
                                lang:rus ,
                                lang:spa ,
                                lang:swe ,
                                lang:zho ;
          dcterms:identifier 56 ;
          skos:notation 56 ;
          rdfs:label "composite solid" ;

  skos:definition "connected set of solids adjoining one another along shared boundary surfaces"@en ;
  skos:definition "مجموعة مجسمات متصلة ومجاورة بعضها ببعض على طول أسطح الحدود المشتركه"@ar ;
  skos:definition "samlet sæt af legemer, der er forbundet med hinanden langs fælles grænseflader"@da ;
  skos:definition "verbundene Menge von Körpern, die gegenseitig entlang von gemeinsamen Grenzflächen verbunden sind"@de ;
  skos:definition "komposiitti, joka koostuu toisissaan kiinni olevista kappaleista"@fi ;
  skos:definition "ensemble de solides connectés attenants l&#39;un à l&#39;autre le long d&#39;une frontière surfacique partagée"@fr ;
  skos:definition "共有された境界曲面に沿って互いに隣接する立体の連結した集合。"@ja ;
  skos:definition "공유 경계 표면을 따라 서로 연결된 입방체의 집합"@ko ;
  skos:definition "set terhubung pepejal bersebelahan di sepanjang permukaan sempadan yang dikongsi"@ms ;
  skos:definition "spójny zbiór brył dołączonych, przylegających jedna do drugiej poprzez współdzielone powierzchnie graniczne"@pl ;
  skos:definition "связное  множество тел, примыкающих друг к другу по общим ограничивающим поверхностям"@ru ;
  skos:definition "conjunto conectado de sólidos que son colindantes unos con otros a través de las superficies de frontera que comparten"@es ;
  skos:definition "samling kroppar där varje kropp delar gränsyta med minst en av de övriga kropparna"@sv ;
  skos:definition "沿着共享边界曲面相邻且相连的体的集合。"@zh ;

  skos:prefLabel "composite solid"@en ;
  skos:prefLabel "مجسم مركب"@ar ;
  skos:prefLabel "sammensat legeme"@da ;
  skos:prefLabel "zusammenhängender Körper"@de ;
  skos:prefLabel "komposiittikappale"@fi ;
  skos:prefLabel "solide composite"@fr ;
  skos:prefLabel "合成立体"@ja ;
  skos:prefLabel "합성 입방체"@ko ;
  skos:prefLabel "pepejal komposit"@ms ;
  skos:prefLabel "bryła kompozytowa"@pl ;
  skos:prefLabel "составное тело"@ru ;
  skos:prefLabel "sólido compuesto"@es ;
  skos:prefLabel "sammansatt kropp"@sv ;
  skos:prefLabel "组合体"@zh ;
  
          geolexica:origin lang:araRegistry ,
                           lang:danRegistry ,
                           lang:deuRegistry ,
                           lang:engRegistry ,
                           lang:finRegistry ,
                           lang:fraRegistry ,
                           lang:korRegistry ,
                           lang:jpnRegistry ,
                           lang:rusRegistry ,
                           lang:polRegistry ,
                           lang:msaRegistry ,
                           lang:spaRegistry ,
                           lang:sweRegistry ,
                           lang:zhoRegistry ;
          lang:deu-note notes:NoteTransUnavail ;
          lang:msa-note notes:NoteTransUnavail ;
          lang:swe-note notes:NoteTransUnavail .


###  https://isotc211.geolexica.org/ld/concepts#composite_surface
:composite_surface rdf:type owl:NamedIndividual ,
                   skos:Concept ;
          skos:inScheme geolexica:GeolexicaConceptScheme ;
          geolexica:hasInfo info:Info57 ;
          geolexica:hasReview reviews:Review57 ;
          geolexica:hasLDAPI ldapi:ldapi57-json ,
                             ldapi:ldapi57-jsonld ,
                             ldapi:ldapi57-rdfxml ,
                             ldapi:ldapi57-skosrdf ;
          geolexica:hasLangCode lang:ara ,
                                lang:dan ,
                                lang:deu ,
                                lang:eng ,
                                lang:fin ,
                                lang:fra ,
                                lang:kor ,
                                lang:pol ,
                                lang:jpn ,
                                lang:msa ,
                                lang:rus ,
                                lang:spa ,
                                lang:swe ,
                                lang:zho ;
          dcterms:identifier 57 ;
          skos:notation 57 ;
          rdfs:label "composite surface" ;

  skos:definition "connected set of surfaces adjoining one another along shared boundary curves"@en ;
  skos:definition "مجموعة أسطح متصلة ببعضها  ومجاورة بعضها لبعض على طول منحنيات الحدود المشتركه"@ar ;
  skos:definition "samlet sæt af flader, der er forbundet med hinanden langs fælles grænsekurv"@da ;
  skos:definition "verbundene Menge von Flächen, die gegenseitig entlang von gemeinsamen Grenzkurven verbunden sind"@de ;
  skos:definition "komposiitti, joka koostuu toisissaan kiinni olevista pinnoista"@fi ;
  skos:definition "ensemble connecté de surfaces jointes le long d&#39;une frontière curviligne partagée"@fr ;
  skos:definition "共有された境界曲線に沿って互いに隣接する曲面の連結な集合。"@ja ;
  skos:definition "공유 경계 곡선을 따라 서로 연결된 표면의 집합"@ko ;
  skos:definition "set permukaan terhubung yang bersebelahan satu sama lain di sepanjang lengkungan sempadan bersama"@ms ;
  skos:definition "spójny zbiór powierzchni przylegających jedna do drugiej poprzez współdzielone krzywe graniczne"@pl ;
  skos:definition "связное множество поверхностей, примыкающих друг к другу по общим граничным кривым"@ru ;
  skos:definition "conjunto conectado de superficies que son colindantes unas con otras a través de las curvas de frontera que comparten"@es ;
  skos:definition "samling ytor där varje yta delar gränslinje med minst en av de övriga ytorna"@sv ;
  skos:definition "沿着共享边界曲线相邻并相连的曲面的集合。"@zh ;

  skos:prefLabel "composite surface"@en ;
  skos:prefLabel "سطح مركَّب"@ar ;
  skos:prefLabel "sammensat flade"@da ;
  skos:prefLabel "zusammenhängende Fläche"@de ;
  skos:prefLabel "komposiittipinta"@fi ;
  skos:prefLabel "surface composite"@fr ;
  skos:prefLabel "合成曲面"@ja ;
  skos:prefLabel "합성 표면"@ko ;
  skos:prefLabel "permukaan komposit"@ms ;
  skos:prefLabel "powierzchnia kompozytowa"@pl ;
  skos:prefLabel "составная поверхность"@ru ;
  skos:prefLabel "superficie compuesta"@es ;
  skos:prefLabel "sammansatt yta"@sv ;
  skos:prefLabel "组合曲面"@zh ;
  
          geolexica:origin lang:araRegistry ,
                           lang:danRegistry ,
                           lang:deuRegistry ,
                           lang:engRegistry ,
                           lang:finRegistry ,
                           lang:fraRegistry ,
                           lang:korRegistry ,
                           lang:jpnRegistry ,
                           lang:rusRegistry ,
                           lang:polRegistry ,
                           lang:msaRegistry ,
                           lang:spaRegistry ,
                           lang:sweRegistry ,
                           lang:zhoRegistry ;
          lang:deu-note notes:NoteTransUnavail ;
          lang:msa-note notes:NoteTransUnavail ;
          lang:swe-note notes:NoteTransUnavail .


###  https://isotc211.geolexica.org/ld/concepts#computational_geometry
:computational_geometry rdf:type owl:NamedIndividual ,
                   skos:Concept ;
          skos:inScheme geolexica:GeolexicaConceptScheme ;
          geolexica:hasInfo info:Info61 ;
          geolexica:hasReview reviews:Review61 ;
          geolexica:hasLDAPI ldapi:ldapi61-json ,
                             ldapi:ldapi61-jsonld ,
                             ldapi:ldapi61-rdfxml ,
                             ldapi:ldapi61-skosrdf ;
          geolexica:hasLangCode lang:ara ,
                                lang:dan ,
                                lang:deu ,
                                lang:eng ,
                                lang:fin ,
                                lang:fra ,
                                lang:kor ,
                                lang:pol ,
                                lang:jpn ,
                                # lang:msa ,
                                lang:rus ,
                                lang:spa ,
                                lang:swe ,
                                lang:zho ;
          dcterms:identifier 61 ;
          skos:notation 61 ;
          rdfs:label "computational geometry" ;

  skos:definition "manipulation of and calculations with geometric representations for the implementation of geometric operations"@en ;
  skos:definition "المعالجات والطرق الحسابية للتمثيل الهندسي لتنفيذ العمليات الهندسية الفراغيه"@ar ;
  skos:definition "manipulationer og beregninger af geometriske repræsentationer med det formål at udføre geometriske operationer"@da ;
  skos:definition "geometriailmentymien käsittely ja niillä laskeminen geometristen operaatioiden suorittamiseksi"@fi ;
  skos:definition "manipulation et calculs de représentations géométriques pour l&#39;implémentation d&#39;opérations géométriques"@fr ;
  skos:definition "幾何演算を実装するための，幾何表現に関する操作及び計算。"@ja ;
  skos:definition "기하 연산을 구현하기 위한 기하 표현의 계산과 조작"@ko ;
  skos:definition "działania i obliczenia na reprezentacjach geometrycznych dla celów implementacji operacji geometrycznych"@pl ;
  skos:definition "манипуляции и вычисления, призводимые с геометрическими представлениями  при реализации геометрических операций"@ru ;
  skos:definition "cálculo y manipulación de representaciones geométricas para la implementación de operaciones geométricas"@es ;
  skos:definition "bearbetning och beräkning utgående från geometrisk representation för att bestämma geometriska förhållanden"@sv ;
  skos:definition "几何表达式的处理与计算，用于几何操作的实现。"@zh ;

  skos:prefLabel "computational geometry"@en ;
  skos:prefLabel "الهندسة الفراغية الحسابية"@ar ;
  skos:prefLabel "algoritmisk geometri"@da ;
  skos:prefLabel "algorithmische Geometrie"@de ;
  skos:prefLabel "laskennallinen geometria"@fi ;
  skos:prefLabel "géométrie calculée"@fr ;
  skos:prefLabel "計算幾何"@ja ;
  skos:prefLabel "계산 기하"@ko ;
  skos:prefLabel "hitungan geometri"@ms ;
  skos:prefLabel "geometria obliczeniowa"@pl ;
  skos:prefLabel "вычислительная геометрия"@ru ;
  skos:prefLabel "geometría computacional"@es ;
  skos:prefLabel "beräkningsgeometri"@sv ;
  skos:prefLabel "计算几何"@zh ;

          geolexica:origin lang:araRegistry ,
                           lang:danRegistry ,
                           lang:deuRegistry ,
                           lang:engRegistry ,
                           lang:finRegistry ,
                           lang:fraRegistry ,
                           lang:korRegistry ,
                           lang:jpnRegistry ,
                           lang:rusRegistry ,
                           lang:polRegistry ,
                        #    lang:msaRegistry ,
                           lang:spaRegistry ,
                           lang:sweRegistry ,
                           lang:zhoRegistry ;
          lang:deu-note notes:NoteTransUnavail, notes:DefnTransUnavail ;
          lang:msa-note notes:NoteTransUnavail, notes:DefnTransUnavail ;
          lang:swe-note notes:NoteTransUnavail .


###  https://isotc211.geolexica.org/ld/concepts#computational_topology
:computational_topology rdf:type owl:NamedIndividual ,
                   skos:Concept ;
          skos:inScheme geolexica:GeolexicaConceptScheme ;
          geolexica:hasInfo info:Info62 ;
          geolexica:hasReview reviews:Review62 ;
          geolexica:hasLDAPI ldapi:ldapi62-json ,
                             ldapi:ldapi62-jsonld ,
                             ldapi:ldapi62-rdfxml ,
                             ldapi:ldapi62-skosrdf ;
          geolexica:hasLangCode lang:ara ,
                                lang:dan ,
                                lang:deu ,
                                lang:eng ,
                                lang:fin ,
                                lang:fra ,
                                lang:kor ,
                                lang:pol ,
                                lang:jpn ,
                                lang:msa ,
                                lang:rus ,
                                lang:spa ,
                                lang:swe ,
                                lang:zho ;
          dcterms:identifier 62 ;
          skos:notation 62 ;
          rdfs:label "computational topology" ;

  skos:definition "topological concepts, structures and algebra that aid, enhance or define operations on topological objects usually performed in computational geometry"@en ;
  skos:definition "المفاهيم والهياكل والجبر الطوبولوجي التي تساعد أو تعزز أو تعرِّف العمليات الحسابية التي تجرى على الكيانات الطوبولوجية والتي يتم إجراؤها عادة في إطار الهندسة الفراغية الحسابية"@ar ;
  skos:definition "topologiske begreber, strukturer og algebra, som hjælper, forstærker eller definerer operationer på topologiske objekter, og som sædvanligvis anvendes i algoritmisk geometri"@da ;
  skos:definition "topologiset käsitteet, rakenteet ja algebra, joilla tuetaan, tehostetaan tai määritellään topologisille objekteille tavallisesti laskennallisessa geometriassa suoritettavia operaatioita"@fi ;
  skos:definition "concepts topologiques, structures et algèbres aidant, améliorant ou définissant des opérations sur des objets topologiques exécutées habituellement sur une géométrie calculée"@fr ;
  skos:definition "通常，計算幾何において実行される位相オブジェクトの演算の支援，拡張又は定義を行う位相的な概念，構造及び代数。"@ja ;
  skos:definition "계산 기하에서 위상 객체에 대하여 일반적으로 수행되는 위상 개념, 구조, 대수 및 부가적 확장 또는 정의 연산"@ko ;
  skos:definition "pojęcia topologiczne, struktury i algebra, które wspomagają, rozszerzają lub definiują operacje na obiektach topologicznych, wykonywane zwykle w geometrii obliczeniowej"@pl ;
  skos:definition "топологические принципы, структуры и алгебра, нацеленные на то, чтобы расширить или определить операции с топологическими объектами, выполняемые обычно средствами вычислительной геометрии"@ru ;
  skos:definition "álgebra, estructuras y conceptos topológicos que apoyan, amplian o definen operaciones, normalmente ejecutadas sobre objetos geométricos"@es ;
  skos:definition "topologiska begrepp, strukturer och algebra som underlättar, förbättrar eller definierar operationer på topologiska objekt, vanligtvis utförda med beräkningsgeometri"@sv ;
  skos:definition "在计算几何中通常用来辅助、增强或定义在拓扑对象上进行操作的拓扑概念、拓扑结构和拓扑代数。"@zh ;

  skos:prefLabel "computational topology"@en ;
  skos:prefLabel "الطوبولوجيا الحسابيه"@ar ;
  skos:prefLabel "algoritmisk topologi"@da ;
  skos:prefLabel "algorithmische Topologie"@de ;
  skos:prefLabel "laskennallinen topologia"@fi ;
  skos:prefLabel "topologie calculée"@fr ;
  skos:prefLabel "計算位相幾何"@ja ;
  skos:prefLabel "계산 위상"@ko ;
  skos:prefLabel "hitungan topografi"@ms ;
  skos:prefLabel "topologia obliczeniowa"@pl ;
  skos:prefLabel "вычислительная топология"@ru ;
  skos:prefLabel "topología computacional"@es ;
  skos:prefLabel "beräkningstopologi"@sv ;
  skos:prefLabel "计算拓扑"@zh ;

          geolexica:origin lang:araRegistry ,
                           lang:danRegistry ,
                           lang:deuRegistry ,
                           lang:engRegistry ,
                           lang:finRegistry ,
                           lang:fraRegistry ,
                           lang:korRegistry ,
                           lang:jpnRegistry ,
                           lang:rusRegistry ,
                           lang:polRegistry ,
                           lang:msaRegistry ,
                           lang:spaRegistry ,
                           lang:sweRegistry ,
                           lang:zhoRegistry ;
          lang:deu-note notes:NoteTransUnavail, notes:DefnTransUnavail ;
          lang:msa-note notes:NoteTransUnavail, notes:DefnTransUnavail ;
          lang:swe-note notes:NoteTransUnavail .


###  https://isotc211.geolexica.org/ld/concepts#computational_viewpoint
:computational_viewpoint rdf:type owl:NamedIndividual ,
                   skos:Concept ;
          skos:inScheme geolexica:GeolexicaConceptScheme ;
          geolexica:hasInfo info:Info63 ;
          geolexica:hasReview reviews:Review63 ;
          geolexica:hasLDAPI ldapi:ldapi63-json ,
                             ldapi:ldapi63-jsonld ,
                             ldapi:ldapi63-rdfxml ,
                             ldapi:ldapi63-skosrdf ;
          geolexica:hasLangCode lang:ara ,
                                lang:dan ,
                                lang:deu ,
                                lang:eng ,
                                lang:fin ,
                                lang:fra ,
                                lang:kor ,
                                lang:pol ,
                                # lang:jpn ,
                                # lang:msa ,
                                lang:rus ,
                                lang:spa ,
                                lang:swe ,
                                lang:zho ;
          dcterms:identifier 63 ;
          skos:notation 63 ;
          rdfs:label "computational viewpoint" ;

  skos:definition "viewpoint on a system and its environment that enables distribution through functional decomposition of the system into objects which interact at interfaces"@en ;
  skos:definition "وجهة نظر حول نظام معين وبيئته التي تتيح إمكانية التوزيع من خلال التحليل الوظيفي للنظام إلى كيانات تتفاعل من خلال واجهات حاسب آلي"@ar ;
  skos:definition "synsvinkel på et system og dets omgivelser, som muliggør distribution gennem funktionel opdeling af systemet i objekter, der interagerer ved grænseflader (RM-ODP)"@da ;
  skos:definition "järjestelmän ja sen ympäristön tarkastelun näkökulma, joka kiinnittää huomiota siihen, miten järjestelmä toiminnallisesti jaetaan rajapintojen kautta vuorovaikuttaviin objekteihin"@fi ;
  skos:definition "point de vue sur un système et son environnement qui permet la répartition selon une décomposition fonctionnelle du système en objets interagissant à leurs interfaces"@fr ;
  skos:definition "시스템을 인터페이스를 통해 상호 작용하는 기능적 객체들로 분해함으로써 분산 처리를 가능하게 하는 개방형 시스템 및 그 환경에 대한 관점"@ko ;
  skos:definition "punkt widzenia (4.7) przyjęty dla systemu oraz jego otoczenia, który za pomocą dekompozycji funkcjonalnej umożliwia rozproszenie systemu na obiekty współpracujące ze sobą poprzez interfejsy"@pl ;
  skos:definition "точка зрения на систему и ее среду, предполагающая распределенную обработку через функциональную декомпозицию системы на объекты, которые взаимодействуют через интерфейсы"@ru ;
  skos:definition "punto de vista de un sistema y su entorno que permite la distribución a través de la descomposición funcional del sistema en objetos que interactúan con interfaces"@es ;
  skos:definition "perspektiv på ett system och dess omgivning som ger möjlighet att dela upp systemet i funktioner som samverkar via gränssnitt"@sv ;
  skos:definition "基于ODP系统及其环境能实现分布处理的视角，这个环境通过系统的功能分解能够在接口上实现对象交互。"@zh ;

  skos:prefLabel "computational viewpoint"@en ;
  skos:prefLabel "وجهة النظر الحسابية"@ar ;
  skos:prefLabel "beregningsmæssig synsvinkel"@da ;
  skos:prefLabel "Implementierungssicht"@de ;
  skos:prefLabel "toiminnallinen näkökulma"@fi ;
  skos:prefLabel "point de vue informatique"@fr ;
  skos:prefLabel "계산 관점"@ko ;
  skos:prefLabel "obliczeniowy punkt widzenia"@pl ;
  skos:prefLabel "вычислительный аспект"@ru ;
  skos:prefLabel "punto de vista computacional"@es ;
  skos:prefLabel "bearbetningsperspektiv"@sv ;
  skos:prefLabel "计算视角"@zh ;

          geolexica:origin lang:araRegistry ,
                           lang:danRegistry ,
                           lang:deuRegistry ,
                           lang:engRegistry ,
                           lang:finRegistry ,
                           lang:fraRegistry ,
                           lang:korRegistry ,
                        #    lang:jpnRegistry ,
                           lang:rusRegistry ,
                           lang:polRegistry ,
                        #    lang:msaRegistry ,
                           lang:spaRegistry ,
                           lang:sweRegistry ,
                           lang:zhoRegistry ;
          lang:deu-note notes:DefnTransUnavail .

###  https://isotc211.geolexica.org/ld/concepts#concept
:concept rdf:type owl:NamedIndividual ,
                   skos:Concept ;
          skos:inScheme geolexica:GeolexicaConceptScheme ;
          geolexica:hasInfo info:Info64 ;
          geolexica:hasReview reviews:Review64 ;
          geolexica:hasLDAPI ldapi:ldapi64-json ,
                             ldapi:ldapi64-jsonld ,
                             ldapi:ldapi64-rdfxml ,
                             ldapi:ldapi64-skosrdf ;
          geolexica:hasLangCode lang:ara ,
                                lang:dan ,
                                lang:deu ,
                                lang:eng ,
                                lang:fin ,
                                # lang:fra ,
                                # lang:kor ,
                                # lang:pol ,
                                # lang:jpn ,
                                lang:msa ,
                                lang:rus ,
                                lang:spa ,
                                lang:swe ;
                                # lang:zho ;
          dcterms:identifier 64 ;
          skos:notation 64 ;
          rdfs:label "concept" ;
  skos:definition "unit of knowledge created by a unique combination of characteristics"@en ;
  skos:definition "وحدة معرفية نشأت عن طريق مزيج فريد من المزايا"@ar ;
  skos:definition "enhed af viden skabt ved en unik kombination af karakteristika"@da ;
  skos:definition "특성의 독특한 조합을 통해 창조된 지식의 단위"@ko ;
  skos:definition "pengertian am atau idea yg mendasari sesuatu"@ms ;
  skos:definition "единица знаний, созданная уникальной комбинацией характеристик"@ru ;
  skos:definition "unidad de conocimiento creada por una combinación única de características"@es ;
  skos:definition "kunskapsenhet som skapats genom en unik kombination av kännetecken"@sv ;

  skos:prefLabel "concept"@en ;
  skos:prefLabel "مفهوم"@ar ;
  skos:prefLabel "begreb"@da ;
  skos:prefLabel "Konzept"@de ;
  skos:prefLabel "개념"@ko ;
  skos:prefLabel "Konsep"@ms ;
  skos:prefLabel "концепция (понятие)"@ru ;
  skos:prefLabel "concepto"@es ;
  skos:prefLabel "begrepp"@sv ;

          geolexica:origin lang:araRegistry ,
                           lang:danRegistry ,
                           lang:deuRegistry ,
                           lang:engRegistry ,
                        #    lang:finRegistry ,
                        #    lang:fraRegistry ,
                           lang:korRegistry ,
                        #    lang:jpnRegistry ,
                           lang:rusRegistry ,
                        #    lang:polRegistry ,
                           lang:msaRegistry ,
                           lang:spaRegistry ,
                           lang:sweRegistry ;
                        #    lang:zhoRegistry ;
          lang:deu-note notes:NoteTransUnavail, notes:DefnTransUnavail ;
          lang:kor-note notes:NoteTransUnavail ;
          lang:msa-note notes:NoteTransUnavail ;
          lang:swe-note notes:NoteTransUnavail .


###  https://isotc211.geolexica.org/ld/concepts#concept_system
:concept_system rdf:type owl:NamedIndividual ,
                   skos:Concept ;
          skos:inScheme geolexica:GeolexicaConceptScheme ;
          geolexica:hasInfo info:Info66 ;
          geolexica:hasReview reviews:Review66 ;
          geolexica:hasLDAPI ldapi:ldapi66-json ,
                             ldapi:ldapi66-jsonld ,
                             ldapi:ldapi66-rdfxml ,
                             ldapi:ldapi66-skosrdf ;
          geolexica:hasLangCode lang:ara ,
                                lang:dan ,
                                lang:deu ,
                                lang:eng ,
                                # lang:fin ,
                                # lang:fra ,
                                lang:kor ,
                                # lang:pol ,
                                # lang:jpn ,
                                lang:msa ,
                                lang:rus ,
                                lang:spa ,
                                lang:swe ,
                                lang:zho ;
          dcterms:identifier 66 ;
          skos:notation 66 ;
          rdfs:label "composite surface" ;

  skos:definition "set of concepts structured according to the relations among them"@en ;
  skos:definition "مجموعة مفاهيم بنيت وفقا للعلاقات القائمة بينها"@ar ;
  skos:definition "sæt af begreber, der er struktureret efter relationerne imellem dem"@da ;
  skos:definition "개념간 관계에 따라 구조화된 개념 집합"@ko ;
  skos:definition "совокупность понятий, структурированных в соответствии с отношениями между ними"@ru ;
  skos:definition "conjunto de conceptos estructurado según las relaciones que los unen"@es ;
  skos:definition "uppsättning begrepp och deras inbördes relationer"@sv ;

  skos:prefLabel "concept system"@en ;
  skos:prefLabel "منظومة مفاهيم"@ar ;
  skos:prefLabel "begrebssystem"@da ;
  skos:prefLabel "System von Konzepten"@de ;
  skos:prefLabel "개념 체계"@ko ;
  skos:prefLabel "Konsep sistem"@ms ;
  skos:prefLabel "система понятий"@ru ;
  skos:prefLabel "sistema de conceptos"@es ;
  skos:prefLabel "begreppssystem"@sv ;
  
          geolexica:origin lang:araRegistry ,
                           lang:danRegistry ,
                           lang:deuRegistry ,
                           lang:engRegistry ,
                        #    lang:finRegistry ,
                        #    lang:fraRegistry ,
                           lang:korRegistry ,
                        #    lang:jpnRegistry ,
                           lang:rusRegistry ,
                        #    lang:polRegistry ,
                           lang:msaRegistry ,
                           lang:spaRegistry ,
                           lang:sweRegistry ;
                        #    lang:zhoRegistry ;
          lang:deu-note notes:DefnTransUnavail ;
          lang:msa-note notes:DefnTransUnavail .


###  https://isotc211.geolexica.org/ld/concepts#conceptual_formalism
:conceptual_formalism rdf:type owl:NamedIndividual ,
                   skos:Concept ;
          skos:inScheme geolexica:GeolexicaConceptScheme ;
          geolexica:hasInfo info:Info67 ;
          geolexica:hasReview reviews:Review67 ;
          geolexica:hasLDAPI ldapi:ldapi67-json ,
                             ldapi:ldapi67-jsonld ,
                             ldapi:ldapi67-rdfxml ,
                             ldapi:ldapi67-skosrdf ;
          geolexica:hasLangCode lang:ara ,
                                lang:dan ,
                                lang:deu ,
                                lang:eng ,
                                lang:fin ,
                                lang:fra ,
                                lang:kor ,
                                # lang:pol ,
                                # lang:jpn ,
                                # lang:msa ,
                                lang:rus ,
                                lang:spa ,
                                lang:swe ,
                                lang:zho ;
          dcterms:identifier 67 ;
          skos:notation 67 ;
          rdfs:label "conceptual formalism" ;

  skos:definition "set of modelling concepts used to describe a conceptual model"@en ;
  skos:definition "مجموعة من المفاهيم النموذجيه المستخدمه لوصف نموذج مفاهيمي"@ar ;
  skos:definition "sæt af modelleringsbegreber, der anvendes til at beskrive en begrebsmodel"@da ;
  skos:definition "Zusammenstellung von Modellierungskonzepten zur Beschreibung eines konzeptuellen Modells"@de ;
  skos:definition "käsiteskeeman kuvaamiseen käytetty mallinnuskäsitejoukko"@fi ;
  skos:definition "ensemble de concepts de modélisation utilisés pour décrire un modèle conceptuel"@fr ;
  skos:definition "개념적 모델을 기술하기 위해 사용된 모델링 개념의 집합"@ko ;
  skos:definition "набор моделирующих понятий, используемых для описания концептуальной модели"@ru ;
  skos:definition "conjunto de conceptos de modelado utilizados para describir un modelo conceptual"@es ;
  skos:definition "uppsättning modelleringsbegrepp som används för att beskriva en begreppsmodell"@sv ;
  skos:definition "用于描述概念模型的一组建模概念。"@zh ;

  skos:prefLabel "conceptual formalism"@en ;
  skos:prefLabel "تكوين مفاهيمي"@ar ;
  skos:prefLabel "konceptuel formalisme"@da ;
  skos:prefLabel "konzeptueller Formalismus"@de ;
  skos:prefLabel "käsitteellinen formalismi"@fi ;
  skos:prefLabel "formalisme conceptuel"@fr ;
  skos:prefLabel "개념적 형식"@ko ;
  skos:prefLabel "концептуальный формализм"@ru ;
  skos:prefLabel "formalismo conceptual"@es ;
  skos:prefLabel "begreppsformalism"@sv ;
  skos:prefLabel "概念形式化体系"@zh ;
  
          geolexica:origin lang:araRegistry ,
                           lang:danRegistry ,
                           lang:deuRegistry ,
                           lang:engRegistry ,
                           lang:finRegistry ,
                           lang:fraRegistry ,
                           lang:korRegistry ,
                        #    lang:jpnRegistry ,
                           lang:rusRegistry ,
                        #    lang:polRegistry ,
                        #    lang:msaRegistry ,
                           lang:spaRegistry ,
                           lang:sweRegistry ,
                           lang:zhoRegistry ;
          lang:deu-note notes:DefnTransUnavail, notes:ExTransUnavail ;
          lang:swe-note notes:DefnTransUnavail, notes:ExTransUnavail .

###  https://isotc211.geolexica.org/ld/concepts#conceptual_model
:conceptual_model rdf:type owl:NamedIndividual ,
                   skos:Concept ;
          skos:inScheme geolexica:GeolexicaConceptScheme ;
          geolexica:hasInfo info:Info68 ;
          geolexica:hasReview reviews:Review68 ;
          geolexica:hasLDAPI ldapi:ldapi68-json ,
                             ldapi:ldapi68-jsonld ,
                             ldapi:ldapi68-rdfxml ,
                             ldapi:ldapi68-skosrdf ;
          geolexica:hasLangCode lang:ara ,
                                lang:dan ,
                                lang:deu ,
                                lang:eng ,
                                lang:fin ,
                                lang:fra ,
                                lang:kor ,
                                # lang:pol ,
                                # lang:jpn ,
                                lang:msa ,
                                lang:rus ,
                                lang:spa ,
                                lang:swe ,
                                lang:zho ;
          dcterms:identifier 68 ;
          skos:notation 68 ;
          rdfs:label "conceptual model" ;

  skos:definition "model that defines concepts of a universe of discourse"@en ;
  skos:definition "نموذج يحدد المفاهيم الخاصة بالمجموعة الشاملة محل البحث"@ar ;
  skos:definition "model, der definerer begreber i et universe of discourse"@da ;
  skos:definition "Modell, das einen abstrahierten Bereich der realen Welt abbildet"@de ;
  skos:definition "tietomalli, joka määrittelee tarkastelun kohteena olevat kohdemaailman käsitteet ja niiden väliset suhteet"@fi ;
  skos:definition "modèle définissant les concepts de l&#39;univers du discours"@fr ;
  skos:definition "논의의 영역의 개념을 정의한 모델"@ko ;
  skos:definition "Satu skim yang menerangkan model konseptual dalam pangkalan data"@ms ;
  skos:definition "модель, определяющая понятия предметной области"@ru ;
  skos:definition "modelo que define conceptos de un universo de discurso"@es ;
  skos:definition "modell som, för ett visst syfte, beskriver begrepp, deras egenskaper och inbördes relationer"@sv ;
  skos:definition "定义一个论域概念的模型。"@zh ;

  skos:prefLabel "conceptual model"@en ;
  skos:prefLabel "نموذج مفاهيمي"@ar ;
  skos:prefLabel "konceptuel model"@da ;
  skos:prefLabel "konzeptuelles Modell"@de ;
  skos:prefLabel "käsitemalli"@fi ;
  skos:prefLabel "modèle conceptuel"@fr ;
  skos:prefLabel "개념적 모델"@ko ;
  skos:prefLabel "model konseptual"@ms ;
  skos:prefLabel "концептуальная модель"@ru ;
  skos:prefLabel "modelo conceptual"@es ;
  skos:prefLabel "begreppsmodell"@sv ;
  skos:prefLabel "概念模型"@zh ;
  
          geolexica:origin lang:araRegistry ,
                           lang:danRegistry ,
                           lang:deuRegistry ,
                           lang:engRegistry ,
                           lang:finRegistry ,
                           lang:fraRegistry ,
                           lang:korRegistry ,
                        #    lang:jpnRegistry ,
                           lang:rusRegistry ,
                        #    lang:polRegistry ,
                           lang:msaRegistry ,
                           lang:spaRegistry ,
                           lang:sweRegistry ,
                           lang:zhoRegistry .

###  https://isotc211.geolexica.org/ld/concepts#conceptual_schema
:conceptual_schema rdf:type owl:NamedIndividual ,
                   skos:Concept ;
          skos:inScheme geolexica:GeolexicaConceptScheme ;
          geolexica:hasInfo info:Info69 ;
          geolexica:hasReview reviews:Review69 ;
          geolexica:hasLDAPI ldapi:ldapi69-json ,
                             ldapi:ldapi69-jsonld ,
                             ldapi:ldapi69-rdfxml ,
                             ldapi:ldapi69-skosrdf ;
          geolexica:hasLangCode lang:ara ,
                                lang:dan ,
                                lang:deu ,
                                lang:eng ,
                                lang:fin ,
                                lang:fra ,
                                lang:kor ,
                                lang:nld ,
                                # lang:pol ,
                                # lang:jpn ,
                                lang:msa ,
                                lang:rus ,
                                lang:spa ,
                                lang:swe ,
                                lang:zho ;
          dcterms:identifier 69 ;
          skos:notation 69 ;
          rdfs:label "conceptual schema" ;

  skos:definition "formal description of a conceptual model"@en ;
  skos:definition "وصف منهجي للنموذج المفاهيمي"@ar ;
  skos:definition "formel beskrivelse af en konceptuel model"@da ;
  skos:definition "formale Beschreibung eines konzeptuellen Modells"@de ;
  skos:definition "käsitemallin määrämuotoinen esitys"@fi ;
  skos:definition "description formelle d&#39;un modèle conceptuel"@fr ;
  skos:definition "개념적 모델의 정형화된 기술"@ko ;
  skos:definition "skema yang menjelaskan sesuatu model konseptual"@ms ;
  skos:definition "formele definitie van objecten, attributen, relaties en regels in een bepaald domein"@nl ;
  skos:definition "формальное описание концептуальной модели"@ru ;
  skos:definition "descripción formal de un modelo conceptual"@es ;
  skos:definition "formell beskrivning av en begreppsmodell"@sv ;
  skos:definition "概念模型的形式化描述。"@zh ;

 skos:prefLabel "conceptual schema"@en ;
  skos:prefLabel "مُخطَّطْ مفاهيمي"@ar ;
  skos:prefLabel "konceptuelt skema"@da ;
  skos:prefLabel "konzeptuelles Schema"@de ;
  skos:prefLabel "käsiteskeema"@fi ;
  skos:prefLabel "schéma conceptuel"@fr ;
  skos:prefLabel "개념적 스키마"@ko ;
  skos:prefLabel "skema Konseptual"@ms ;
  skos:prefLabel "informatiemodel"@nl ;
  skos:prefLabel "концептуальня схема"@ru ;
  skos:prefLabel "esquema conceptual"@es ;
  skos:prefLabel "begreppsschema"@sv ;
  skos:prefLabel "概念模式"@zh ;
  
  skos:altLabel "käsitekaavio"@fi ;
  
  geolexica:origin lang:araRegistry ,
                lang:danRegistry ,
                lang:deuRegistry ,
                lang:engRegistry ,
                lang:finRegistry ,
                lang:fraRegistry ,
                lang:korRegistry ,
                lang:nldRegistry ,
        #    lang:jpnRegistry ,
                lang:rusRegistry ,
        #    lang:polRegistry ,
                lang:msaRegistry ,
                lang:spaRegistry ,
                lang:sweRegistry ,
                lang:zhoRegistry .

###  https://isotc211.geolexica.org/ld/concepts#conceptual_schema_language
:conceptual_schema_language rdf:type owl:NamedIndividual ,
                   skos:Concept ;
          skos:inScheme geolexica:GeolexicaConceptScheme ;
          geolexica:hasInfo info:Info70 ;
          geolexica:hasReview reviews:Review70 ;
          geolexica:hasLDAPI ldapi:ldapi70-json ,
                             ldapi:ldapi70-jsonld ,
                             ldapi:ldapi70-rdfxml ,
                             ldapi:ldapi70-skosrdf ;
        geolexica:hasLangCode lang:ara ,
                        lang:dan ,
                        lang:deu ,
                        lang:eng ,
                        lang:fin ,
                        lang:fra ,
                        lang:kor ,
                        # lang:nld ,
                        # lang:pol ,
                        # lang:jpn ,
                        lang:msa ,
                        lang:rus ,
                        lang:spa ,
                        lang:swe ,
                        lang:zho ;
          dcterms:identifier 70 ;
          skos:notation 70 ;
          rdfs:label "conceptual schema language" ;

  skos:definition "formal language based on a conceptual formalism for the purpose of representing conceptual schemas"@en ;
  skos:definition "لغة رسمية مبنية على التكوين المفاهيمي  لغرض تمثيل المخططات المفاهيمية( التصورية)"@ar ;
  skos:definition "formelt sprog baseret på en konceptuel formalisme til repræsentation af konceptuelle skemaer"@da ;
  skos:definition "formale Sprache, die auf einem konzeptuellen Formalismus zur Darstellung konzeptueller Schemata basiert"@de ;
  skos:definition "määrämuotoinen kieli käsiteskeemojen tuottamista varten"@fi ;
  skos:definition "langage formel basé sur un formalisme conceptuel destiné à représenter des schémas conceptuels"@fr ;
  skos:definition "개념적 스키마의 표현을 위해 개념적 형식에 근거한 형식 언어"@ko ;
  skos:definition "формальный язык представления концептуальных схем, основанный на концептуальном формализме"@ru ;
  skos:definition "lenguaje formal basado en un formalismo conceptual con el propósito de representar esquemas conceptuales"@es ;
  skos:definition "formellt språk som är baserat på begreppsformalism och som används för att representera begreppsscheman"@sv ;
  skos:definition "表达概念模式的形式化语言。"@zh ;

  skos:prefLabel "conceptual schema language"@en ;
  skos:prefLabel "لغة المُخطَّطْ المفاهيمي"@ar ;
  skos:prefLabel "konceptuelt modelleringssprog"@da ;
  skos:prefLabel "Modellierungsprache"@de ;
  skos:prefLabel "mallinnuskieli"@fi ;
  skos:prefLabel "langage de schéma conceptuel"@fr ;
  skos:prefLabel "개념적 스키마 언어"@ko ;
  skos:prefLabel "skema bahasa  Konseptual"@ms ;
  skos:prefLabel "язык концептуальных схем"@ru ;
  skos:prefLabel "lenguaje de esquemas conceptuales"@es ;
  skos:prefLabel "begreppsschemaspråk"@sv ;
  skos:prefLabel "概念模式语言"@zh ;
  
  geolexica:origin lang:araRegistry ,
                lang:danRegistry ,
                lang:deuRegistry ,
                lang:engRegistry ,
                lang:finRegistry ,
                lang:fraRegistry ,
                lang:korRegistry ,
                # lang:nldRegistry ,
                # lang:jpnRegistry ,
                lang:rusRegistry ,
                # lang:polRegistry ,
                lang:msaRegistry ,
                lang:spaRegistry ,
                lang:sweRegistry ,
                lang:zhoRegistry ;
          lang:deu-note notes:DefnTransUnavail, notes:ExTransUnavail ;
          lang:msa-note notes:DefnTransUnavail, notes:NoteTransUnavail, notes:ExTransUnavail ;
          lang:dan-note notes:ExTransUnavail ;
          lang:kor-note notes:ExTransUnavail ;
          lang:swe-note notes:NoteTransUnavail, notes:ExTransUnavail .

###  https://isotc211.geolexica.org/ld/concepts#conformance
:conformance rdf:type owl:NamedIndividual ,
                   skos:Concept ;
          skos:inScheme geolexica:GeolexicaConceptScheme ;
          geolexica:hasInfo info:Info71 ;
        #   geolexica:hasReview reviews:Review71 ;
          geolexica:hasLDAPI ldapi:ldapi71-json ,
                             ldapi:ldapi71-jsonld ,
                             ldapi:ldapi71-rdfxml ,
                             ldapi:ldapi71-skosrdf ;
        geolexica:hasLangCode lang:ara ,
                        lang:dan ,
                        lang:deu ,
                        lang:eng ,
                        lang:fin ,
                        lang:fra ,
                        lang:kor ,
                        # lang:nld ,
                        # lang:pol ,
                        lang:jpn ,
                        lang:msa ,
                        lang:rus ,
                        lang:spa ,
                        lang:swe ,
                        lang:zho ;
          dcterms:identifier 71 ;
          skos:notation 71 ;
          rdfs:label "conformance" ;

  skos:definition "fulfilment of specified requirements"@en ;
  skos:definition "الوفاء بمتطلبات محددة"@ar ;
  skos:definition "opfyldelse af specificerede krav"@da ;
  skos:definition "Erfüllung festgelegter Anforderungen"@de ;
  skos:definition "laatuvaatimustason mukaisten vaatimusten täyttyminen"@fi ;
  skos:definition "satisfaction des exigences spécifiées"@fr ;
  skos:definition "規定された要件をすべて満足すること。"@ja ;
  skos:definition "명시된 요구 사항을 구현한 것에 대한 충실도"@ko ;
  skos:definition "memenuhi keperluan spesifikasi yang ditetapkan"@ms ;
  skos:definition "выполнение заданных требований"@ru ;
  skos:definition "cumplimiento de los requisitos especificados"@es ;
  skos:definition "uppfyllande av specificerade krav"@sv ;
  skos:definition "满足规定的要求。"@zh ;

  skos:prefLabel "conformance"@en ;
  skos:prefLabel "مطابقة"@ar ;
  skos:prefLabel "overensstemmelse"@da ;
  skos:prefLabel "Konformität"@de ;
  skos:prefLabel "vaatimuksenmukaisuus"@fi ;
  skos:prefLabel "conformité"@fr ;
  skos:prefLabel "適合，適合性"@ja ;
  skos:prefLabel "적합성"@ko ;
  skos:prefLabel "Pematuhan"@ms ;
  skos:prefLabel "соответствие"@ru ;
  skos:prefLabel "conformidad"@es ;
  skos:prefLabel "överensstämmelse"@sv ;
  skos:prefLabel "一致性"@zh ;
  
  geolexica:origin lang:araRegistry ,
                lang:danRegistry ,
                lang:deuRegistry ,
                lang:engRegistry ,
                lang:finRegistry ,
                lang:fraRegistry ,
                lang:korRegistry ,
                # lang:nldRegistry ,
                lang:jpnRegistry ,
                lang:rusRegistry ,
                # lang:polRegistry ,
                lang:msaRegistry ,
                lang:spaRegistry ,
                lang:sweRegistry ,
                lang:zhoRegistry ;
          lang:fra-note notes:NoteTransDiff .

###  https://isotc211.geolexica.org/ld/concepts#conformance_assess_process
:conformance_assess_process rdf:type owl:NamedIndividual ,
                   skos:Concept ;
          skos:inScheme geolexica:GeolexicaConceptScheme ;
          geolexica:hasInfo info:Info72 ;
          geolexica:hasReview reviews:Review72 ;
          geolexica:hasLDAPI ldapi:ldapi72-json ,
                             ldapi:ldapi72-jsonld ,
                             ldapi:ldapi72-rdfxml ,
                             ldapi:ldapi72-skosrdf ;
        geolexica:hasLangCode lang:ara ,
                        lang:dan ,
                        lang:deu ,
                        lang:eng ,
                        lang:fin ,
                        lang:fra ,
                        lang:kor ,
                        # lang:nld ,
                        # lang:pol ,
                        lang:jpn ,
                        # lang:msa ,
                        lang:rus ,
                        lang:spa ,
                        lang:swe ,
                        lang:zho ;
          dcterms:identifier 72 ;
          skos:notation 72 ;
          rdfs:label "conformance assessment process" ;

  skos:definition "process for assessing the conformance of an implementation to an International Standard"@en ;
  skos:definition "عملية لتقييم مطابقة التنفيذ للمعيار الدولي"@ar ;
  skos:definition "proces til vurdering af overensstemmelsen af en implementering i forhold til en international standard"@da ;
  skos:definition "prosessi, jossa arvioidaan, miten toteutus täyttää kansainvälisen standardin vaatimukset"@fi ;
  skos:definition "processus évaluant la conformité d&#39;une implémentation d&#39;une Norme Internationale"@fr ;
  skos:definition "ある規格への実装の適合性を評価する過程。"@ja ;
  skos:definition "표준 표준에 따라 적합성을 만족하도록 구현되었는지를 평가하는 과정"@ko ;
  skos:definition "процесс, призванный оценить степень соответствия реализации требованиям конкретного международного стандарта"@ru ;
  skos:definition "proceso para evaluar la conformidad de una implementación con una norma internacional"@es ;
  skos:definition "process för att bedöma i vilken grad en implementering överensstämmer med en standard"@sv ;
  skos:definition "对某项国际标准实现的一致性评价过程。"@zh ;

  skos:prefLabel "conformance assessment process"@en ;
  skos:prefLabel "عملية تقييم المطابقة"@ar ;
  skos:prefLabel "overensstemmelse, proces til vurdering af"@da ;
  skos:prefLabel "Konformitätsauswertungsprozess"@de ;
  skos:prefLabel "vaatimuksenmukaisuuden arviointi"@fi ;
  skos:prefLabel "processus d&#39;évaluation de conformité"@fr ;
  skos:prefLabel "適合性評価過程"@ja ;
  skos:prefLabel "적합성 평가 과정"@ko ;
  skos:prefLabel "процесс оценки соответствия"@ru ;
  skos:prefLabel "proceso de evaluación de la conformidad"@es ;
  skos:prefLabel "process för överensstämmelsebedömning"@sv ;
  skos:prefLabel "一致性评价过程"@zh ;
  
  geolexica:origin lang:araRegistry ,
                lang:danRegistry ,
                lang:deuRegistry ,
                lang:engRegistry ,
                lang:finRegistry ,
                lang:fraRegistry ,
                lang:korRegistry ,
                # lang:nldRegistry ,
                lang:jpnRegistry ,
                lang:rusRegistry ,
                # lang:polRegistry ,
                # lang:msaRegistry ,
                lang:spaRegistry ,
                lang:sweRegistry ,
                lang:zhoRegistry ;
          lang:deu-note notes:DefnTransUnavail .

###  https://isotc211.geolexica.org/ld/concepts#conformance_clause
:conformance_clause rdf:type owl:NamedIndividual ,
                   skos:Concept ;
          skos:inScheme geolexica:GeolexicaConceptScheme ;
          geolexica:hasInfo info:Info73 ;
       #  geolexica:hasReview reviews:Review73 ;
          geolexica:hasLDAPI ldapi:ldapi73-json ,
                             ldapi:ldapi73-jsonld ,
                             ldapi:ldapi73-rdfxml ,
                             ldapi:ldapi73-skosrdf ;
        geolexica:hasLangCode lang:ara ,
                        lang:dan ,
                        lang:deu ,
                        lang:eng ,
                        lang:fin ,
                        lang:fra ,
                        lang:kor ,
                        # lang:nld ,
                        # lang:pol ,
                        lang:jpn ,
                        # lang:msa ,
                        lang:rus ,
                        lang:spa ,
                        lang:swe ,
                        lang:zho ;
          dcterms:identifier 73 ;
          skos:notation 73 ;
          rdfs:label "conformance clause" ;

  skos:definition "clause defining what is necessary in order to meet the requirements of the International Standard"@en ;
  skos:definition "شرط يوضح ما هو ضروري للوفاء بمتطلبات المعاير الدولي"@ar ;
  skos:definition "klausul, der definerer, hvad der er nødvendigt for at opfylde kravene i den internationale standard"@da ;
  skos:definition "määrittely, jossa todetaan, mikä on välttämätöntä kansainvälisen standardin vaatimusten täyttymiseksi"@fi ;
  skos:definition "clause définissant ce qui est nécessaire pour satisfaire les exigences de la norme Internationale"@fr ;
  skos:definition "規格の要件を満たすために必要なことを示した箇条。"@ja ;
  skos:definition "표준의 요구사항 충족을 위해 필요한 것이 무엇인지를 정의하는 조항"@ko ;
  skos:definition "раздел, определяющий, что необходимо для соответствия требованиям конкретного международного стандарта"@ru ;
  skos:definition "capítulo que define qué es necesario para satisfacer los requisitos de la norma internacional"@es ;
  skos:definition "avsnitt i standard om vad som är nödvändigt för att standardens krav ska anses uppfyllda"@sv ;
  skos:definition "为满足标准要求而必须规定的条款。"@zh ;

  skos:prefLabel "conformance clause"@en ;
  skos:prefLabel "شرط المطابقة"@ar ;
  skos:prefLabel "overensstemmelsesklausul"@da ;
  skos:prefLabel "Konformitätsabschnitt"@de ;
  skos:prefLabel "vaatimuksenmukaisuuden määrittely"@fi ;
  skos:prefLabel "clause de conformité"@fr ;
  skos:prefLabel "適合性の箇条"@ja ;
  skos:prefLabel "적합성 조항"@ko ;
  skos:prefLabel "раздел о соответствии"@ru ;
  skos:prefLabel "claúsula de conformidad"@es ;
  skos:prefLabel "överensstämmelseavsnitt"@sv ;
  skos:prefLabel "一致性条款"@zh ;
  
  geolexica:origin lang:araRegistry ,
                lang:danRegistry ,
                lang:deuRegistry ,
                lang:engRegistry ,
                lang:finRegistry ,
                lang:fraRegistry ,
                lang:korRegistry ,
                # lang:nldRegistry ,
                # lang:jpnRegistry ,
                lang:rusRegistry ,
                # lang:polRegistry ,
                lang:msaRegistry ,
                lang:spaRegistry ,
                lang:sweRegistry ,
                lang:zhoRegistry ;
          lang:deu-note notes:DefnTransUnavail ;
          lang:fra-note notes:NoteTransDiff .

###  https://isotc211.geolexica.org/ld/concepts#conformance_quality_level
:conformance_quality_level rdf:type owl:NamedIndividual ,
                   skos:Concept ;
          skos:inScheme geolexica:GeolexicaConceptScheme ;
          geolexica:hasInfo info:Info74 ;
          geolexica:hasReview reviews:Review74 ;
          geolexica:hasLDAPI ldapi:ldapi74-json ,
                             ldapi:ldapi74-jsonld ,
                             ldapi:ldapi74-rdfxml ,
                             ldapi:ldapi74-skosrdf ;
        geolexica:hasLangCode lang:ara ,
                        lang:dan ,
                        lang:deu ,
                        lang:eng ,
                        lang:fin ,
                        lang:fra ,
                        lang:kor ,
                        # lang:nld ,
                        # lang:pol ,
                        lang:jpn ,
                        # lang:msa ,
                        lang:rus ,
                        lang:spa ,
                        lang:swe ,
                        lang:zho ;
          dcterms:identifier 74 ;
          skos:notation 74 ;
          rdfs:label "conformance quality level" ;

  skos:definition "threshold value or set of threshold values for data quality results used to determine how well a dataset meets the criteria set forth in its product specification or user requirements"@en ;
  skos:definition "القيمة الحدية أو مجموعة القيم الحدية لنتائج فحص الجودة التي تستخدم لمعرفة مدى مطابقة مجموعة بيانات للمعايير المحددة لمواصفات إنتاجها أو لمتطلبات المستخدم"@ar ;
  skos:definition "tærskelværdi eller sæt af tærskelværdier for resultater af datakvalitet, som anvendes til at bestemme, hvor godt et datasæt opfylder kriterierne i produktspecifikationen eller brugerkravene"@da ;
  skos:definition "Schwellenwert oder Reihe von Schwellenwerten zur Ermittlung der Qualität von Daten, mit denen bestimmt wird, wie gut ein Datensatz die in dessen Datenprodukt-Spezifikation oder den Benutzeranforderungen festgelegten Kriterien erfüllt"@de ;
  skos:definition "kynnysarvo tai kynnysarvojen joukko, jonka avulla voidaan selvittää, kuinka hyvin tietoaineisto vastaa käyttäjän vaatimuksia tai tietotuotemäärittelyä"@fi ;
  skos:definition "valeur seuil ou ensemble de valeurs seuil devant être atteint par des résultats d&#39;évaluation de la qualité et utilisé pour déterminer dans quelle mesure un jeu de données respecte les critères exposés dans sa spécification de produit ou les exigences utilisateur"@fr ;
  skos:definition "데이터셋이 제품 사양이나 사용자의 요구사항을 만족했는지를 결정하는데 사용되는 데이터 품질 결과에 대한 임계 값 또는 임계 값의 집합"@ko ;
  skos:definition "пороговое значение или набор пороговых значений для  оценки качества данных, по которым определяют степень соответствия  спецификации продукта или потребностям пользователя"@ru ;
  skos:definition "valor umbral o conjunto de valores umbral, para los resultados de la calidad de datos, empleados para determinar lo bien que un conjunto de datos se adecua a los criterios expuestos en sus especificaciones de producto o en los requerimientos de usuario"@es ;
  skos:definition "ett eller flera tröskelvärden för datas kvalitet vilka används för att bedöma hur väl en datamängd uppfyller användarkraven eller kraven i dataproduktspecifikationen"@sv ;
  skos:definition "数据质量结果的一个或一组阀值，用于确定数据集符合产品规范所规定或用户要求的程度。"@zh ;

  skos:prefLabel "conformance quality level"@en ;
  skos:prefLabel "مستوى جودة المطابقة"@ar ;
  skos:prefLabel "overensstemmelse, kvalitetsniveau af"@da ;
  skos:prefLabel "Qualitätskonformitätsschwellwert"@de ;
  skos:prefLabel "laatuvaatimustaso"@fi ;
  skos:prefLabel "niveau de conformité"@fr ;
  skos:prefLabel "적합성 품질 수준"@ko ;
  skos:prefLabel "уровень соответствия качества"@ru ;
  skos:prefLabel "nivel de calidad de conformidad"@es ;
  skos:prefLabel "målvärde för datakvalitet"@sv ;
  skos:prefLabel "一致性质量级别"@zh ;
  
  geolexica:origin lang:araRegistry ,
                lang:danRegistry ,
                lang:deuRegistry ,
                lang:engRegistry ,
                lang:finRegistry ,
                lang:fraRegistry ,
                lang:korRegistry ,
                # lang:nldRegistry ,
                # lang:jpnRegistry ,
                lang:rusRegistry ,
                # lang:polRegistry ,
                lang:msaRegistry ,
                lang:spaRegistry ,
                lang:sweRegistry ,
                lang:zhoRegistry .

###  https://isotc211.geolexica.org/ld/concepts#conformance_test_report
:conformance_test_report rdf:type owl:NamedIndividual ,
                   skos:Concept ;
          skos:inScheme geolexica:GeolexicaConceptScheme ;
          geolexica:hasInfo info:Info75 ;
          geolexica:hasReview reviews:Review75 ;
          geolexica:hasLDAPI ldapi:ldapi75-json ,
                             ldapi:ldapi75-jsonld ,
                             ldapi:ldapi75-rdfxml ,
                             ldapi:ldapi75-skosrdf ;
        geolexica:hasLangCode lang:ara ,
                        lang:dan ,
                        lang:deu ,
                        lang:eng ,
                        lang:fin ,
                        lang:fra ,
                        lang:kor ,
                        # lang:nld ,
                        # lang:pol ,
                        lang:jpn ,
                        # lang:msa ,
                        lang:rus ,
                        lang:spa ,
                        lang:swe ,
                        lang:zho ;
          dcterms:identifier 75 ;
          skos:notation 75 ;
          rdfs:label "conformance test report" ;

  skos:definition "summary of the conformance to the International Standard as well as all the details of the testing that supports the given overall summary"@en ;
  skos:definition "ملخص مطابقة المعيار الدولي وكذلك جميع تفاصيل الاختبار التي تؤيد الملخص الإجمالي المعطى"@ar ;
  skos:definition "opsummering af overensstemmelsen med den internationale standard samt detaljer om testen, der understøtter den givne samlede opsummering"@da ;
  skos:definition "yhteenveto kansainvälisen standardin vaatimusten täyttymisestä sekä yksityiskohtaiset testitiedot, joihin yhteenveto perustuu"@fi ;
  skos:definition "résumé de la conformité à la Norme Internationale et détails des tests ayant abouti au résumé donné"@fr ;
  skos:definition "規格への適合の全体概要報告及びその全体概要の基となる試験結果の詳細報告。"@ja ;
  skos:definition "시험의 상세 내용과 표준에 대한 적합성 여부를 요약한 보고서"@ko ;
  skos:definition "резюме соответствия конкретному международному стандарту, а также детальные результаты тестирования, которые подтверждают данное сводное резюме"@ru ;
  skos:definition "resumen de la conformidad con la Norma Internacional así como de todos los detalles de las pruebas que justifican el resumen global incluido"@es ;
  skos:definition "redovisning av någots överensstämmelse med en standard samt detaljer som underbygger detta"@sv ;
  skos:definition "与具体标准一致性程度的概要以及支持给出这一总体概要的全部测试细节。"@zh ;

  skos:prefLabel "conformance test report"@en ;
  skos:prefLabel "تقرير اختبار المطابقة"@ar ;
  skos:prefLabel "overensstemmelse, testrapport"@da ;
  skos:prefLabel "Konformitätsprüfbericht"@de ;
  skos:prefLabel "vaatimuksenmukaisuuden testausraportti"@fi ;
  skos:prefLabel "compte-rendu de test de conformité"@fr ;
  skos:prefLabel "適合性試験報告書"@ja ;
  skos:prefLabel "적합성 시험 보고서"@ko ;
  skos:prefLabel "отчет о тестировании на соответствие"@ru ;
  skos:prefLabel "informe de prueba de conformidad"@es ;
  skos:prefLabel "överensstämmelseredovisning"@sv ;
  skos:prefLabel "一致性测试报告"@zh ;
  
  geolexica:origin lang:araRegistry ,
                lang:danRegistry ,
                lang:deuRegistry ,
                lang:engRegistry ,
                lang:finRegistry ,
                lang:fraRegistry ,
                lang:korRegistry ,
                # lang:nldRegistry ,
                lang:jpnRegistry ,
                lang:rusRegistry ,
                # lang:polRegistry ,
                # lang:msaRegistry ,
                lang:spaRegistry ,
                lang:sweRegistry ,
                lang:zhoRegistry ;
          lang:deu-note notes:DefnTransUnavail .

###  https://isotc211.geolexica.org/ld/concepts#conformance_testing
:conformance_testing rdf:type owl:NamedIndividual ,
                   skos:Concept ;
          skos:inScheme geolexica:GeolexicaConceptScheme ;
          geolexica:hasInfo info:Info76 ;
        #   geolexica:hasReview reviews:Review76 ;
          geolexica:hasLDAPI ldapi:ldapi76-json ,
                             ldapi:ldapi76-jsonld ,
                             ldapi:ldapi76-rdfxml ,
                             ldapi:ldapi76-skosrdf ;
        geolexica:hasLangCode lang:ara ,
                        lang:dan ,
                        lang:deu ,
                        lang:eng ,
                        lang:fin ,
                        lang:fra ,
                        lang:kor ,
                        # lang:nld ,
                        # lang:pol ,
                        lang:jpn ,
                        # lang:msa ,
                        lang:rus ,
                        lang:spa ,
                        lang:swe ,
                        lang:zho ;
          dcterms:identifier 76 ;
          skos:notation 76 ;
          rdfs:label "conformance testings" ;

  skos:definition "testing of a product to determine the extent to which the product is a conforming implementation"@en ;
  skos:definition "اختبار منتج لمعرفة مدى مطابقته للتنفيذ"@ar ;
  skos:definition "test af et produkt for at afgøre, i hvor høj grad produktet opfylder kravene til implementeringen"@da ;
  skos:definition "tuotteen testaaminen sen selvittämiseksi, missä määrin tuote on vaatimuksenmukainen toteutus"@fi ;
  skos:definition "test d&#39;un produit pour déterminer dans quelle mesure l&#39;implémentation du produit est conforme"@fr ;
  skos:definition "製品の実装の適合の度合を決めるために，その製品に対して行う試験。"@ja ;
  skos:definition "구현된 제품의 적합 정도를 결정하기 위한 시험"@ko ;
  skos:definition "тестирование продукта с целью определения степени его соответствия установленным требованиям"@ru ;
  skos:definition "prueba de un producto para determinar hasta qué punto el producto es una implementación conforme"@es ;
  skos:definition "aktivitet för att avgöra i vilken grad angivna krav uppfylls"@sv ;
  skos:definition "对产品进行的测试，以便确定该产品一致性实现的程度。"@zh ;

  skos:prefLabel "conformance testing"@en ;
  skos:prefLabel "اختبار المطابقة"@ar ;
  skos:prefLabel "overensstemmelse, test af"@da ;
  skos:prefLabel "Konformitätsprüfung"@de ;
  skos:prefLabel "vaatimuksenmukaisuuden testaus"@fi ;
  skos:prefLabel "test de conformité"@fr ;
  skos:prefLabel "適合性試験"@ja ;
  skos:prefLabel "적합성 시험"@ko ;
  skos:prefLabel "тестирование на соответствие"@ru ;
  skos:prefLabel "prueba de conformidad"@es ;
  skos:prefLabel "test av överensstämmelse"@sv ;
  skos:prefLabel "一致性测试"@zh ;
  
  geolexica:origin lang:araRegistry ,
                lang:danRegistry ,
                lang:deuRegistry ,
                lang:engRegistry ,
                lang:finRegistry ,
                lang:fraRegistry ,
                lang:korRegistry ,
                # lang:nldRegistry ,
                lang:jpnRegistry ,
                lang:rusRegistry ,
                # lang:polRegistry ,
                # lang:msaRegistry ,
                lang:spaRegistry ,
                lang:sweRegistry ,
                lang:zhoRegistry ;
          lang:deu-note notes:DefnTransUnavail ;
          lang:fra-note notes:NoteTransDiff .

###  https://isotc211.geolexica.org/ld/concepts#conforming_implementation
:conforming_implementation rdf:type owl:NamedIndividual ,
                   skos:Concept ;
          skos:inScheme geolexica:GeolexicaConceptScheme ;
          geolexica:hasInfo info:Info77 ;
        #   geolexica:hasReview reviews:Review77 ;
          geolexica:hasLDAPI ldapi:ldapi77-json ,
                             ldapi:ldapi77-jsonld ,
                             ldapi:ldapi77-rdfxml ,
                             ldapi:ldapi77-skosrdf ;
        geolexica:hasLangCode lang:ara ,
                        lang:dan ,
                        lang:deu ,
                        lang:eng ,
                        lang:fin ,
                        lang:fra ,
                        lang:kor ,
                        # lang:nld ,
                        # lang:pol ,
                        lang:jpn ,
                        # lang:msa ,
                        lang:rus ,
                        lang:spa ,
                        lang:swe ,
                        lang:zho ;
          dcterms:identifier 77 ;
          skos:notation 77 ;
          rdfs:label "conforming implementation" ;

  skos:definition "implementation which satisfies the requirements"@en ;
  skos:definition "التنفيذ الذي يحقق المتطلبات"@ar ;
  skos:definition "implementering, der opfylder kravene"@da ;
  skos:definition "toteutus, joka täyttää vaatimukset"@fi ;
  skos:definition "implémentation satisfaisant les exigences"@fr ;
  skos:definition "適合性要件を満たしている実装。"@ja ;
  skos:definition "적합성 요건을 만족시키는 구현"@ko ;
  skos:definition "реализация, удовлетворяющая требованиям"@ru ;
  skos:definition "implementación que satisface los requisitos de conformidad"@es ;
  skos:definition "implementering som uppfyller angivna krav"@sv ;
  skos:definition "满足要求的实现。"@zh ;

  skos:prefLabel "conforming implementation"@en ;
  skos:prefLabel "تنفيذ مطابِق"@ar ;
  skos:prefLabel "overensstemmende implementering"@da ;
  skos:prefLabel "konforme Implementierung"@de ;
  skos:prefLabel "vaatimuksenmukainen toteutus"@fi ;
  skos:prefLabel "implémentation conforme"@fr ;
  skos:prefLabel "適合実装"@ja ;
  skos:prefLabel "적합성 구현"@ko ;
  skos:prefLabel "корректная реализация"@ru ;
  skos:prefLabel "implementación conforme"@es ;
  skos:prefLabel "överensstämmande implementering"@sv ;
  skos:prefLabel "一致性实现"@zh ;
  
  geolexica:origin lang:araRegistry ,
                lang:danRegistry ,
                lang:deuRegistry ,
                lang:engRegistry ,
                lang:finRegistry ,
                lang:fraRegistry ,
                lang:korRegistry ,
                # lang:nldRegistry ,
                lang:jpnRegistry ,
                lang:rusRegistry ,
                # lang:polRegistry ,
                # lang:msaRegistry ,
                lang:spaRegistry ,
                lang:sweRegistry ,
                lang:zhoRegistry ;
          lang:deu-note notes:DefnTransUnavail ;
          lang:fra-note notes:NoteTransDiff .

###  https://isotc211.geolexica.org/ld/concepts#connected
:connected rdf:type owl:NamedIndividual ,
                   skos:Concept ;
          skos:inScheme geolexica:GeolexicaConceptScheme ;
          geolexica:hasInfo info:Info78 ;
          geolexica:hasReview reviews:Review78 ;
          geolexica:hasLDAPI ldapi:ldapi78-json ,
                             ldapi:ldapi78-jsonld ,
                             ldapi:ldapi78-rdfxml ,
                             ldapi:ldapi78-skosrdf ;
        geolexica:hasLangCode lang:ara ,
                        lang:dan ,
                        lang:deu ,
                        lang:eng ,
                        lang:fin ,
                        lang:fra ,
                        lang:kor ,
                        # lang:nld ,
                        lang:pol ,
                        lang:jpn ,
                        lang:msa ,
                        lang:rus ,
                        lang:spa ,
                        lang:swe ,
                        lang:zho ;
          dcterms:identifier 77 ;
          skos:notation 77 ;
          rdfs:label "connected" ;

  skos:definition "property of a geometric object implying that any two direct positions on the object can be placed on a curve that remains totally within the object"@en ;
  skos:definition "خاصية كيان هندسي تتضمن أن أي موقعين مباشرين على الكيان المذكور يمكن وضعهما على منحنى يظل بكامله داخل الكيان"@ar ;
  skos:definition "egenskab ved et geometrisk objekt, som angiver, at enhver af to direkte positioner på objektet kan placeres på en kurve, der forbliver helt inde i objektet"@da ;
  skos:definition "geometrisen objektin ominaisuus, joka edellyttää, että mitkä hyvänsä kaksi objektin pistettä voidaan sijoittaa käyrälle, joka on kokonaan objektin sisällä"@fi ;
  skos:definition "propriété d&#39;un objet géométrique impliquant que tout couple de positions directes de l&#39;objet peut être placé sur une courbe restant totalement dans l&#39;objet"@fr ;
  skos:definition "オブジェクトの任意の二つの直接位置がそのオブジェクト内に完全に含まれる曲線上に配置できることを意味する幾何オブジェクトの性質。"@ja ;
  skos:definition "객체에서 임의의 두 개의 직접 위치가 그 객체 내부에 완전하게 포함되는 곡선상에 위치할 수 있는 것을 의미하는 기하 객체의 특성"@ko ;
  skos:definition "właściwość obiektu geometrycznego oznaczająca, że dowolne dwa położenia bezpośrednie na tym obiekcie mogą być umieszczone na krzywej, która całkowicie pozostaje wewnątrz tego obiektu"@pl ;
  skos:definition "свойство геометрического объекта, предполагающее, что любые две точки в пределах объекта могут быть помещены на кривую, полностью лежащую внутри этого объекта"@ru ;
  skos:definition "propiedad de un objeto geométrico que implica que cualesquiera dos posiciones directas en el objeto pueden ser puestas sobre una curva que permance totalmente dentro de ese objeto"@es ;
  skos:definition "(inom geometri); sådan att en linje genom två  godtyckligt valda punkter hos ett geometriskt objekt befinner sig inom objektet"@sv ;
  skos:definition "几何对象的一种特性，指这个几何对象内的任何两个直接位置可以都位于完全在这个对象内的一条曲线上。"@zh ;

  skos:prefLabel "connected"@en ;
  skos:prefLabel "متصل"@ar ;
  skos:prefLabel "forbundet"@da ;
  skos:prefLabel "verbunden"@de ;
  skos:prefLabel "yhtenäinen"@fi ;
  skos:prefLabel "connexe"@fr ;
  skos:prefLabel "連結"@ja ;
  skos:prefLabel "연결"@ko ;
  skos:prefLabel "hubungan"@ms ;
  skos:prefLabel "spójny"@pl ;
  skos:prefLabel "связный"@ru ;
  skos:prefLabel "conectado"@es ;
  skos:prefLabel "sammanhängande"@sv ;
  skos:prefLabel "连通"@zh ;
  
  geolexica:origin lang:araRegistry ,
                lang:danRegistry ,
                lang:deuRegistry ,
                lang:engRegistry ,
                lang:finRegistry ,
                lang:fraRegistry ,
                lang:korRegistry ,
                # lang:nldRegistry ,
                lang:jpnRegistry ,
                lang:rusRegistry ,
                lang:polRegistry ,
                lang:msaRegistry ,
                lang:spaRegistry ,
                lang:sweRegistry ,
                lang:zhoRegistry ;
          lang:deu-note notes:DefnTransUnavail , notes:NoteTransUnavail ;
          lang:swe-note notes:NoteTransUnavail ;
          lang:msa-note notes:DefnTransUnavail , notes:NoteTransUnavail .

###  https://isotc211.geolexica.org/ld/concepts#connected_node
:connected_node rdf:type owl:NamedIndividual ,
                   skos:Concept ;
          skos:inScheme geolexica:GeolexicaConceptScheme ;
          geolexica:hasInfo info:Info79 ;
          geolexica:hasReview reviews:Review79 ;
          geolexica:hasLDAPI ldapi:ldapi79-json ,
                             ldapi:ldapi79-jsonld ,
                             ldapi:ldapi79-rdfxml ,
                             ldapi:ldapi79-skosrdf ;
        geolexica:hasLangCode lang:ara ,
                        lang:dan ,
                        lang:deu ,
                        lang:eng ,
                        lang:fin ,
                        lang:fra ,
                        lang:kor ,
                        # lang:nld ,
                        lang:pol ,
                        lang:jpn ,
                        # lang:msa ,
                        lang:rus ,
                        lang:spa ,
                        lang:swe ,
                        lang:zho ;
          dcterms:identifier 79 ;
          skos:notation 79 ;
          rdfs:label "connected node" ;

  skos:definition "node that starts or ends one or more edges"@en ;
  skos:definition "عقدة تبدأ منها أو تنتهي إليها حافة واحدة أو أكثر"@ar ;
  skos:definition "knude, der starter eller slutter en eller flere kanter"@da ;
  skos:definition "solmupiste, joka toimii yhden tai useamman linkin alku- tai loppupisteenä"@fi ;
  skos:definition "nœud de début ou de fin d&#39;une ou plusieurs arêtes"@fr ;
  skos:definition "一つ以上のエッジが開始又は終了するノード。"@ja ;
  skos:definition "한 개 이상의 변으로 시작하거나 끝나는 절점"@ko ;
  skos:definition "węzeł, który zaczyna lub kończy co najmniej jedną krawędź"@pl ;
  skos:definition "узел, в котором начинаются или заканчиваются  одно или несколько ребер"@ru ;
  skos:definition "nodo en el que empiezan o acaban uno o más arcos"@es ;
  skos:definition "nod som inleder eller avslutar en eller flera länkar"@sv ;
  skos:definition "起始于或终止于一条或多条边的结点。"@zh ;

  skos:prefLabel "connected node"@en ;
  skos:prefLabel "عقدة موصلة"@ar ;
  skos:prefLabel "forbundet knude"@da ;
  skos:prefLabel "Verbindungsknoten"@de ;
  skos:prefLabel "yhdistävä solmu"@fi ;
  skos:prefLabel "nœud connexe"@fr ;
  skos:prefLabel "連結ノード"@ja ;
  skos:prefLabel "연결 절점"@ko ;
  skos:prefLabel "węzeł dołączony"@pl ;
  skos:prefLabel "сопряженный узел"@ru ;
  skos:prefLabel "nodo conectado"@es ;
  skos:prefLabel "ansluten nod"@sv ;
  skos:prefLabel "相连结点"@zh ;
  
  geolexica:origin lang:araRegistry ,
                lang:danRegistry ,
                lang:deuRegistry ,
                lang:engRegistry ,
                lang:finRegistry ,
                lang:fraRegistry ,
                lang:korRegistry ,
                # lang:nldRegistry ,
                lang:jpnRegistry ,
                lang:rusRegistry ,
                lang:polRegistry ,
                # lang:msaRegistry ,
                lang:spaRegistry ,
                lang:sweRegistry ,
                lang:zhoRegistry ;
          lang:deu-note notes:DefnTransUnavail .

###  https://isotc211.geolexica.org/ld/concepts#constraintUML
:constraintUML rdf:type owl:NamedIndividual ,
                   skos:Concept ;
          skos:inScheme geolexica:GeolexicaConceptScheme ;
          geolexica:hasInfo info:Info81 ;
          geolexica:hasReview reviews:Review81 ;
          geolexica:hasLDAPI ldapi:ldapi81-json ,
                             ldapi:ldapi81-jsonld ,
                             ldapi:ldapi81-rdfxml ,
                             ldapi:ldapi81-skosrdf ;
        geolexica:hasLangCode lang:ara ,
                        lang:dan ,
                        lang:deu ,
                        lang:eng ,
                        lang:fin ,
                        lang:fra ,
                        lang:kor ,
                        # lang:nld ,
                        # lang:pol ,
                        # lang:jpn ,
                        # lang:msa ,
                        lang:rus ,
                        lang:spa ,
                        lang:swe ,
                        lang:zho ;
          dcterms:identifier 81 ;
          skos:notation 81 ;
          rdfs:label "constraint (UML)" ;

  skos:definition "semantic condition or restriction"@en ;
  skos:definition "شرط أو قيد يتعلق بمعاني ودلالات المفردات اللغوية"@ar ;
  skos:definition "semantisk betingelse eller begrænsning"@da ;
  skos:definition "semanttinen ehto tai rajoitus"@fi ;
  skos:definition "condition ou restriction sémantique"@fr ;
  skos:definition "의미론적 조건 또는 제한"@ko ;
  skos:definition "семантическое условие или особое требование"@ru ;
  skos:definition "restricción o  condición semántica"@es ;
  skos:definition "(i UML); begränsning i beteende för en klass"@sv ;
  skos:definition "语义条件或限制。"@zh ;

  skos:prefLabel "constraint (UML);"@en ;
  skos:prefLabel "قيد (UML);"@ar ;
  skos:prefLabel "restriktion (UML);"@da ;
  skos:prefLabel "Einschränkung (UML);"@de ;
  skos:prefLabel "rajoite (UML);"@fi ;
  skos:prefLabel "contrainte (UML);"@fr ;
  skos:prefLabel "제약 조건 (UML);"@ko ;
  skos:prefLabel "ограничение (UML);"@ru ;
  skos:prefLabel "restricción (UML);"@es ;
  skos:prefLabel "restriktion (UML);"@sv ;
  skos:prefLabel "约束(UML);"@zh ;
  
  geolexica:origin lang:araRegistry ,
                lang:danRegistry ,
                lang:deuRegistry ,
                lang:engRegistry ,
                lang:finRegistry ,
                lang:fraRegistry ,
                lang:korRegistry ,
                # lang:nldRegistry ,
                # lang:jpnRegistry ,
                lang:rusRegistry ,
                # lang:polRegistry ,
                # lang:msaRegistry ,
                lang:spaRegistry ,
                lang:sweRegistry ,
                lang:zhoRegistry ;
          lang:deu-note notes:DefnTransUnavail , notes:NoteTransUnavail ;
          lang:swe-note notes:NoteTransUnavail .


###  https://isotc211.geolexica.org/ld/concepts#content_model
:content_model rdf:type owl:NamedIndividual ,
                   skos:Concept ;
          skos:inScheme geolexica:GeolexicaConceptScheme ;
          geolexica:hasInfo info:Info82 ;
        #   geolexica:hasReview reviews:Review82 ;
          geolexica:hasLDAPI ldapi:ldapi82-json ,
                             ldapi:ldapi82-jsonld ,
                             ldapi:ldapi82-rdfxml ,
                             ldapi:ldapi82-skosrdf ;
        geolexica:hasLangCode lang:ara ,
                        # lang:dan ,
                        lang:deu ,
                        lang:eng ,
                        # lang:fin ,
                        # lang:fra ,
                        lang:kor ,
                        # lang:nld ,
                        # lang:pol ,
                        # lang:jpn ,
                        # lang:msa ,
                        lang:rus ,
                        lang:spa ,
                        lang:swe ;
                        # lang:zho ;
          dcterms:identifier 82 ;
          skos:notation 82 ;
          rdfs:label "content model" ;

  skos:definition "information view of an application schemas"@en ;
  skos:definition "جانب المعلومات لمخطط التطبيق"@ar ;
  skos:definition "응용 스키마의 정보창"@ko ;
  skos:definition "информационное представление схем приложений"@ru ;
  skos:definition "vista informativa de un esquema de aplicación"@es ;
  skos:definition "informationsperspektiv på ett applikationsschema"@sv ;

  skos:prefLabel "content model"@en ;
  skos:prefLabel "نموذج المحتوى"@ar ;
  skos:prefLabel "Inhaltsmodell"@de ;
  skos:prefLabel "내용 모형"@ko ;
  skos:prefLabel "модель контента"@ru ;
  skos:prefLabel "modelo de contenido"@es ;
  skos:prefLabel "innehållsmodell"@sv ;
  
  geolexica:origin lang:araRegistry ,
                # lang:danRegistry ,
                lang:deuRegistry ,
                lang:engRegistry ,
                # lang:finRegistry ,
                # lang:fraRegistry ,
                lang:korRegistry ,
                # lang:nldRegistry ,
                # lang:jpnRegistry ,
                lang:rusRegistry ,
                # lang:polRegistry ,
                # lang:msaRegistry ,
                lang:spaRegistry ,
                lang:sweRegistry ;
                # lang:zhoRegistry ;
          lang:deu-note notes:DefnTransUnavail , notes:NoteTransUnavail ;
          lang:kor-note notes:NoteTransUnavail ;
          lang:swe-note notes:NoteTransUnavail .


###  https://isotc211.geolexica.org/ld/concepts#continuous_coverage
:continuous_coverage rdf:type owl:NamedIndividual ,
                   skos:Concept ;
          skos:inScheme geolexica:GeolexicaConceptScheme ;
          geolexica:hasInfo info:Info83 ;
        #   geolexica:hasReview reviews:Review83 ;
          geolexica:hasLDAPI ldapi:ldapi83-json ,
                             ldapi:ldapi83-jsonld ,
                             ldapi:ldapi83-rdfxml ,
                             ldapi:ldapi83-skosrdf ;
        geolexica:hasLangCode lang:ara ,
                        lang:dan ,
                        lang:deu ,
                        lang:eng ,
                        lang:fin ,
                        lang:fra ,
                        lang:kor ,
                        # lang:nld ,
                        lang:pol ,
                        # lang:jpn ,
                        lang:msa ,
                        lang:rus ,
                        lang:spa ,
                        lang:swe ,
                        lang:zho ;
          dcterms:identifier 83 ;
          skos:notation 83 ;
          rdfs:label "continuous coverage" ;

  skos:definition "coverage that returns different values for the same feature attribute at different direct positions within a single spatial object, temporal object, or spatiotemporal object in its domain"@en ;
  skos:definition "تغطية تعيد قيم مختلفة لخاصية المعلم نفسه ، التي تكون على مواقع مباشرة مختلفة ضمن كيان مكاني واحد ،أو كيان زماني أو كيان مكاني-زماني ، في نطاقها"@ar ;
  skos:definition "coverage, der giver forskellige værdier for samme featureattribut på forskellige direkte positioner inden for et enkelt spatialt objekt, temporale objekt eller temporalt-spatialt objekt i sit domæne"@da ;
  skos:definition "paikkatietojatkumo, jonka alueella olevan spatiaalisen, temporaalisen tai spatiotemporaalisen objektin sisällä sama kohteen ominaisuus saa eri arvot eri koordinaattipisteissä"@fi ;
  skos:definition "couverture qui retourne des valeurs différentes pour le même attribut d&#39;entité à différentes positions directes à l&#39;intérieur de tout objet spatial, temporel ou spatiotemporel dans son domaine"@fr ;
  skos:definition "동일한 피처(공간 객체, 시간 객체, 시공간 객체) 속성값이 영역 내 서로 다른 직접 위치에서 다른 값을 갖는 커버리지"@ko ;
  skos:definition "pokrycie, które przyjmuje różne wartości tego samego atrybutu obiektu w różnych położeniach bezpośrednich w obrębie pojedynczego obiektu przestrzennego, czasowego lub czasoprzestrzennego z jego dziedziny"@pl ;
  skos:definition "покрытие, возвращающее разные значения одного атрибута для различных  точек в пределах одного пространственного , временнóго или пространственно-временнóго объекта в его области определения"@ru ;
  skos:definition "cobertura que devuelve valores diferentes para el mismo atributo de objeto geográfico en diferentes posiciones directas dentro de un único objeto espacial, objeto temporal, u objeto espacio-temporal en su dominio"@es ;
  skos:definition "domänobjekttyp vars objekt definierar en domän inom vilket objektets uppgifter varierar kontinuerligt med positionen"@sv ;
  skos:definition "在一个数据覆盖域中，单独的空间对象、时间对象或时空对象的相同要素属性在不同的直接位置返回不同值的覆盖。"@zh ;

  skos:prefLabel "continuous coverage"@en ;
  skos:prefLabel "تغطية مستمرة"@ar ;
  skos:prefLabel "coverage,  sammenhængende"@da ;
  skos:prefLabel "stetiges Coverage"@de ;
  skos:prefLabel "jatkuva paikkatietojatkumo"@fi ;
  skos:prefLabel "couverture continue"@fr ;
  skos:prefLabel "연속 커버리지"@ko ;
  skos:prefLabel "liputan selanjar"@ms ;
  skos:prefLabel "pokrycie ciągłe"@pl ;
  skos:prefLabel "непрерывное покрытие"@ru ;
  skos:prefLabel "cobertura continua"@es ;
  skos:prefLabel "kontinuerlig domänobjekttyp"@sv ;
  skos:prefLabel "连续覆盖"@zh ;
  
  geolexica:origin lang:araRegistry ,
                lang:danRegistry ,
                lang:deuRegistry ,
                lang:engRegistry ,
                lang:finRegistry ,
                lang:fraRegistry ,
                lang:korRegistry ,
                # lang:nldRegistry ,
                # lang:jpnRegistry ,
                lang:rusRegistry ,
                lang:polRegistry ,
                lang:msaRegistry ,
                lang:spaRegistry ,
                lang:sweRegistry ,
                lang:zhoRegistry ;
          lang:deu-note notes:DefnTransUnavail , notes:NoteTransUnavail ;
          lang:fra-note notes:NoteTransDiff ;
          lang:msa-note notes:DefnTransUnavail , notes:NoteTransUnavail ;
          lang:swe-note notes:NoteTransUnavail .


###  https://isotc211.geolexica.org/ld/concepts#control_body
:control_body rdf:type owl:NamedIndividual ,
                   skos:Concept ;
          skos:inScheme geolexica:GeolexicaConceptScheme ;
          geolexica:hasInfo info:Info84 ;
          geolexica:hasReview reviews:Review84 ;
          geolexica:hasLDAPI ldapi:ldapi84-json ,
                             ldapi:ldapi84-jsonld ,
                             ldapi:ldapi84-rdfxml ,
                             ldapi:ldapi84-skosrdf ;
        geolexica:hasLangCode lang:ara ,
                        lang:dan ,
                        lang:deu ,
                        lang:eng ,
                        lang:fin ,
                        lang:fra ,
                        lang:kor ,
                        # lang:nld ,
                        lang:pol ,
                        # lang:jpn ,
                        # lang:msa ,
                        lang:rus ,
                        lang:spa ,
                        lang:swe ,
                        lang:zho ;
          dcterms:identifier 84 ;
          skos:notation 84 ;
          rdfs:label "control body" ;

  skos:definition "group of technical experts that makes decisions regarding the content of a register"@en ;
  skos:definition "مجموعة من الخبراء الفنيين تختص باتخاذ القرارات فيما يتعلق بمحتويات كل سجل"@ar ;
  skos:definition "gruppe af tekniske eksperter, der træffer beslutninger om indholdet af et register"@da ;
  skos:definition "Expertengruppe, welche über den Inhalt eines Registers entscheidet"@de ;
  skos:definition "teknisten asiantuntijoiden ryhmä, joka tekee rekisterin sisältöä koskevat päätökset"@fi ;
  skos:definition "groupe d&#39;experts techniques qui prend des décisions quant au contenu d&#39;un registre"@fr ;
  skos:definition "등록물의 내용에 대한 결정권을 갖는 전문가 집단"@ko ;
  skos:definition "grupa ekspertów technicznych podejmująca decyzje dotyczące zawartosci rejestru"@pl ;
  skos:definition "группа технических экспертов, которая принимает решения по содержанию реестра"@ru ;
  skos:definition "grupo de expertos técnicos que decide el contenido de un registro"@es ;
  skos:definition "grupp som fattar övergripande beslut gällande ett projekt eller en löpande verksamhet"@sv ;
  skos:definition "对注册表内容作决定的技术专家组。"@zh ;

  skos:prefLabel "control body"@en ;
  skos:prefLabel "جهاز الرقابة"@ar ;
  skos:prefLabel "kontrolorgan"@da ;
  skos:prefLabel "Koordinierungsgremium"@de ;
  skos:prefLabel "ohjausryhmä"@fi ;
  skos:prefLabel "organisme de contrôle"@fr ;
  skos:prefLabel "통제 기구"@ko ;
  skos:prefLabel "organ nadzorujący"@pl ;
  skos:prefLabel "управляющий орган"@ru ;
  skos:prefLabel "organismo de control"@es ;
  skos:prefLabel "styrgrupp"@sv ;
  skos:prefLabel "控制组"@zh ;
  
  geolexica:origin lang:araRegistry ,
                lang:danRegistry ,
                lang:deuRegistry ,
                lang:engRegistry ,
                lang:finRegistry ,
                lang:fraRegistry ,
                lang:korRegistry ,
                # lang:nldRegistry ,
                # lang:jpnRegistry ,
                lang:rusRegistry ,
                lang:polRegistry ,
                # lang:msaRegistry ,
                lang:spaRegistry ,
                lang:sweRegistry ,
                lang:zhoRegistry ;
          lang:rus-note notes:NoteTransDiff .

###  https://isotc211.geolexica.org/ld/concepts#conversion_rule
:conversion_rule rdf:type owl:NamedIndividual ,
                   skos:Concept ;
          skos:inScheme geolexica:GeolexicaConceptScheme ;
          geolexica:hasInfo info:Info85 ;
          geolexica:hasReview reviews:Review85 ;
          geolexica:hasLDAPI ldapi:ldapi85-json ,
                             ldapi:ldapi85-jsonld ,
                             ldapi:ldapi85-rdfxml ,
                             ldapi:ldapi85-skosrdf ;
        geolexica:hasLangCode lang:ara ,
                        lang:dan ,
                        lang:deu ,
                        lang:eng ,
                        lang:fin ,
                        lang:fra ,
                        lang:kor ,
                        # lang:nld ,
                        # lang:pol ,
                        # lang:jpn ,
                        lang:msa ,
                        lang:rus ,
                        lang:spa ,
                        lang:swe ,
                        lang:zho ;
          dcterms:identifier 85 ;
          skos:notation 85 ;
          rdfs:label "conversion rule" ;

  skos:definition "rule for converting instances in the input data structure to instances in the output data structure"@en ;
  skos:definition "قاعدة لتحويل حالات في هيكل البيانات المدخلة إلى حالات في هياكل البيانات المخرجة"@ar ;
  skos:definition "regel for at konvertere instanser i inputdatastrukturen til instanser i outputdatastrukturen"@da ;
  skos:definition "sääntö, jota sovelletaan tiedon muuntamisessa"@fi ;
  skos:definition "règle utilisée pour convertir les instances de la structure de données entrante en instances de la structure de données sortante"@fr ;
  skos:definition "입력 데이터 구조의 인스턴스를 출력 자료 구조의 인스턴스로 바꾸는 규칙"@ko ;
  skos:definition "правило преобразования экземпляров во входных структурах данных в экземпляры  выходных  структур данных"@ru ;
  skos:definition "regla para convertir instancias de la estructura de datos de entrada a instancias de la estructura de datos de salida"@es ;
  skos:definition "regel för att översätta data enligt en datastruktur till data enligt en annan datastruktur"@sv ;
  skos:definition "将输入数据结构的实例转换成输出数据结构实例的规则。"@zh ;

  skos:prefLabel "conversion rule"@en ;
  skos:prefLabel "قاعدة التحويل"@ar ;
  skos:prefLabel "konverteringsregel"@da ;
  skos:prefLabel "Konvertierungsregel"@de ;
  skos:prefLabel "muunnossääntö"@fi ;
  skos:prefLabel "règle de conversion"@fr ;
  skos:prefLabel "전환 규칙"@ko ;
  skos:prefLabel "undang-undang penukaran"@ms ;
  skos:prefLabel "правило преобразования"@ru ;
  skos:prefLabel "regla de conversión"@es ;
  skos:prefLabel "översättningsregel"@sv ;
  skos:prefLabel "转换规则"@zh ;
  skos:altLabel "muunnossääntö"@fi ;
  
  geolexica:origin lang:araRegistry ,
                lang:danRegistry ,
                lang:deuRegistry ,
                lang:engRegistry ,
                lang:finRegistry ,
                lang:fraRegistry ,
                lang:korRegistry ,
                # lang:nldRegistry ,
                # lang:jpnRegistry ,
                lang:rusRegistry ,
                # lang:polRegistry ,
                lang:msaRegistry ,
                lang:spaRegistry ,
                lang:sweRegistry ,
                lang:zhoRegistry ;
          lang:deu-note notes:DefnTransUnavail ;
          lang:msa-note notes:DefnTransUnavail .


###  https://isotc211.geolexica.org/ld/concepts#convex_hull
:convex_hull rdf:type owl:NamedIndividual ,
                   skos:Concept ;
          skos:inScheme geolexica:GeolexicaConceptScheme ;
          geolexica:hasInfo info:Info86 ;
          geolexica:hasReview reviews:Review86 ;
          geolexica:hasLDAPI ldapi:ldapi86-json ,
                             ldapi:ldapi86-jsonld ,
                             ldapi:ldapi86-rdfxml ,
                             ldapi:ldapi86-skosrdf ;
        geolexica:hasLangCode lang:ara ,
                        lang:dan ,
                        lang:deu ,
                        lang:eng ,
                        lang:fin ,
                        lang:fra ,
                        lang:kor ,
                        # lang:nld ,
                        # lang:pol ,
                        # lang:jpn ,
                        # lang:msa ,
                        lang:rus ,
                        lang:spa ,
                        lang:swe ,
                        lang:zho ;
          dcterms:identifier 86 ;
          skos:notation 86 ;
          rdfs:label "convex hull" ;

  skos:definition "smallest convex set containing a given geometric object"@en ;
  skos:definition "أصغر مجموعة محدَّبة تحتوي على جسم هندسي محدَّد"@ar ;
  skos:definition "mindste konvekse mængde, der kan indeholde et givet geometrisk objekt"@da ;
  skos:definition "pienin konveksi joukko, joka sisältää annetun geometrisen objektin"@fi ;
  skos:definition "plus petit ensemble convexe contenant un objet géométrique donné"@fr ;
  skos:definition "기하 객체를 포함하는 최소의 볼록 집합"@ko ;
  skos:definition "наименьшее из выпуклых множеств, содержащее данный геометрический объект"@ru ;
  skos:definition "conjunto convexo más pequeño que contiene un objeto geométrico dado"@es ;
  skos:definition "den minsta konvexa mängden som innehåller ett givet geometriskt objekt"@sv ;
  skos:definition "包含给定的几何对象的最小凸集。"@zh ;

  skos:prefLabel "convex hull"@en ;
  skos:prefLabel "هيكل محدَّب"@ar ;
  skos:prefLabel "konvekst hylster"@da ;
  skos:prefLabel "konvexe Hülle"@de ;
  skos:prefLabel "konveksi peite"@fi ;
  skos:altLabel "konveksi verho"@fi ;
  skos:prefLabel "enveloppe convexe"@fr ;
  skos:prefLabel "볼록 외곽"@ko ;
  skos:prefLabel "выпуклая оболочка"@ru ;
  skos:prefLabel "cierre convexo"@es ;
  skos:prefLabel "konvext hölje"@sv ;
  skos:prefLabel "凸包"@zh ;
  
  geolexica:origin lang:araRegistry ,
                lang:danRegistry ,
                lang:deuRegistry ,
                lang:engRegistry ,
                lang:finRegistry ,
                lang:fraRegistry ,
                lang:korRegistry ,
                # lang:nldRegistry ,
                # lang:jpnRegistry ,
                lang:rusRegistry ,
                # lang:polRegistry ,
                # lang:msaRegistry ,
                lang:spaRegistry ,
                lang:sweRegistry ,
                lang:zhoRegistry ;
          lang:deu-note notes:DefnTransUnavail, notes:NoteTransUnavail .


###  https://isotc211.geolexica.org/ld/concepts#convex_set
:convex_set rdf:type owl:NamedIndividual ,
                   skos:Concept ;
          skos:inScheme geolexica:GeolexicaConceptScheme ;
          geolexica:hasInfo info:Info87 ;
          geolexica:hasReview reviews:Review87 ;
          geolexica:hasLDAPI ldapi:ldapi87-json ,
                             ldapi:ldapi87-jsonld ,
                             ldapi:ldapi87-rdfxml ,
                             ldapi:ldapi87-skosrdf ;
        geolexica:hasLangCode lang:ara ,
                        lang:dan ,
                        lang:deu ,
                        lang:eng ,
                        lang:fin ,
                        lang:fra ,
                        lang:kor ,
                        # lang:nld ,
                        # lang:pol ,
                        # lang:jpn ,
                        # lang:msa ,
                        lang:rus ,
                        lang:spa ,
                        lang:swe ,
                        lang:zho ;
          dcterms:identifier 87 ;
          skos:notation 87 ;
          rdfs:label "convex set" ;

  skos:definition "geometric set in which any direct position on the straight-line segment joining any two direct positions in the geometric set is also contained in the geometric set"@en ;
  skos:definition "مجموعة هندسية يكون كل موقع مباشر على المقطع المستقيم الذي يصل بين أي موقعين مباشرين فيها مشمولا هو الآخر في المجموعة"@ar ;
  skos:definition "geometrisk mængde, i hvilket det gælder, at uanset hvilke to punkter vi tager i mængden og tager linjestykket mellem disse, er linjestykket fuldt indeholdt i mængden."@da ;
  skos:definition "geometrinen joukko, jossa mikä hyvänsä kahta pistettä yhdistävällä suoralla oleva piste sisältyy tähän geometriseen joukkoon"@fi ;
  skos:definition "ensemble géométrique dans laquelle n&#39;importe quelle position directe sur le segment de droite joignant deux points dans l&#39;ensemble géométrique est également contenue dans l&#39;ensemble géométrique"@fr ;
  skos:definition "내부의 임의 두 직접 위치를 잇는 직선 조각상의 모든 점을 포함할 수 있는 기하 집합"@ko ;
  skos:definition "геометрическое множество, в котором любой отрезок прямой, соединяющий две любые точки данного множества, также принадлежит этому геометрическому множеству"@ru ;
  skos:definition "conjunto geométrico en el que cualquier posición directa del segmento que une dos posiciones directas cualesquiera del conjunto geométrico, también está contenida en el conjunto geométrico"@es ;
  skos:definition "punktmängd sådan att varje punkt längs en sträcka mellan två godtyckligt valda punkter i mängden också ligger i mängden"@sv ;
  skos:definition "一种几何集，在几何集中连接任意两个直接位置的直线段上的任意直接位置都包含在该几何集合中。"@zh ;

  skos:prefLabel "convex set"@en ;
  skos:prefLabel "مجموعة محدَّبة"@ar ;
  skos:prefLabel "konveks mængde"@da ;
  skos:prefLabel "konvexe Menge"@de ;
  skos:prefLabel "konveksi joukko"@fi ;
  skos:prefLabel "ensemble convexe"@fr ;
  skos:prefLabel "볼록 집합"@ko ;
  skos:prefLabel "выпуклое множество"@ru ;
  skos:prefLabel "conjunto convexo"@es ;
  skos:prefLabel "konvex mängd"@sv ;
  skos:prefLabel "凸集"@zh ;
  
  geolexica:origin lang:araRegistry ,
                lang:danRegistry ,
                lang:deuRegistry ,
                lang:engRegistry ,
                lang:finRegistry ,
                lang:fraRegistry ,
                lang:korRegistry ,
                # lang:nldRegistry ,
                # lang:jpnRegistry ,
                lang:rusRegistry ,
                # lang:polRegistry ,
                # lang:msaRegistry ,
                lang:spaRegistry ,
                lang:sweRegistry ,
                lang:zhoRegistry ;
          lang:deu-note notes:DefnTransUnavail, notes:NoteTransUnavail ;
          lang:swe-note notes:NoteTransUnavail .


###  https://isotc211.geolexica.org/ld/concepts#coordinate
:coordinate rdf:type owl:NamedIndividual ,
                   skos:Concept ;
          skos:inScheme geolexica:GeolexicaConceptScheme ;
          geolexica:hasInfo info:Info88 ;
          geolexica:hasReview reviews:Review88 ;
          geolexica:hasLDAPI ldapi:ldapi88-json ,
                             ldapi:ldapi88-jsonld ,
                             ldapi:ldapi88-rdfxml ,
                             ldapi:ldapi88-skosrdf ;
        geolexica:hasLangCode lang:ara ,
                        lang:dan ,
                        lang:deu ,
                        lang:eng ,
                        lang:fin ,
                        lang:fra ,
                        lang:kor ,
                        lang:nld ,
                        lang:pol ,
                        # lang:jpn ,
                        lang:msa ,
                        lang:rus ,
                        lang:spa ,
                        lang:swe ,
                        lang:zho ;
          dcterms:identifier 88 ;
          skos:notation 88 ;
          rdfs:label "coordinate" ;

  skos:definition "one of a sequence of n numbers designating the position of a point in n-dimensional space"@en ;
  skos:definition "واحد من سلسلة أعداد (ع) تحدد موقع نقطة في حيز مكاني أبعاده (ع)"@ar ;
  skos:definition "et af en sekvens af n tal, der betegner positionen af et punkt i det n-dimensionale rum"@da ;
  skos:definition "eine aus der Folge von n Zahlen, die die Position eines Punktes im n-dimensionalen Raum beschreiben"@de ;
  skos:definition "kukin n:stä järjestetystä lukuarvosta, jotka määrittelevät pisteen sijainnin valitussa n-ulotteisessa avaruudessa"@fi ;
  skos:definition "élément d&#39;un n-uplet désignant la position d&#39;un point dans un espace de dimension n"@fr ;
  skos:definition "n차원의 공간에서 점의 위치를 표현하는 n개의 숫자 연속"@ko ;
  skos:definition "pasangan nombor yg menentukan kedudukan sesuatu titik pd ruang yg ukurannya diberikan"@ms ;
  skos:definition "getal in een sequentie van n getallen om de positie van een punt in een n-dimensionale ruimte te bepalen"@nl ;
  skos:definition "jedna liczba z sekwencji n liczb oznaczających pozycję punktu w przestrzeni n-wymiarowej"@pl ;
  skos:definition "число из упорядоченного набора N чисел, описывающих положение пункта в N-мерном пространстве"@ru ;
  skos:definition "cualquiera de los n números de una secuencia que designa la posición de un punto en un sistema n-dimensional"@es ;
  skos:definition "ett av de n tal som tillsammans anger en punkts läge i ett n-dimesionellt rum"@sv ;
  skos:definition "表示一个点在n维空间中位置的n个数值组成的有序数之一。"@zh ;

  skos:prefLabel "coordinate"@en ;
  skos:prefLabel "إحداثي"@ar ;
  skos:prefLabel "koordinat"@da ;
  skos:prefLabel "Koordinate"@de ;
  skos:prefLabel "koordinaatti"@fi ;
  skos:prefLabel "coordonnée"@fr ;
  skos:prefLabel "좌표"@ko ;
  skos:prefLabel "koordinat"@ms ;
  skos:prefLabel "coördinaat"@nl ;
  skos:prefLabel "współrzędna"@pl ;
  skos:prefLabel "координата"@ru ;
  skos:prefLabel "coordenada"@es ;
  skos:prefLabel "koordinat"@sv ;
  skos:prefLabel "坐标"@zh ;
  skos:altLabel "coordinate"@nl ;
  
  geolexica:origin lang:araRegistry ,
                lang:danRegistry ,
                lang:deuRegistry ,
                lang:engRegistry ,
                lang:finRegistry ,
                lang:fraRegistry ,
                lang:korRegistry ,
                lang:nldRegistry ,
                # lang:jpnRegistry ,
                lang:rusRegistry ,
                lang:polRegistry ,
                lang:msaRegistry ,
                lang:spaRegistry ,
                lang:sweRegistry ,
                lang:zhoRegistry ;
          lang:deu-note notes:DefnTransUnavail ;
          lang:msa-note notes:NoteTransUnavail ; 
          lang:swe-note notes:NoteTransUnavail .

###  https://isotc211.geolexica.org/ld/concepts#coordinate_dimension
:coordinate_dimension rdf:type owl:NamedIndividual ,
                   skos:Concept ;
          skos:inScheme geolexica:GeolexicaConceptScheme ;
          geolexica:hasInfo info:Info90 ;
          geolexica:hasReview reviews:Review90 ;
          geolexica:hasLDAPI ldapi:ldapi90-json ,
                             ldapi:ldapi90-jsonld ,
                             ldapi:ldapi90-rdfxml ,
                             ldapi:ldapi90-skosrdf ;
        geolexica:hasLangCode lang:ara ,
                        lang:dan ,
                        lang:deu ,
                        lang:eng ,
                        lang:fin ,
                        lang:fra ,
                        lang:kor ,
                        # lang:nld ,
                        lang:pol ,
                        lang:jpn ,
                        # lang:msa ,
                        lang:rus ,
                        lang:spa ,
                        lang:swe ,
                        lang:zho ;
          dcterms:identifier 90 ;
          skos:notation 90 ;
          rdfs:label "coordinate dimension" ;

  skos:definition "number of measurements or axes needed to describe a position in a coordinate system"@en ;
  skos:definition "عدد القياسات أو المحاور المطلوبة لوصف موقع ما في إطار نظام إحداثي"@ar ;
  skos:definition "antallet af målinger eller akser, der er nødvendige for at kunne beskrive en position i et koordinatsystem"@da ;
  skos:definition "niiden mittojen tai akselien lukumäärä, jotka tarvitaan sijainnin ilmaisemiseksi koordinaatistossa"@fi ;
  skos:definition "nombre de mesures ou d&#39;axes nécessaires pour décrire une position dans un système de coordonnées"@fr ;
  skos:definition "ある座標系における位置を記述するために必要な計測値又は座標軸の数。"@ja ;
  skos:definition "좌표 체계에서 위치를 기술하는 데 필요한 측정 또는 축의 수"@ko ;
  skos:definition "liczba pomiarów lub osi potrzebnych do opisania położenia w układzie współrzędnych"@pl ;
  skos:definition "количество измерений или осей, необходимое для описания положения в системе координат"@ru ;
  skos:definition "número de mediciones o ejes necesarios para describir una posición en un sistema de coordenadas"@es ;
  skos:definition "antal bestämningar eller axlar som behövs för att ange en position i ett koordinatsystem"@sv ;
  skos:definition "在一个坐标系中，描述一个位置所需的量测或坐标轴的个数。"@zh ;

  skos:prefLabel "coordinate dimension"@en ;
  skos:prefLabel "البعد الإحداثي"@ar ;
  skos:prefLabel "koordinatdimension"@da ;
  skos:prefLabel "Koordinatendimension"@de ;
  skos:prefLabel "koordinaatiston ulottuvuus"@fi ;
  skos:prefLabel "dimension de coordonnées"@fr ;
  skos:prefLabel "座標次元"@ja ;
  skos:prefLabel "좌표 차원"@ko ;
  skos:prefLabel "wymiar współrzędnych"@pl ;
  skos:prefLabel "размерность координат"@ru ;
  skos:prefLabel "dimensión de coordenadas"@es ;
  skos:prefLabel "koordinatdimension"@sv ;
  skos:prefLabel "坐标维数"@zh ;
  
  geolexica:origin lang:araRegistry ,
                lang:danRegistry ,
                lang:deuRegistry ,
                lang:engRegistry ,
                lang:finRegistry ,
                lang:fraRegistry ,
                lang:korRegistry ,
                # lang:nldRegistry ,
                lang:jpnRegistry ,
                lang:rusRegistry ,
                lang:polRegistry ,
                # lang:msaRegistry ,
                lang:spaRegistry ,
                lang:sweRegistry ,
                lang:zhoRegistry ;
          lang:deu-note notes:DefnTransUnavail .


###  https://isotc211.geolexica.org/ld/concepts#coordinate_operation
:coordinate_operation rdf:type owl:NamedIndividual ,
                   skos:Concept ;
          skos:inScheme geolexica:GeolexicaConceptScheme ;
          geolexica:hasInfo info:Info91 ;
          geolexica:hasReview reviews:Review91 ;
          geolexica:hasLDAPI ldapi:ldapi91-json ,
                             ldapi:ldapi91-jsonld ,
                             ldapi:ldapi91-rdfxml ,
                             ldapi:ldapi91-skosrdf ;
        geolexica:hasLangCode lang:ara ,
                        lang:dan ,
                        lang:deu ,
                        lang:eng ,
                        lang:fin ,
                        lang:fra ,
                        lang:kor ,
                        lang:nld ,
                        lang:pol ,
                        # lang:jpn ,
                        # lang:msa ,
                        lang:rus ,
                        lang:spa ,
                        lang:swe ,
                        lang:zho ;
          dcterms:identifier 91 ;
          skos:notation 91 ;
          rdfs:label "coordinate operation" ;

  skos:definition "change of coordinates, based on a one-to-one relationship, from one coordinate reference system to another"@en ;
  skos:definition "تغيير للإحداثيات lبنى على علاقة تقابل واحد لواحد من نظام إحداثيات مرجعي معين إلى آخر"@ar ;
  skos:definition "ændring af koordinater baseret på en 1 til 1-relation fra et koordinatsystem til et andet"@da ;
  skos:definition "eineindeutige Koordinatenänderung von einem Koordinatenreferenzsystem in ein anderes"@de ;
  skos:definition "koordinaattien muuntaminen yksi yhteen -suhteessa koordinaattijärjestelmästä toiseen"@fi ;
  skos:definition "changement de coordonnées, basé sur une relation 1:1, d&#39;un système de coordonnées de référence à un autre"@fr ;
  skos:definition "하나의 좌표 참조 체계로부터 다른 좌표 참조 체계로의 1대1 관계를 갖는 좌표 변경"@ko ;
  skos:definition "verandering van coördinaten, gebaseerd op een één op één relatie van het ene coördinaatreferentiesysteem tot het andere."@nl ;
  skos:definition "zamiana współrzędnych, oparta na związku jeden do jednego, jednego systemu odniesienia na współrzędne drugiego systemu odniesienia"@pl ;
  skos:definition "изменение координат пространственных объектов с использованием их математической связи при переходе от одной системы координат к другой"@ru ;
  skos:definition "cambio de coordenadas, basado en una relación uno a uno, desde un sistema de referencia de coordenadas a otro"@es ;
  skos:definition "omräkning av punkters koordinatvärden,  baserad på ett ett-till-ett-förhållande, från ett koordinatbaserat referenssystem till ett annat"@sv ;
  skos:definition "从一个坐标参照系到另一个参照坐标系一一对应的坐标改变。"@zh ;

  skos:prefLabel "coordinate operation"@en ;
  skos:prefLabel "عملية إحداثية"@ar ;
  skos:prefLabel "koordinatoperation"@da ;
  skos:prefLabel "Koordinatenoperation"@de ;
  skos:prefLabel "koordinaattioperaatio"@fi ;
  skos:altLabel "koordinaatteihin liittyvä laskentaoperaatio"@fi ;
  skos:prefLabel "opération sur les coordonnées"@fr ;
  skos:prefLabel "좌표 연산"@ko ;
  skos:prefLabel "coördinaatbewerking"@nl ;
  skos:prefLabel "operacja na współrzędnych"@pl ;
  skos:prefLabel "операции с координатами"@ru ;
  skos:prefLabel "operación de coordenadas"@es ;
  skos:prefLabel "koordinatomräkning"@sv ;
  skos:prefLabel "坐标操作"@zh ;
  
  geolexica:origin lang:araRegistry ,
                lang:danRegistry ,
                lang:deuRegistry ,
                lang:engRegistry ,
                lang:finRegistry ,
                lang:fraRegistry ,
                lang:korRegistry ,
                lang:nldRegistry ,
                # lang:jpnRegistry ,
                lang:rusRegistry ,
                lang:polRegistry ,
                # lang:msaRegistry ,
                lang:spaRegistry ,
                lang:sweRegistry ,
                lang:zhoRegistry ;
          lang:deu-note notes:DefnTransUnavail ;
          lang:swe-note notes:DefnTransUnavail .


###  https://isotc211.geolexica.org/ld/concepts#coordinate_system
:coordinate_system rdf:type owl:NamedIndividual ,
                   skos:Concept ;
          skos:inScheme geolexica:GeolexicaConceptScheme ;
          geolexica:hasInfo info:Info93 ;
          geolexica:hasReview reviews:Review93 ;
          geolexica:hasLDAPI ldapi:ldapi93-json ,
                             ldapi:ldapi93-jsonld ,
                             ldapi:ldapi93-rdfxml ,
                             ldapi:ldapi93-skosrdf ;
        geolexica:hasLangCode lang:ara ,
                        lang:dan ,
                        lang:deu ,
                        lang:eng ,
                        lang:fin ,
                        lang:fra ,
                        lang:kor ,
                        lang:nld ,
                        lang:pol ,
                        # lang:jpn ,
                        # lang:msa ,
                        lang:rus ,
                        lang:spa ,
                        lang:swe ,
                        lang:zho ;
          dcterms:identifier 93 ;
          skos:notation 93 ;
          rdfs:label "coordinate system" ;

  skos:definition "set of mathematical rules for specifying how coordinates are to be assigned to points"@en ;
  skos:definition "مجموعة من القواعد الرياضية لتحديد كيفية تعيين الإحداثيات للنقاط"@ar ;
  skos:definition "sæt af matematiske regler, der specificerer, hvordan koordinater henføres til punkter"@da ;
  skos:definition "Menge mathematischer Regeln zur Festlegung, wie Koordinaten Punkten zuzuordnen sind"@de ;
  skos:definition "matemaattisten sääntöjen joukko, jolla määritellään se, miten pisteille annetaan koordinaatit"@fi ;
  skos:definition "ensemble de règles mathématiques spécifiant comment les coordonnées doivent être affectées aux points"@fr ;
  skos:definition "점에 어떤 좌표를 부여할지를 규정하기 위한 수학적 규칙의 집합"@ko ;
  skos:definition "set van wiskundige regels voor het toekennen van coördinaten aan punten"@nl ;
  skos:definition "zbiór reguł matematycznych określających w jaki sposób punktom przypisywane są współrzędne"@pl ;
  skos:definition "набор математических правил, описывающих, как координаты должны быть соотнесены с точками пространства"@ru ;
  skos:definition "conjunto de reglas matemáticas que especifican cómo las coordenadas deben ser asignadas a los puntos"@es ;
  skos:definition "uppsättning av matematiska regler för hur koordinater ska anges för punkter+E730"@sv ;
  skos:definition "给点赋予坐标的数学规则集。"@zh ;

  skos:prefLabel "coordinate system"@en ;
  skos:prefLabel "نظام إحداثيات"@ar ;
  skos:prefLabel "koordinatsystem"@da ;
  skos:prefLabel "Koordinatensystem"@de ;
  skos:prefLabel "koordinaatisto"@fi ;
  skos:prefLabel "système de coordonnées"@fr ;
  skos:prefLabel "좌표 체계"@ko ;
  skos:prefLabel "coördinaatsysteem"@nl ;
  skos:prefLabel "układ współrzędnych"@pl ;
  skos:prefLabel "система координат"@ru ;
  skos:prefLabel "sistema de coordenadas"@es ;
  skos:prefLabel "koordinatsystem"@sv ;
  skos:prefLabel "坐标系"@zh ;
  
  geolexica:origin lang:araRegistry ,
                lang:danRegistry ,
                lang:deuRegistry ,
                lang:engRegistry ,
                lang:finRegistry ,
                lang:fraRegistry ,
                lang:korRegistry ,
                lang:nldRegistry ,
                # lang:jpnRegistry ,
                lang:rusRegistry ,
                lang:polRegistry ,
                # lang:msaRegistry ,
                lang:spaRegistry ,
                lang:sweRegistry ,
                lang:zhoRegistry .


###  https://isotc211.geolexica.org/ld/concepts#Coordinated_Universal_Time
:Coordinated_Universal_Time rdf:type owl:NamedIndividual ,
                   skos:Concept ;
          skos:inScheme geolexica:GeolexicaConceptScheme ;
          geolexica:hasInfo info:Info96 ;
        #   geolexica:hasReview reviews:Review96 ;
          geolexica:hasLDAPI ldapi:ldapi96-json ,
                             ldapi:ldapi96-jsonld ,
                             ldapi:ldapi96-rdfxml ,
                             ldapi:ldapi96-skosrdf ;
        geolexica:hasLangCode lang:ara ,
                        lang:dan ,
                        lang:deu ,
                        lang:eng ,
                        lang:fin ,
                        lang:fra ,
                        lang:kor ,
                        # lang:nld ,
                        # lang:pol ,
                        # lang:jpn ,
                        # lang:msa ,
                        lang:rus ,
                        lang:spa ,
                        # lang:swe ,
                        lang:zho ;
          dcterms:identifier 96 ;
          skos:notation 96 ;
          rdfs:label "Coordinated Universal Time (UTC)" ;

  skos:definition "time scale maintained by the Bureau International des Poids et Mesures (International Bureau of Weights and Measures) and the International Earth Rotation Service (IERS) that forms the basis of a coordinated dissemination of standard frequencies and time"@en ;
  skos:definition "المقياس الزمني المعتمد لدى المكتب العالمي للأوزان والقياسات والخدمة العالمية لدوران كوكب الأرض والذي يمثل الأساس الذي يقوم عليه النشر القياسي المجمع عليه عالميا للذبذبات القياسية والتوقيت القياسي"@ar ;
  skos:definition "tidsskala, der varetages af Bureau International des Poids et Mesures (International Bureau of Weights and Measures) og International Earth Rotation Service (IERS), og som danner grundlaget for en koordineret udbredelse af standardfrekvenser og standardtid"@da ;
  skos:definition "toimielinten Bureau International des Poids et Mesures (International Bureau of Weights and Measures) ja International Earth Rotation Service (IERS) ylläpitämä aika-asteikko, joka muodostaa pohjan standardifrekvenssien ja -ajan koordinoidulle jakamiselle"@fi ;
  skos:definition "échelle de temps maintenue par le Bureau international des Poids et Mesures et l&#39;International Earth Rotation Service (IERS) qui forme la base d&#39;une diffusion coordonnée des fréquences étalon et de l&#39;heure"@fr ;
  skos:definition "国際度量衡局（International Bureau of Weights and Measures）及び国際地球回転観測事業（International Earth Rotation Service）によって維持管理されている時間尺度。標準周波数及び時刻信号に関する標準電波の基礎となるもの[ITU-R Rec.TF.686-1(1997)]。"@ja ;
  skos:definition "제 도량형 협회와 표준시와 표준 주파수를 보급하는 국제 지구 자전 협회(IERS: International Earth Rotation Service)가 유지 관리하는 시간 척도"@ko ;
  skos:definition "шкала времени, утвержденная Международным бюро мер и весов (МБМВ) и Международной службой вращения Земли (МСВЗ), и служащая основой скоординированной передачи стандартных частот и трансляции сигналов времени"@ru ;
  skos:definition "escala temporal según la Oficina Internacional de Pesos y Medidas (Bureau International des Poids et Mesures) y el Servicio Internacional de Rotación de la Tierra, IERS (International Earth Rotation Service), que constituye la base de una difusión coordinada de las frecuencias estándar y señales horarias"@es ;
  skos:definition "由国际计量局与国际地球自转服务局（IERS)维护的时标，它构成协调发布标准频率和时间信号基础。"@zh ;

  skos:prefLabel "Coordinated Universal Time (UTC)"@en ;
  skos:prefLabel "التوقيت العالمي (UTC)"@ar ;
  skos:prefLabel "UTC, Coordinated Universal Time"@da ;
  skos:prefLabel "koordinierte Weltzeit (UTC)"@de ;
  skos:prefLabel "koordinoitu yleisaika"@fi ;
  skos:prefLabel "Temps Universel Coordonné (UTC)"@fr ;
  skos:prefLabel "協定世界時，UTC"@ja ;
  skos:prefLabel "협정 세계시"@ko ;
  skos:prefLabel "всемирное координированное время"@ru ;
  skos:prefLabel "Tiempo Universal Coordinado (UTC)"@es ;
  skos:prefLabel "协调世界时"@zh ;
  
  geolexica:origin lang:araRegistry ,
                lang:danRegistry ,
                lang:deuRegistry ,
                lang:engRegistry ,
                lang:finRegistry ,
                lang:fraRegistry ,
                lang:korRegistry ,
                # lang:nldRegistry ,
                lang:jpnRegistry ,
                lang:rusRegistry ,
                # lang:polRegistry ,
                # lang:msaRegistry ,
                lang:spaRegistry ,
                # lang:sweRegistry ,
                lang:zhoRegistry .


###  https://isotc211.geolexica.org/ld/concepts#cost_function
:cost_function rdf:type owl:NamedIndividual ,
                   skos:Concept ;
          skos:inScheme geolexica:GeolexicaConceptScheme ;
          geolexica:hasInfo info:Info97 ;
        #   geolexica:hasReview reviews:Review97 ;
          geolexica:hasLDAPI ldapi:ldapi97-json ,
                             ldapi:ldapi97-jsonld ,
                             ldapi:ldapi97-rdfxml ,
                             ldapi:ldapi97-skosrdf ;
        geolexica:hasLangCode lang:ara ,
                        lang:dan ,
                        lang:deu ,
                        lang:eng ,
                        lang:fin ,
                        lang:fra ,
                        lang:kor ,
                        # lang:nld ,
                        # lang:pol ,
                        # lang:jpn ,
                        # lang:msa ,
                        lang:rus ,
                        lang:spa ,
                        lang:swe ,
                        lang:zho ;
          dcterms:identifier 97 ;
          skos:notation 97 ;
          rdfs:label "cost function" ;

  skos:definition "function that associates a measure (cost) to a route"@en ;
  skos:definition "دالة تربط بين القياس (التكلفة) وطريق أو مسار معين"@ar ;
  skos:definition "funktion, der forbinder et mål (omkostning) med en rute"@da ;
  skos:definition "toiminto, joka liittää reittiin mitattavan kustannussuureen"@fi ;
  skos:definition "fonction qui associe une mesure (coût) à un itinéraire"@fr ;
  skos:definition "경로 측정(비용)과 관련된 함수"@ko ;
  skos:definition "функция, связывающая меру  (стоимость) передвижения с маршрутом движения"@ru ;
  skos:definition "función que asocia una medida (costo) a una ruta"@es ;
  skos:definition "(inom ekonomi) funktion som anger samband mellan kostnad och produktion"@sv ;
  skos:definition "与路径关联的成本的函数。"@zh ;

  skos:prefLabel "cost function"@en ;
  skos:prefLabel "دالة التكلفة"@ar ;
  skos:prefLabel "omkostningsfunktion"@da ;
  skos:prefLabel "Kostenfunktion"@de ;
  skos:prefLabel "kustannusfunktio"@fi ;
  skos:prefLabel "fonction de coût"@fr ;
  skos:prefLabel "비용 함수"@ko ;
  skos:prefLabel "функция стоимости"@ru ;
  skos:prefLabel "función de costo"@es ;
  skos:prefLabel "kostnadsfunktion"@sv ;
  skos:prefLabel "成本函数"@zh ;
  
  geolexica:origin lang:araRegistry ,
                lang:danRegistry ,
                lang:deuRegistry ,
                lang:engRegistry ,
                lang:finRegistry ,
                lang:fraRegistry ,
                lang:korRegistry ,
                # lang:nldRegistry ,
                # lang:jpnRegistry ,
                lang:rusRegistry ,
                # lang:polRegistry ,
                # lang:msaRegistry ,
                lang:spaRegistry ,
                lang:sweRegistry ,
                lang:zhoRegistry ;
        lang:deu-note notes:DefnTransUnavail, notes:NoteTransUnavail ;
        lang:fra-note notes:NoteTransDiff ;
        lang:swe-note notes:NoteTransUnavail .


###  https://isotc211.geolexica.org/ld/concepts#coverage
:coverage rdf:type owl:NamedIndividual ,
                   skos:Concept ;
          skos:inScheme geolexica:GeolexicaConceptScheme ;
          geolexica:hasInfo info:Info99 ;
        #   geolexica:hasReview reviews:Review99 ;
          geolexica:hasLDAPI ldapi:ldapi99-json ,
                             ldapi:ldapi99-jsonld ,
                             ldapi:ldapi99-rdfxml ,
                             ldapi:ldapi99-skosrdf ;
        geolexica:hasLangCode lang:ara ,
                        lang:dan ,
                        lang:deu ,
                        lang:eng ,
                        lang:fin ,
                        lang:fra ,
                        lang:kor ,
                        # lang:nld ,
                        lang:pol ,
                        # lang:jpn ,
                        lang:msa ,
                        lang:rus ,
                        lang:spa ,
                        lang:swe ,
                        lang:zho ;
          dcterms:identifier 99 ;
          skos:notation 99 ;
          rdfs:label "coverage" ;

  skos:definition "feature that acts as a function to return values from its range for any direct position within its spatial, temporal or spatiotemporal domain"@en ;
  skos:definition "معلم يعمل كوظيفة لإعادة القيم من نطاق تفاوته بالنسبة لأي موقع مباشر يقع ضمن نطاقه المكاني أو نطاقه الزماني أو نطاقه المكاني-الزماني"@ar ;
  skos:definition "feature, der virker som en funktion, som returnerer værdier fra sin værdimængde, for enhver direkte position inden for dens rumlige, temporale eller rumlig-temporale domæne"@da ;
  skos:definition "Feature, das in Form einer Funktion für jeden räumlichen, zeitlichen oder raum-zeitlichen Punkt innerhalb seines Definitionsbereichs einen Wertevektor liefert"@de ;
  skos:definition "alueen kattavana jatkumona esitetty paikkatietokohde"@fi ;
  skos:definition "entité agissant comme une fonction retournant des valeurs de sa gamme de valeurs pour toute position directe dans son domaine spatial, temporel ou spatiotemporel"@fr ;
  skos:definition "시공간 영역(공간, 시간, 시공간) 내에서 함수처럼 그 범위 내의 특정 직접 위치에 대한 값을 반환하는 피처"@ko ;
  skos:definition "sesuatu yg meliputi (menyeliputi, memenuhi, menutupi) sesuatu"@ms ;
  skos:definition "obiekt , który działa jak funkcja zwracająca wartości ze swojego zakresu dla każdego położenia bezpośredniego należącego do jej dziedziny przestrzennej, czasowej lub czasoprzestrzennej"@pl ;
  skos:definition "модель объекта, представляющая собой функцию, возвращающую значения из диапазона допустимых значений для каждой точки в пространственной, временнóй или пространственно-временнóй области определения"@ru ;
  skos:definition "objeto geográfico que actúa como una función que devuelve valores de su rango para cualquier posición directa dentro de su dominio  espacial, temporal o espacio-temporal"@es ;
  skos:definition "objekttyp vars objekt definierar ett rumslig, temporal eller rumstemporal domän inom vilket objektets uppgifter kan variera med positionen"@sv ;
  skos:definition "在空间域、时间域或时空域中，为任意直接位置充当函数，从其值域中返回数值的要素。"@zh ;

  skos:prefLabel "coverage"@en ;
  skos:prefLabel "التغطية"@ar ;
  skos:prefLabel "coverage"@da ;
  skos:prefLabel "Coverage"@de ;
  skos:prefLabel "paikkatietojatkumo"@fi ;
  skos:prefLabel "couverture"@fr ;
  skos:prefLabel "커버리지"@ko ;
  skos:prefLabel "liputan"@ms ;
  skos:prefLabel "pokrycie"@pl ;
  skos:prefLabel "покрытие"@ru ;
  skos:prefLabel "cobertura"@es ;
  skos:prefLabel "domänobjekttyp"@sv ;
  skos:prefLabel "覆盖"@zh ;
  
  geolexica:origin lang:araRegistry ,
                lang:danRegistry ,
                lang:deuRegistry ,
                lang:engRegistry ,
                lang:finRegistry ,
                lang:fraRegistry ,
                lang:korRegistry ,
                # lang:nldRegistry ,
                # lang:jpnRegistry ,
                lang:rusRegistry ,
                lang:polRegistry ,
                lang:msaRegistry ,
                lang:spaRegistry ,
                lang:sweRegistry ,
                lang:zhoRegistry ;
        lang:deu-note notes:DefnTransUnavail, notes:NoteTransUnavail ;
        lang:msa-note notes:ExTransUnavail, notes:NoteTransUnavail ;
        lang:fra-note notes:NoteTransDiff ;
        lang:swe-note notes:ExTransUnavail .


###  https://isotc211.geolexica.org/ld/concepts#coverage_geometry
:coverage_geometry rdf:type owl:NamedIndividual ,
                   skos:Concept ;
          skos:inScheme geolexica:GeolexicaConceptScheme ;
          geolexica:hasInfo info:Info100 ;
        #   geolexica:hasReview reviews:Review100 ;
          geolexica:hasLDAPI ldapi:ldapi100-json ,
                             ldapi:ldapi100-jsonld ,
                             ldapi:ldapi100-rdfxml ,
                             ldapi:ldapi100-skosrdf ;
        geolexica:hasLangCode lang:ara ,
                        lang:dan ,
                        lang:deu ,
                        lang:eng ,
                        lang:fin ,
                        lang:fra ,
                        lang:kor ,
                        # lang:nld ,
                        # lang:pol ,
                        # lang:jpn ,
                        lang:msa ,
                        lang:rus ,
                        lang:spa ,
                        lang:swe ,
                        lang:zho ;
          dcterms:identifier 100 ;
          skos:notation 100 ;
          rdfs:label "coverage geometry" ;

  skos:definition "configuration of the domain of a coverage described in terms of coordinates"@en ;
  skos:definition "تكوين نطاق التغطية الموصوف من خلال الإحداثيات"@ar ;
  skos:definition "konfiguration af domænet for en coverage beskrevet i form af koordinater"@da ;
  skos:definition "koordinaattien avulla ilmaistu paikkatietojatkumon kokoonpano"@fi ;
  skos:definition "configuration du domaine d&#39;une couverture décrite en termes de coordonnées"@fr ;
  skos:definition "좌표로 기술된 커버리지의 시공간적 영역에 대한 구성"@ko ;
  skos:definition "konfiguracja dziedziny pokrycia opisana współrzędnymi"@pl ;
  skos:definition "конфигурация области определения покрытия, описываемая в терминах координат"@ru ;
  skos:definition "configuración del dominio de una cobertura en términos de coordenadas"@es ;
  skos:definition "koordinatbaserad beskrivning av den domän som definieras av ett domänobjekt"@sv ;
  skos:definition "按照坐标描述的数据覆盖的域结构。"@zh ;

  skos:prefLabel "coverage geometry"@en ;
  skos:prefLabel "هندسة التغطية"@ar ;
  skos:prefLabel "coverage-geometri"@da ;
  skos:prefLabel "Coveragegeometrie"@de ;
  skos:prefLabel "paikkatietojatkumon geometria"@fi ;
  skos:prefLabel "géométrie de couverture"@fr ;
  skos:prefLabel "커버리지 기하"@ko ;
  skos:prefLabel "geometria pokrycia"@pl ;
  skos:prefLabel "геометрия покрытия"@ru ;
  skos:prefLabel "geometría de la cobertura"@es ;
  skos:prefLabel "domängeometri"@sv ;
  skos:prefLabel "覆盖几何"@zh ;
  
  geolexica:origin lang:araRegistry ,
                lang:danRegistry ,
                lang:deuRegistry ,
                lang:engRegistry ,
                lang:finRegistry ,
                lang:fraRegistry ,
                lang:korRegistry ,
                # lang:nldRegistry ,
                # lang:jpnRegistry ,
                lang:rusRegistry ,
                # lang:polRegistry ,
                lang:msaRegistry ,
                lang:spaRegistry ,
                lang:sweRegistry ,
                lang:zhoRegistry ;
        lang:deu-note notes:DefnTransUnavail ;
        lang:fra-note notes:NoteTransDiff .


###  https://isotc211.geolexica.org/ld/concepts#coverage_geometry
:coverage_geometry rdf:type owl:NamedIndividual ,
                   skos:Concept ;
          skos:inScheme geolexica:GeolexicaConceptScheme ;
          geolexica:hasInfo info:Info100 ;
        #   geolexica:hasReview reviews:Review100 ;
          geolexica:hasLDAPI ldapi:ldapi100-json ,
                             ldapi:ldapi100-jsonld ,
                             ldapi:ldapi100-rdfxml ,
                             ldapi:ldapi100-skosrdf ;
        geolexica:hasLangCode lang:ara ,
                        lang:dan ,
                        lang:deu ,
                        lang:eng ,
                        lang:fin ,
                        lang:fra ,
                        lang:kor ,
                        # lang:nld ,
                        # lang:pol ,
                        # lang:jpn ,
                        lang:msa ,
                        lang:rus ,
                        lang:spa ,
                        lang:swe ,
                        lang:zho ;
          dcterms:identifier 100 ;
          skos:notation 100 ;
          rdfs:label "coverage geometry" ;

  skos:definition "configuration of the domain of a coverage described in terms of coordinates"@en ;
  skos:definition "تكوين نطاق التغطية الموصوف من خلال الإحداثيات"@ar ;
  skos:definition "konfiguration af domænet for en coverage beskrevet i form af koordinater"@da ;
  skos:definition "koordinaattien avulla ilmaistu paikkatietojatkumon kokoonpano"@fi ;
  skos:definition "configuration du domaine d&#39;une couverture décrite en termes de coordonnées"@fr ;
  skos:definition "좌표로 기술된 커버리지의 시공간적 영역에 대한 구성"@ko ;
  skos:definition "konfiguracja dziedziny pokrycia opisana współrzędnymi"@pl ;
  skos:definition "конфигурация области определения покрытия, описываемая в терминах координат"@ru ;
  skos:definition "configuración del dominio de una cobertura en términos de coordenadas"@es ;
  skos:definition "koordinatbaserad beskrivning av den domän som definieras av ett domänobjekt"@sv ;
  skos:definition "按照坐标描述的数据覆盖的域结构。"@zh ;

  skos:prefLabel "coverage geometry"@en ;
  skos:prefLabel "هندسة التغطية"@ar ;
  skos:prefLabel "coverage-geometri"@da ;
  skos:prefLabel "Coveragegeometrie"@de ;
  skos:prefLabel "paikkatietojatkumon geometria"@fi ;
  skos:prefLabel "géométrie de couverture"@fr ;
  skos:prefLabel "커버리지 기하"@ko ;
  skos:prefLabel "geometria pokrycia"@pl ;
  skos:prefLabel "геометрия покрытия"@ru ;
  skos:prefLabel "geometría de la cobertura"@es ;
  skos:prefLabel "domängeometri"@sv ;
  skos:prefLabel "覆盖几何"@zh ;
  
  geolexica:origin lang:araRegistry ,
                lang:danRegistry ,
                lang:deuRegistry ,
                lang:engRegistry ,
                lang:finRegistry ,
                lang:fraRegistry ,
                lang:korRegistry ,
                # lang:nldRegistry ,
                # lang:jpnRegistry ,
                lang:rusRegistry ,
                # lang:polRegistry ,
                lang:msaRegistry ,
                lang:spaRegistry ,
                lang:sweRegistry ,
                lang:zhoRegistry ;
        lang:deu-note notes:DefnTransUnavail ;
        lang:fra-note notes:NoteTransDiff .


###  https://isotc211.geolexica.org/ld/concepts#curve
:curve rdf:type owl:NamedIndividual ,
                   skos:Concept ;
          skos:inScheme geolexica:GeolexicaConceptScheme ;
          geolexica:hasInfo info:Info101 ;
          geolexica:hasReview reviews:Review101 ;
          geolexica:hasLDAPI ldapi:ldapi101-json ,
                             ldapi:ldapi101-jsonld ,
                             ldapi:ldapi101-rdfxml ,
                             ldapi:ldapi101-skosrdf ;
        geolexica:hasLangCode lang:ara ,
                        lang:dan ,
                        lang:deu ,
                        lang:eng ,
                        lang:fin ,
                        lang:fra ,
                        lang:kor ,
                        # lang:nld ,
                        lang:pol ,
                        lang:jpn ,
                        lang:msa ,
                        lang:rus ,
                        lang:spa ,
                        lang:swe ,
                        lang:zho ;
          dcterms:identifier 101 ;
          skos:notation 101 ;
          rdfs:label "curve" ;

  skos:definition "1-dimensional geometric primitive, representing the continuous image of a line"@en ;
  skos:definition "عنصر هندسي بسيط ذو بعد واحد يمثل الصورة المتصلة  للخط"@ar ;
  skos:definition "1-dimensional geometrisk grundform, der repræsenterer et kontinuert billede af en linje"@da ;
  skos:definition "eindimensionales geometrisches Primitiv, das das kontinuierliche Abbild einer Linie darstellt"@de ;
  skos:definition "yksiulotteinen geometrinen primitiivi, joka muodostuu joukosta peräkkäisiä toisiinsa yhdistettyjä pisteitä"@fi ;
  skos:definition "primitive géométrique à une dimension représentant l&#39;image continue d&#39;une ligne"@fr ;
  skos:definition "直線の連続な像を表現する一次元の幾何プリミティブ。"@ja ;
  skos:definition "선의 연속적 이미지를 표현하는 1차원 기하 원시 객체"@ko ;
  skos:definition "sesuatu yg bentuknya melengkung"@ms ;
  skos:definition "1-wymiarowy prosty element geometryczny reprezentujący ciągły obraz linii"@pl ;
  skos:definition "одномерный геометрический примитив, представляющий непрерывный образ линии"@ru ;
  skos:definition "primitiva geométrica unidimensional que representa la imagen continua de una línea"@es ;
  skos:definition "endimensionellt geometriskt grundelement"@sv ;
  skos:definition "一维几何单形，表达一条线的连续映像。"@zh ;

  skos:prefLabel "curve"@en ;
  skos:prefLabel "منحنى"@ar ;
  skos:prefLabel "kurve"@da ;
  skos:prefLabel "Kurve"@de ;
  skos:prefLabel "käyrä"@fi ;
  skos:prefLabel "courbe"@fr ;
  skos:prefLabel "曲線"@ja ;
  skos:prefLabel "곡선"@ko ;
  skos:prefLabel "lengkungan"@ms ;
  skos:prefLabel "krzywa"@pl ;
  skos:prefLabel "кривая"@ru ;
  skos:prefLabel "curva"@es ;
  skos:prefLabel "linje"@sv ;
  skos:prefLabel "曲线"@zh ;
  
  geolexica:origin lang:araRegistry ,
                lang:danRegistry ,
                lang:deuRegistry ,
                lang:engRegistry ,
                lang:finRegistry ,
                lang:fraRegistry ,
                lang:korRegistry ,
                # lang:nldRegistry ,
                lang:jpnRegistry ,
                lang:rusRegistry ,
                lang:polRegistry ,
                lang:msaRegistry ,
                lang:spaRegistry ,
                lang:sweRegistry ,
                lang:zhoRegistry ;
        lang:deu-note notes:NoteTransUnavail ;
        lang:msa-note notes:NoteTransUnavail .


###  https://isotc211.geolexica.org/ld/concepts#curve_segment
:curve_segment rdf:type owl:NamedIndividual ,
                   skos:Concept ;
          skos:inScheme geolexica:GeolexicaConceptScheme ;
          geolexica:hasInfo info:Info102 ;
          geolexica:hasReview reviews:Review102 ;
          geolexica:hasLDAPI ldapi:ldapi102-json ,
                             ldapi:ldapi102-jsonld ,
                             ldapi:ldapi102-rdfxml ,
                             ldapi:ldapi102-skosrdf ;
        geolexica:hasLangCode lang:ara ,
                        lang:dan ,
                        lang:deu ,
                        lang:eng ,
                        lang:fin ,
                        lang:fra ,
                        lang:kor ,
                        # lang:nld ,
                        lang:pol ,
                        lang:jpn ,
                        # lang:msa ,
                        lang:rus ,
                        lang:spa ,
                        lang:swe ,
                        lang:zho ;
          dcterms:identifier 102 ;
          skos:notation 102 ;
          rdfs:label "curve segment" ;

  skos:definition "1-dimensional geometric object used to represent a continuous component of a curve using homogeneous interpolation and definition methods"@en ;
  skos:definition "كيان هندسي ذو بعد واحد يستخدم ليمثل مكونا متصلا لمنحنى باستخدام طرق استكمال وتعريف متجانسة"@ar ;
  skos:definition "1-dimensionalt geometrisk objekt, der anvendes til at repræsentere en kontinuert komponent af en kurve ved hjælp af homogene interpolations- og definitionsmetoder"@da ;
  skos:definition "käyrän osa, jolla on yhtenäinen interpolointi"@fi ;
  skos:definition "objet géométrique à une dimension utilisé pour représenter un composant continu d&#39;une courbe utilisant des méthodes de définition et une interpolation homogènes"@fr ;
  skos:definition "一定の内挿及び定義の方法を用いて曲線の連続した部分を表現するために用いる一次元の幾何オブジェクト。"@ja ;
  skos:definition "동일한 보간법 및 정의 방법으로 곡선의 연속적인 컴포넌트의 표현에 사용되는 1차원 기하객체"@ko ;
  skos:definition "1-wymiarowy obiekt geometryczny stosowany do przedstawienia ciągłego składnika krzywej, za pomocą homogenicznych metod interpolacji i definiowania"@pl ;
  skos:definition "одномерный геометрический объект, используемый для представления непрерывного отрезка кривой с применением методов однородной интерполяции и определения"@ru ;
  skos:definition "objeto geométrico unidimensional que se utiliza para representar una componente continua de una curva que usa métodos de interpolación y definición homogéneos"@es ;
  skos:definition "linje som ingår i en samling av linjer som tillsammans, och vanligen genom homogen interpolation, representerar en linje"@sv ;
  skos:definition "一维几何对象，用来表达一条曲线的连续组分，这条曲线具有相似的插值和定义方法。"@zh ;

  skos:prefLabel "curve segment"@en ;
  skos:prefLabel "مقطع منحنى"@ar ;
  skos:prefLabel "kurvesegment"@da ;
  skos:prefLabel "Kurvenabschnitt"@de ;
  skos:prefLabel "käyräsegmentti"@fi ;
  skos:prefLabel "segment de courbe"@fr ;
  skos:prefLabel "曲線分"@ja ;
  skos:prefLabel "곡선 분절"@ko ;
  skos:prefLabel "segment krzywej"@pl ;
  skos:prefLabel "сегмент кривой"@ru ;
  skos:prefLabel "segmento de curva"@es ;
  skos:prefLabel "linjesegment"@sv ;
  skos:prefLabel "曲线段"@zh ;
  
  geolexica:origin lang:araRegistry ,
                lang:danRegistry ,
                lang:deuRegistry ,
                lang:engRegistry ,
                lang:finRegistry ,
                lang:fraRegistry ,
                lang:korRegistry ,
                # lang:nldRegistry ,
                lang:jpnRegistry ,
                lang:rusRegistry ,
                lang:polRegistry ,
                # lang:msaRegistry ,
                lang:spaRegistry ,
                lang:sweRegistry ,
                lang:zhoRegistry ;
        lang:deu-note notes:DefnTransUnavail , notes:NoteTransUnavail .


###  https://isotc211.geolexica.org/ld/concepts#cycle_geometry
:cycle_geometry rdf:type owl:NamedIndividual ,
                   skos:Concept ;
          skos:inScheme geolexica:GeolexicaConceptScheme ;
          geolexica:hasInfo info:Info103 ;
          geolexica:hasReview reviews:Review103 ;
          geolexica:hasLDAPI ldapi:ldapi103-json ,
                             ldapi:ldapi103-jsonld ,
                             ldapi:ldapi103-rdfxml ,
                             ldapi:ldapi103-skosrdf ;
        geolexica:hasLangCode lang:ara ,
                        lang:dan ,
                        lang:deu ,
                        lang:eng ,
                        lang:fin ,
                        lang:fra ,
                        lang:kor ,
                        # lang:nld ,
                        lang:pol ,
                        lang:jpn ,
                        # lang:msa ,
                        lang:rus ,
                        lang:spa ,
                        lang:swe ,
                        lang:zho ;
          dcterms:identifier 103 ;
          skos:notation 103 ;
          rdfs:label "cycle (geometry)" ;

  skos:definition "spatial object without a boundary"@en ;
  skos:definition "كيان مكاني بلا حدود"@ar ;
  skos:definition "om rumligt objekt uden en grænse"@da ;
  skos:definition "sijaintiobjekti, jolla ei ole rajausta"@fi ;
  skos:definition "objet spatial sans frontière"@fr ;
  skos:definition "境界をもたない空間オブジェクト。"@ja ;
  skos:definition "경계가 없는 공간 객체"@ko ;
  skos:definition "(geometria) obiekt przestrzenny bez granicy"@pl ;
  skos:definition "пространственный объект, не имеющий границы"@ru ;
  skos:definition "objeto espacial sin frontera"@es ;
  skos:definition "rumsligt objekt med ändlig utsträckning men utan avgränsning"@sv ;
  skos:definition "(几何学)没有边界的空间对象。"@zh ;

  skos:prefLabel "cycle(geometry)"@en ;
  skos:prefLabel "دورة (هندسة)"@ar ;
  skos:prefLabel "lukket(geometri)"@da ;
  skos:prefLabel "Ring (Geometrie)"@de ;
  skos:prefLabel "silmukka (geometria)"@fi ;
  skos:prefLabel "cycle (géométrie)"@fr ;
  skos:prefLabel "輪体"@ja ;
  skos:prefLabel "순환(기하)"@ko ;
  skos:prefLabel "cykl"@pl ;
  skos:prefLabel "цикл (геометрия)"@ru ;
  skos:prefLabel "ciclo (geometría)"@es ;
  skos:prefLabel "cykliskt objekt"@sv ;
  skos:prefLabel "圈"@zh ;
  
  geolexica:origin lang:araRegistry ,
                lang:danRegistry ,
                lang:deuRegistry ,
                lang:engRegistry ,
                lang:finRegistry ,
                lang:fraRegistry ,
                lang:korRegistry ,
                # lang:nldRegistry ,
                lang:jpnRegistry ,
                lang:rusRegistry ,
                lang:polRegistry ,
                # lang:msaRegistry ,
                lang:spaRegistry ,
                lang:sweRegistry ,
                lang:zhoRegistry ;
        lang:deu-note notes:DefnTransUnavail , notes:NoteTransUnavail .


###  https://isotc211.geolexica.org/ld/concepts#data
:data rdf:type owl:NamedIndividual ,
                   skos:Concept ;
          skos:inScheme geolexica:GeolexicaConceptScheme ;
          geolexica:hasInfo info:Info104 ;
          geolexica:hasReview reviews:Review104 ;
          geolexica:hasLDAPI ldapi:ldapi104-json ,
                             ldapi:ldapi104-jsonld ,
                             ldapi:ldapi104-rdfxml ,
                             ldapi:ldapi104-skosrdf ;
        geolexica:hasLangCode lang:ara ,
                        lang:dan ,
                        lang:deu ,
                        lang:eng ,
                        lang:fin ,
                        lang:fra ,
                        lang:kor ,
                        # lang:nld ,
                        # lang:pol ,
                        # lang:jpn ,
                        lang:msa ,
                        lang:rus ,
                        lang:spa ,
                        lang:swe ,
                        lang:zho ;
          dcterms:identifier 104 ;
          skos:notation 104 ;
          rdfs:label "data" ;

  skos:definition "reinterpretable representation of information in a formalised manner suitable for communication, interpretation, or processing"@en ;
  skos:definition "تمثيل للمعلومات قابل لإعادة التفسير بطريقة رسمية مناسبة لأغراض الاتصال والتفسير والمعالجة"@ar ;
  skos:definition "genfortolkelig repræsentation af informationer på en formaliseret måde, så de kan kommunikeres, fortolkes eller bearbejdes"@da ;
  skos:definition "formalisierte eineindeutige Darstellung von Information, geeignet für den Austausch, die Interpretation und die Verarbeitung"@de ;
  skos:definition "tiedon määrämuotoinen, uudelleen tulkittavissa oleva esitys, joka soveltuu viestintään, tulkintaan tai prosessointiin"@fi ;
  skos:definition "représentation réinterprétable d’une information de façon formelle et adaptée à la communication, à l’interprétation ou au traitement"@fr ;
  skos:definition "정보를 의사소통, 해석, 처리에 적합한 형식으로 재해석 가능하도록 표현한 것"@ko ;
  skos:definition "формализованное представление информации, допускающее  неоднозначное толкование и пригодное для коммуникации, интерпретации или обработки"@ru ;
  skos:definition "representación reinterpretable de la información de manera formal adecuada para la comunicación, la interpretación o el procesamiento"@es ;
  skos:definition "representation av fakta, begrepp eller instruktioner i form lämpad för överföring, tolkning eller bearbetning av människor eller maskiner"@sv ;
  skos:definition "为便于交流、解释或处理，对信息的可再解释的形式化表示。"@zh ;

  skos:prefLabel "data"@en ;
  skos:prefLabel "بيانات"@ar ;
  skos:prefLabel "data"@da ;
  skos:prefLabel "Daten"@de ;
  skos:prefLabel "data"@fi ;
  skos:prefLabel "donnée"@fr ;
  skos:prefLabel "데이터"@ko ;
  skos:prefLabel "data"@ms ;
  skos:prefLabel "данные"@ru ;
  skos:prefLabel "datos"@es ;
  skos:prefLabel "data"@sv ;
  skos:prefLabel "数据"@zh ;
  
  geolexica:origin lang:araRegistry ,
                lang:danRegistry ,
                lang:deuRegistry ,
                lang:engRegistry ,
                lang:finRegistry ,
                lang:fraRegistry ,
                lang:korRegistry ,
                # lang:nldRegistry ,
                # lang:jpnRegistry ,
                lang:rusRegistry ,
                # lang:polRegistry ,
                lang:msaRegistry ,
                lang:spaRegistry ,
                lang:sweRegistry ,
                lang:zhoRegistry ;
        lang:msa-note notes:DefnTransUnavail .


###  https://isotc211.geolexica.org/ld/concepts#data_element
:data_element rdf:type owl:NamedIndividual ,
                   skos:Concept ;
          skos:inScheme geolexica:GeolexicaConceptScheme ;
          geolexica:hasInfo info:Info105 ;
          geolexica:hasReview reviews:Review105 ;
          geolexica:hasLDAPI ldapi:ldapi105-json ,
                             ldapi:ldapi105-jsonld ,
                             ldapi:ldapi105-rdfxml ,
                             ldapi:ldapi105-skosrdf ;
        geolexica:hasLangCode lang:ara ,
                        lang:dan ,
                        lang:deu ,
                        lang:eng ,
                        lang:fin ,
                        lang:fra ,
                        lang:kor ,
                        # lang:nld ,
                        # lang:pol ,
                        # lang:jpn ,
                        # lang:msa ,
                        lang:rus ,
                        lang:spa ,
                        lang:swe ,
                        lang:zho ;
          dcterms:identifier 105 ;
          skos:notation 105 ;
          rdfs:label "data element" ;

  skos:definition "unit of data that, in a certain context, is considered indivisible"@en ;
  skos:definition "وحدة بيانات تعتبر ، في سياق معين ، غير قابلة للتجزئة"@ar ;
  skos:definition "dataenhed, som i en bestemt kontekst anses for at være udelelig"@da ;
  skos:definition "tietyssä yhteydessä jakamattomana pidettävä tietoyksikkö"@fi ;
  skos:definition "unité de donnée qui, dans un certain contexte, est considérée comme indivisible"@fr ;
  skos:definition "특정 상황에서 더 이상 나누어질 수 없는 데이터 단위"@ko ;
  skos:definition "порция данных, в контексте использования которой отсутствует способ выделения из нее порции, отличной от нее самой"@ru ;
  skos:definition "unidad de datos que, en un contexto dado, se considera indivisible"@es ;
  skos:definition "data som vid en given tillämpning behandlas som en helhet"@sv ;
  skos:definition "在特定的环境中，认为不能再分的数据单元。"@zh ;

  skos:prefLabel "data element"@en ;
  skos:prefLabel "عنصر بيانات"@ar ;
  skos:prefLabel "dataelement"@da ;
  skos:prefLabel "Datenelement"@de ;
  skos:prefLabel "tietoelementti"@fi ;
  skos:prefLabel "élément de donnée"@fr ;
  skos:prefLabel "데이터 요소"@ko ;
  skos:prefLabel "элемент данных"@ru ;
  skos:prefLabel "elemento de datos"@es ;
  skos:prefLabel "dataelement"@sv ;
  skos:prefLabel "数据元素"@zh ;
  
  geolexica:origin lang:araRegistry ,
                lang:danRegistry ,
                lang:deuRegistry ,
                lang:engRegistry ,
                lang:finRegistry ,
                lang:fraRegistry ,
                lang:korRegistry ,
                # lang:nldRegistry ,
                # lang:jpnRegistry ,
                lang:rusRegistry ,
                # lang:polRegistry ,
                # lang:msaRegistry ,
                lang:spaRegistry ,
                lang:sweRegistry ,
                lang:zhoRegistry ;
        lang:deu-note notes:DefnTransUnavail .


###  https://isotc211.geolexica.org/ld/concepts#data_interchange
:data_interchange rdf:type owl:NamedIndividual ,
                   skos:Concept ;
          skos:inScheme geolexica:GeolexicaConceptScheme ;
          geolexica:hasInfo info:Info107 ;
          geolexica:hasReview reviews:Review107 ;
          geolexica:hasLDAPI ldapi:ldapi107-json ,
                             ldapi:ldapi107-jsonld ,
                             ldapi:ldapi107-rdfxml ,
                             ldapi:ldapi107-skosrdf ;
        geolexica:hasLangCode lang:ara ,
                        lang:dan ,
                        lang:deu ,
                        lang:eng ,
                        lang:fin ,
                        lang:fra ,
                        lang:kor ,
                        # lang:nld ,
                        # lang:pol ,
                        # lang:jpn ,
                        # lang:msa ,
                        lang:rus ,
                        lang:spa ,
                        lang:swe ,
                        lang:zho ;
          dcterms:identifier 107 ;
          skos:notation 107 ;
          rdfs:label "data interchange" ;

  skos:definition "delivery, receipt and interpretation of data"@en ;
  skos:definition "إيصال البيانات واستلامها وتفسيرها"@ar ;
  skos:definition "levering, modtagelse og fortolkning af data"@da ;
  skos:definition "tiedon jakaminen, vastaanottaminen ja tulkinta"@fi ;
  skos:definition "livraison, réception et interprétation de données"@fr ;
  skos:definition "데이터의 송수신 및 해석을 위한 처리 과정"@ko ;
  skos:definition "передача, прием и интепретация данных"@ru ;
  skos:definition "entrega, recepción e interpretación de datos"@es ;
  skos:definition "leverans, mottagning och tolkning av data"@sv ;
  skos:definition "数据的传输、接收和解释。"@zh ;

  skos:prefLabel "data interchange"@en ;
  skos:prefLabel "تبادل البيانات"@ar ;
  skos:prefLabel "dataudveksling"@da ;
  skos:prefLabel "Datenaustausch"@de ;
  skos:prefLabel "tiedonvaihto"@fi ;
  skos:prefLabel "échange de données"@fr ;
  skos:prefLabel "데이터 교환"@ko ;
  skos:prefLabel "обмен данными"@ru ;
  skos:prefLabel "intercambio de datos"@es ;
  skos:prefLabel "datautbyte"@sv ;
  skos:prefLabel "数据交换"@zh ;
  
  geolexica:origin lang:araRegistry ,
                lang:danRegistry ,
                lang:deuRegistry ,
                lang:engRegistry ,
                lang:finRegistry ,
                lang:fraRegistry ,
                lang:korRegistry ,
                # lang:nldRegistry ,
                # lang:jpnRegistry ,
                lang:rusRegistry ,
                # lang:polRegistry ,
                # lang:msaRegistry ,
                lang:spaRegistry ,
                lang:sweRegistry ,
                lang:zhoRegistry ;
        lang:deu-note notes:DefnTransUnavail .


###  https://isotc211.geolexica.org/ld/concepts#data_level
:data_level rdf:type owl:NamedIndividual ,
                   skos:Concept ;
          skos:inScheme geolexica:GeolexicaConceptScheme ;
          geolexica:hasInfo info:Info108 ;
          geolexica:hasReview reviews:Review108 ;
          geolexica:hasLDAPI ldapi:ldapi108-json ,
                             ldapi:ldapi108-jsonld ,
                             ldapi:ldapi108-rdfxml ,
                             ldapi:ldapi108-skosrdf ;
        geolexica:hasLangCode lang:ara ,
                        lang:dan ,
                        lang:deu ,
                        lang:eng ,
                        lang:fin ,
                        lang:fra ,
                        lang:kor ,
                        # lang:nld ,
                        # lang:pol ,
                        # lang:jpn ,
                        # lang:msa ,
                        lang:rus ,
                        lang:spa ,
                        # lang:swe ,
                        lang:zho ;
          dcterms:identifier 108 ;
          skos:notation 108 ;
          rdfs:label "data level" ;

  skos:definition "level containing data describing specific instances"@en ;
  skos:definition "مستوى يحتوي على بيانات تصف حالات محددة"@ar ;
  skos:definition "niveau med data, der beskriver specifikke instanser"@da ;
  skos:definition "taso, joka koostuu tiettyjä ilmentymiä kuvaavasta tiedosta"@fi ;
  skos:definition "niveau contenant des données décrivant des instances spécifiques"@fr ;
  skos:definition "특정 인스턴스를 기술하고 있는 데이터가 포함된 레벨"@ko ;
  skos:definition "уровень, содержащий данные, описывающие конкретные экземпляры"@ru ;
  skos:definition "nivel que contiene datos que describen instancias específicas"@es ;
  skos:definition "含有描述特定实例数据的层。"@zh ;

  skos:prefLabel "data level"@en ;
  skos:prefLabel "مستوى البيانات"@ar ;
  skos:prefLabel "dataniveau"@da ;
  skos:prefLabel "Datenebene"@de ;
  skos:prefLabel "tietotaso"@fi ;
  skos:prefLabel "niveau des données"@fr ;
  skos:prefLabel "데이터 층위"@ko ;
  skos:altLabel "데이터 레벨"@ko ;
  skos:prefLabel "уровень данных"@ru ;
  skos:prefLabel "nivel de datos"@es ;
  skos:prefLabel "数据层"@zh ;
  
  geolexica:origin lang:araRegistry ,
                lang:danRegistry ,
                lang:deuRegistry ,
                lang:engRegistry ,
                lang:finRegistry ,
                lang:fraRegistry ,
                lang:korRegistry ,
                # lang:nldRegistry ,
                # lang:jpnRegistry ,
                lang:rusRegistry ,
                # lang:polRegistry ,
                # lang:msaRegistry ,
                lang:spaRegistry ,
                # lang:sweRegistry ,
                lang:zhoRegistry ;
        lang:deu-note notes:DefnTransUnavail .


###  https://isotc211.geolexica.org/ld/concepts#data_product
:data_product rdf:type owl:NamedIndividual ,
                   skos:Concept ;
          skos:inScheme geolexica:GeolexicaConceptScheme ;
          geolexica:hasInfo info:Info110 ;
        #   geolexica:hasReview reviews:Review110 ;
          geolexica:hasLDAPI ldapi:ldapi110-json ,
                             ldapi:ldapi110-jsonld ,
                             ldapi:ldapi110-rdfxml ,
                             ldapi:ldapi110-skosrdf ;
        geolexica:hasLangCode lang:ara ,
                        lang:dan ,
                        lang:deu ,
                        lang:eng ,
                        lang:fin ,
                        lang:fra ,
                        lang:kor ,
                        # lang:nld ,
                        # lang:pol ,
                        # lang:jpn ,
                        # lang:msa ,
                        lang:rus ,
                        lang:spa ,
                        lang:swe ,
                        lang:zho ;
          dcterms:identifier 110 ;
          skos:notation 110 ;
          rdfs:label "data product" ;

  skos:definition "dataset or dataset series that conforms to a data product specification"@en ;
  skos:definition "مجموعة بيانات أو سلسلة مجموعة بيانات مطابقة لمواصفات منتج بيانات معين"@ar ;
  skos:definition "yhden tai useamman tietoaineiston tai tietoaineistosarjan tiedoista koottu tuote, joka voidaan luovuttaa sellaisenaan tai sisällön perusteella rajattuna tiettyyn käyttötarkoitukseen"@fi ;
  skos:definition "jeu de données ou série de jeux de données conforme à une spécification de produit (de données)"@fr ;
  skos:definition "데이터 제품 사양을 따르는 데이터셋 또는 데이터셋 시리즈"@ko ;
  skos:definition "набор данных или ряд наборов данных, которые соответствуют спецификации информационного продукта"@ru ;
  skos:definition "conjunto de datos o serie de conjuntos de datos conforme a unas especificaciones de producto de datos"@es ;
  skos:definition "specificerad datamängd eller serie av datamängder som erbjuds eller efterfrågas"@sv ;
  skos:definition "与数据产品规范一致的数据集或数据集系列。"@zh ;

  skos:prefLabel "data product"@en ;
  skos:prefLabel "منتج بيانات"@ar ;
  skos:prefLabel "Datenprodukt"@de ;
  skos:prefLabel "tietotuote"@fi ;
  skos:prefLabel "produit (de données)"@fr ;
  skos:prefLabel "데이터 제품"@ko ;
  skos:prefLabel "информационный продукт"@ru ;
  skos:prefLabel "producto de datos"@es ;
  skos:prefLabel "dataprodukt"@sv ;
  skos:prefLabel "数据产品"@zh ;
  
  geolexica:origin lang:araRegistry ,
                lang:danRegistry ,
                lang:deuRegistry ,
                lang:engRegistry ,
                lang:finRegistry ,
                lang:fraRegistry ,
                lang:korRegistry ,
                # lang:nldRegistry ,
                # lang:jpnRegistry ,
                lang:rusRegistry ,
                # lang:polRegistry ,
                # lang:msaRegistry ,
                lang:spaRegistry ,
                lang:sweRegistry ,
                lang:zhoRegistry ;
        lang:deu-note notes:DefnTransUnavail ;
        lang:fra-note notes:NoteTransDiff .


###  https://isotc211.geolexica.org/ld/concepts#data_product_specification
:data_product_specification rdf:type owl:NamedIndividual ,
                   skos:Concept ;
          skos:inScheme geolexica:GeolexicaConceptScheme ;
          geolexica:hasInfo info:Info111 ;
        #   geolexica:hasReview reviews:Review111 ;
          geolexica:hasLDAPI ldapi:ldapi111-json ,
                             ldapi:ldapi111-jsonld ,
                             ldapi:ldapi111-rdfxml ,
                             ldapi:ldapi111-skosrdf ;
        geolexica:hasLangCode lang:ara ,
                        lang:dan ,
                        lang:deu ,
                        lang:eng ,
                        lang:fin ,
                        lang:fra ,
                        lang:kor ,
                        # lang:nld ,
                        # lang:pol ,
                        # lang:jpn ,
                        # lang:msa ,
                        lang:rus ,
                        lang:spa ,
                        lang:swe ,
                        lang:zho ;
          dcterms:identifier 111 ;
          skos:notation 111 ;
          rdfs:label "data product specification" ;

  skos:definition "detailed description of a dataset or dataset series together with additional information that will enable it to be created, supplied to and used by another party"@en ;
  skos:definition "وصف تفصيلي لمجموعة بيانات أو سلسلة مجموعة بيانات مع معلومات إضافية تمكن من إنشائها وتقديمها إلى طرف آخر لاستخدامها"@ar ;
  skos:definition "detaillierte Beschreibung eines Datensatzes oder einer Serie von Datensätzen verbunden mit ergänzenden Informationen, die deren Erstellung, Lieferung an und Nutzung durch Dritte ermöglicht"@de ;
  skos:definition "dokumentti, jossa tietotuote kuvataan yksityiskohtaisesti tuotannon, myynnin, käytön tai jonkin muun toiminnan tarpeisiin"@fi ;
  skos:definition "description détaillée d&#39;un jeu de données ou d&#39;une série de jeux de données comprenant également des informations supplémentaires permettant leur création, fourniture  et utilisation par une tierce partie"@fr ;
  skos:definition "데이터 제품에 대하여 제3자가 이를 생성, 공급, 사용하는 데 필요한 정보를 제공하는 데이터셋 또는 데이터셋 시리즈의 상세 설명"@ko ;
  skos:definition "детальное описание набора данных или ряда наборов данных, а также дополнительная информация, обеспечивающая  его (их) создание, поставку и использование другой стороной"@ru ;
  skos:definition "descripción detallada de un conjunto de datos o de una serie de conjuntos de datos junto con la información adicional que permite su creación, suministro y utilización por otras partes"@es ;
  skos:definition "dokumentation som definierar en dataprodukt och de krav som kan ställas på dataprodukten"@sv ;
  skos:definition "数据集或数据集系列的详细描述及补充说明，从而使其他方能够创建、提供和使用数据集或数据集系列。"@zh ;

  skos:prefLabel "data product specification"@en ;
  skos:prefLabel "مواصفات منتج بيانات"@ar ;
  skos:prefLabel "Datenproduktspezifikation"@de ;
  skos:prefLabel "tietotuotemäärittely"@fi ;
  skos:altLabel "tietotuoteseloste"@fi ;
  skos:prefLabel "spécification de produit (de données)"@fr ;
  skos:prefLabel "데이터 제품 사양"@ko ;
  skos:prefLabel "спецификация информационного продукта"@ru ;
  skos:prefLabel "especificaciones de producto de datos"@es ;
  skos:prefLabel "dataproduktspecifikation"@sv ;
  skos:prefLabel "数据产品规范"@zh ;
  
  geolexica:origin lang:araRegistry ,
                lang:danRegistry ,
                lang:deuRegistry ,
                lang:engRegistry ,
                lang:finRegistry ,
                lang:fraRegistry ,
                lang:korRegistry ,
                # lang:nldRegistry ,
                # lang:jpnRegistry ,
                lang:rusRegistry ,
                # lang:polRegistry ,
                # lang:msaRegistry ,
                lang:spaRegistry ,
                lang:sweRegistry ,
                lang:zhoRegistry ;
        lang:deu-note notes:DefnTransUnavail ;
        lang:fra-note notes:NoteTransDiff .


###  https://isotc211.geolexica.org/ld/concepts#data_quality_date
:data_quality_date rdf:type owl:NamedIndividual ,
                   skos:Concept ;
          skos:inScheme geolexica:GeolexicaConceptScheme ;
          geolexica:hasInfo info:Info112 ;
          geolexica:hasReview reviews:Review112 ;
          geolexica:hasLDAPI ldapi:ldapi112-json ,
                             ldapi:ldapi112-jsonld ,
                             ldapi:ldapi112-rdfxml ,
                             ldapi:ldapi112-skosrdf ;
        geolexica:hasLangCode lang:ara ,
                        lang:dan ,
                        lang:deu ,
                        lang:eng ,
                        lang:fin ,
                        lang:fra ,
                        lang:kor ,
                        # lang:nld ,
                        lang:pol ,
                        lang:jpn ,
                        # lang:msa ,
                        lang:rus ,
                        lang:spa ,
                        lang:swe ,
                        lang:zho ;
          dcterms:identifier 112 ;
          skos:notation 112 ;
          rdfs:label "data quality date" ;

  skos:definition "date or range of dates on which a data quality measure is applied"@en ;
  skos:definition "التاريخ أو النطاق الزمني الذي طبق فيه قياس جودة البيانات"@ar ;
  skos:definition "dato eller periode hvor et mål for datakvalitet foretages"@da ;
  skos:definition "päiväys tai aikaväli, jona laatumittaria sovelletaan"@fi ;
  skos:definition "date ou gamme de dates à laquelle la mesure de qualité de donnée est effectuée"@fr ;
  skos:definition "あるデータ品質評価尺度を適用した日付又は期間。"@ja ;
  skos:definition "데이터 품질 측정을 실시한 일자 또는 범위"@ko ;
  skos:definition "data lub zakres dat, do których odnosi się pomiar jakości danych"@pl ;
  skos:definition "дата или период, к которым относится мера качества данных"@ru ;
  skos:definition "fecha o rango de fechas en las que se realiza una medida de calidad de datos"@es ;
  skos:definition "衡量数据质量的日期或日期范围。"@zh ;

  skos:prefLabel "data quality date"@en ;
  skos:prefLabel "تاريخ جودة البيانات"@ar ;
  skos:prefLabel "datakvalitet, dato for"@da ;
  skos:prefLabel "Datum der Datenqualitätsangabe"@de ;
  skos:prefLabel "laatumittauksen päiväys"@fi ;
  skos:prefLabel "date de la qualité des données"@fr ;
  skos:prefLabel "データ品質評価日付"@ja ;
  skos:prefLabel "데이터 품질 일자"@ko ;
  skos:prefLabel "data oceny jakości danych"@pl ;
  skos:prefLabel "период действия меры качества данных"@ru ;
  skos:prefLabel "fecha de la calidad de datos"@es ;
  skos:prefLabel "数据质量日期"@zh ;
  
  geolexica:origin lang:araRegistry ,
                lang:danRegistry ,
                lang:deuRegistry ,
                lang:engRegistry ,
                lang:finRegistry ,
                lang:fraRegistry ,
                lang:korRegistry ,
                # lang:nldRegistry ,
                lang:jpnRegistry ,
                lang:rusRegistry ,
                lang:polRegistry ,
                # lang:msaRegistry ,
                lang:spaRegistry ,
                lang:sweRegistry ,
                lang:zhoRegistry ;
        lang:deu-note notes:DefnTransUnavail .


###  https://isotc211.geolexica.org/ld/concepts#data_quality_element
:data_quality_element rdf:type owl:NamedIndividual ,
                   skos:Concept ;
          skos:inScheme geolexica:GeolexicaConceptScheme ;
          geolexica:hasInfo info:Info113 ;
          geolexica:hasReview reviews:Review113 ;
          geolexica:hasLDAPI ldapi:ldapi113-json ,
                             ldapi:ldapi113-jsonld ,
                             ldapi:ldapi113-rdfxml ,
                             ldapi:ldapi113-skosrdf ;
        geolexica:hasLangCode lang:ara ,
                        lang:dan ,
                        lang:deu ,
                        lang:eng ,
                        lang:fin ,
                        lang:fra ,
                        lang:kor ,
                        # lang:nld ,
                        # lang:pol ,
                        # lang:jpn ,
                        # lang:msa ,
                        lang:rus ,
                        lang:spa ,
                        lang:swe ,
                        lang:zho ;
          dcterms:identifier 113 ;
          skos:notation 113 ;
          rdfs:label "data quality element" ;

  skos:definition "quantitative component documenting the quality of a dataset"@en ;
  skos:definition "المكون الكمي لتوثيق الجودة لمجموعة بيانات"@ar ;
  skos:definition "kvantitativ komponent, der dokumenterer kvaliteten af et datasæt"@da ;
  skos:definition "tekijä, joka kuvaa laadun tiettyä näkökulmaa"@fi ;
  skos:definition "composant quantitatif documentant la qualité d&#39;un jeu de données"@fr ;
  skos:definition "품질정보를 기술하는 데이터셋의 정량적 컴포넌트"@ko ;
  skos:definition "количественный компонент, определяющий качество набора данных"@ru ;
  skos:definition "componente cuantitativo que documenta la calidad de un conjunto de datos"@es ;
  skos:definition "kvantitativ, inneboende egenskap hos en datamängd på vilken krav på datakvalitet kan ställas"@sv ;
  skos:definition "定量描述数据集质量的组成部分。"@zh ;

  skos:prefLabel "data quality element"@en ;
  skos:prefLabel "عنصر جودة البيانات"@ar ;
  skos:prefLabel "datakvalitetselement"@da ;
  skos:prefLabel "Datenqualitätselement"@de ;
  skos:prefLabel "laatutekijä"@fi ;
  skos:prefLabel "élément de qualité des données"@fr ;
  skos:prefLabel "데이터 품질 요소"@ko ;
  skos:prefLabel "элемент качества данных"@ru ;
  skos:prefLabel "elemento de la calidad de datos"@es ;
  skos:prefLabel "datakvalitetsegenskap"@sv ;
  skos:prefLabel "数据质量元素"@zh ;
  
  geolexica:origin lang:araRegistry ,
                lang:danRegistry ,
                lang:deuRegistry ,
                lang:engRegistry ,
                lang:finRegistry ,
                lang:fraRegistry ,
                lang:korRegistry ,
                # lang:nldRegistry ,
                # lang:jpnRegistry ,
                lang:rusRegistry ,
                # lang:polRegistry ,
                # lang:msaRegistry ,
                lang:spaRegistry ,
                lang:sweRegistry ,
                lang:zhoRegistry ;
        lang:deu-note notes:DefnTransUnavail, notes:NoteTransUnavail ;
        lang:swe-note notes:NoteTransUnavail .


###  https://isotc211.geolexica.org/ld/concepts#data_quality_eval_procedure
:data_quality_eval_procedure rdf:type owl:NamedIndividual ,
                   skos:Concept ;
          skos:inScheme geolexica:GeolexicaConceptScheme ;
          geolexica:hasInfo info:Info114 ;
          geolexica:hasReview reviews:Review114 ;
          geolexica:hasLDAPI ldapi:ldapi114-json ,
                             ldapi:ldapi114-jsonld ,
                             ldapi:ldapi114-rdfxml ,
                             ldapi:ldapi114-skosrdf ;
        geolexica:hasLangCode lang:ara ,
                        lang:dan ,
                        lang:deu ,
                        lang:eng ,
                        lang:fin ,
                        lang:fra ,
                        lang:kor ,
                        # lang:nld ,
                        lang:pol ,
                        lang:jpn ,
                        # lang:msa ,
                        lang:rus ,
                        lang:spa ,
                        lang:swe ,
                        lang:zho ;
          dcterms:identifier 114 ;
          skos:notation 114 ;
          rdfs:label "data quality evaluation procedure" ;

  skos:definition "operation(s) used in applying and reporting quality evaluation methods and their results"@en ;
  skos:definition "عملية (أو عمليات) تستخدم في تطبيق طرق تقييم الجودة ونتائجها والإبلاغ عن ذلك"@ar ;
  skos:definition "operation(er), som indgår i anvendelsen af metoder til kvalitetsvurdering, og benyttes til at rapportere resultaterne heraf"@da ;
  skos:definition "tiedon laadun arviointi"@fi ;
  skos:definition "opération(s) effectuée(s) pour l&#39;application et la description des méthodes d&#39;évaluation de la qualité et de leurs résultats"@fr ;
  skos:definition "品質評価手法を適用し，その結果を報告するときの作業工程。"@ja ;
  skos:definition "품질 산출 방법을 적용하여 그 결과를 보고하는 절차"@ko ;
  skos:definition "działania wykonywane w celu stosowania metod oceny jakości oraz przedstawiania ich wyników"@pl ;
  skos:definition "операция (- и), используемая (-ые) при применении методов оценки и составлении соответствующих отчетов"@ru ;
  skos:definition "operación(es) utilizada(s) en la aplicación y difusión de los métodos de evaluación de la calidad y de sus resultados"@es ;
  skos:definition "应用和报告质量评价方法及评价结果的操作。"@zh ;

  skos:prefLabel "data quality evaluation procedure"@en ;
  skos:prefLabel "إجراءات تقييم جودة البيانات"@ar ;
  skos:prefLabel "datakvalitet, procedure til vurdering af"@da ;
  skos:prefLabel "Verfahren zur Datenqualitätsbestimmung"@de ;
  skos:prefLabel "tiedon laadun arviointi"@fi ;
  skos:prefLabel "procédure d&#39;évaluation de la qualité des données"@fr ;
  skos:prefLabel "データ品質評価手順"@ja ;
  skos:prefLabel "데이터 품질 평가 절차"@ko ;
  skos:prefLabel "procedura określania jakości danych"@pl ;
  skos:prefLabel "процедура оценки качества данных"@ru ;
  skos:prefLabel "procedimiento de evaluación de la calidad de datos"@es ;
  skos:prefLabel "数据质量评价过程"@zh ;
  
  geolexica:origin lang:araRegistry ,
                lang:danRegistry ,
                lang:deuRegistry ,
                lang:engRegistry ,
                lang:finRegistry ,
                lang:fraRegistry ,
                lang:korRegistry ,
                # lang:nldRegistry ,
                lang:jpnRegistry ,
                lang:rusRegistry ,
                lang:polRegistry ,
                # lang:msaRegistry ,
                lang:spaRegistry ,
                lang:sweRegistry ,
                lang:zhoRegistry ;
        lang:deu-note notes:DefnTransUnavail .


###  https://isotc211.geolexica.org/ld/concepts#data_quality_measure
:data_quality_measure rdf:type owl:NamedIndividual ,
                   skos:Concept ;
          skos:inScheme geolexica:GeolexicaConceptScheme ;
          geolexica:hasInfo info:Info115 ;
          geolexica:hasReview reviews:Review115 ;
          geolexica:hasLDAPI ldapi:ldapi115-json ,
                             ldapi:ldapi115-jsonld ,
                             ldapi:ldapi115-rdfxml ,
                             ldapi:ldapi115-skosrdf ;
        geolexica:hasLangCode lang:ara ,
                        lang:dan ,
                        lang:deu ,
                        lang:eng ,
                        lang:fin ,
                        lang:fra ,
                        lang:kor ,
                        # lang:nld ,
                        lang:pol ,
                        lang:jpn ,
                        # lang:msa ,
                        lang:rus ,
                        lang:spa ,
                        lang:swe ,
                        lang:zho ;
          dcterms:identifier 115 ;
          skos:notation 115 ;
          rdfs:label "data quality measure" ;

 skos:definition "evaluation of a data quality subelement"@en ;
  skos:definition "تقييم عنصر فرعي لجودة البيانات"@ar ;
  skos:definition "evaluering af et datakvalitetsdelelement"@da ;
  skos:definition "laatutekijän mittari"@fi ;
  skos:definition "évaluation d&#39;un sous-élément de qualité des données"@fr ;
  skos:definition "データ品質副要素の評価尺度。"@ja ;
  skos:definition "데이터 품질 하위 요소의 산출"@ko ;
  skos:definition "ocena elementu podrzędnego jakości danych"@pl ;
  skos:definition "измеряемое значение подэлемента качества данных"@ru ;
  skos:definition "evaluación de un subelemento de calidad de datos"@es ;
  skos:definition "kvantitativ bestämning som ligger till grund för utvärderingen av en datakvalitetsegenskap"@sv ;
  skos:definition "数据质量子元素的取值。"@zh ;

  skos:prefLabel "data quality measure"@en ;
  skos:prefLabel "قياس جودة البيانات"@ar ;
  skos:prefLabel "datakvalitet, mål for"@da ;
  skos:prefLabel "Datenqualitätsmaß"@de ;
  skos:prefLabel "laatumittari"@fi ;
  skos:prefLabel "mesure de qualité des données"@fr ;
  skos:prefLabel "データ品質評価尺度"@ja ;
  skos:prefLabel "데이터 품질 측정"@ko ;
  skos:prefLabel "miara jakości danych"@pl ;
  skos:prefLabel "мера качества данных"@ru ;
  skos:prefLabel "medida de la calidad de datos"@es ;
  skos:prefLabel "datakvalitetsmått"@sv ;
  skos:prefLabel "数据质量度量"@zh ;
  
  geolexica:origin lang:araRegistry ,
                lang:danRegistry ,
                lang:deuRegistry ,
                lang:engRegistry ,
                lang:finRegistry ,
                lang:fraRegistry ,
                lang:korRegistry ,
                # lang:nldRegistry ,
                lang:jpnRegistry ,
                lang:rusRegistry ,
                lang:polRegistry ,
                # lang:msaRegistry ,
                lang:spaRegistry ,
                lang:sweRegistry ,
                lang:zhoRegistry ;
        lang:deu-note notes:DefnTransUnavail , notes:ExTransUnavail ; 
        lang:swe-note notes:ExTransUnavail .


###  https://isotc211.geolexica.org/ld/concepts#data_quality_over_element
:data_quality_over_element rdf:type owl:NamedIndividual ,
                   skos:Concept ;
          skos:inScheme geolexica:GeolexicaConceptScheme ;
          geolexica:hasInfo info:Info116 ;
          geolexica:hasReview reviews:Review116 ;
          geolexica:hasLDAPI ldapi:ldapi116-json ,
                             ldapi:ldapi116-jsonld ,
                             ldapi:ldapi116-rdfxml ,
                             ldapi:ldapi116-skosrdf ;
        geolexica:hasLangCode lang:ara ,
                        lang:dan ,
                        lang:deu ,
                        lang:eng ,
                        lang:fin ,
                        lang:fra ,
                        lang:kor ,
                        # lang:nld ,
                        # lang:pol ,
                        # lang:jpn ,
                        # lang:msa ,
                        lang:rus ,
                        lang:spa ,
                        lang:swe ,
                        lang:zho ;
          dcterms:identifier 116 ;
          skos:notation 116 ;
          rdfs:label "data quality overview element" ;

  skos:definition "non-quantitative component documenting the quality of a dataset"@en ;
  skos:definition "مكون غير كمي يوثق لجودة مجموعة بيانات معيَّنة"@ar ;
  skos:definition "ikke-kvantitativ komponent, der dokumenterer kvaliteten af et datasæt"@da ;
  skos:definition "tietotuotteen laatukuvauksen kuvailevaa laatutietoa ilmentävä laatutekijä"@fi ;
  skos:definition "composant non-quantitatif documentant la qualité d&#39;un jeu de données"@fr ;
  skos:definition "데이터셋의 품질을 기술하는 비정량적 컴포넌트"@ko ;
  skos:definition "неколичественный компонент, определяющий качество набора данных"@ru ;
  skos:definition "componente no cuantitativo que documenta la calidad de un conjunto de datos"@es ;
  skos:definition "cke-kvantitativ, inneboende egenskap hos en datamängd på vilken krav på datakvalitet kan ställas"@sv ;
  skos:definition "说明数据集质量的非量化组成部分。"@zh ;

  skos:prefLabel "data quality overview element"@en ;
  skos:prefLabel "عنصر الاستعراض العام لجودة البيانات"@ar ;
  skos:prefLabel "datakvalitet, element til at få overblik over"@da ;
  skos:prefLabel "Überblickselement für die Datenqualität"@de ;
  skos:prefLabel "kuvaileva laatutekijä"@fi ;
  skos:prefLabel "élément d&#39;aperçu de la qualité des données"@fr ;
  skos:prefLabel "데이터 품질 개관 요소"@ko ;
  skos:prefLabel "описательный элемент качества данных"@ru ;
  skos:prefLabel "elemento general de la calidad de datos"@es ;
  skos:prefLabel "datakvalitetsbeskrivning"@sv ;
  skos:prefLabel "数据质量概述元素"@zh ;
  
  geolexica:origin lang:araRegistry ,
                lang:danRegistry ,
                lang:deuRegistry ,
                lang:engRegistry ,
                lang:finRegistry ,
                lang:fraRegistry ,
                lang:korRegistry ,
                # lang:nldRegistry ,
                # lang:jpnRegistry ,
                lang:rusRegistry ,
                # lang:polRegistry ,
                # lang:msaRegistry ,
                lang:spaRegistry ,
                lang:sweRegistry ,
                lang:zhoRegistry ;
        lang:deu-note notes:DefnTransUnavail , notes:NoteTransUnavail ; 
        lang:swe-note notes:NoteTransUnavail .


###  https://isotc211.geolexica.org/ld/concepts#data_quality_result
:data_quality_result rdf:type owl:NamedIndividual ,
                   skos:Concept ;
          skos:inScheme geolexica:GeolexicaConceptScheme ;
          geolexica:hasInfo info:Info117 ;
          geolexica:hasReview reviews:Review117 ;
          geolexica:hasLDAPI ldapi:ldapi117-json ,
                             ldapi:ldapi117-jsonld ,
                             ldapi:ldapi117-rdfxml ,
                             ldapi:ldapi117-skosrdf ;
        geolexica:hasLangCode lang:ara ,
                        lang:dan ,
                        lang:deu ,
                        lang:eng ,
                        lang:fin ,
                        lang:fra ,
                        lang:kor ,
                        # lang:nld ,
                        # lang:pol ,
                        # lang:jpn ,
                        # lang:msa ,
                        lang:rus ,
                        lang:spa ,
                        lang:swe ,
                        lang:zho ;
          dcterms:identifier 117 ;
          skos:notation 117 ;
          rdfs:label "data quality result" ;

  skos:definition "value or set of values resulting from applying a data quality measure or the outcome of evaluating the obtained value or set of values against a specified conformance quality level"@en ;
  skos:definition "قيمة أو مجموعة قيم ناتجة عن تطبيق قياس معيَّن لجودة البيانات أو ناتج تقييم القيمة أو القيم المتحصلة مقابل مستوى محدد من الجودة المطابقة"@ar ;
  skos:definition "1) værdi eller sæt af værdier opnået ved at anvende et mål for datakvalitet. 2) resultatet af at evaluere de(n) opnåede værdi(er) i forhold til et specificeret kvalitetsniveau af overensstemmelse."@da ;
  skos:definition "arvo tai arvojoukko, joka saadaan soveltamalla laatumittaria tai vertaamalla mitattuja tuloksia ennalta määrättyyn laatuvaatimustasoon, tai tekstimuotoinen, subjektiiviseen arvioon perustuva kuvaus laadusta"@fi ;
  skos:definition "valeur ou ensemble de valeurs résultant de l&#39;application d&#39;une mesure de qualité de donnée ou le résultat de la comparaison de la valeur obtenue (ou ensemble de valeurs) par rapport au niveau de conformité spécifié"@fr ;
  skos:definition "データ品質評価尺度を適用した結果の値若しくは値の集合，又は規定された適合品質水準を満たすか否かを，取得した値又は値の集合を用いて評価した結果。"@ja ;
  skos:definition "데이터 품질 측정의 결과 값이나 값의 집합 또는 이를 정해진 적합성 품질 수준에 따라 평가한 결과"@ko ;
  skos:definition "wartość lub zbiór wartości wynikających z zastosowania miary jakości danych lub rezultat oceny otrzymanej wartości lub zbioru wartości względem określonego wymaganego poziomu jakości"@pl ;
  skos:definition "значение или набор значений, получаемые в результате применения меры качества данных, или результат сопоставления полученного значения (набора значений) с заданным уровнем соответствия качеству"@ru ;
  skos:definition "valor, o conjunto de valores, que resultan de la aplicación de una medida de calidad, o bien proceden de la evaluación del valor, o conjunto de valores obtenidos, frente a un nivel de calidad de conformidad especificado"@es ;
  skos:definition "värden som erhålls vid tillämpning av ett datakvalitetsmått eller vid utvärdering av sådana värden mot en specificerad överensstämmelsenivå för datakvalitet"@sv ;
  skos:definition "数据质量度量得到的一个值或一组值，或者将获取一个值或一组值同规定的一致性质量级别相比较得到的评价结果。"@zh ;

  skos:prefLabel "data quality result"@en ;
  skos:prefLabel "نتيجة جودة البيانات"@ar ;
  skos:prefLabel "datakvalitetsresultat"@da ;
  skos:prefLabel "Datenqualitätsangabe"@de ;
  skos:prefLabel "laatutulos"@fi ;
  skos:prefLabel "résultat de qualité des données"@fr ;
  skos:prefLabel "データ品質評価結果"@ja ;
  skos:prefLabel "데이터 품질 결과"@ko ;
  skos:prefLabel "wynik oceny jakości danych"@pl ;
  skos:prefLabel "результат оценки качества данных"@ru ;
  skos:prefLabel "resultado de la calidad de datos"@es ;
  skos:prefLabel "datakvalitetsreultat"@sv ;
  skos:prefLabel "数据质量结果"@zh ;
  
  geolexica:origin lang:araRegistry ,
                lang:danRegistry ,
                lang:deuRegistry ,
                lang:engRegistry ,
                lang:finRegistry ,
                lang:fraRegistry ,
                lang:korRegistry ,
                # lang:nldRegistry ,
                # lang:jpnRegistry ,
                lang:rusRegistry ,
                # lang:polRegistry ,
                # lang:msaRegistry ,
                lang:spaRegistry ,
                lang:sweRegistry ,
                lang:zhoRegistry ;
        lang:deu-note notes:DefnTransUnavail , notes:ExTransUnavail ; 
        lang:swe-note notes:ExTransUnavail .


###  https://isotc211.geolexica.org/ld/concepts#data_quality_scope
:data_quality_scope rdf:type owl:NamedIndividual ,
                   skos:Concept ;
          skos:inScheme geolexica:GeolexicaConceptScheme ;
          geolexica:hasInfo info:Info118 ;
          geolexica:hasReview reviews:Review118 ;
          geolexica:hasLDAPI ldapi:ldapi118-json ,
                             ldapi:ldapi118-jsonld ,
                             ldapi:ldapi118-rdfxml ,
                             ldapi:ldapi118-skosrdf ;
        geolexica:hasLangCode lang:ara ,
                        lang:dan ,
                        lang:deu ,
                        lang:eng ,
                        lang:fin ,
                        lang:fra ,
                        lang:kor ,
                        # lang:nld ,
                        lang:pol ,
                        lang:jpn ,
                        # lang:msa ,
                        lang:rus ,
                        lang:spa ,
                        lang:swe ,
                        lang:zho ;
          dcterms:identifier 118 ;
          skos:notation 118 ;
          rdfs:label "data quality scope" ;

  skos:definition "extent or characteristic(s) of the data for which quality information is reported"@en ;
  skos:definition "حدود أو خاصية (أو خصائص) البيانات التي يتم تقديم بيانات الجودة عنها"@ar ;
  skos:definition "omfang af eller egenskaber ved de data, for hvilke der rapporteres kvalitetsinformation"@da ;
  skos:definition "tiedot, joihin tiedon laadun arviointi kohdistuu ja jotka on valittu sijainnillisen tai ajallisen kattavuuden ja/tai yhteisten ominaisuuksien perusteella"@fi ;
  skos:definition "étendue ou caractéristique(s) des données pour lesquelles les informations de qualité sont rapportées"@fr ;
  skos:definition "品質情報を報告するデータの範囲又は特性。"@ja ;
  skos:definition "품질 정보가 기록된 데이터의 범위 혹은 특성"@ko ;
  skos:definition "zasięg lub cechy danych, dla których przedstawiana jest informacja o jakości"@pl ;
  skos:definition "область или характеристика (-и) данных, в отношении которых выдается информация о качестве"@ru ;
  skos:definition "alcance o características de los datos para los que se informa sobre la calidad"@es ;
  skos:definition "specifik del hos en datamängd eller en dataprodukt som har identifierats för att ett eller flera datakvalitetsmått antas vara konstanta inom delen"@sv ;
  skos:definition "被报告质量信息的数据的范围或特征。"@zh ;

  skos:prefLabel "data quality scope"@en ;
  skos:prefLabel "نطاق جودة البيانات"@ar ;
  skos:prefLabel "datakvalitet, omfang af"@da ;
  skos:prefLabel "Geltungsbereich der Datenqualitätsangabe"@de ;
  skos:prefLabel "laatukuvauksen laajuus"@fi ;
  skos:prefLabel "domaine d&#39;application des informations sur la qualité des données"@fr ;
  skos:prefLabel "データ品質適用範囲"@ja ;
  skos:prefLabel "데이터 품질 범위"@ko ;
  skos:prefLabel "zakres jakości danych"@pl ;
  skos:prefLabel "область определения качества данных"@ru ;
  skos:prefLabel "ámbito de la calidad de datos"@es ;
  skos:prefLabel "datakvalitetsdelomfattning"@sv ;
  skos:prefLabel "数据质量范围"@zh ;
  
  geolexica:origin lang:araRegistry ,
                lang:danRegistry ,
                lang:deuRegistry ,
                lang:engRegistry ,
                lang:finRegistry ,
                lang:fraRegistry ,
                lang:korRegistry ,
                # lang:nldRegistry ,
                lang:jpnRegistry ,
                lang:rusRegistry ,
                lang:polRegistry ,
                # lang:msaRegistry ,
                lang:spaRegistry ,
                lang:sweRegistry ,
                lang:zhoRegistry ;
        lang:deu-note notes:DefnTransUnavail , notes:NoteTransUnavail ; 
        lang:swe-note notes:NoteTransUnavail .

###  https://isotc211.geolexica.org/ld/concepts#data_quality_subelement
:data_quality_subelement rdf:type owl:NamedIndividual ,
                   skos:Concept ;
          skos:inScheme geolexica:GeolexicaConceptScheme ;
          geolexica:hasInfo info:Info119 ;
          geolexica:hasReview reviews:Review119 ;
          geolexica:hasLDAPI ldapi:ldapi119-json ,
                             ldapi:ldapi119-jsonld ,
                             ldapi:ldapi119-rdfxml ,
                             ldapi:ldapi119-skosrdf ;
        geolexica:hasLangCode lang:ara ,
                        lang:dan ,
                        lang:deu ,
                        lang:eng ,
                        lang:fin ,
                        lang:fra ,
                        lang:kor ,
                        # lang:nld ,
                        lang:pol ,
                        lang:jpn ,
                        # lang:msa ,
                        lang:rus ,
                        lang:spa ,
                        lang:swe ,
                        lang:zho ;
          dcterms:identifier 119 ;
          skos:notation 119 ;
          rdfs:label "data quality subelement" ;

  skos:definition "component of a data quality element describing a certain aspect of that data quality element"@en ;
  skos:definition "مكون عنصر جودة بيانات يصف جانبا محدداً من ذلك العنصر"@ar ;
  skos:definition "komponent af et datakvalitetselement, der beskriver et bestemt aspekt ved det pågældende datakvalitetselement"@da ;
  skos:definition "osatekijä, joka kuvailee mitattavan laatutekijän tiettyä näkökulmaa"@fi ;
  skos:definition "composant d&#39;un élément de qualité des données décrivant un certain aspect de cet élément de qualité des données"@fr ;
  skos:definition "データ品質要素のある側面を記述するデータ品質要素の構成要素。"@ja ;
  skos:definition "데이터 품질 요소의 특정한 측면을 설명하는 컴포넌트"@ko ;
  skos:definition "składnik elementu jakości danych opisujący wybrany pewien aspekt tego elementu jakości danych"@pl ;
  skos:definition "компонент элемента качества данных, описывающий определенный аспект этого элемента качества данных"@ru ;
  skos:definition "componente de un elemento de la calidad que describe un cierto aspecto de éste"@es ;
  skos:definition "数据质量元素的组成部分，描述数据质量元素的某一方面。"@zh ;
  
  skos:prefLabel "data quality subelement"@en ;
  skos:prefLabel "العنصر الفرعي لجودة البيانات"@ar ;
  skos:prefLabel "datakvalitetsdelelement"@da ;
  skos:prefLabel "Unterelement zur Angabe der Datenqualität"@de ;
  skos:prefLabel "mitattavan laatutekijän osatekijä"@fi ;
  skos:prefLabel "sous-élément de qualité des données"@fr ;
  skos:prefLabel "データ品質副要素"@ja ;
  skos:prefLabel "데이터 품질 하위 요소"@ko ;
  skos:prefLabel "element podrzędny jakości danych"@pl ;
  skos:prefLabel "подэлемент качества данных"@ru ;
  skos:prefLabel "subelemento de la calidad de datos"@es ;
  skos:prefLabel "数据质量子元素"@zh ;
  
  geolexica:origin lang:araRegistry ,
                lang:danRegistry ,
                lang:deuRegistry ,
                lang:engRegistry ,
                lang:finRegistry ,
                lang:fraRegistry ,
                lang:korRegistry ,
                # lang:nldRegistry ,
                lang:jpnRegistry ,
                lang:rusRegistry ,
                lang:polRegistry ,
                # lang:msaRegistry ,
                lang:spaRegistry ,
                lang:sweRegistry ,
                lang:zhoRegistry ;
        lang:deu-note notes:DefnTransUnavail .

###  https://isotc211.geolexica.org/ld/concepts#data_quality_value_type
:data_quality_value_type rdf:type owl:NamedIndividual ,
                   skos:Concept ;
          skos:inScheme geolexica:GeolexicaConceptScheme ;
          geolexica:hasInfo info:Info120 ;
          geolexica:hasReview reviews:Review120 ;
          geolexica:hasLDAPI ldapi:ldapi120-json ,
                             ldapi:ldapi120-jsonld ,
                             ldapi:ldapi120-rdfxml ,
                             ldapi:ldapi120-skosrdf ;
        geolexica:hasLangCode lang:ara ,
                        lang:dan ,
                        lang:deu ,
                        lang:eng ,
                        lang:fin ,
                        lang:fra ,
                        lang:kor ,
                        # lang:nld ,
                        lang:pol ,
                        lang:jpn ,
                        # lang:msa ,
                        lang:rus ,
                        lang:spa ,
                        lang:swe ,
                        lang:zho ;
          dcterms:identifier 120 ;
          skos:notation 120 ;
          rdfs:label "data quality value type" ;

  skos:definition "value type for reporting a data quality result"@en ;
  skos:definition "نوع القيمة الخاصة بالإبلاغ عن نتائج جودة البيانات"@ar ;
  skos:definition "værditype til rapportering af et datakvalitetsresultat"@da ;
  skos:definition "laatutuloksen raportoinnissa käytetty arvotyyppi"@fi ;
  skos:definition "type de valeur destiné à rapporter un résultat de qualité des données"@fr ;
  skos:definition "データ品質評価結果を報告するための値の型。"@ja ;
  skos:definition "데이터 품질 결과를 보고하는 값의 유형"@ko ;
  skos:definition "typ wartości do przedstawiania wyniku oceny jakości danych"@pl ;
  skos:definition "тип величин для представления результатов  оценки качества данных"@ru ;
  skos:definition "tipo de valor para informar de un resultado de la calidad de datos"@es ;
  skos:definition "typ av värde som används för att ange ett datakvalitetsresultat"@sv ;
  skos:definition "记录数据质量结果的值的类型。"@zh ;

  skos:prefLabel "data quality value type"@en ;
  skos:prefLabel "نوع قيمة جودة البيانات"@ar ;
  skos:prefLabel "datakvalitet, værditype for"@da ;
  skos:prefLabel "Wertetyp der Datenqualitätsangabe"@de ;
  skos:prefLabel "laatuarvon tyyppi"@fi ;
  skos:prefLabel "type de valeur de qualité des données"@fr ;
  skos:prefLabel "データ品質評価値型"@ja ;
  skos:prefLabel "데이터 품질 값 유형"@ko ;
  skos:prefLabel "typ wartości jakości danych"@pl ;
  skos:prefLabel "тип значения качества данных"@ru ;
  skos:prefLabel "tipo de valor de la calidad de datos"@es ;
  skos:prefLabel "datakvalitetsresultattyp"@sv ;
  skos:prefLabel "数据质量值类型"@zh ;
  
  geolexica:origin lang:araRegistry ,
                lang:danRegistry ,
                lang:deuRegistry ,
                lang:engRegistry ,
                lang:finRegistry ,
                lang:fraRegistry ,
                lang:korRegistry ,
                # lang:nldRegistry ,
                lang:jpnRegistry ,
                lang:rusRegistry ,
                lang:polRegistry ,
                # lang:msaRegistry ,
                lang:spaRegistry ,
                lang:sweRegistry ,
                lang:zhoRegistry ;
        lang:deu-note notes:DefnTransUnavail , notes:NoteTransUnavail , notes:ExTransUnavail  ;
        lang:swe-note notes:NoteTransUnavail , notes:ExTransUnavail .


###  https://isotc211.geolexica.org/ld/concepts#data_quality_value_unit
:data_quality_value_unit rdf:type owl:NamedIndividual ,
                   skos:Concept ;
          skos:inScheme geolexica:GeolexicaConceptScheme ;
          geolexica:hasInfo info:Info121 ;
          geolexica:hasReview reviews:Review121 ;
          geolexica:hasLDAPI ldapi:ldapi121-json ,
                             ldapi:ldapi121-jsonld ,
                             ldapi:ldapi121-rdfxml ,
                             ldapi:ldapi121-skosrdf ;
        geolexica:hasLangCode lang:ara ,
                        lang:dan ,
                        lang:deu ,
                        lang:eng ,
                        lang:fin ,
                        lang:fra ,
                        lang:kor ,
                        # lang:nld ,
                        lang:pol ,
                        lang:jpn ,
                        # lang:msa ,
                        lang:rus ,
                        lang:spa ,
                        lang:swe ,
                        lang:zho ;
          dcterms:identifier 121 ;
          skos:notation 121 ;
          rdfs:label "data quality value unit" ;

  skos:definition "value unit for reporting a data quality result"@en ;
  skos:definition "وحدة القيمة الخاصة بالإبلاغ عن نتائج جودة البيانات"@ar ;
  skos:definition "værdienhed til rapportering af et datakvalitetsresultat"@da ;
  skos:definition "laatutuloksen raportoinnissa käytetty arvoyksikkö"@fi ;
  skos:definition "unité de valeur destiné à rapporter un résultat de qualité des données"@fr ;
  skos:definition "データ品質評価結果を報告するための値の単位。"@ja ;
  skos:definition "데이터 품질 결과를 보고하는 값의 단위"@ko ;
  skos:definition "jednostka wartości do przedstawiania wyniku oceny jakości danych"@pl ;
  skos:definition "единица измерения для представления результатов оценки качества данных"@ru ;
  skos:definition "unidad empleada para informar sobre un resultado de la calidad de un conjunto de datos"@es ;
  skos:definition "måttenhet som används för att ange ett datakvalitetsresultat"@sv ;
  skos:definition "记录数据质量结果的值的单位。"@zh ;

  skos:prefLabel "data quality value unit"@en ;
  skos:prefLabel "وحدة قيمة جودة البيانات"@ar ;
  skos:prefLabel "værdienhed for datakvalitet"@da ;
  skos:prefLabel "Einheit der Datenqualitätsangabe"@de ;
  skos:prefLabel "laatuarvon yksikkö"@fi ;
  skos:prefLabel "unité de valeur de qualité des données"@fr ;
  skos:prefLabel "データ品質評価値単位"@ja ;
  skos:prefLabel "데이터 품질 값 단위"@ko ;
  skos:prefLabel "jednostka wartości jakości danych"@pl ;
  skos:prefLabel "единица измерения качества данных"@ru ;
  skos:prefLabel "unidad del valor de la calidad de datos"@es ;
  skos:prefLabel "datakvalitetsresultatenhet"@sv ;
  skos:prefLabel "数据质量值单位"@zh ;
  
  geolexica:origin lang:araRegistry ,
                lang:danRegistry ,
                lang:deuRegistry ,
                lang:engRegistry ,
                lang:finRegistry ,
                lang:fraRegistry ,
                lang:korRegistry ,
                # lang:nldRegistry ,
                lang:jpnRegistry ,
                lang:rusRegistry ,
                lang:polRegistry ,
                # lang:msaRegistry ,
                lang:spaRegistry ,
                lang:sweRegistry ,
                lang:zhoRegistry ;
        lang:deu-note notes:DefnTransUnavail , notes:NoteTransUnavail , notes:ExTransUnavail  ;
        lang:swe-note notes:NoteTransUnavail , notes:ExTransUnavail .


###  https://isotc211.geolexica.org/ld/concepts#data_transfer
:data_transfer rdf:type owl:NamedIndividual ,
                   skos:Concept ;
          skos:inScheme geolexica:GeolexicaConceptScheme ;
          geolexica:hasInfo info:Info122 ;
          geolexica:hasReview reviews:Review122 ;
          geolexica:hasLDAPI ldapi:ldapi122-json ,
                             ldapi:ldapi122-jsonld ,
                             ldapi:ldapi122-rdfxml ,
                             ldapi:ldapi122-skosrdf ;
        geolexica:hasLangCode lang:ara ,
                        lang:dan ,
                        lang:deu ,
                        lang:eng ,
                        lang:fin ,
                        lang:fra ,
                        lang:kor ,
                        # lang:nld ,
                        # lang:pol ,
                        # lang:jpn ,
                        # lang:msa ,
                        lang:rus ,
                        lang:spa ,
                        lang:swe ,
                        lang:zho ;
          dcterms:identifier 122 ;
          skos:notation 122 ;
          rdfs:label "data transfer" ;

  skos:definition "movement of data from one point to another over a medium"@en ;
  skos:definition "حركة البيانات من نقطة إلى أخرى من خلال وسيط"@ar ;
  skos:definition "flytning af data fra et sted til et andet vha. et medie"@da ;
  skos:definition "tiedon siirtäminen pisteestä toiseen viestintävälineen kautta"@fi ;
  skos:definition "mouvement de donnée d&#39;un point à un autre via un media"@fr ;
  skos:definition "매체를 통해 한 지점에서 다른 지점으로 데이터를 이동시키는 것"@ko ;
  skos:definition "перемещение данных из одного места в другое в той или иной среде"@ru ;
  skos:definition "movimiento de datos de un punto a otro a través de un medio"@es ;
  skos:definition "överföring av data från en plats till en annan med hjälp av ett medium"@sv ;
  skos:definition "数据通过介质从一点到另一点的传送。"@zh ;

  skos:prefLabel "data transfer"@en ;
  skos:prefLabel "نقل البيانات"@ar ;
  skos:prefLabel "dataoverførsel"@da ;
  skos:prefLabel "Datenübertragung"@de ;
  skos:prefLabel "tiedonsiirto"@fi ;
  skos:prefLabel "transfert de données"@fr ;
  skos:prefLabel "데이터 전송"@ko ;
  skos:prefLabel "передача данных"@ru ;
  skos:prefLabel "transferencia de datos"@es ;
  skos:prefLabel "dataöverföring"@sv ;
  skos:prefLabel "数据传输"@zh ;
  
  geolexica:origin lang:araRegistry ,
                lang:danRegistry ,
                lang:deuRegistry ,
                lang:engRegistry ,
                lang:finRegistry ,
                lang:fraRegistry ,
                lang:korRegistry ,
                # lang:nldRegistry ,
                # lang:jpnRegistry ,
                lang:rusRegistry ,
                # lang:polRegistry ,
                # lang:msaRegistry ,
                lang:spaRegistry ,
                lang:sweRegistry ,
                lang:zhoRegistry ;
        lang:deu-note notes:DefnTransUnavail , notes:NoteTransUnavail ;
        lang:swe-note notes:NoteTransUnavail  .

###  https://isotc211.geolexica.org/ld/concepts#data_type
:data_type rdf:type owl:NamedIndividual ,
                   skos:Concept ;
          skos:inScheme geolexica:GeolexicaConceptScheme ;
          geolexica:hasInfo info:Info123 ;
          geolexica:hasReview reviews:Review123 ;
          geolexica:hasLDAPI ldapi:ldapi123-json ,
                             ldapi:ldapi123-jsonld ,
                             ldapi:ldapi123-rdfxml ,
                             ldapi:ldapi123-skosrdf ;
        geolexica:hasLangCode lang:ara ,
                        lang:dan ,
                        lang:deu ,
                        lang:eng ,
                        lang:fin ,
                        lang:fra ,
                        lang:kor ,
                        # lang:nld ,
                        lang:pol ,
                        # lang:jpn ,
                        # lang:msa ,
                        lang:rus ,
                        lang:spa ,
                        lang:swe ,
                        lang:zho ;
          dcterms:identifier 123 ;
          skos:notation 123 ;
          rdfs:label "data type" ;

  skos:definition "specification of a value domain with operations allowed on values in this domain"@en ;
  skos:definition "مواصفات نطاق قيمة محدد مع العمليات المسموح بإجرائها على القيم في حدود هذا النطاق"@ar ;
  skos:definition "specifikation af et værdidomæne inkl. de tilladte operationer på værdier deri"@da ;
  skos:definition "Festlegung eines Wertebereichs mit Operationen, die für Werte in diesem Bereich zulässig sind"@de ;
  skos:definition "tietoyksiköiden tai -rakenteiden ja niihin liittyvien toimintojen määrittely"@fi ;
  skos:definition "spécification d’un domaine de valeurs et d’opérations autorisées sur les valeurs de ce domaine"@fr ;
  skos:definition "영역 내의 값을 바탕으로 연산을 통해 나올 수 있는 허용된 값 영역의 사양"@ko ;
  skos:definition "określenie dziedziny wartości dopuszczalnych i operacji dozwolonych na wartościach z tej dziedziny [ISO 19103]"@pl ;
  skos:definition "комплекс характеристик, наличие которых у группы данных позволяет выделить ее из множества других данных"@ru ;
  skos:definition "especificación de un dominio de valores con unas operaciones permitidas sobre los valores de ese dominio"@es ;
  skos:definition "specifikation av en värdedomän och de operationer som är tillåtna på domänens värden"@sv ;
  skos:definition "允许在值域内对值进行操作的值域的说明。"@zh ;

  skos:prefLabel "data type"@en ;
  skos:prefLabel "نوع البيانات"@ar ;
  skos:prefLabel "datatype"@da ;
  skos:prefLabel "Datentyp"@de ;
  skos:prefLabel "tietotyyppi"@fi ;
  skos:prefLabel "type de donnée"@fr ;
  skos:prefLabel "데이터 유형"@ko ;
  skos:prefLabel "typ danych"@pl ;
  skos:prefLabel "тип данных"@ru ;
  skos:prefLabel "tipo de datos"@es ;
  skos:prefLabel "datatyp"@sv ;
  skos:prefLabel "数据类型"@zh ;
  
  geolexica:origin lang:araRegistry ,
                lang:danRegistry ,
                lang:deuRegistry ,
                lang:engRegistry ,
                lang:finRegistry ,
                lang:fraRegistry ,
                lang:korRegistry ,
                # lang:nldRegistry ,
                # lang:jpnRegistry ,
                lang:rusRegistry ,
                lang:polRegistry ,
                # lang:msaRegistry ,
                lang:spaRegistry ,
                lang:sweRegistry ,
                lang:zhoRegistry ;
        lang:deu-note notes:ExTransUnavail , notes:NoteTransUnavail ;
        lang:rus-note notes:NoteTransDiff  ;
        lang:swe-note notes:ExTransUnavail , notes:NoteTransUnavail   .

###  https://isotc211.geolexica.org/ld/concepts#dataset
:dataset rdf:type owl:NamedIndividual ,
                   skos:Concept ;
          skos:inScheme geolexica:GeolexicaConceptScheme ;
          geolexica:hasInfo info:Info124 ;
          geolexica:hasReview reviews:Review124 ;
          geolexica:hasLDAPI ldapi:ldapi124-json ,
                             ldapi:ldapi124-jsonld ,
                             ldapi:ldapi124-rdfxml ,
                             ldapi:ldapi124-skosrdf ;
        geolexica:hasLangCode lang:ara ,
                        lang:dan ,
                        lang:deu ,
                        lang:eng ,
                        lang:fin ,
                        lang:fra ,
                        lang:kor ,
                        # lang:nld ,
                        lang:pol ,
                        lang:jpn ,
                        lang:msa ,
                        lang:rus ,
                        lang:spa ,
                        lang:swe ,
                        lang:zho ;
          dcterms:identifier 124 ;
          skos:notation 124 ;
          rdfs:label "dataset" ;

  skos:definition "identifiable collection of data"@en ;
  skos:definition "مجموعة من البيانات المميزة"@ar ;
  skos:definition "identificerbar samling af data"@da ;
  skos:definition "identifizierbare Sammlung von Daten"@de ;
  skos:definition "yksilöitävissä oleva kokoelma tietoja"@fi ;
  skos:definition "collection identifiable de données"@fr ;
  skos:definition "他と識別可能なデータの集まり。"@ja ;
  skos:definition "식별 가능한 데이터의 모음"@ko ;
  skos:definition "kumpulan data yang boleh dikenal pasti sama ada dataset statik atau dataset dinamik"@ms ;
  skos:definition "identyfikowalna kolekcja danych"@pl ;
  skos:definition "идентифицированная совокупность данных"@ru ;
  skos:definition "colección identificable de datos"@es ;
  skos:definition "identifierbar samling data"@sv ;
  skos:definition "可识别的数据集合。"@zh ;

  skos:prefLabel "dataset"@en ;
  skos:prefLabel "مجموعة بيانات"@ar ;
  skos:prefLabel "datasæt"@da ;
  skos:prefLabel "Datensatz"@de ;
  skos:prefLabel "tietoaineisto"@fi ;
  skos:prefLabel "jeu de données"@fr ;
  skos:prefLabel "データ集合"@ja ;
  skos:prefLabel "데이터셋"@ko ;
  skos:prefLabel "dataset"@ms ;
  skos:prefLabel "zbiór danych"@pl ;
  skos:prefLabel "набор данных"@ru ;
  skos:prefLabel "conjunto de datos"@es ;
  skos:prefLabel "datamängd"@sv ;
  skos:prefLabel "数据集"@zh ;
  
  geolexica:origin lang:araRegistry ,
                lang:danRegistry ,
                lang:deuRegistry ,
                lang:engRegistry ,
                lang:finRegistry ,
                lang:fraRegistry ,
                lang:korRegistry ,
                # lang:nldRegistry ,
                lang:jpnRegistry ,
                lang:rusRegistry ,
                lang:polRegistry ,
                lang:msaRegistry ,
                lang:spaRegistry ,
                lang:sweRegistry ,
                lang:zhoRegistry ;
        lang:deu-note notes:NoteTransUnavail ;
        lang:msa-note notes:NoteTransUnavail ;
        lang:swe-note notes:NoteTransUnavail   .


###  https://isotc211.geolexica.org/ld/concepts#dataset_series
:dataset_series rdf:type owl:NamedIndividual ,
                   skos:Concept ;
          skos:inScheme geolexica:GeolexicaConceptScheme ;
          geolexica:hasInfo info:Info125 ;
          geolexica:hasReview reviews:Review125 ;
          geolexica:hasLDAPI ldapi:ldapi125-json ,
                             ldapi:ldapi125-jsonld ,
                             ldapi:ldapi125-rdfxml ,
                             ldapi:ldapi125-skosrdf ;
        geolexica:hasLangCode lang:ara ,
                        lang:dan ,
                        lang:deu ,
                        lang:eng ,
                        lang:fin ,
                        lang:fra ,
                        lang:kor ,
                        # lang:nld ,
                        lang:pol ,
                        lang:jpn ,
                        lang:msa ,
                        lang:rus ,
                        lang:spa ,
                        lang:swe ,
                        lang:zho ;
          dcterms:identifier 125 ;
          skos:notation 125 ;
          rdfs:label "dataset series" ;

  skos:definition "collection of datasets sharing the same product specification"@en ;
  skos:definition "تجميع لمجموعة بيانات لها نفس مواصفات المنتج"@ar ;
  skos:definition "samling af datasæt med samme produktspecifikation"@da ;
  skos:definition "Sammlung von Datensätzen mit gemeinsamer Datenproduktspezifikation"@de ;
  skos:definition "kokoelma tietoaineistoja, joihin liittyy pääosin sama metatietosisältö"@fi ;
  skos:definition "collection de jeux de données partageant la même spécification de produit"@fr ;
  skos:definition "同じ製品仕様書を使って作成したデータ集合の集まり。"@ja ;
  skos:definition "동일한 제품 사양을 통해 작성된 데이터셋의 모음"@ko ;
  skos:definition "kumpulan dataset yang menggunakan spesifikasi produk yang sama"@ms ;
  skos:definition "kolekcja zbiorów danych zgodnych z tą samą specyfikacją produktu"@pl ;
  skos:definition "совокупность наборов данных на основе общей спецификации продукта"@ru ;
  skos:definition "colección de conjuntos de datos que comparten una misma especificación de producto"@es ;
  skos:definition "uppsättning datamängder som har samma dataproduktspecifikation"@sv ;
  skos:definition "符合相同产品规范的数据集集合。"@zh ;

  skos:prefLabel "dataset series"@en ;
  skos:prefLabel "سلسلة مجموعة بيانات"@ar ;
  skos:prefLabel "datasætserie"@da ;
  skos:prefLabel "Serie von Datensätzen"@de ;
  skos:prefLabel "tietoaineistosarja"@fi ;
  skos:prefLabel "série de jeux de données"@fr ;
  skos:prefLabel "データ集合系列"@ja ;
  skos:prefLabel "데이터셋 시리즈"@ko ;
  skos:prefLabel "siri data"@ms ;
  skos:prefLabel "seria zbiorów danych"@pl ;
  skos:prefLabel "комплект наборов данных"@ru ;
  skos:prefLabel "serie de conjuntos de datos"@es ;
  skos:prefLabel "datamängdsserie"@sv ;
  skos:prefLabel "数据集系列"@zh ;
  
  geolexica:origin lang:araRegistry ,
                lang:danRegistry ,
                lang:deuRegistry ,
                lang:engRegistry ,
                lang:finRegistry ,
                lang:fraRegistry ,
                lang:korRegistry ,
                # lang:nldRegistry ,
                lang:jpnRegistry ,
                lang:rusRegistry ,
                lang:polRegistry ,
                lang:msaRegistry ,
                lang:spaRegistry ,
                lang:sweRegistry ,
                lang:zhoRegistry .

###  https://isotc211.geolexica.org/ld/concepts#day
:day rdf:type owl:NamedIndividual ,
                   skos:Concept ;
          skos:inScheme geolexica:GeolexicaConceptScheme ;
          geolexica:hasInfo info:Info127 ;
        #   geolexica:hasReview reviews:Review127 ;
          geolexica:hasLDAPI ldapi:ldapi127-json ,
                             ldapi:ldapi127-jsonld ,
                             ldapi:ldapi127-rdfxml ,
                             ldapi:ldapi127-skosrdf ;
        geolexica:hasLangCode lang:ara ,
                        lang:dan ,
                        lang:deu ,
                        lang:eng ,
                        lang:fin ,
                        lang:fra ,
                        lang:kor ,
                        # lang:nld ,
                        lang:pol ,
                        lang:jpn ,
                        lang:msa ,
                        lang:rus ,
                        lang:spa ,
                        lang:swe ,
                        lang:zho ;
          dcterms:identifier 127 ;
          skos:notation 127 ;
          rdfs:label "day" ;

  skos:definition "period having a duration nominally equivalent to the periodic time of the Earth&#39;s rotation around its axis"@en ;
  skos:definition "فترة زمنية يمتد أمدها الزمني الاسمي بما يساوي الوقت الذي تستغرقه الكرة الأرضية للدوران حول محورها"@ar ;
  skos:definition "tidsrum af en varighed, der nominelt svarer til den tid, det tager jorden at dreje omkring sin egen akse"@da ;
  skos:definition "ajanjakso, joka teoreettisesti kestää ajan, joka kuluu Maan pyörähtämiseen akselinsa ympäri"@fi ;
  skos:definition "période ayant une durée nominalement équivalente à la période de temps de la rotation de la Terre autour de son axe"@fr ;
  skos:definition "地球の自転周期にほぼ等しい持続時間をもつ期間。"@ja ;
  skos:definition "지구 자전 주기와 명목상 같은 지속 기간을 갖는 기간"@ko ;
  skos:definition "okres, którego czas trwania jest nominalnie równoważny z czasem cyklicznym obrotu Ziemi wokół własnej osi"@pl ;
  skos:definition "период времени, продолжительность которого номинально равна периоду обращения Земли вокруг ее оси"@ru ;
  skos:definition "período de duración nominalmente equivalente al período de tiempo de rotación de la Tierra alrededor de su eje"@es ;
  skos:definition "den tid jorden behöver för att rotera ett varv kring sin axel"@sv ;
  skos:definition "相当于地球自转周期的持续时间的时段。"@zh ;

  skos:prefLabel "day"@en ;
  skos:prefLabel "يوم"@ar ;
  skos:prefLabel "døgn"@da ;
  skos:prefLabel "Tag"@de ;
  skos:prefLabel "päivä"@fi ;
  skos:prefLabel "jour"@fr ;
  skos:prefLabel "日"@ja ;
  skos:prefLabel "일"@ko ;
  skos:prefLabel "hari"@ms ;
  skos:prefLabel "dzień"@pl ;
  skos:prefLabel "день"@ru ;
  skos:prefLabel "día"@es ;
  skos:prefLabel "dygn"@sv ;
  skos:prefLabel "日"@zh ;
  
  geolexica:origin lang:araRegistry ,
                lang:danRegistry ,
                lang:deuRegistry ,
                lang:engRegistry ,
                lang:finRegistry ,
                lang:fraRegistry ,
                lang:korRegistry ,
                # lang:nldRegistry ,
                lang:jpnRegistry ,
                lang:rusRegistry ,
                lang:polRegistry ,
                lang:msaRegistry ,
                lang:spaRegistry ,
                lang:sweRegistry ,
                lang:zhoRegistry ;
        lang:deu-note notes:DefnTransUnavail ;
        lang:fra-note notes:NoteTransDiff ;
        lang:msa-note notes:DefnTransUnavail .


###  https://isotc211.geolexica.org/ld/concepts#definition
:definition rdf:type owl:NamedIndividual ,
                   skos:Concept ;
          skos:inScheme geolexica:GeolexicaConceptScheme ;
          geolexica:hasInfo info:Info128 ;
          geolexica:hasReview reviews:Review128 ;
          geolexica:hasLDAPI ldapi:ldapi128-json ,
                             ldapi:ldapi128-jsonld ,
                             ldapi:ldapi128-rdfxml ,
                             ldapi:ldapi128-skosrdf ;
        geolexica:hasLangCode lang:ara ,
                        lang:dan ,
                        lang:deu ,
                        lang:eng ,
                        # lang:fin ,
                        # lang:fra ,
                        lang:kor ,
                        # lang:nld ,
                        # lang:pol ,
                        # lang:jpn ,
                        lang:msa ,
                        lang:rus ,
                        lang:spa ,
                        lang:swe ;
                        # lang:zho ;
          dcterms:identifier 128 ;
          skos:notation 128 ;
          rdfs:label "definition" ;

  skos:definition "representation of a concept by a descriptive statement which serves to differentiate it from related concepts"@en ;
  skos:definition "توضيح لمفهوم بجملة وصفية لتمييزه عن  المفاهيم الاخرى ذات العلاقة"@ar ;
  skos:definition "beskrivelse af et begreb ved et deskriptivt udsagn, der tjener til at skelne det fra beslægtede begreber"@da ;
  skos:definition "연관 개념들과 차별화하기 위한 묘사적 기술을 통한 개념 표현"@ko ;
  skos:definition "представление понятия описательным утверждением, которое служит для того, чтобы отличить его от связанных понятий"@ru ;
  skos:definition "representación de un concepto mediante un enunciado descriptivo que permite diferenciarlo de otros conceptos relacionados"@es ;
  skos:definition "beskrivning som ska avgränsa begreppet mot relaterade begrepp"@sv ;

  skos:prefLabel "definition"@en ;
  skos:prefLabel "تعريف"@ar ;
  skos:prefLabel "definition"@da ;
  skos:prefLabel "Definition"@de ;
  skos:prefLabel "정의"@ko ;
  skos:prefLabel "kejelasan"@ms ;
  skos:prefLabel "определение"@ru ;
  skos:prefLabel "definición"@es ;
  skos:prefLabel "definition"@sv ;
  
  geolexica:origin lang:araRegistry ,
                lang:danRegistry ,
                lang:deuRegistry ,
                lang:engRegistry ,
                # lang:finRegistry ,
                # lang:fraRegistry ,
                lang:korRegistry ,
                # lang:nldRegistry ,
                # lang:jpnRegistry ,
                lang:rusRegistry ,
                # lang:polRegistry ,
                lang:msaRegistry ,
                lang:spaRegistry ,
                lang:sweRegistry ;
                # lang:zhoRegistry ;
        lang:deu-note notes:DefnTransUnavail ;
        lang:msa-note notes:DefnTransUnavail .


###  https://isotc211.geolexica.org/ld/concepts#Delaunay_triangulation
:Delaunay_triangulation rdf:type owl:NamedIndividual ,
                   skos:Concept ;
          skos:inScheme geolexica:GeolexicaConceptScheme ;
          geolexica:hasInfo info:Info129 ;
        #   geolexica:hasReview reviews:Review129 ;
          geolexica:hasLDAPI ldapi:ldapi129-json ,
                             ldapi:ldapi129-jsonld ,
                             ldapi:ldapi129-rdfxml ,
                             ldapi:ldapi129-skosrdf ;
        geolexica:hasLangCode lang:ara ,
                        lang:dan ,
                        lang:deu ,
                        lang:eng ,
                        lang:fin ,
                        lang:fra ,
                        lang:kor ,
                        # lang:nld ,
                        lang:pol ,
                        # lang:jpn ,
                        # lang:msa ,
                        lang:rus ,
                        lang:spa ,
                        lang:swe ,
                        lang:zho ;
          dcterms:identifier 129 ;
          skos:notation 129 ;
          rdfs:label "Delaunay triangulation" ;

  skos:definition "network of triangles such that  the circle passing through the vertices of any triangle does not contain, in its interior, the vertex of any other triangle"@en ;
  skos:definition "شبكة مثلثات مرتبة بحيث أن الدائرة التي تمر عبر رؤوس أي مثلث لا تحتوي في داخلها على رأس أي من المثلثات الأخرى"@ar ;
  skos:definition "netværk af trekanter dannet således, at der inden for ingen af de cirkler, som går igennem trekanternes toppunkter, ligger en anden trekants toppunkt"@da ;
  skos:definition "sellainen kolmioiden verkosto, jossa minkä hyvänsä kolmion kärkien kautta kulkeva ympyrä ei pidä sisällään minkään muun kolmion kärkeä"@fi ;
  skos:definition "réseau de triangles tel que le cercle passant par les sommets de n&#39;importe quel triangle ne contient pas, dans son intérieur, le sommet d&#39;un autre triangle"@fr ;
  skos:definition "삼각형을 구성하는 세 개의 정점을 지나는 원의 내부에 다른 삼각형의 어느 정점도 포함하지 않는 삼각망"@ko ;
  skos:definition "taka siatka trójkątów, dla której okrąg przechodzący przez wierzchołki dowolnego trójkąta nie zawiera w swoim wnętrzu wierzchołka żadnego innego trójkąta"@pl ;
  skos:definition "сеть треугольников, в пределах которой внутри окружности, описанной вокруг любого треугольника, нет вершин другого треугольника"@ru ;
  skos:definition "red de triángulos tal que el círculo que pasa a través de los vértices de cualquier triángulo no contiene, en su interior, el vértice de ningún otro triángulo"@es ;
  skos:definition "nät av trianglar där varje triangel är ur utformad så att en cirkel som omskriver triangeln endast innehåller den egna triangelns hörn"@sv ;
  skos:definition "任意三角形的外接圆内不含其他三角形顶点的三角网。"@zh ;

  skos:prefLabel "Delaunay triangulation"@en ;
  skos:prefLabel "تثليث ديلوناي"@ar ;
  skos:prefLabel "Delaunay-triangulation"@da ;
  skos:prefLabel "Delaunay Triangulation"@de ;
  skos:prefLabel "Delaunayn kolmiointi"@fi ;
  skos:prefLabel "triangulation de Delaunay"@fr ;
  skos:prefLabel "델로니 삼각 분할"@ko ;
  skos:prefLabel "triangulacja Delaunaya"@pl ;
  skos:prefLabel "триангуляция Делоне"@ru ;
  skos:prefLabel "triangulación de Delaunay"@es ;
  skos:prefLabel "Delaunay-triangelnät"@sv ;
  skos:prefLabel "Delaunay三角网"@zh ;
  
  geolexica:origin lang:araRegistry ,
                lang:danRegistry ,
                lang:deuRegistry ,
                lang:engRegistry ,
                lang:finRegistry ,
                lang:fraRegistry ,
                lang:korRegistry ,
                # lang:nldRegistry ,
                # lang:jpnRegistry ,
                lang:rusRegistry ,
                lang:polRegistry ,
                # lang:msaRegistry ,
                lang:spaRegistry ,
                lang:sweRegistry ,
                lang:zhoRegistry ;
        lang:deu-note notes:DefnTransUnavail ;
        lang:fra-note notes:NoteTransDiff .

###  https://isotc211.geolexica.org/ld/concepts#dependencyUML
:dependencyUML rdf:type owl:NamedIndividual ,
                   skos:Concept ;
          skos:inScheme geolexica:GeolexicaConceptScheme ;
          geolexica:hasInfo info:Info130 ;
          geolexica:hasReview reviews:Review130 ;
          geolexica:hasLDAPI ldapi:ldapi130-json ,
                             ldapi:ldapi130-jsonld ,
                             ldapi:ldapi130-rdfxml ,
                             ldapi:ldapi130-skosrdf ;
        geolexica:hasLangCode lang:ara ,
                        lang:dan ,
                        lang:deu ,
                        lang:eng ,
                        lang:fin ,
                        lang:fra ,
                        lang:kor ,
                        # lang:nld ,
                        # lang:pol ,
                        # lang:jpn ,
                        # lang:msa ,
                        lang:rus ,
                        lang:spa ,
                        lang:swe ,
                        lang:zho ;
          dcterms:identifier 130 ;
          skos:notation 130 ;
          rdfs:label "dependency (UML)" ;

  skos:definition "relationship between two modelling elements, in which a change to one modelling element (the independent element) will affect the other modelling element (the dependent element)"@en ;
  skos:definition "علاقة متبادلة بين عنصرين للنمذجة يكون فيها للتغيير في أحد العنصرين (وهو العنصر المستقل ) تأثير على العنصر الآخر ( أي العنصر التابع )"@ar ;
  skos:definition "relation mellem to elementer (klasser), hvor en ændring af det ene element (det uafhængige element) vil påvirke det andet element (det afhængige element)"@da ;
  skos:definition "kahden mallinnuselementin välinen suhde, jossa yhteen mallinnuselementtiin (riippumaton elementti) kohdistuva muutos vaikuttaa toiseen (riippuvainen elementti)"@fi ;
  skos:definition "relation entre deux éléments du modèle, dans laquelle un changement d&#39;un élément du modèle (l&#39;élément indépendant) affectera l&#39;autre élément du modèle (l&#39;élément dépendant)"@fr ;
  skos:definition "하나의 모델링 요소(독립 요소)가 변경되었을 때 다른 모델링 요소(종속 요소)에 영향을 미치는 두 모델링 요소 간의 관계"@ko ;
  skos:definition "отношение двух моделируемых элементов, при котором изменение одного из них (независимого) может повлиять на другой (зависимый)"@ru ;
  skos:definition "relación entre dos elementos de modelado en el que un cambio en uno de los elementos (elementos independientes) afecta a otros elementos de modelado (elementos dependientes)"@es ;
  skos:definition "relationship between two modelling elements, in which a change to one modelling element (the independent element) will affect the other modelling element (the dependent element)"@sv ;
  skos:definition "两个建模元素之间的关系，一个建模元素（独立元素）发生改变会影响另一个建模元素（依赖元素）。"@zh ;

  skos:prefLabel "dependency (UML)"@en ;
  skos:prefLabel "التبعية  ( UML  )"@ar ;
  skos:prefLabel "afhængighed (UML)"@da ;
  skos:prefLabel "Abhängigkeit (UML)"@de ;
  skos:prefLabel "riippuvuus (UML)"@fi ;
  skos:prefLabel "dépendance (UML)"@fr ;
  skos:prefLabel "의존 (UML)"@ko ;
  skos:prefLabel "зависимость (UML)"@ru ;
  skos:prefLabel "dependencia (UML)"@es ;
  skos:prefLabel "dependency (UML)"@sv ;
  skos:prefLabel "依赖(UML)"@zh ;
  
  geolexica:origin lang:araRegistry ,
                lang:danRegistry ,
                lang:deuRegistry ,
                lang:engRegistry ,
                lang:finRegistry ,
                lang:fraRegistry ,
                lang:korRegistry ,
                # lang:nldRegistry ,
                # lang:jpnRegistry ,
                lang:rusRegistry ,
                # lang:polRegistry ,
                # lang:msaRegistry ,
                lang:spaRegistry ,
                lang:sweRegistry ,
                lang:zhoRegistry ;
        lang:deu-note notes:DefnTransUnavail .

###  https://isotc211.geolexica.org/ld/concepts#deprecated_term
:deprecated_term rdf:type owl:NamedIndividual ,
                   skos:Concept ;
          skos:inScheme geolexica:GeolexicaConceptScheme ;
          geolexica:hasInfo info:Info131 ;
          geolexica:hasReview reviews:Review131 ;
          geolexica:hasLDAPI ldapi:ldapi131-json ,
                             ldapi:ldapi131-jsonld ,
                             ldapi:ldapi131-rdfxml ,
                             ldapi:ldapi131-skosrdf ;
        geolexica:hasLangCode lang:ara ,
                        lang:dan ,
                        lang:deu ,
                        lang:eng ,
                        # lang:fin ,
                        # lang:fra ,
                        lang:kor ,
                        # lang:nld ,
                        # lang:pol ,
                        # lang:jpn ,
                        # lang:msa ,
                        lang:rus ,
                        lang:spa ,
                        lang:swe ;
                        # lang:zho ;
          dcterms:identifier 131 ;
          skos:notation 131 ;
          rdfs:label "deprecated term" ;

  skos:definition "term rated according to the scale of the term acceptability rating as undesired"@en ;
  skos:definition "مصطلح صنف وفقا لمقياس تصنيف قبول المصطلحات غير مرغوب"@ar ;
  skos:definition "term, klassificeret efter en skala for tilladte termer som uønsket"@da ;
  skos:definition "용어 수용가능성 등급체계에서 불필요 등급을 부여받은 용어"@ko ;
  skos:definition "термин, оцененный по шкале рейтинга приемлемости термина как нежелательный"@ru ;
  skos:definition "término clasificado de acuerdo a la escala de aceptación como indeseable"@es ;
  skos:definition "term som bedömts vara olämplig för ett visst begrepp"@sv ;
  
  skos:prefLabel "deprecated term"@en ;
  skos:prefLabel "مصطلح مهمل"@ar ;
  skos:prefLabel "frarådet term"@da ;
  skos:prefLabel "nicht mehr gültiger Begriff"@de ;
  skos:prefLabel "사용되지 않는 용어"@ko ;
  skos:prefLabel "нерекомендуемый термин"@ru ;
  skos:prefLabel "término desaprobado"@es ;
  skos:prefLabel "avrådd term"@sv ;
  
  geolexica:origin lang:araRegistry ,
                lang:danRegistry ,
                lang:deuRegistry ,
                lang:engRegistry ,
                # lang:finRegistry ,
                # lang:fraRegistry ,
                lang:korRegistry ,
                # lang:nldRegistry ,
                # lang:jpnRegistry ,
                lang:rusRegistry ,
                # lang:polRegistry ,
                # lang:msaRegistry ,
                lang:spaRegistry ,
                lang:sweRegistry ;
                # lang:zhoRegistry ;
        lang:deu-note notes:DefnTransUnavail .

###  https://isotc211.geolexica.org/ld/concepts#Dijkstra_graph
:Dijkstra_graph rdf:type owl:NamedIndividual ,
                   skos:Concept ;
          skos:inScheme geolexica:GeolexicaConceptScheme ;
          geolexica:hasInfo info:Info133 ;
        #   geolexica:hasReview reviews:Review133 ;
          geolexica:hasLDAPI ldapi:ldapi133-json ,
                             ldapi:ldapi133-jsonld ,
                             ldapi:ldapi133-rdfxml ,
                             ldapi:ldapi133-skosrdf ;
        geolexica:hasLangCode lang:ara ,
                        lang:dan ,
                        lang:deu ,
                        lang:eng ,
                        lang:fin ,
                        lang:fra ,
                        lang:kor ,
                        # lang:nld ,
                        # lang:pol ,
                        # lang:jpn ,
                        # lang:msa ,
                        lang:rus ,
                        lang:spa ,
                        lang:swe ,
                        lang:zho ;
          dcterms:identifier 133 ;
          skos:notation 133 ;
          rdfs:label "Dijkstra graph" ;

  skos:definition "positively weighted directed graph appropriately configured to execute a shortest path search"@en ;
  skos:definition "رسم بياني موجهاً وموزوناً إيجابياً وبالشكل المناسب لتنفيذ البحث عن أقصر الطرق"@ar ;
  skos:definition "positivt vægtet retningsbestemt graf, der er konfigureret til at udføre en søgning efter korteste vej"@da ;
  skos:definition "positiivisesti painotettu suunnattu verkko, joka on konfiguroitu hakemaan suorin reitti"@fi ;
  skos:definition "graphe dirigé, pondéré positivement, convenablement configuré pour exécuter une recherche de chemin le plus court"@fr ;
  skos:definition "최단 경로 탐색을 위해 적합하게 설정된 양의 가중 방향 그래프"@ko ;
  skos:definition "неотрицательно взвешенный ориентированный граф, специально сконфигурированный для выполнения операции поиска кратчайшего пути"@ru ;
  skos:definition "grafo dirigido positivamente ponderado y  configurado de manera apropiada para ejecutar una búsqueda del camino más corto"@es ;
  skos:definition "viktad och riktad graf som utgör underlag för Dijkstras algoritm, vilken söker den kortaste vägen mellan två punkter (eller noder)"@sv ;
  skos:definition "Dijkstra曲线图是通过适当配置、权值为正的有向图，用于执行最短路径的搜索。"@zh ;

  skos:prefLabel "Dijkstra graph"@en ;
  skos:prefLabel "الرسم البياني لـدجكسترا &quot;"@ar ;
  skos:prefLabel "Dijkstra-graf"@da ;
  skos:prefLabel "Dijkstra Graph"@de ;
  skos:prefLabel "Dijkstran verkko"@fi ;
  skos:altLabel "Dijkstran graafi"@fi ;
  skos:prefLabel "graphe de Dijkstra"@fr ;
  skos:prefLabel "다익스트라 그래프"@ko ;
  skos:prefLabel "граф Дейкстры"@ru ;
  skos:prefLabel "grafo de Dijkstra"@es ;
  skos:prefLabel "Dijkstragraf"@sv ;
  skos:prefLabel "Dijkstra曲线图"@zh ;
  
  geolexica:origin lang:araRegistry ,
                lang:danRegistry ,
                lang:deuRegistry ,
                lang:engRegistry ,
                lang:finRegistry ,
                lang:fraRegistry ,
                lang:korRegistry ,
                # lang:polRegistry ,
                # lang:msaRegistry ,
                # lang:nldRegistry ,
                # lang:jpnRegistry ,
                lang:rusRegistry ,
                lang:spaRegistry ,
                lang:sweRegistry ,
                lang:zhoRegistry ;
        lang:deu-note notes:DefnTransUnavail , notes:NoteTransUnavail ;
        lang:swe-note notes:NoteTransUnavail ;
        lang:fra-note notes:NoteTransDiff .


###  https://isotc211.geolexica.org/ld/concepts#direct_eval_method
:direct_eval_method rdf:type owl:NamedIndividual ,
                   skos:Concept ;
          skos:inScheme geolexica:GeolexicaConceptScheme ;
          geolexica:hasInfo info:Info134 ;
          geolexica:hasReview reviews:Review134 ;
          geolexica:hasLDAPI ldapi:ldapi134-json ,
                             ldapi:ldapi134-jsonld ,
                             ldapi:ldapi134-rdfxml ,
                             ldapi:ldapi134-skosrdf ;
        geolexica:hasLangCode lang:ara ,
                        lang:dan ,
                        lang:deu ,
                        lang:eng ,
                        lang:fin ,
                        lang:fra ,
                        lang:kor ,
                        # lang:nld ,
                        # lang:pol ,
                        # lang:jpn ,
                        # lang:msa ,
                        lang:rus ,
                        lang:spa ,
                        lang:swe ,
                        lang:zho ;
          dcterms:identifier 134 ;
          skos:notation 134 ;
          rdfs:label "direct evaluation method" ;

  skos:definition "method of evaluating the quality of a dataset based on inspection of the items within the dataset"@en ;
  skos:definition "طريقة لتقييم الجودة لمجموعة بيانات تبني على فحص البنود أو المواد التي تحتوي عليها المجموعة ."@ar ;
  skos:definition "metode til vurdering af kvaliteten af et datasæt baseret på undersøgelse af elementerne i datasættet"@da ;
  skos:definition "Verfahren zur Bewertung der Qualität eines Datensatzes, das auf der Überprüfung der Elemente innerhalb des Datensatzes beruht"@de ;
  skos:definition "laadun arviointimenetelmä, jossa tietoaineiston laatu määritellään tietoaineistoon sisältyvän tiedon tarkastuksen perusteella"@fi ;
  skos:definition "méthode d&#39;évaluation de la qualité d&#39;un jeu de données basée sur l&#39;inspection des éléments du jeu de données"@fr ;
  skos:definition "데이터셋 내의 항목 검사에 의거한 데이터셋 품질 평가 방법"@ko ;
  skos:definition "метод оценки качества набора данных, основанный на проверке элементов набора данных"@ru ;
  skos:definition "método de evaluación de la calidad de un conjunto de datos basado en la inspección de sus ítems dentro del conjunto de datos"@es ;
  skos:definition "metod för att utvärdera kvaliteten av hos en datamängd baserat på inspektion av enheterna uppgifterna inom datamängden"@sv ;
  skos:definition "以数据集内部检验单元检验为基础的数据集质量评价方法。"@zh ;

  skos:prefLabel "direct evaluation method"@en ;
  skos:prefLabel "طريقة التقييم المباشر"@ar ;
  skos:prefLabel "direkte vurderingsmetode"@da ;
  skos:prefLabel "(direktes) Bewertungsverfahren"@de ;
  skos:prefLabel "suora laadun arviointimenetelmä"@fi ;
  skos:prefLabel "méthode d&#39;évaluation directe"@fr ;
  skos:prefLabel "직접 평가법"@ko ;
  skos:prefLabel "метод прямой оценки"@ru ;
  skos:prefLabel "método directo de evaluación"@es ;
  skos:prefLabel "direkt utvärdering"@sv ;
  skos:prefLabel "直接评价法"@zh ;
  
  geolexica:origin lang:araRegistry ,
                lang:danRegistry ,
                lang:deuRegistry ,
                lang:engRegistry ,
                lang:finRegistry ,
                lang:fraRegistry ,
                lang:korRegistry ,
                # lang:polRegistry ,
                # lang:msaRegistry ,
                # lang:nldRegistry ,
                # lang:jpnRegistry ,
                lang:rusRegistry ,
                lang:spaRegistry ,
                lang:sweRegistry ,
                lang:zhoRegistry .

###  https://isotc211.geolexica.org/ld/concepts#direct_position
:direct_position rdf:type owl:NamedIndividual ,
                   skos:Concept ;
          skos:inScheme geolexica:GeolexicaConceptScheme ;
          geolexica:hasInfo info:Info135 ;
          geolexica:hasReview reviews:Review135 ;
          geolexica:hasLDAPI ldapi:ldapi135-json ,
                             ldapi:ldapi135-jsonld ,
                             ldapi:ldapi135-rdfxml ,
                             ldapi:ldapi135-skosrdf ;
        geolexica:hasLangCode lang:ara ,
                        lang:dan ,
                        lang:deu ,
                        lang:eng ,
                        lang:fin ,
                        lang:fra ,
                        lang:kor ,
                        # lang:nld ,
                        lang:pol ,
                        lang:jpn ,
                        lang:msa ,
                        lang:rus ,
                        lang:spa ,
                        lang:swe ,
                        lang:zho ;
          dcterms:identifier 135 ;
          skos:notation 135 ;
          rdfs:label "direct position" ;

  skos:definition "position described by a single set of coordinates within a coordinate reference system"@en ;
  skos:definition "موقع تصفه مجموعة إحداثيات واحدة ضمن نظام إحداثيات مرجعي"@ar ;
  skos:definition "position beskrevet ved et enkelt sæt af koordinater i et koordinatsystem"@da ;
  skos:definition "Position, die durch einen einzelnen Koordinatensatz in einem Koordinatenreferenzsystem beschrieben wird"@de ;
  skos:definition "koordinaattijärjestelmän ja sen mukaisten koordinaattien avulla ilmaistu sijainti"@fi ;
  skos:definition "position décrite par un ensemble unique de coordonnées dans un système de référence de coordonnées"@fr ;
  skos:definition "座標参照系の中で一つの座標によって記述された位置。"@ja ;
  skos:definition "좌표 참조 체계 내에서 단일 좌표 집합에 의해 기술되는 위치"@ko ;
  skos:definition "położenie opisane przez pojedynczy zbiór współrzędnych w systemie odniesienia opartym na współrzędnych"@pl ;
  skos:definition "местоположение,  описываемое единичным  множеством координат в некоторой координатной системе отсчета"@ru ;
  skos:definition "posición descrita por un único conjunto de coordenadas dentro de un sistema de referencia de coordenadas"@es ;
  skos:definition "läge beskrivet av en viss uppsättning koordinater i ett koordinatsystem"@sv ;
  skos:definition "用坐标参照系中的一组坐标描述的位置。"@zh ;

  skos:prefLabel "direct position"@en ;
  skos:prefLabel "موقع مباشر"@ar ;
  skos:prefLabel "direkte position"@da ;
  skos:prefLabel "direkte Position"@de ;
  skos:prefLabel "suora sijainti"@fi ;
  skos:altLabel "koordinaattitieto"@fi ;
  skos:prefLabel "position directe"@fr ;
  skos:prefLabel "直接位置"@ja ;
  skos:prefLabel "직접 위치"@ko ;
  skos:prefLabel "kedudukan langsung"@ms ;
  skos:prefLabel "położenie bezpośrednie"@pl ;
  skos:prefLabel "(координатная) точка"@ru ;
  skos:prefLabel "posición directa"@es ;
  skos:prefLabel "geografiskt läge"@sv ;
  skos:prefLabel "直接位置"@zh ;
  
  geolexica:origin lang:araRegistry ,
                lang:danRegistry ,
                lang:deuRegistry ,
                lang:engRegistry ,
                lang:finRegistry ,
                lang:fraRegistry ,
                lang:korRegistry ,
                lang:polRegistry ,
                lang:msaRegistry ,
                # lang:nldRegistry ,
                lang:jpnRegistry ,
                lang:rusRegistry ,
                lang:spaRegistry ,
                lang:sweRegistry ,
                lang:zhoRegistry ;
        lang:msa-note notes:DefnTransUnavail .

###  https://isotc211.geolexica.org/ld/concepts#directed_edge
:directed_edge rdf:type owl:NamedIndividual ,
                   skos:Concept ;
          skos:inScheme geolexica:GeolexicaConceptScheme ;
          geolexica:hasInfo info:Info136 ;
          geolexica:hasReview reviews:Review136 ;
          geolexica:hasLDAPI ldapi:ldapi136-json ,
                             ldapi:ldapi136-jsonld ,
                             ldapi:ldapi136-rdfxml ,
                             ldapi:ldapi136-skosrdf ;
        geolexica:hasLangCode lang:ara ,
                        lang:dan ,
                        lang:deu ,
                        lang:eng ,
                        lang:fin ,
                        lang:fra ,
                        lang:kor ,
                        # lang:nld ,
                        lang:pol ,
                        lang:jpn ,
                        # lang:msa ,
                        lang:rus ,
                        lang:spa ,
                        lang:swe ,
                        lang:zho ;
          dcterms:identifier 136 ;
          skos:notation 136 ;
          rdfs:label "directed edge" ;

  skos:definition "directed topological object that represents an association between an edge and one of its orientations"@en ;
  skos:definition "كائن طوبولوجي موجه يمثل ربطاً بين حافة معينة وأحد اتجاهاتها"@ar ;
  skos:definition "retningsbestemt topologisk objekt, der repræsenterer en forbindelse mellem en kant og en af dens orienteringer"@da ;
  skos:definition "suunnattu topologinen objekti, joka kuvaa särmän ja sen suunnan välistä yhteyttä"@fi ;
  skos:definition "objet topologique orienté représentant une association entre une arête et une de ses orientations"@fr ;
  skos:definition "エッジとその向きの一つとの間の関連を表す有向位相オブジェクト。"@ja ;
  skos:definition "하나의 변과 그 변이 갖는 방향성 간의 연관으로 표현된 방향성 위상 객체"@ko ;
  skos:definition "skierowany obiekt topologiczny, który reprezentuje powiązanie między krawędzią a jedną z jej orientacji"@pl ;
  skos:definition "ориентированный топологический объект, который представляет связь между ребром и одним из его направлений"@ru ;
  skos:definition "objeto topológico orientado que representa una asociación entre un arco y una de sus orientaciones"@es ;
  skos:definition "orienterad topologiskt objekt som anger sambandet mellan en länk och en av dess orienteringar"@sv ;
  skos:definition "有向拓扑对象，表达边和它的一个方向之间的关联。"@zh ;

  skos:prefLabel "directed edge"@en ;
  skos:prefLabel "حافة موجهة"@ar ;
  skos:prefLabel "retningsbestemt kant"@da ;
  skos:prefLabel "gerichtete Kante"@de ;
  skos:prefLabel "suunnattu särmä"@fi ;
  skos:altLabel "linkki"@fi ;
  skos:prefLabel "arête orientée"@fr ;
  skos:prefLabel "有向エッジ"@ja ;
  skos:prefLabel "방향성 변"@ko ;
  skos:altLabel "방향성 에지"@ko ;
  skos:prefLabel "krawędź skierowana"@pl ;
  skos:prefLabel "ориентированное ребро"@ru ;
  skos:prefLabel "arco orientado"@es ;
  skos:prefLabel "orienterad länk"@sv ;
  skos:prefLabel "有向边"@zh ;
  
  geolexica:origin lang:araRegistry ,
                lang:danRegistry ,
                lang:deuRegistry ,
                lang:engRegistry ,
                lang:finRegistry ,
                lang:fraRegistry ,
                lang:korRegistry ,
                lang:polRegistry ,
                # lang:msaRegistry ,
                # lang:nldRegistry ,
                lang:jpnRegistry ,
                lang:rusRegistry ,
                lang:spaRegistry ,
                lang:sweRegistry ,
                lang:zhoRegistry ;
        lang:deu-note notes:DefnTransUnavail , notes:NoteTransUnavail .

###  https://isotc211.geolexica.org/ld/concepts#directed_face
:directed_face rdf:type owl:NamedIndividual ,
                   skos:Concept ;
          skos:inScheme geolexica:GeolexicaConceptScheme ;
          geolexica:hasInfo info:Info137 ;
          geolexica:hasReview reviews:Review137 ;
          geolexica:hasLDAPI ldapi:ldapi137-json ,
                             ldapi:ldapi137-jsonld ,
                             ldapi:ldapi137-rdfxml ,
                             ldapi:ldapi137-skosrdf ;
        geolexica:hasLangCode lang:ara ,
                        lang:dan ,
                        lang:deu ,
                        lang:eng ,
                        lang:fin ,
                        lang:fra ,
                        lang:kor ,
                        # lang:nld ,
                        lang:pol ,
                        lang:jpn ,
                        # lang:msa ,
                        lang:rus ,
                        lang:spa ,
                        lang:swe ,
                        lang:zho ;
          dcterms:identifier 137 ;
          skos:notation 137 ;
          rdfs:label "directed face" ;

  skos:definition "directed topological object that represents an association between a face and one of its orientations"@en ;
  skos:definition "كائن طوبولوجي موجه يمثل ربطاً بين واجهة معينة وأحد اتجاهاتها"@ar ;
  skos:definition "retningsbestemt topologisk objekt, der repræsenterer en forbindelse mellem en flade og en af dens orienteringer"@da ;
  skos:definition "suunnattu topologinen objekti, joka kuvaa tahkon ja jonkin sen suunnan välistä yhteyttä"@fi ;
  skos:definition "objet topologique orienté représentant une association entre une face et une de ses orientations"@fr ;
  skos:definition "フェイスとその向きの一つとの間の関連を表す有向位相オブジェクト。"@ja ;
  skos:definition "하나의 면과 그 면이 갖는 방향성 간의 연관으로 표현된 방향성 위상 객체"@ko ;
  skos:definition "skierowany obiekt topologiczny, który reprezentuje powiązanie między ścianą a jedną z jej orientacji"@pl ;
  skos:definition "ориентированный топологический объект, который представляет связь между гранью и одним из ее направлений"@ru ;
  skos:definition "objeto topológico orientado que representa una asociación entre una cara y una de sus orientaciones"@es ;
  skos:definition "orienterat topologiskt objekt som anger sambandet mellan ett topologiskt område och en av dess orienteringar"@sv ;
  skos:definition "有向拓扑对象，表达面和它的一个方向之间的关联。"@zh ;
  
  skos:prefLabel "directed face"@en ;
  skos:prefLabel "واجهة موجهة"@ar ;
  skos:prefLabel "retningsbestemt flade"@da ;
  skos:prefLabel "gerichtete Masche"@de ;
  skos:prefLabel "suunnattu tahko"@fi ;
  skos:prefLabel "face orientée"@fr ;
  skos:prefLabel "有向フェイス"@ja ;
  skos:prefLabel "방향성 면"@ko ;
  skos:altLabel "방향성 페이스"@ko ;
  skos:prefLabel "ściana skierowana"@pl ;
  skos:prefLabel "ориентированная грань"@ru ;
  skos:prefLabel "cara orientada"@es ;
  skos:prefLabel "orienterat område"@sv ;
  skos:prefLabel "有向面"@zh ;
  
  geolexica:origin lang:araRegistry ,
                lang:danRegistry ,
                lang:deuRegistry ,
                lang:engRegistry ,
                lang:finRegistry ,
                lang:fraRegistry ,
                lang:korRegistry ,
                lang:polRegistry ,
                # lang:msaRegistry ,
                # lang:nldRegistry ,
                lang:jpnRegistry ,
                lang:rusRegistry ,
                lang:spaRegistry ,
                lang:sweRegistry ,
                lang:zhoRegistry ;
        lang:deu-note notes:DefnTransUnavail , notes:NoteTransUnavail ; 
        lang:swe-note notes:NoteTransUnavail  .

###  https://isotc211.geolexica.org/ld/concepts#directed_node
:directed_node rdf:type owl:NamedIndividual ,
                   skos:Concept ;
          skos:inScheme geolexica:GeolexicaConceptScheme ;
          geolexica:hasInfo info:Info138 ;
          geolexica:hasReview reviews:Review138 ;
          geolexica:hasLDAPI ldapi:ldapi138-json ,
                             ldapi:ldapi138-jsonld ,
                             ldapi:ldapi138-rdfxml ,
                             ldapi:ldapi138-skosrdf ;
        geolexica:hasLangCode lang:ara ,
                        lang:dan ,
                        lang:deu ,
                        lang:eng ,
                        lang:fin ,
                        lang:fra ,
                        lang:kor ,
                        # lang:nld ,
                        lang:pol ,
                        lang:jpn ,
                        # lang:msa ,
                        lang:rus ,
                        lang:spa ,
                        lang:swe ,
                        lang:zho ;
          dcterms:identifier 138 ;
          skos:notation 138 ;
          rdfs:label "directed node" ;

  skos:definition "directed topological object that represents an association between a node and one of its orientations"@en ;
  skos:definition "كائن طوبولوجي موجه يمثل ربطاً بين عقدة معينة وأحد اتجاهاتها"@ar ;
  skos:definition "retningsbestemt topologisk objekt, der repræsenterer en forbindelse mellem en knude og en af dens orienteringer"@da ;
  skos:definition "suunnattu topologinen objekti, joka kuvaa solmupisteen ja jonkin sen suunnan välistä yhteyttä"@fi ;
  skos:definition "objet topologique orienté représentant une association entre un noeud et une de ses orientations"@fr ;
  skos:definition "ノードとその向きの一つとの間の関連を表す有向位相オブジェクト。"@ja ;
  skos:definition "하나의 절점과 그 절점이 갖는 방향성 간의 연관으로 표현된 방향성 위상 객체"@ko ;
  skos:definition "skierowany obiekt topologiczny, który reprezentuje powiązanie między węzłem a jedną z jego orientacji"@pl ;
  skos:definition "ориентированный топологический объект, который представляет связь между узлом и одним из его направлений"@ru ;
  skos:definition "objeto topológico orientado que representa una asociación entre un nodo y una de sus orientaciones"@es ;
  skos:definition "orienterat topologiskt objekt som anger sambandet mellan en nod och en av dess orienteringar"@sv ;
  skos:definition "有向拓扑对象，表达结点和它的一个方向之间的关联。"@zh ;
  
  skos:prefLabel "directed node"@en ;
  skos:prefLabel "عقدة موجهة"@ar ;
  skos:prefLabel "retningsbestemt knude"@da ;
  skos:prefLabel "gerichteter Knoten"@de ;
  skos:prefLabel "suunnattu solmu"@fi ;
  skos:prefLabel "nœud orienté"@fr ;
  skos:prefLabel "有向ノード"@ja ;
  skos:prefLabel "방향성 절점"@ko ;
  skos:prefLabel "węzeł skierowany"@pl ;
  skos:prefLabel "ориентированный узел"@ru ;
  skos:prefLabel "nodo orientado"@es ;
  skos:prefLabel "orienterad nod"@sv ;
  skos:prefLabel "有向结点"@zh ;
  
  geolexica:origin lang:araRegistry ,
                lang:danRegistry ,
                lang:deuRegistry ,
                lang:engRegistry ,
                lang:finRegistry ,
                lang:fraRegistry ,
                lang:korRegistry ,
                lang:polRegistry ,
                # lang:msaRegistry ,
                # lang:nldRegistry ,
                lang:jpnRegistry ,
                lang:rusRegistry ,
                lang:spaRegistry ,
                lang:sweRegistry ,
                lang:zhoRegistry ;
        lang:deu-note notes:DefnTransUnavail , notes:NoteTransUnavail ; 
        lang:swe-note notes:NoteTransUnavail  .


###  https://isotc211.geolexica.org/ld/concepts#directed_solid
:directed_solid rdf:type owl:NamedIndividual ,
                   skos:Concept ;
          skos:inScheme geolexica:GeolexicaConceptScheme ;
          geolexica:hasInfo info:Info139 ;
          geolexica:hasReview reviews:Review139 ;
          geolexica:hasLDAPI ldapi:ldapi139-json ,
                             ldapi:ldapi139-jsonld ,
                             ldapi:ldapi139-rdfxml ,
                             ldapi:ldapi139-skosrdf ;
        geolexica:hasLangCode lang:ara ,
                        lang:dan ,
                        lang:deu ,
                        lang:eng ,
                        lang:fin ,
                        lang:fra ,
                        lang:kor ,
                        # lang:nld ,
                        lang:pol ,
                        lang:jpn ,
                        # lang:msa ,
                        lang:rus ,
                        lang:spa ,
                        lang:swe ,
                        lang:zho ;
          dcterms:identifier 139 ;
          skos:notation 139 ;
          rdfs:label "directed solid" ;

  skos:definition "directed topological object that represents an association between a topological solid and one of its orientations"@en ;
  skos:definition "كائن طوبولوجي موجه يمثل ربطاً بين مجسم طوبولوجي وأحد اتجاهاته"@ar ;
  skos:definition "retningsbestemt topologisk objekt, der repræsenterer en fobindelse mellem et topologisk legeme og en af dets orienteringer"@da ;
  skos:definition "suunnattu topologinen objekti, joka kuvaa topologisen kappaleen ja jonkin sen suunnan välistä yhteyttä"@fi ;
  skos:definition "objet topologique orienté représentant une association entre un solide topologique et une de ses orientations"@fr ;
  skos:definition "位相立体とその向きの一つとの間の関連を表す有向位相オブジェクト。"@ja ;
  skos:definition "하나의 위상 입방체와 그 입방체가 갖는 방향성 간의 연관으로 표현된 방향성 위상 객체"@ko ;
  skos:definition "skierowany obiekt topologiczny, który reprezentuje powiązanie między bryłą topologiczną a jedną z jej orientacji"@pl ;
  skos:definition "ориентированный топологический объект, который представляет связь между топологическим телом  и одним из его направлений"@ru ;
  skos:definition "objeto topológico orientado que representa una asociación entre un sólido topológico y una de sus orientaciones"@es ;
  skos:definition "orienterat topologiskt objekt som anger sambandet mellan ett topologisk kropp och en av dess orienteringar"@sv ;
  skos:definition "有向拓扑对象，表达拓扑体和它的一个方向之间的关联。"@zh ;
  
  skos:prefLabel "directed solid"@en ;
  skos:prefLabel "مجسم موجه"@ar ;
  skos:prefLabel "retningsbestemt legeme"@da ;
  skos:prefLabel "gerichteter Körper"@de ;
  skos:prefLabel "suunnattu kappale"@fi ;
  skos:prefLabel "solide orienté"@fr ;
  skos:prefLabel "有向位相立体"@ja ;
  skos:prefLabel "방향성 입방체"@ko ;
  skos:prefLabel "bryła skierowana"@pl ;
  skos:prefLabel "ориентированное тело"@ru ;
  skos:prefLabel "sólido orientado"@es ;
  skos:prefLabel "orienterad topologisk kropp"@sv ;
  skos:prefLabel "有向体"@zh ;
  
  geolexica:origin lang:araRegistry ,
                lang:danRegistry ,
                lang:deuRegistry ,
                lang:engRegistry ,
                lang:finRegistry ,
                lang:fraRegistry ,
                lang:korRegistry ,
                lang:polRegistry ,
                # lang:msaRegistry ,
                # lang:nldRegistry ,
                lang:jpnRegistry ,
                lang:rusRegistry ,
                lang:spaRegistry ,
                lang:sweRegistry ,
                lang:zhoRegistry ;
        lang:deu-note notes:DefnTransUnavail , notes:NoteTransUnavail ; 
        lang:swe-note notes:NoteTransUnavail  .


###  https://isotc211.geolexica.org/ld/concepts#directed_topo_object
:directed_topo_object rdf:type owl:NamedIndividual ,
                   skos:Concept ;
          skos:inScheme geolexica:GeolexicaConceptScheme ;
          geolexica:hasInfo info:Info140 ;
          geolexica:hasReview reviews:Review140 ;
          geolexica:hasLDAPI ldapi:ldapi140-json ,
                             ldapi:ldapi140-jsonld ,
                             ldapi:ldapi140-rdfxml ,
                             ldapi:ldapi140-skosrdf ;
        geolexica:hasLangCode lang:ara ,
                        lang:dan ,
                        lang:deu ,
                        lang:eng ,
                        lang:fin ,
                        lang:fra ,
                        lang:kor ,
                        # lang:nld ,
                        lang:pol ,
                        lang:jpn ,
                        # lang:msa ,
                        lang:rus ,
                        lang:spa ,
                        lang:swe ,
                        lang:zho ;
          dcterms:identifier 140 ;
          skos:notation 140 ;
          rdfs:label "directed topological object" ;

  skos:definition "topological object that represents a logical association between a topological primitive and one of its orientations"@en ;
  skos:definition "كائن طوبولوجي يمثل ربطاً منطقياً بين عنصر طوبولوجي بسيط وأحد اتجاهاته"@ar ;
  skos:definition "topologisk objekt, der repræsenterer en logisk forbindelse mellem en topologisk grundform og en af dets orienteringer"@da ;
  skos:definition "topologinen objekti, joka kuvaa topologisen primitiivin ja jonkin sen suunnan välistä loogista yhteyttä"@fi ;
  skos:definition "objet topologique représentant une association logique entre une primitive topologique et une de ses orientations"@fr ;
  skos:definition "位相プリミティブとその向きの一つとの間の論理的な関連を表す位相オブジェクト。"@ja ;
  skos:definition "하나의 위상 원시 객체와 그 위상 원시 객체가 갖는 방향성 간의 연관으로 표현된 위상객체"@ko ;
  skos:definition "obiekt topologiczny reprezentujący powiązanie logiczne między prostym elementem topologicznym a jedną z jego orientacji"@pl ;
  skos:definition "топологический объект, который представляет логическую связь между топологическим примитивом и одним из его направлений"@ru ;
  skos:definition "objeto topológico orientado que representa una asociación entre un objeto topológico y una de sus orientaciones"@es ;
  skos:definition "topologiskt objekt som anger det logiska sambandet mellan ett topologisk grundelement och en av dess orienteringar"@sv ;
  skos:definition "拓扑对象，表达拓扑单形和它的一个方向之间的逻辑关联。"@zh ;
  
  skos:prefLabel "directed topological object"@en ;
  skos:prefLabel "كائن طوبولوجي موجه"@ar ;
  skos:prefLabel "retningsbestemt topologisk objekt"@da ;
  skos:prefLabel "gerichtetes topologisches Objekt"@de ;
  skos:prefLabel "suunnattu topologinen objekti"@fi ;
  skos:prefLabel "objet topologique orienté"@fr ;
  skos:prefLabel "有向位相オブジェクト"@ja ;
  skos:prefLabel "방향성 위상 객체"@ko ;
  skos:prefLabel "skierowany obiekt topologiczny"@pl ;
  skos:prefLabel "ориентированный топологический объект"@ru ;
  skos:prefLabel "objeto topológico orientado"@es ;
  skos:prefLabel "orienterat topologiskt objekt"@sv ;
  skos:prefLabel "有向拓扑对象"@zh ;
  
  geolexica:origin lang:araRegistry ,
                lang:danRegistry ,
                lang:deuRegistry ,
                lang:engRegistry ,
                lang:finRegistry ,
                lang:fraRegistry ,
                lang:korRegistry ,
                lang:polRegistry ,
                # lang:msaRegistry ,
                # lang:nldRegistry ,
                lang:jpnRegistry ,
                lang:rusRegistry ,
                lang:spaRegistry ,
                lang:sweRegistry ,
                lang:zhoRegistry ;
        lang:deu-note notes:DefnTransUnavail .


###  Generated by the OWL API (version 4.5.9.2019-02-01T07:24:44Z) https://github.com/owlcs/owlapi
# 